<?xml version="1.0" encoding="utf-8"?>
<rdf:RDF
   xmlns:bffi-meta="http://urn.fi/URN:NBN:fi:schema:bffi-meta:"
   xmlns:dct="http://purl.org/dc/terms/"
   xmlns:owl="http://www.w3.org/2002/07/owl#"
   xmlns:rdf="http://www.w3.org/1999/02/22-rdf-syntax-ns#"
   xmlns:rdfs="http://www.w3.org/2000/01/rdf-schema#"
   xmlns:skos="http://www.w3.org/2004/02/skos/core#"
>
  <rdf:Description rdf:nodeID="n3340e60e05a148bda7f556ae223dde3ab5">
    <rdf:first rdf:resource="http://urn.fi/URN:NBN:fi:schema:bffi:Item"/>
    <rdf:rest rdf:resource="http://www.w3.org/1999/02/22-rdf-syntax-ns#nil"/>
  </rdf:Description>
  <rdf:Description rdf:about="http://urn.fi/URN:NBN:fi:schema:bffi:MetadataLicensor">
    <dct:modified>2024-06-19 (New)</dct:modified>
    <rdfs:label xml:lang="en">Metadata licensor</rdfs:label>
    <rdfs:label xml:lang="fi">Metatiedon tekijänoikeus</rdfs:label>
    <rdf:type rdf:resource="http://www.w3.org/2002/07/owl#Class"/>
    <owl:equivalentClass rdf:resource="http://id.loc.gov/ontologies/bflc/MetadataLicensor"/>
    <rdfs:subClassOf rdf:resource="http://urn.fi/URN:NBN:fi:schema:bffi:Agent"/>
    <skos:definition xml:lang="en">BFLC definition: Organization that licenses the intellectual property rights to the data contained in the description.</skos:definition>
  </rdf:Description>
  <rdf:Description rdf:about="http://urn.fi/URN:NBN:fi:schema:bffi:contentOfRepresentativeExpression">
    <dct:modified>2024-04-16 (New)</dct:modified>
    <rdfs:label xml:lang="en">content type of representative expression</rdfs:label>
    <rdfs:label xml:lang="fi">edustavan ekspression sisältötyyppi</rdfs:label>
    <rdfs:domain rdf:resource="http://urn.fi/URN:NBN:fi:schema:bffi:Work"/>
    <rdfs:range rdf:resource="http://urn.fi/URN:NBN:fi:schema:bffi:Content"/>
    <rdf:type rdf:resource="http://www.w3.org/2002/07/owl#ObjectProperty"/>
    <bffi-meta:exactMatch rdf:resource="http://rdaregistry.info/Elements/w/P10349"/>
    <rdfs:subPropertyOf rdf:resource="http://id.loc.gov/ontologies/bibframe/content"/>
  </rdf:Description>
  <rdf:Description rdf:about="http://urn.fi/URN:NBN:fi:schema:bffi:exclusionGRing">
    <dct:modified>2024-04-16 (New)</dct:modified>
    <rdfs:label xml:lang="en">cartographic G ring area excluded</rdfs:label>
    <rdfs:label xml:lang="fi">poissulkeva G-kehä</rdfs:label>
    <rdfs:domain rdf:resource="http://urn.fi/URN:NBN:fi:schema:bffi:Cartographic"/>
    <rdfs:range rdf:resource="http://www.w3.org/2000/01/rdf-schema#Literal"/>
    <rdf:type rdf:resource="http://www.w3.org/2002/07/owl#DatatypeProperty"/>
    <owl:equivalentProperty rdf:resource="http://id.loc.gov/ontologies/bibframe/exclusionGRing"/>
    <skos:definition xml:lang="en">BIBFRAME definition: Coordinate pairs that identify the closed non-intersecting boundary of the area contained within the G-polygon outer ring that is excluded.</skos:definition>
  </rdf:Description>
  <rdf:Description rdf:about="http://urn.fi/URN:NBN:fi:schema:bffi:associatedResource">
    <dct:modified>2024-09-16 (New)</dct:modified>
    <rdfs:label xml:lang="en">associated resource</rdfs:label>
    <rdfs:label xml:lang="fi">liittyvä aineisto</rdfs:label>
    <rdfs:domain rdf:resource="http://urn.fi/URN:NBN:fi:schema:bffi:Relation"/>
    <rdfs:range rdf:nodeID="n3340e60e05a148bda7f556ae223dde3ab1"/>
    <rdf:type rdf:resource="http://www.w3.org/2002/07/owl#ObjectProperty"/>
    <owl:equivalentProperty rdf:resource="http://id.loc.gov/ontologies/bibframe/associatedResource"/>
    <skos:definition xml:lang="en">BIBFRAME definition: Associated resource</skos:definition>
  </rdf:Description>
  <rdf:Description rdf:about="http://urn.fi/URN:NBN:fi:schema:bffi:heldBy">
    <dct:modified>2025-01-02 (New)</dct:modified>
    <rdfs:label xml:lang="en">held by</rdfs:label>
    <rdfs:label xml:lang="fi">haltija</rdfs:label>
    <rdfs:domain rdf:resource="http://urn.fi/URN:NBN:fi:schema:bffi:Item"/>
    <rdfs:range rdf:resource="http://www.w3.org/2000/01/rdf-schema#Resource"/>
    <rdf:type rdf:resource="http://www.w3.org/2002/07/owl#ObjectProperty"/>
    <owl:equivalentProperty rdf:resource="http://id.loc.gov/ontologies/bibframe/heldBy"/>
    <bffi-meta:narrowMatch rdf:resource="http://rdaregistry.info/Elements/i/P40021"/>
    <skos:definition xml:lang="en">BIBFRAME definition: Entity holding the item or from which it is available.</skos:definition>
  </rdf:Description>
  <rdf:Description rdf:about="http://urn.fi/URN:NBN:fi:schema:bffi:SourceConsulted">
    <dct:modified>2024-06-19 (New)</dct:modified>
    <rdfs:label xml:lang="en">Source consulted</rdfs:label>
    <rdfs:label xml:lang="fi">Käytetty lähde</rdfs:label>
    <rdf:type rdf:resource="http://www.w3.org/2002/07/owl#Class"/>
  </rdf:Description>
  <rdf:Description rdf:about="http://urn.fi/URN:NBN:fi:schema:bffi:Kit">
    <dct:modified>2024-02-23 (New)</dct:modified>
    <rdfs:label xml:lang="en">Kit</rdfs:label>
    <rdfs:label xml:lang="fi">Moniviestin</rdfs:label>
    <rdf:type rdf:resource="http://www.w3.org/2002/07/owl#Class"/>
    <owl:equivalentClass rdf:resource="http://id.loc.gov/ontologies/bibframe/Kit"/>
    <rdfs:subClassOf rdf:resource="http://urn.fi/URN:NBN:fi:schema:bffi:MixedMaterial"/>
    <skos:definition xml:lang="en">BIBFRAME definition: Resource that contains a mixture of various components issued as a unit and intended primarily for instructional purposes</skos:definition>
  </rdf:Description>
  <rdf:Description rdf:about="http://urn.fi/URN:NBN:fi:schema:bffi:enumerationAndChronology">
    <dct:modified>2024-02-23 (New)</dct:modified>
    <rdfs:label xml:lang="en">enumeration and chronology</rdfs:label>
    <rdfs:label xml:lang="fi">numerointi- ja julkaisuaikatiedot</rdfs:label>
    <rdfs:domain rdf:resource="http://urn.fi/URN:NBN:fi:schema:bffi:Item"/>
    <rdfs:range rdf:resource="http://urn.fi/URN:NBN:fi:schema:bffi:EnumerationAndChronology"/>
    <rdf:type rdf:resource="http://www.w3.org/2002/07/owl#ObjectProperty"/>
    <owl:equivalentProperty rdf:resource="http://id.loc.gov/ontologies/bibframe/enumerationAndChronology"/>
    <skos:definition xml:lang="en">BIBFRAME definition: Numbering and dates of issues or items held.</skos:definition>
  </rdf:Description>
  <rdf:Description rdf:about="http://urn.fi/URN:NBN:fi:schema:bffi:simpleDate">
    <dct:modified>2024-02-23 (New)</dct:modified>
    <rdfs:label xml:lang="en">date of provision activity</rdfs:label>
    <rdfs:label xml:lang="fi">tuottamiseen liittyvä vuosiluku</rdfs:label>
    <rdfs:domain rdf:resource="http://urn.fi/URN:NBN:fi:schema:bffi:ProvisionActivity"/>
    <rdfs:range rdf:resource="http://www.w3.org/2000/01/rdf-schema#Literal"/>
    <rdf:type rdf:resource="http://www.w3.org/2002/07/owl#DatatypeProperty"/>
    <owl:equivalentProperty rdf:resource="http://id.loc.gov/ontologies/bflc/simpleDate"/>
    <skos:definition xml:lang="en">BFLC definition: Date of publication, distribution, manufacture or production as transcribed from the resource</skos:definition>
  </rdf:Description>
  <rdf:Description rdf:about="http://urn.fi/URN:NBN:fi:schema:bffi:originDate">
    <dct:modified>2024-02-23 (New)</dct:modified>
    <rdfs:label xml:lang="en">origin date</rdfs:label>
    <rdfs:label xml:lang="fi">teoksen ajankohta</rdfs:label>
    <rdfs:domain rdf:resource="http://urn.fi/URN:NBN:fi:schema:bffi:Work"/>
    <rdfs:range rdf:resource="http://www.w3.org/2000/01/rdf-schema#Literal"/>
    <rdf:type rdf:resource="http://www.w3.org/2002/07/owl#DatatypeProperty"/>
    <owl:equivalentProperty rdf:resource="http://id.loc.gov/ontologies/bibframe/originDate"/>
    <bffi-meta:exactMatch rdf:resource="http://rdaregistry.info/Elements/w/P10219"/>
    <rdfs:subPropertyOf rdf:resource="http://urn.fi/URN:NBN:fi:schema:bffi:date"/>
    <skos:definition xml:lang="en">BIBFRAME definition: Date or date range associated with the creation of a Work.</skos:definition>
  </rdf:Description>
  <rdf:Description rdf:about="http://urn.fi/URN:NBN:fi:schema:bffi:captureOfRepresentativeExpression">
    <dct:modified>2024-11-22 (New)</dct:modified>
    <rdfs:label xml:lang="en">capture of content of representative expression</rdfs:label>
    <rdfs:label xml:lang="fi">edustavan ekspression taltiointitiedot</rdfs:label>
    <rdfs:domain rdf:nodeID="n2ee3b3232b574a15b2a1faf6555dee4fb1"/>
    <rdfs:range rdf:resource="http://urn.fi/URN:NBN:fi:schema:bffi:Capture"/>
    <rdf:type rdf:resource="http://www.w3.org/2002/07/owl#ObjectProperty"/>
    <bffi-meta:narrowMatch rdf:resource="http://rdaregistry.info/Elements/w/P10350"/>
    <bffi-meta:narrowMatch rdf:resource="http://rdaregistry.info/Elements/w/P10354"/>
    <rdfs:subPropertyOf rdf:resource="http://id.loc.gov/ontologies/bibframe/capture"/>
  </rdf:Description>
  <rdf:Description rdf:about="http://urn.fi/URN:NBN:fi:schema:bffi:dissertation">
    <dct:modified>2024-02-23 (New)</dct:modified>
    <rdfs:label xml:lang="en">dissertation information</rdfs:label>
    <rdfs:label xml:lang="fi">tieto väitöskirjasta tai muusta opinnäytteestä</rdfs:label>
    <rdfs:domain rdf:nodeID="n3fb00cccae3f45e2923b7c06d0716eb2b1"/>
    <rdfs:range rdf:resource="http://urn.fi/URN:NBN:fi:schema:bffi:Dissertation"/>
    <rdf:type rdf:resource="http://www.w3.org/2002/07/owl#ObjectProperty"/>
    <owl:equivalentProperty rdf:resource="http://id.loc.gov/ontologies/bibframe/dissertation"/>
    <bffi-meta:exactMatch rdf:resource="http://rdaregistry.info/Elements/w/P10209"/>
    <skos:definition xml:lang="en">BIBFRAME definition: Work presented as part of the formal requirements for an academic degree.</skos:definition>
  </rdf:Description>
  <rdf:Description rdf:about="http://urn.fi/URN:NBN:fi:schema:bffi:manifestationOfExpression">
    <owl:inverseOf rdf:resource="http://urn.fi/URN:NBN:fi:schema:bffi:expressionManifested"/>
    <dct:modified>2024-02-23 (New)</dct:modified>
    <rdfs:label xml:lang="en">manifestation of expression</rdfs:label>
    <rdfs:label xml:lang="fi">ekspression manifestaatio</rdfs:label>
    <rdfs:domain rdf:resource="http://urn.fi/URN:NBN:fi:schema:bffi:Expression"/>
    <rdfs:range rdf:resource="http://urn.fi/URN:NBN:fi:schema:bffi:Manifestation"/>
    <rdf:type rdf:resource="http://www.w3.org/2002/07/owl#ObjectProperty"/>
    <bffi-meta:broadMatch rdf:resource="http://id.loc.gov/ontologies/bibframe/hasInstance"/>
    <bffi-meta:exactMatch rdf:resource="http://rdaregistry.info/Elements/e/P20059"/>
    <rdfs:subPropertyOf rdf:resource="http://urn.fi/URN:NBN:fi:schema:bffi:relatedTo"/>
  </rdf:Description>
  <rdf:Description rdf:about="http://urn.fi/URN:NBN:fi:schema:bffi:SerialExpression">
    <dct:modified>2024-02-23 (New)</dct:modified>
    <rdfs:label xml:lang="en">Serial expression</rdfs:label>
    <rdfs:label xml:lang="fi">Sarjamaisesti ilmestynyt ekspressio</rdfs:label>
    <rdf:type rdf:resource="http://www.w3.org/2002/07/owl#Class"/>
    <bffi-meta:broadMatch rdf:resource="http://id.loc.gov/ontologies/bibframe/Serial"/>
    <rdfs:subClassOf rdf:resource="http://urn.fi/URN:NBN:fi:schema:bffi:Expression"/>
    <owl:disjointWith rdf:resource="http://urn.fi/URN:NBN:fi:schema:bffi:SeriesExpression"/>
  </rdf:Description>
  <rdf:Description rdf:about="http://urn.fi/URN:NBN:fi:schema:bffi:hasRepresentativeExpression">
    <dct:modified>2024-02-23 (New)</dct:modified>
    <rdfs:label xml:lang="en">representative expression</rdfs:label>
    <rdfs:label xml:lang="fi">edustava ekspressio</rdfs:label>
    <rdfs:domain rdf:resource="http://urn.fi/URN:NBN:fi:schema:bffi:Work"/>
    <rdfs:range rdf:resource="http://urn.fi/URN:NBN:fi:schema:bffi:Expression"/>
    <rdf:type rdf:resource="http://www.w3.org/2002/07/owl#ObjectProperty"/>
    <bffi-meta:broadMatch rdf:resource="http://id.loc.gov/ontologies/bibframe/hasExpression"/>
    <bffi-meta:exactMatch rdf:resource="http://rdaregistry.info/Elements/w/P10346"/>
    <rdfs:subPropertyOf rdf:resource="http://urn.fi/URN:NBN:fi:schema:bffi:relatedTo"/>
    <owl:inverseOf rdf:resource="http://urn.fi/URN:NBN:fi:schema:bffi:representativeExpressionOf"/>
  </rdf:Description>
  <rdf:Description rdf:about="http://urn.fi/URN:NBN:fi:schema:bffi:degree">
    <dct:modified>2024-02-23 (New)</dct:modified>
    <rdfs:label xml:lang="en">degree</rdfs:label>
    <rdfs:label xml:lang="fi">oppiarvo</rdfs:label>
    <rdfs:domain rdf:resource="http://urn.fi/URN:NBN:fi:schema:bffi:Dissertation"/>
    <rdfs:range rdf:resource="http://urn.fi/URN:NBN:fi:schema:bffi:Degree"/>
    <rdf:type rdf:resource="http://www.w3.org/2002/07/owl#ObjectProperty"/>
    <bffi-meta:closeMatch rdf:resource="http://id.loc.gov/ontologies/bibframe/degree"/>
    <bffi-meta:closeMatch rdf:resource="http://rdaregistry.info/Elements/w/P10077"/>
  </rdf:Description>
  <rdf:Description rdf:about="http://urn.fi/URN:NBN:fi:schema:bffi-meta:">
    <dct:description xml:lang="en">Additional linking properties supporting LKD data model.</dct:description>
    <dct:description xml:lang="fi">Sisältää lisäominaisuuksia LKD-tietomallin linkityksiä varten.</dct:description>
    <rdf:type rdf:resource="http://www.w3.org/2002/07/owl#Ontology"/>
    <dct:title xml:lang="fi">Metadataontologia LKD-tietomallin tueksi</dct:title>
    <dct:title xml:lang="en">Metadata ontology for LKD data model</dct:title>
    <dct:license rdf:resource="http://creativecommons.org/publicdomain/zero/1.0/"/>
  </rdf:Description>
  <rdf:Description rdf:nodeID="n5cd48ce8767a480c888bcf43bfaa8780b1">
    <rdf:type rdf:resource="http://www.w3.org/2002/07/owl#Class"/>
    <owl:unionOf rdf:nodeID="n5cd48ce8767a480c888bcf43bfaa8780b2"/>
  </rdf:Description>
  <rdf:Description rdf:nodeID="ne27b8fc3c7014a3a99b60051d23322e1b3">
    <rdf:first rdf:resource="http://urn.fi/URN:NBN:fi:schema:bffi:Expression"/>
    <rdf:rest rdf:nodeID="ne27b8fc3c7014a3a99b60051d23322e1b4"/>
  </rdf:Description>
  <rdf:Description rdf:about="http://urn.fi/URN:NBN:fi:schema:bffi:cartographicProjection">
    <dct:modified>2024-04-16 (New)</dct:modified>
    <rdfs:label xml:lang="en">cartographic projection</rdfs:label>
    <rdfs:label xml:lang="fi">karttaprojektio</rdfs:label>
    <rdfs:domain rdf:resource="http://urn.fi/URN:NBN:fi:schema:bffi:CartographyExpression"/>
    <rdfs:range rdf:resource="http://urn.fi/URN:NBN:fi:schema:bffi:Projection"/>
    <rdf:type rdf:resource="http://www.w3.org/2002/07/owl#ObjectProperty"/>
    <bffi-meta:exactMatch rdf:resource="http://rdaregistry.info/Elements/e/P20216"/>
    <rdfs:subPropertyOf rdf:resource="http://id.loc.gov/ontologies/bibframe/projection"/>
  </rdf:Description>
  <rdf:Description rdf:about="http://urn.fi/URN:NBN:fi:schema:bffi:Illustration">
    <dct:modified>2024-02-23 (New)</dct:modified>
    <rdfs:label xml:lang="en">Illustrative content</rdfs:label>
    <rdfs:label xml:lang="fi">Kuvasisältö</rdfs:label>
    <bffi-meta:relatedValueVocabulary rdf:resource="http://urn.fi/URN:NBN:fi:au:mts:m439"/>
    <rdf:type rdf:resource="http://www.w3.org/2002/07/owl#Class"/>
    <owl:equivalentClass rdf:resource="http://id.loc.gov/ontologies/bibframe/Illustration"/>
    <rdfs:seeAlso rdf:resource="http://rdaregistry.info/termList/IllusContent/"/>
    <skos:definition xml:lang="en">BIBFRAME definition: Information about content intended to illustrate a resource</skos:definition>
  </rdf:Description>
  <rdf:Description rdf:about="http://urn.fi/URN:NBN:fi:schema:bffi:bookFormat">
    <dct:modified>2024-09-16 (New)</dct:modified>
    <rdfs:label xml:lang="en">book format</rdfs:label>
    <rdfs:label xml:lang="fi">bibliografinen koko</rdfs:label>
    <rdfs:domain rdf:resource="http://urn.fi/URN:NBN:fi:schema:bffi:Manifestation"/>
    <rdfs:range rdf:resource="http://urn.fi/URN:NBN:fi:schema:bffi:BookFormat"/>
    <rdf:type rdf:resource="http://www.w3.org/2002/07/owl#ObjectProperty"/>
    <owl:equivalentProperty rdf:resource="http://id.loc.gov/ontologies/bibframe/bookFormat"/>
    <bffi-meta:exactMatch rdf:resource="http://rdaregistry.info/Elements/m/P30197"/>
    <skos:definition xml:lang="en">BIBFRAME definition: Result of folding a printed sheet to form a gathering of leaves.</skos:definition>
  </rdf:Description>
  <rdf:Description rdf:about="http://urn.fi/URN:NBN:fi:schema:bffi:AppliesTo">
    <dct:modified>2025-01-02 (New)</dct:modified>
    <rdfs:label xml:lang="en">Applies to</rdfs:label>
    <rdfs:label xml:lang="fi">Aineiston osa</rdfs:label>
    <rdf:type rdf:resource="http://www.w3.org/2002/07/owl#Class"/>
    <owl:equivalentClass rdf:resource="http://id.loc.gov/ontologies/bflc/AppliesTo"/>
    <skos:definition xml:lang="en">BFLC definition: The component of a resource to which a characteristic applies.</skos:definition>
  </rdf:Description>
  <rdf:Description rdf:about="http://urn.fi/URN:NBN:fi:schema:bffi:intendedAudience">
    <dct:modified>2024-02-23 (New)</dct:modified>
    <rdfs:label xml:lang="en">intended audience</rdfs:label>
    <rdfs:label xml:lang="fi">kohderyhmä</rdfs:label>
    <rdfs:domain rdf:nodeID="n0a20977f4ff64f88b13306bf2d732ab6b1"/>
    <rdfs:range rdf:resource="http://urn.fi/URN:NBN:fi:schema:bffi:IntendedAudience"/>
    <rdf:type rdf:resource="http://www.w3.org/2002/07/owl#ObjectProperty"/>
    <owl:equivalentProperty rdf:resource="http://id.loc.gov/ontologies/bibframe/intendedAudience"/>
    <bffi-meta:narrowMatch rdf:resource="http://rdaregistry.info/Elements/e/P20322"/>
    <bffi-meta:narrowMatch rdf:resource="http://rdaregistry.info/Elements/m/P30305"/>
    <skos:definition xml:lang="en">BIBFRAME definition: Information that identifies the specific audience or intellectual level for which the content of the resource is considered appropriate.</skos:definition>
  </rdf:Description>
  <rdf:Description rdf:nodeID="n90e14c5f212f40b8a6a776d86788ca21b4">
    <rdf:first rdf:resource="http://urn.fi/URN:NBN:fi:schema:bffi:Manifestation"/>
    <rdf:rest rdf:nodeID="n90e14c5f212f40b8a6a776d86788ca21b5"/>
  </rdf:Description>
  <rdf:Description rdf:about="http://urn.fi/URN:NBN:fi:schema:bffi:GovernmentPubType">
    <dct:modified>2025-01-02 (New)</dct:modified>
    <rdfs:label xml:lang="en">Government Publication Type</rdfs:label>
    <rdfs:label xml:lang="fi">Virallisjulkaisun tyyppi</rdfs:label>
    <rdf:type rdf:resource="http://www.w3.org/2002/07/owl#Class"/>
    <owl:equivalentClass rdf:resource="http://id.loc.gov/ontologies/bflc/GovernmentPubType"/>
    <skos:definition xml:lang="en">BFLC definition: Information recording that the resource is published or produced by or for an international, national, state, provincial, or local government agency, or by any subdivision of such a body.</skos:definition>
  </rdf:Description>
  <rdf:Description rdf:about="http://urn.fi/URN:NBN:fi:schema:bffi-meta:closeMatch">
    <dct:modified>2024-02-23 (New)</dct:modified>
    <rdfs:subPropertyOf rdf:resource="http://purl.org/dc/terms/relation"/>
    <skos:definition xml:lang="fi">Merkitykseltään lähes vastaava luokka tai ominaisuus jossakin toisessa ontologiassa tai skeemassa.</skos:definition>
    <skos:definition xml:lang="en">Semantically similar class or property in another ontology or scheme.</skos:definition>
    <rdfs:label xml:lang="fi">lähes vastaava</rdfs:label>
    <rdfs:label xml:lang="en">close match</rdfs:label>
    <rdf:type rdf:resource="http://www.w3.org/2002/07/owl#AnnotationProperty"/>
    <owl:equivalentProperty rdf:resource="https://www.svde.org/ontology/closeMatch"/>
  </rdf:Description>
  <rdf:Description rdf:about="http://urn.fi/URN:NBN:fi:schema:bffi:representativeExpressionOf">
    <owl:inverseOf rdf:resource="http://urn.fi/URN:NBN:fi:schema:bffi:hasRepresentativeExpression"/>
    <dct:modified>2024-02-23 (New)</dct:modified>
    <rdfs:label xml:lang="en">is representative expression of</rdfs:label>
    <rdfs:label xml:lang="fi">edustava ekspressio teokselle</rdfs:label>
    <rdfs:domain rdf:resource="http://urn.fi/URN:NBN:fi:schema:bffi:Expression"/>
    <rdfs:range rdf:resource="http://urn.fi/URN:NBN:fi:schema:bffi:Work"/>
    <rdf:type rdf:resource="http://www.w3.org/2002/07/owl#ObjectProperty"/>
    <bffi-meta:broadMatch rdf:resource="http://id.loc.gov/ontologies/bibframe/expressionOf"/>
    <bffi-meta:exactMatch rdf:resource="http://rdaregistry.info/Elements/e/P20325"/>
    <rdfs:subPropertyOf rdf:resource="http://urn.fi/URN:NBN:fi:schema:bffi:relatedTo"/>
  </rdf:Description>
  <rdf:Description rdf:about="http://urn.fi/URN:NBN:fi:schema:bffi:BookFormat">
    <dct:modified>2024-09-16 (New)</dct:modified>
    <rdfs:label xml:lang="en">Book format</rdfs:label>
    <rdfs:label xml:lang="fi">Bibliografinen koko</rdfs:label>
    <bffi-meta:relatedValueVocabulary rdf:resource="http://urn.fi/URN:NBN:fi:au:mts:m50"/>
    <rdf:type rdf:resource="http://www.w3.org/2002/07/owl#Class"/>
    <owl:equivalentClass rdf:resource="http://id.loc.gov/ontologies/bibframe/BookFormat"/>
    <rdfs:seeAlso rdf:resource="http://rdaregistry.info/termList/bookFormat/"/>
    <skos:definition xml:lang="en">BIBFRAME definition: Result of folding a printed sheet to form a gathering of leaves</skos:definition>
  </rdf:Description>
  <rdf:Description rdf:about="http://urn.fi/URN:NBN:fi:schema:bffi:Arrangement">
    <dct:modified>2024-11-22 (New)</dct:modified>
    <rdfs:label xml:lang="en">Arrangement</rdfs:label>
    <rdfs:label xml:lang="fi">Sovitus</rdfs:label>
    <rdf:type rdf:resource="http://www.w3.org/2002/07/owl#Class"/>
    <owl:equivalentClass rdf:resource="http://id.loc.gov/ontologies/bibframe/Arrangement"/>
    <rdfs:seeAlso rdf:resource="http://rdaregistry.info/termList/RDATerms/1008"/>
    <rdfs:subClassOf rdf:resource="http://urn.fi/URN:NBN:fi:schema:bffi:Expression"/>
    <skos:definition xml:lang="en">BIBFRAME definition: Resource that represents an arrangement of another resource</skos:definition>
  </rdf:Description>
  <rdf:Description rdf:about="http://urn.fi/URN:NBN:fi:schema:bffi:musicFormat">
    <dct:modified>2024-02-23 (New)</dct:modified>
    <rdfs:label xml:lang="en">format of notated music</rdfs:label>
    <rdfs:label xml:lang="fi">nuottiaineiston muoto</rdfs:label>
    <rdfs:domain rdf:resource="http://urn.fi/URN:NBN:fi:schema:bffi:NotatedMusic"/>
    <rdfs:range rdf:resource="http://urn.fi/URN:NBN:fi:schema:bffi:MusicFormat"/>
    <rdf:type rdf:resource="http://www.w3.org/2002/07/owl#ObjectProperty"/>
    <owl:equivalentProperty rdf:resource="http://id.loc.gov/ontologies/bibframe/musicFormat"/>
    <bffi-meta:exactMatch rdf:resource="http://rdaregistry.info/Elements/e/P20209"/>
    <skos:definition xml:lang="en">BIBFRAME definition: Layout for content of a resource that is presented in the form of musical notation, such as full score, condensed score, vocal score, etc.</skos:definition>
  </rdf:Description>
  <rdf:Description rdf:about="http://urn.fi/URN:NBN:fi:schema:bffi:PlayingSpeed">
    <dct:modified>2024-11-22 (New)</dct:modified>
    <rdfs:label xml:lang="en">Playing speed</rdfs:label>
    <rdfs:label xml:lang="fi">Toistonopeus</rdfs:label>
    <bffi-meta:relatedValueVocabulary rdf:resource="http://urn.fi/URN:NBN:fi:au:mts:m4"/>
    <rdf:type rdf:resource="http://www.w3.org/2002/07/owl#Class"/>
    <owl:equivalentClass rdf:resource="http://id.loc.gov/ontologies/bibframe/PlayingSpeed"/>
    <rdfs:subClassOf rdf:resource="http://urn.fi/URN:NBN:fi:schema:bffi:SoundCharacteristic"/>
    <skos:definition xml:lang="en">BIBFRAME definition: Speed at which an audio carrier must be operated to produce the sound intended, e.g., 78 rpm, 19 cm/s</skos:definition>
  </rdf:Description>
  <rdf:Description rdf:about="http://urn.fi/URN:NBN:fi:schema:bffi:SeriesWork">
    <owl:disjointWith rdf:resource="http://urn.fi/URN:NBN:fi:schema:bffi:SerialWork"/>
    <dct:modified>2024-02-23 (New)</dct:modified>
    <rdfs:label xml:lang="en">Series work</rdfs:label>
    <rdfs:label xml:lang="fi">Moniosainen teos</rdfs:label>
    <rdf:type rdf:resource="http://www.w3.org/2002/07/owl#Class"/>
    <bffi-meta:broadMatch rdf:resource="http://id.loc.gov/ontologies/bibframe/Series"/>
    <rdfs:subClassOf rdf:resource="http://urn.fi/URN:NBN:fi:schema:bffi:Work"/>
  </rdf:Description>
  <rdf:Description rdf:about="http://urn.fi/URN:NBN:fi:schema:bffi:productionMethod">
    <dct:modified>2024-09-16 (New)</dct:modified>
    <rdfs:label xml:lang="en">production method</rdfs:label>
    <rdfs:label xml:lang="fi">valmistusmenetelmä</rdfs:label>
    <rdfs:domain rdf:resource="http://urn.fi/URN:NBN:fi:schema:bffi:Manifestation"/>
    <rdfs:range rdf:resource="http://urn.fi/URN:NBN:fi:schema:bffi:ProductionMethod"/>
    <rdf:type rdf:resource="http://www.w3.org/2002/07/owl#ObjectProperty"/>
    <owl:equivalentProperty rdf:resource="http://id.loc.gov/ontologies/bibframe/productionMethod"/>
    <bffi-meta:exactMatch rdf:resource="http://rdaregistry.info/Elements/m/P30187"/>
    <skos:definition xml:lang="en">BIBFRAME definition: Process used to produce a resource.</skos:definition>
  </rdf:Description>
  <rdf:Description rdf:about="http://urn.fi/URN:NBN:fi:schema:bffi:aggregatedBy">
    <dct:modified>2024-09-16 (New)</dct:modified>
    <rdfs:label xml:lang="en">aggregated by</rdfs:label>
    <rdfs:label xml:lang="fi">aggregoija</rdfs:label>
    <rdfs:domain rdf:resource="http://urn.fi/URN:NBN:fi:schema:bffi:Expression"/>
    <rdfs:range rdf:resource="http://urn.fi/URN:NBN:fi:schema:bffi:AggregatingExpression"/>
    <rdf:type rdf:resource="http://www.w3.org/2002/07/owl#ObjectProperty"/>
    <bffi-meta:broadMatch rdf:resource="http://id.loc.gov/ontologies/bibframe/relatedTo"/>
    <bffi-meta:exactMatch rdf:resource="http://rdaregistry.info/Elements/e/P20320"/>
    <rdfs:subPropertyOf rdf:resource="http://urn.fi/URN:NBN:fi:schema:bffi:relatedTo"/>
    <owl:inverseOf rdf:resource="http://urn.fi/URN:NBN:fi:schema:bffi:aggregates"/>
  </rdf:Description>
  <rdf:Description rdf:about="http://urn.fi/URN:NBN:fi:schema:bffi:ClassificationUdc">
    <dct:modified>2024-02-23 (New)</dct:modified>
    <rdfs:label xml:lang="en">UDC Classification</rdfs:label>
    <rdfs:label xml:lang="fi">UDK-luokitus</rdfs:label>
    <rdf:type rdf:resource="http://www.w3.org/2002/07/owl#Class"/>
    <owl:equivalentClass rdf:resource="http://id.loc.gov/ontologies/bibframe/ClassificationUdc"/>
    <rdfs:subClassOf rdf:resource="http://urn.fi/URN:NBN:fi:schema:bffi:Classification"/>
    <skos:definition xml:lang="en">BIBFRAME definition: Universal Decimal Classification number used for subject access</skos:definition>
  </rdf:Description>
  <rdf:Description rdf:nodeID="n26a54bed81f14ec98f0dfd0d8091fc72b4">
    <rdf:first rdf:resource="http://urn.fi/URN:NBN:fi:schema:bffi:Manifestation"/>
    <rdf:rest rdf:resource="http://www.w3.org/1999/02/22-rdf-syntax-ns#nil"/>
  </rdf:Description>
  <rdf:Description rdf:about="http://urn.fi/URN:NBN:fi:schema:bffi:PlaybackCharacteristic">
    <dct:modified>2024-11-22 (New)</dct:modified>
    <rdfs:label xml:lang="en">Special playback characteristics</rdfs:label>
    <rdfs:label xml:lang="fi">Äänentoiston erityisominaisuudet</rdfs:label>
    <bffi-meta:relatedValueVocabulary rdf:resource="http://urn.fi/URN:NBN:fi:au:mts:m315"/>
    <rdf:type rdf:resource="http://www.w3.org/2002/07/owl#Class"/>
    <owl:equivalentClass rdf:resource="http://id.loc.gov/ontologies/bibframe/PlaybackCharacteristic"/>
    <rdfs:seeAlso rdf:resource="http://rdaregistry.info/termList/specPlayback/"/>
    <rdfs:subClassOf rdf:resource="http://urn.fi/URN:NBN:fi:schema:bffi:SoundCharacteristic"/>
    <skos:definition xml:lang="en">BIBFRAME definition: Equalization system, noise reduction system, etc., used in making an audio recording, e.g., CCIR standard, CX encoded, Dolby</skos:definition>
  </rdf:Description>
  <rdf:Description rdf:about="http://urn.fi/URN:NBN:fi:schema:bffi:Media">
    <dct:modified>2024-02-23 (New)</dct:modified>
    <rdfs:label xml:lang="en">Media type</rdfs:label>
    <rdfs:label xml:lang="fi">Mediatyyppi</rdfs:label>
    <bffi-meta:relatedValueVocabulary rdf:resource="http://urn.fi/URN:NBN:fi:au:mts:m777"/>
    <rdf:type rdf:resource="http://www.w3.org/2002/07/owl#Class"/>
    <owl:equivalentClass rdf:resource="http://id.loc.gov/ontologies/bibframe/Media"/>
    <rdfs:seeAlso rdf:resource="http://rdaregistry.info/termList/RDAMediaType/"/>
    <skos:definition xml:lang="en">BIBFRAME definition: Categorization reflecting the general type of intermediation device required to view, play, run, etc., the content of a resource</skos:definition>
  </rdf:Description>
  <rdf:Description rdf:about="http://urn.fi/URN:NBN:fi:schema:bffi:expressionManifested">
    <dct:modified>2024-02-23 (New)</dct:modified>
    <rdfs:label xml:lang="en">expression manifested</rdfs:label>
    <rdfs:label xml:lang="fi">manifestaatioon sisältyvä ekspressio</rdfs:label>
    <rdfs:domain rdf:resource="http://urn.fi/URN:NBN:fi:schema:bffi:Manifestation"/>
    <rdfs:range rdf:resource="http://urn.fi/URN:NBN:fi:schema:bffi:Expression"/>
    <rdf:type rdf:resource="http://www.w3.org/2002/07/owl#ObjectProperty"/>
    <bffi-meta:broadMatch rdf:resource="http://id.loc.gov/ontologies/bibframe/instanceOf"/>
    <bffi-meta:exactMatch rdf:resource="http://rdaregistry.info/Elements/m/P30139"/>
    <rdfs:subPropertyOf rdf:resource="http://urn.fi/URN:NBN:fi:schema:bffi:relatedTo"/>
    <owl:inverseOf rdf:resource="http://urn.fi/URN:NBN:fi:schema:bffi:manifestationOfExpression"/>
  </rdf:Description>
  <rdf:Description rdf:about="http://urn.fi/URN:NBN:fi:schema:bffi:physicalLocation">
    <dct:modified>2024-04-16 (New)</dct:modified>
    <rdfs:label xml:lang="en">location of item</rdfs:label>
    <rdfs:label xml:lang="fi">kappaleen sijainti</rdfs:label>
    <rdfs:domain rdf:resource="http://urn.fi/URN:NBN:fi:schema:bffi:Item"/>
    <rdfs:range rdf:resource="http://www.w3.org/2000/01/rdf-schema#Literal"/>
    <rdf:type rdf:resource="http://www.w3.org/2002/07/owl#DatatypeProperty"/>
    <owl:equivalentProperty rdf:resource="http://id.loc.gov/ontologies/bibframe/physicalLocation"/>
    <bffi-meta:exactMatch rdf:resource="http://rdaregistry.info/Elements/i/P40162"/>
    <skos:definition xml:lang="en">BIBFRAME definition: Location in the holding agency where the item is shelved or stored.</skos:definition>
  </rdf:Description>
  <rdf:Description rdf:about="http://urn.fi/URN:NBN:fi:schema:bffi:date">
    <dct:modified>2024-02-23 (New)</dct:modified>
    <rdfs:label xml:lang="en">date</rdfs:label>
    <rdfs:label xml:lang="fi">ajankohta</rdfs:label>
    <rdfs:domain rdf:resource="http://www.w3.org/2000/01/rdf-schema#Resource"/>
    <rdfs:range rdf:resource="http://www.w3.org/2000/01/rdf-schema#Literal"/>
    <rdf:type rdf:resource="http://www.w3.org/2002/07/owl#DatatypeProperty"/>
    <bffi-meta:closeMatch rdf:resource="http://rdaregistry.info/Elements/x/P00011"/>
    <rdfs:subPropertyOf rdf:resource="http://id.loc.gov/ontologies/bibframe/date"/>
  </rdf:Description>
  <rdf:Description rdf:nodeID="nbf7db4a78c624ed983d40041e8bb0721b2">
    <rdf:first rdf:resource="http://urn.fi/URN:NBN:fi:schema:bffi:Manifestation"/>
    <rdf:rest rdf:nodeID="nbf7db4a78c624ed983d40041e8bb0721b3"/>
  </rdf:Description>
  <rdf:Description rdf:about="http://urn.fi/URN:NBN:fi:schema:bffi:MusicWork">
    <dct:modified>2024-11-22 (New)</dct:modified>
    <rdfs:label xml:lang="en">Music work</rdfs:label>
    <rdfs:label xml:lang="fi">Musiikkiteos</rdfs:label>
    <rdf:type rdf:resource="http://www.w3.org/2002/07/owl#Class"/>
    <bffi-meta:closeMatch rdf:resource="http://id.loc.gov/ontologies/bibframe/NotatedMusic"/>
    <bffi-meta:closeMatch rdf:resource="http://id.loc.gov/ontologies/bibframe/MusicAudio"/>
    <rdfs:subClassOf rdf:resource="http://urn.fi/URN:NBN:fi:schema:bffi:Work"/>
  </rdf:Description>
  <rdf:Description rdf:about="http://urn.fi/URN:NBN:fi:schema:bffi:copyrightRegistration">
    <dct:modified>2024-02-23 (New)</dct:modified>
    <rdfs:label xml:lang="en">copyright registration information</rdfs:label>
    <rdfs:label xml:lang="fi">tekijänoikeus- tai vapaakappaletiedot</rdfs:label>
    <rdfs:domain rdf:resource="http://urn.fi/URN:NBN:fi:schema:bffi:Manifestation"/>
    <rdfs:range rdf:resource="http://urn.fi/URN:NBN:fi:schema:bffi:CopyrightRegistration"/>
    <rdf:type rdf:resource="http://www.w3.org/2002/07/owl#ObjectProperty"/>
    <owl:equivalentProperty rdf:resource="http://id.loc.gov/ontologies/bibframe/copyrightRegistration"/>
    <skos:definition xml:lang="en">BIBFRAME definition: Copyright and Legal Deposit registration information</skos:definition>
  </rdf:Description>
  <rdf:Description rdf:about="http://urn.fi/URN:NBN:fi:schema:bffi-meta:exactMatch">
    <dct:modified>2024-02-23 (New)</dct:modified>
    <rdf:type rdf:resource="http://www.w3.org/2002/07/owl#AnnotationProperty"/>
    <skos:definition xml:lang="en">Semantically exactly matching class or property in another ontology or scheme.</skos:definition>
    <skos:definition xml:lang="fi">Merkitykseltään vastaava luokka tai ominaisuus jossakin toisessa ontologiassa tai skeemassa.</skos:definition>
    <rdfs:subPropertyOf rdf:resource="http://purl.org/dc/terms/relation"/>
    <rdfs:label xml:lang="fi">tarkasti vastaava</rdfs:label>
    <rdfs:label xml:lang="en">exact match</rdfs:label>
  </rdf:Description>
  <rdf:Description rdf:about="http://urn.fi/URN:NBN:fi:schema:bffi:appliesTo">
    <dct:modified>2025-01-02 (New)</dct:modified>
    <rdfs:label xml:lang="en">applies to</rdfs:label>
    <rdfs:label xml:lang="fi">aineiston osa</rdfs:label>
    <rdfs:domain rdf:nodeID="n68bca78492684c1398be6f6d4f77765db1"/>
    <rdfs:range rdf:resource="http://urn.fi/URN:NBN:fi:schema:bffi:AppliesTo"/>
    <rdf:type rdf:resource="http://www.w3.org/2002/07/owl#ObjectProperty"/>
    <owl:equivalentProperty rdf:resource="http://id.loc.gov/ontologies/bflc/appliesTo"/>
    <skos:definition xml:lang="en">BFLC definition: The component of a resource to which a characteristic applies.</skos:definition>
  </rdf:Description>
  <rdf:Description rdf:about="http://urn.fi/URN:NBN:fi:schema:bffi:place">
    <dct:modified>2024-02-23 (New)</dct:modified>
    <rdfs:label xml:lang="en">place</rdfs:label>
    <rdfs:label xml:lang="fi">paikka</rdfs:label>
    <rdfs:domain rdf:resource="http://www.w3.org/2000/01/rdf-schema#Resource"/>
    <rdfs:range rdf:resource="http://urn.fi/URN:NBN:fi:schema:bffi:Place"/>
    <rdf:type rdf:resource="http://www.w3.org/2002/07/owl#ObjectProperty"/>
    <rdfs:subPropertyOf rdf:resource="http://id.loc.gov/ontologies/bibframe/place"/>
  </rdf:Description>
  <rdf:Description rdf:about="http://urn.fi/URN:NBN:fi:schema:bffi:simplePlace">
    <dct:modified>2024-02-23 (New)</dct:modified>
    <rdfs:label xml:lang="en">place</rdfs:label>
    <rdfs:label xml:lang="fi">auktorisoimaton paikka</rdfs:label>
    <rdfs:domain rdf:resource="http://urn.fi/URN:NBN:fi:schema:bffi:ProvisionActivity"/>
    <rdfs:range rdf:resource="http://www.w3.org/2000/01/rdf-schema#Literal"/>
    <rdf:type rdf:resource="http://www.w3.org/2002/07/owl#DatatypeProperty"/>
    <owl:equivalentProperty rdf:resource="http://id.loc.gov/ontologies/bflc/simplePlace"/>
    <bffi-meta:closeMatch rdf:resource="http://rdaregistry.info/Elements/p/P70001"/>
    <skos:definition xml:lang="en">BFLC definition: Location of publication, distribution, manufacture or production as transcribed from the resource</skos:definition>
  </rdf:Description>
  <rdf:Description rdf:about="http://urn.fi/URN:NBN:fi:schema:bffi:editionStatement">
    <dct:modified>2024-02-23 (New)</dct:modified>
    <rdfs:label xml:lang="en">edition statement</rdfs:label>
    <rdfs:label xml:lang="fi">painosmerkintö</rdfs:label>
    <rdfs:domain rdf:resource="http://urn.fi/URN:NBN:fi:schema:bffi:Manifestation"/>
    <rdfs:range rdf:resource="http://www.w3.org/2000/01/rdf-schema#Literal"/>
    <rdf:type rdf:resource="http://www.w3.org/2002/07/owl#DatatypeProperty"/>
    <owl:equivalentProperty rdf:resource="http://id.loc.gov/ontologies/bibframe/editionStatement"/>
    <bffi-meta:narrowMatch rdf:resource="http://rdaregistry.info/Elements/m/P30121"/>
    <bffi-meta:narrowMatch rdf:resource="http://rdaregistry.info/Elements/m/P30115"/>
    <bffi-meta:narrowMatch rdf:resource="http://rdaregistry.info/Elements/m/P30118"/>
    <bffi-meta:narrowMatch rdf:resource="http://rdaregistry.info/Elements/m/P30112"/>
    <skos:definition xml:lang="en">BIBFRAME definition: Information identifying the edition or version of the resource and associated statements of responsibility for the edition; usually transcribed.</skos:definition>
  </rdf:Description>
  <rdf:Description rdf:about="http://urn.fi/URN:NBN:fi:schema:bffi:holding">
    <dct:modified>2024-04-16 (New)</dct:modified>
    <rdfs:label xml:lang="en">holding</rdfs:label>
    <rdfs:label xml:lang="fi">kokoelman kappale</rdfs:label>
    <rdfs:domain rdf:resource="http://urn.fi/URN:NBN:fi:schema:bffi:CollectionManifestation"/>
    <rdfs:range rdf:resource="http://urn.fi/URN:NBN:fi:schema:bffi:Item"/>
    <rdf:type rdf:resource="http://www.w3.org/2002/07/owl#ObjectProperty"/>
    <bffi-meta:broadMatch rdf:resource="http://id.loc.gov/ontologies/bibframe/hasItem"/>
    <bffi-meta:exactMatch rdf:resource="http://rdaregistry.info/Elements/m/P30460"/>
    <rdfs:subPropertyOf rdf:resource="http://urn.fi/URN:NBN:fi:schema:bffi:relatedTo"/>
  </rdf:Description>
  <rdf:Description rdf:about="http://urn.fi/URN:NBN:fi:schema:bffi:appliedMaterial">
    <dct:modified>2024-09-16 (New)</dct:modified>
    <rdfs:label xml:lang="en">applied material</rdfs:label>
    <rdfs:label xml:lang="fi">päällimateriaali</rdfs:label>
    <rdfs:domain rdf:resource="http://urn.fi/URN:NBN:fi:schema:bffi:Manifestation"/>
    <rdfs:range rdf:resource="http://urn.fi/URN:NBN:fi:schema:bffi:AppliedMaterial"/>
    <rdf:type rdf:resource="http://www.w3.org/2002/07/owl#ObjectProperty"/>
    <owl:equivalentProperty rdf:resource="http://id.loc.gov/ontologies/bibframe/appliedMaterial"/>
    <bffi-meta:exactMatch rdf:resource="http://rdaregistry.info/Elements/m/P30084"/>
    <rdfs:subPropertyOf rdf:resource="http://urn.fi/URN:NBN:fi:schema:bffi:material"/>
    <skos:definition xml:lang="en">BIBFRAME definition: Physical or chemical substance applied to a base material of a resource.</skos:definition>
  </rdf:Description>
  <rdf:Description rdf:about="http://urn.fi/URN:NBN:fi:schema:bffi:extentOfRepresentativeExpression">
    <dct:modified>2024-04-16 (New)</dct:modified>
    <rdfs:label xml:lang="en">extent of representative expression</rdfs:label>
    <rdfs:label xml:lang="fi">edustavan ekspression laajuus</rdfs:label>
    <rdfs:domain rdf:resource="http://urn.fi/URN:NBN:fi:schema:bffi:Work"/>
    <rdfs:range rdf:resource="http://urn.fi/URN:NBN:fi:schema:bffi:Extent"/>
    <rdf:type rdf:resource="http://www.w3.org/2002/07/owl#ObjectProperty"/>
    <bffi-meta:closeMatch rdf:resource="http://id.loc.gov/ontologies/bibframe/extent"/>
    <bffi-meta:exactMatch rdf:resource="http://rdaregistry.info/Elements/w/P10352"/>
  </rdf:Description>
  <rdf:Description rdf:about="http://urn.fi/URN:NBN:fi:schema:bffi:preferredCitation">
    <dct:modified>2024-02-23 (New)</dct:modified>
    <rdfs:label xml:lang="en">preferred citation</rdfs:label>
    <rdfs:label xml:lang="fi">ensisijainen viittausmuoto</rdfs:label>
    <rdfs:domain rdf:resource="http://urn.fi/URN:NBN:fi:schema:bffi:Manifestation"/>
    <rdfs:range rdf:resource="http://www.w3.org/2000/01/rdf-schema#Literal"/>
    <rdf:type rdf:resource="http://www.w3.org/2002/07/owl#DatatypeProperty"/>
    <owl:equivalentProperty rdf:resource="http://id.loc.gov/ontologies/bibframe/preferredCitation"/>
    <bffi-meta:exactMatch rdf:resource="http://rdaregistry.info/Elements/m/P30005"/>
    <skos:definition xml:lang="en">BIBFRAME definition: Citation to the resource preferred by its custodian of the resource.</skos:definition>
  </rdf:Description>
  <rdf:Description rdf:about="http://urn.fi/URN:NBN:fi:schema:bffi:VideoFormat">
    <dct:modified>2024-11-22 (New)</dct:modified>
    <rdfs:label xml:lang="en">Video format</rdfs:label>
    <rdfs:label xml:lang="fi">Videoformaatti</rdfs:label>
    <bffi-meta:relatedValueVocabulary rdf:resource="http://urn.fi/URN:NBN:fi:au:mts:m191"/>
    <rdf:type rdf:resource="http://www.w3.org/2002/07/owl#Class"/>
    <owl:equivalentClass rdf:resource="http://id.loc.gov/ontologies/bibframe/VideoFormat"/>
    <rdfs:seeAlso rdf:resource="http://rdaregistry.info/termList/videoFormat/"/>
    <rdfs:subClassOf rdf:resource="http://urn.fi/URN:NBN:fi:schema:bffi:VideoCharacteristic"/>
    <skos:definition xml:lang="en">BIBFRAME definition: Standard, etc., used to encode the analog video content of a resource, e.g., Beta, 8mm</skos:definition>
  </rdf:Description>
  <rdf:Description rdf:about="http://urn.fi/URN:NBN:fi:schema:bffi:issuance">
    <dct:modified>2024-02-23 (New)</dct:modified>
    <rdfs:label xml:lang="en">mode of issuance</rdfs:label>
    <rdfs:label xml:lang="fi">julkaisutapa</rdfs:label>
    <rdfs:domain rdf:resource="http://urn.fi/URN:NBN:fi:schema:bffi:Manifestation"/>
    <rdfs:range rdf:resource="http://urn.fi/URN:NBN:fi:schema:bffi:Issuance"/>
    <rdf:type rdf:resource="http://www.w3.org/2002/07/owl#ObjectProperty"/>
    <bffi-meta:broadMatch rdf:resource="http://id.loc.gov/ontologies/bibframe/issuance"/>
    <bffi-meta:exactMatch rdf:resource="http://rdaregistry.info/Elements/m/P30003"/>
  </rdf:Description>
  <rdf:Description rdf:about="http://urn.fi/URN:NBN:fi:schema:bffi:contentAccessibility">
    <dct:modified>2024-09-16 (New)</dct:modified>
    <rdfs:label xml:lang="en">content accessibility information</rdfs:label>
    <rdfs:label xml:lang="fi">saavutettavuussisältö</rdfs:label>
    <rdfs:domain rdf:resource="http://urn.fi/URN:NBN:fi:schema:bffi:Manifestation"/>
    <rdfs:range rdf:resource="http://urn.fi/URN:NBN:fi:schema:bffi:ContentAccessibility"/>
    <rdf:type rdf:resource="http://www.w3.org/2002/07/owl#ObjectProperty"/>
    <owl:equivalentProperty rdf:resource="http://id.loc.gov/ontologies/bibframe/contentAccessibility"/>
    <bffi-meta:exactMatch rdf:resource="http://rdaregistry.info/Elements/m/P30452"/>
    <skos:definition xml:lang="en">BIBFRAME definition: Information that assists those with a sensory impairment for greater understanding of content, e.g., captions.</skos:definition>
  </rdf:Description>
  <rdf:Description rdf:about="http://urn.fi/URN:NBN:fi:schema:bffi:mount">
    <dct:modified>2024-09-16 (New)</dct:modified>
    <rdfs:label xml:lang="en">mount material or object</rdfs:label>
    <rdfs:label xml:lang="fi">tukimateriaali</rdfs:label>
    <rdfs:domain rdf:resource="http://urn.fi/URN:NBN:fi:schema:bffi:Manifestation"/>
    <rdfs:range rdf:resource="http://urn.fi/URN:NBN:fi:schema:bffi:Mount"/>
    <rdf:type rdf:resource="http://www.w3.org/2002/07/owl#ObjectProperty"/>
    <owl:equivalentProperty rdf:resource="http://id.loc.gov/ontologies/bibframe/mount"/>
    <bffi-meta:exactMatch rdf:resource="http://rdaregistry.info/Elements/m/P30186"/>
    <skos:definition xml:lang="en">BIBFRAME definition: Physical material or object used for the support or backing to which the base material of a resource has been attached.</skos:definition>
  </rdf:Description>
  <rdf:Description rdf:about="http://urn.fi/URN:NBN:fi:schema:bffi:Binding">
    <dct:modified>2024-09-16 (New)</dct:modified>
    <rdfs:label xml:lang="en">Binding</rdfs:label>
    <rdfs:label xml:lang="fi">Sidostyyppi</rdfs:label>
    <bffi-meta:relatedValueVocabulary rdf:resource="http://urn.fi/URN:NBN:fi:au:mts:m4402"/>
    <rdf:type rdf:resource="http://www.w3.org/2002/07/owl#Class"/>
    <owl:equivalentClass rdf:resource="http://id.loc.gov/ontologies/bibframe/Binding"/>
    <rdfs:seeAlso rdf:resource="http://rdaregistry.info/termList/RDATypeOfBinding/"/>
    <skos:definition xml:lang="en">BIBFRAME definition: Information about methods used to bind a published or unpublished resource, or other binding information</skos:definition>
  </rdf:Description>
  <rdf:Description rdf:about="http://urn.fi/URN:NBN:fi:schema:bffi:UsePolicy">
    <dct:modified>2024-02-23 (New)</dct:modified>
    <rdfs:label xml:lang="en">Use policy</rdfs:label>
    <rdfs:label xml:lang="fi">Käyttöehdot</rdfs:label>
    <rdf:type rdf:resource="http://www.w3.org/2002/07/owl#Class"/>
    <owl:equivalentClass rdf:resource="http://id.loc.gov/ontologies/bibframe/UsePolicy"/>
    <rdfs:subClassOf rdf:resource="http://urn.fi/URN:NBN:fi:schema:bffi:UsageAndAccessPolicy"/>
    <skos:definition xml:lang="en">BIBFRAME definition: Usage limitations placed on a resource with respect to reproduction, publication, exhibition, etc.</skos:definition>
  </rdf:Description>
  <rdf:Description rdf:about="http://urn.fi/URN:NBN:fi:schema:bffi:generation">
    <dct:modified>2024-09-16 (New)</dct:modified>
    <rdfs:label xml:lang="en">generation</rdfs:label>
    <rdfs:label xml:lang="fi">sukupolvi</rdfs:label>
    <rdfs:domain rdf:resource="http://urn.fi/URN:NBN:fi:schema:bffi:Manifestation"/>
    <rdfs:range rdf:resource="http://urn.fi/URN:NBN:fi:schema:bffi:Generation"/>
    <rdf:type rdf:resource="http://www.w3.org/2002/07/owl#ObjectProperty"/>
    <owl:equivalentProperty rdf:resource="http://id.loc.gov/ontologies/bibframe/generation"/>
    <skos:definition xml:lang="en">BIBFRAME definition: Relationship between an original carrier and the carrier of a reproduction made from the original.</skos:definition>
  </rdf:Description>
  <rdf:Description rdf:about="http://urn.fi/URN:NBN:fi:schema:bffi:Source">
    <dct:modified>2024-02-23 (New)</dct:modified>
    <rdfs:label xml:lang="en">Source</rdfs:label>
    <rdfs:label xml:lang="fi">Lähde</rdfs:label>
    <rdf:type rdf:resource="http://www.w3.org/2002/07/owl#Class"/>
    <owl:equivalentClass rdf:resource="http://id.loc.gov/ontologies/bibframe/Source"/>
    <skos:definition xml:lang="en">BIBFRAME definition: Resource from which value or label came or was derived</skos:definition>
  </rdf:Description>
  <rdf:Description rdf:about="http://urn.fi/URN:NBN:fi:schema:bffi:baseMaterial">
    <dct:modified>2024-09-16 (New)</dct:modified>
    <rdfs:label xml:lang="en">base material</rdfs:label>
    <rdfs:label xml:lang="fi">pohjamateriaali</rdfs:label>
    <rdfs:domain rdf:nodeID="nbf7db4a78c624ed983d40041e8bb0721b1"/>
    <rdfs:range rdf:resource="http://urn.fi/URN:NBN:fi:schema:bffi:BaseMaterial"/>
    <rdf:type rdf:resource="http://www.w3.org/2002/07/owl#ObjectProperty"/>
    <owl:equivalentProperty rdf:resource="http://id.loc.gov/ontologies/bibframe/baseMaterial"/>
    <bffi-meta:exactMatch rdf:resource="http://rdaregistry.info/Elements/m/P30208"/>
    <rdfs:subPropertyOf rdf:resource="http://urn.fi/URN:NBN:fi:schema:bffi:material"/>
    <skos:definition xml:lang="en">BIBFRAME definition: Underlying physical material of a resource.</skos:definition>
  </rdf:Description>
  <rdf:Description rdf:about="http://urn.fi/URN:NBN:fi:schema:bffi:ClassificationLcc">
    <dct:modified>2024-06-19 (New)</dct:modified>
    <rdfs:label xml:lang="en">LCC classification</rdfs:label>
    <rdfs:label xml:lang="fi">Library of Congress -luokitus</rdfs:label>
    <rdf:type rdf:resource="http://www.w3.org/2002/07/owl#Class"/>
    <owl:equivalentClass rdf:resource="http://id.loc.gov/ontologies/bibframe/ClassificationLcc"/>
    <rdfs:subClassOf rdf:resource="http://urn.fi/URN:NBN:fi:schema:bffi:Classification"/>
    <skos:definition xml:lang="en">BIBFRAME definition: Library of Congress Classification number used for subject access</skos:definition>
  </rdf:Description>
  <rdf:Description rdf:about="http://urn.fi/URN:NBN:fi:schema:bffi:NonMusicAudioWork">
    <dct:modified>2024-02-23 (New)</dct:modified>
    <rdfs:label xml:lang="en">Non-music audio work</rdfs:label>
    <rdfs:label xml:lang="fi">Musiikiton ääniteos</rdfs:label>
    <rdf:type rdf:resource="http://www.w3.org/2002/07/owl#Class"/>
    <bffi-meta:broadMatch rdf:resource="http://id.loc.gov/ontologies/bibframe/NonMusicAudio"/>
    <bffi-meta:broadMatch rdf:resource="http://rdaregistry.info/Elements/c/C10001"/>
    <rdfs:subClassOf rdf:resource="http://urn.fi/URN:NBN:fi:schema:bffi:Work"/>
  </rdf:Description>
  <rdf:Description rdf:about="http://urn.fi/URN:NBN:fi:schema:bffi:Note">
    <dct:modified>2024-02-23 (New)</dct:modified>
    <rdfs:label xml:lang="en">Note</rdfs:label>
    <rdfs:label xml:lang="fi">Huomautus</rdfs:label>
    <rdf:type rdf:resource="http://www.w3.org/2002/07/owl#Class"/>
    <owl:equivalentClass rdf:resource="http://id.loc.gov/ontologies/bibframe/Note"/>
    <skos:definition xml:lang="en">BIBFRAME definition: Information, usually in textual form, on attributes of a resource or some aspect of a resource</skos:definition>
  </rdf:Description>
  <rdf:Description rdf:about="http://urn.fi/URN:NBN:fi:schema:bffi:relationship">
    <dct:modified>2024-09-16 (New)</dct:modified>
    <rdfs:label xml:lang="en">relationship</rdfs:label>
    <rdfs:label xml:lang="fi">suhdetyyppi</rdfs:label>
    <rdfs:domain rdf:resource="http://urn.fi/URN:NBN:fi:schema:bffi:Relation"/>
    <rdfs:range rdf:resource="http://urn.fi/URN:NBN:fi:schema:bffi:Relationship"/>
    <rdf:type rdf:resource="http://www.w3.org/2002/07/owl#ObjectProperty"/>
    <owl:equivalentProperty rdf:resource="http://id.loc.gov/ontologies/bibframe/relationship"/>
    <skos:definition xml:lang="en">BIBFRAME definition: Type of relationship between resources</skos:definition>
  </rdf:Description>
  <rdf:Description rdf:about="http://urn.fi/URN:NBN:fi:schema:bffi:governmentPubType">
    <dct:modified>2025-01-02 (New)</dct:modified>
    <rdfs:label xml:lang="en">government publication type</rdfs:label>
    <rdfs:label xml:lang="fi">virallisjulkaisun tyyppi</rdfs:label>
    <rdfs:domain rdf:nodeID="n71c313d9323b40c29dadafedf28680eeb1"/>
    <rdfs:range rdf:resource="http://urn.fi/URN:NBN:fi:schema:bffi:GovernmentPubType"/>
    <rdf:type rdf:resource="http://www.w3.org/2002/07/owl#ObjectProperty"/>
    <owl:equivalentProperty rdf:resource="http://id.loc.gov/ontologies/bflc/governmentPubType"/>
    <skos:definition xml:lang="en">BFLC definition: Information recording that the resource is published or produced by or for an international, national, state, provincial, or local government agency, or by any subdivision of such a body.</skos:definition>
  </rdf:Description>
  <rdf:Description rdf:about="http://urn.fi/URN:NBN:fi:schema:bffi:MovingImageExpression">
    <dct:modified>2024-02-23 (New)</dct:modified>
    <rdfs:label xml:lang="en">Moving image expression</rdfs:label>
    <rdfs:label xml:lang="fi">Liikkuvan kuvan ekspressio</rdfs:label>
    <rdf:type rdf:resource="http://www.w3.org/2002/07/owl#Class"/>
    <bffi-meta:broadMatch rdf:resource="http://id.loc.gov/ontologies/bibframe/MovingImage"/>
    <rdfs:subClassOf rdf:resource="http://urn.fi/URN:NBN:fi:schema:bffi:Expression"/>
    <owl:disjointWith rdf:resource="http://urn.fi/URN:NBN:fi:schema:bffi:MovingImageWork"/>
  </rdf:Description>
  <rdf:Description rdf:about="http://urn.fi/URN:NBN:fi:schema:bffi:legalDate">
    <dct:modified>2024-11-22 (New)</dct:modified>
    <rdfs:label xml:lang="en">date of legal work</rdfs:label>
    <rdfs:label xml:lang="fi">allekirjoittamisen tai voimaantulon ajankohta</rdfs:label>
    <rdfs:domain rdf:resource="http://urn.fi/URN:NBN:fi:schema:bffi:Work"/>
    <rdfs:range rdf:resource="http://www.w3.org/2000/01/rdf-schema#Literal"/>
    <rdf:type rdf:resource="http://www.w3.org/2002/07/owl#DatatypeProperty"/>
    <owl:equivalentProperty rdf:resource="http://id.loc.gov/ontologies/bibframe/legalDate"/>
    <bffi-meta:broadMatch rdf:resource="http://rdaregistry.info/Elements/w/P10219"/>
    <rdfs:subPropertyOf rdf:resource="http://urn.fi/URN:NBN:fi:schema:bffi:date"/>
    <skos:definition xml:lang="en">BIBFRAME definition: Date of legal work, or promulgation of a law, or signing of a treaty.</skos:definition>
  </rdf:Description>
  <rdf:Description rdf:about="http://urn.fi/URN:NBN:fi:schema:bffi:descriptionModifier">
    <dct:modified>2024-06-19 (New)</dct:modified>
    <rdfs:label xml:lang="en">description modifier</rdfs:label>
    <rdfs:label xml:lang="fi">muokkaava taho</rdfs:label>
    <rdfs:domain rdf:resource="http://urn.fi/URN:NBN:fi:schema:bffi:AdminMetadata"/>
    <rdfs:range rdf:resource="http://urn.fi/URN:NBN:fi:schema:bffi:Agent"/>
    <rdf:type rdf:resource="http://www.w3.org/2002/07/owl#ObjectProperty"/>
    <owl:equivalentProperty rdf:resource="http://id.loc.gov/ontologies/bibframe/descriptionModifier"/>
    <bffi-meta:exactMatch rdf:resource="http://rdaregistry.info/Elements/i/P40093"/>
    <skos:definition xml:lang="en">BIBFRAME definition: Agency that modified a description</skos:definition>
  </rdf:Description>
  <rdf:Description rdf:about="http://urn.fi/URN:NBN:fi:schema:bffi:MonographExpression">
    <dct:modified>2024-02-23 (New)</dct:modified>
    <rdfs:label xml:lang="en">Monograph expression</rdfs:label>
    <rdfs:label xml:lang="fi">Monografiaekspressio</rdfs:label>
    <rdf:type rdf:resource="http://www.w3.org/2002/07/owl#Class"/>
    <bffi-meta:broadMatch rdf:resource="http://id.loc.gov/ontologies/bibframe/Monograph"/>
    <rdfs:subClassOf rdf:resource="http://urn.fi/URN:NBN:fi:schema:bffi:Expression"/>
  </rdf:Description>
  <rdf:Description rdf:about="http://urn.fi/URN:NBN:fi:schema:bffi:extensionPlan">
    <dct:modified>2024-04-16 (New)</dct:modified>
    <rdfs:label xml:lang="en">extension plan</rdfs:label>
    <rdfs:label xml:lang="fi">laajennussuunnitelma</rdfs:label>
    <rdfs:domain rdf:resource="http://urn.fi/URN:NBN:fi:schema:bffi:Work"/>
    <rdfs:range rdf:resource="http://urn.fi/URN:NBN:fi:schema:bffi:ExtensionPlan"/>
    <rdf:type rdf:resource="http://www.w3.org/2002/07/owl#ObjectProperty"/>
    <bffi-meta:broadMatch rdf:resource="http://id.loc.gov/ontologies/bibframe/issuance"/>
    <bffi-meta:exactMatch rdf:resource="http://rdaregistry.info/Elements/w/P10365"/>
  </rdf:Description>
  <rdf:Description rdf:about="http://urn.fi/URN:NBN:fi:schema:bffi:lastIssueChronology">
    <dct:modified>2024-02-23 (New)</dct:modified>
    <rdfs:label xml:lang="en">last chronological designation of sequence</rdfs:label>
    <rdfs:label xml:lang="fi">numerointijakson viimeinen aikamäärite</rdfs:label>
    <rdfs:domain rdf:resource="http://urn.fi/URN:NBN:fi:schema:bffi:Manifestation"/>
    <rdfs:range rdf:resource="http://www.w3.org/2000/01/rdf-schema#Literal"/>
    <rdf:type rdf:resource="http://www.w3.org/2002/07/owl#DatatypeProperty"/>
    <bffi-meta:broadMatch rdf:resource="http://id.loc.gov/ontologies/bibframe/lastIssue"/>
    <bffi-meta:exactMatch rdf:resource="http://rdaregistry.info/Elements/m/P30150"/>
  </rdf:Description>
  <rdf:Description rdf:nodeID="n71c313d9323b40c29dadafedf28680eeb2">
    <rdf:first rdf:resource="http://urn.fi/URN:NBN:fi:schema:bffi:Work"/>
    <rdf:rest rdf:nodeID="n71c313d9323b40c29dadafedf28680eeb3"/>
  </rdf:Description>
  <rdf:Description rdf:nodeID="n7333c8087d784d019f2d09a8a88483c5b1">
    <rdf:type rdf:resource="http://www.w3.org/2002/07/owl#Class"/>
    <owl:unionOf rdf:nodeID="n7333c8087d784d019f2d09a8a88483c5b2"/>
  </rdf:Description>
  <rdf:Description rdf:about="http://urn.fi/URN:NBN:fi:schema:bffi:notation">
    <dct:modified>2024-02-23 (New)</dct:modified>
    <rdfs:label xml:lang="en">notation system</rdfs:label>
    <rdfs:label xml:lang="fi">notaatio</rdfs:label>
    <rdfs:domain rdf:resource="http://urn.fi/URN:NBN:fi:schema:bffi:Expression"/>
    <rdfs:range rdf:resource="http://urn.fi/URN:NBN:fi:schema:bffi:Notation"/>
    <rdf:type rdf:resource="http://www.w3.org/2002/07/owl#ObjectProperty"/>
    <owl:equivalentProperty rdf:resource="http://id.loc.gov/ontologies/bibframe/notation"/>
    <bffi-meta:narrowMatch rdf:resource="http://rdaregistry.info/Elements/e/P20061"/>
    <bffi-meta:narrowMatch rdf:resource="http://rdaregistry.info/Elements/e/P20062"/>
    <bffi-meta:narrowMatch rdf:resource="http://rdaregistry.info/Elements/e/P20063"/>
    <bffi-meta:narrowMatch rdf:resource="http://rdaregistry.info/Elements/e/P20064"/>
    <skos:definition xml:lang="en">BIBFRAME definition: Alphabet, script, or symbol system used to convey the content of the resource, including specialized scripts, typefaces, tactile notation, movement notation, and musical notation.</skos:definition>
  </rdf:Description>
  <rdf:Description rdf:about="http://urn.fi/URN:NBN:fi:schema:bffi:role">
    <dct:modified>2024-02-23 (New)</dct:modified>
    <rdfs:label xml:lang="en">contributor role</rdfs:label>
    <rdfs:label xml:lang="fi">rooli</rdfs:label>
    <rdfs:domain rdf:resource="http://urn.fi/URN:NBN:fi:schema:bffi:Contribution"/>
    <rdfs:range rdf:resource="http://urn.fi/URN:NBN:fi:schema:bffi:Role"/>
    <rdf:type rdf:resource="http://www.w3.org/2002/07/owl#ObjectProperty"/>
    <owl:equivalentProperty rdf:resource="http://id.loc.gov/ontologies/bibframe/role"/>
    <bffi-meta:broadMatch rdf:resource="http://rdaregistry.info/Elements/a/P50304"/>
    <skos:definition xml:lang="en">BIBFRAME definition: Function provided by a contributor, e.g., author, illustrator, etc.</skos:definition>
  </rdf:Description>
  <rdf:Description rdf:about="http://urn.fi/URN:NBN:fi:schema:bffi:MixedMaterial">
    <dct:modified>2024-02-23 (New)</dct:modified>
    <rdfs:label xml:lang="en">Mixed material</rdfs:label>
    <rdfs:label xml:lang="fi">Kooste</rdfs:label>
    <rdf:type rdf:resource="http://www.w3.org/2002/07/owl#Class"/>
    <owl:equivalentClass rdf:resource="http://id.loc.gov/ontologies/bibframe/MixedMaterial"/>
    <rdfs:subClassOf rdf:resource="http://urn.fi/URN:NBN:fi:schema:bffi:Expression"/>
    <skos:definition xml:lang="en">BIBFRAME definition: Resource comprised of multiple types which is not driven by software, e.g. an archival collection of text, photographs and sound recordings</skos:definition>
  </rdf:Description>
  <rdf:Description rdf:about="http://urn.fi/URN:NBN:fi:schema:bffi:AccessPolicy">
    <dct:modified>2024-02-23 (New)</dct:modified>
    <rdfs:label xml:lang="en">Access policy</rdfs:label>
    <rdfs:label xml:lang="fi">Pääsyrajoitus</rdfs:label>
    <rdf:type rdf:resource="http://www.w3.org/2002/07/owl#Class"/>
    <owl:equivalentClass rdf:resource="http://id.loc.gov/ontologies/bibframe/AccessPolicy"/>
    <rdfs:subClassOf rdf:resource="http://urn.fi/URN:NBN:fi:schema:bffi:UsageAndAccessPolicy"/>
    <skos:definition xml:lang="en">BIBFRAME definition: Access restrictions and allowances regarding access to a resource, e.g., lending policy, access restrictions, embargos</skos:definition>
  </rdf:Description>
  <rdf:Description rdf:about="http://urn.fi/URN:NBN:fi:schema:bffi:durationOfRepresentativeExpression">
    <dct:modified>2024-11-22 (New)</dct:modified>
    <rdfs:label xml:lang="en">duration of representative expression</rdfs:label>
    <rdfs:label xml:lang="fi">edustavan ekspression kesto</rdfs:label>
    <rdfs:domain rdf:nodeID="n7b5ca739c46d4a329e0fe2325c944dbcb1"/>
    <rdfs:range rdf:resource="http://www.w3.org/2000/01/rdf-schema#Literal"/>
    <rdf:type rdf:resource="http://www.w3.org/2002/07/owl#DatatypeProperty"/>
    <bffi-meta:closeMatch rdf:resource="http://id.loc.gov/ontologies/bibframe/duration"/>
    <bffi-meta:exactMatch rdf:resource="http://rdaregistry.info/Elements/w/P10351"/>
  </rdf:Description>
  <rdf:Description rdf:about="http://urn.fi/URN:NBN:fi:schema:bffi:geographicCoverage">
    <dct:modified>2025-01-02 (New)</dct:modified>
    <rdfs:label xml:lang="en">geographic coverage</rdfs:label>
    <rdfs:label xml:lang="fi">maantieteellinen kattavuus</rdfs:label>
    <rdfs:domain rdf:resource="http://urn.fi/URN:NBN:fi:schema:bffi:Work"/>
    <rdfs:range rdf:resource="http://urn.fi/URN:NBN:fi:schema:bffi:GeographicCoverage"/>
    <rdf:type rdf:resource="http://www.w3.org/2002/07/owl#ObjectProperty"/>
    <owl:equivalentProperty rdf:resource="http://id.loc.gov/ontologies/bibframe/geographicCoverage"/>
    <bffi-meta:closeMatch rdf:resource="http://rdaregistry.info/Elements/w/P10216"/>
    <skos:definition xml:lang="en">BIBFRAME definition: Geographic coverage of the content of the resource.</skos:definition>
  </rdf:Description>
  <rdf:Description rdf:about="http://urn.fi/URN:NBN:fi:schema:bffi:coordinates">
    <dct:modified>2024-02-23 (New)</dct:modified>
    <rdfs:label xml:lang="en">cartographic coordinates</rdfs:label>
    <rdfs:label xml:lang="fi">koordinaatit</rdfs:label>
    <rdfs:domain rdf:resource="http://urn.fi/URN:NBN:fi:schema:bffi:Cartographic"/>
    <rdfs:range rdf:resource="http://www.w3.org/2000/01/rdf-schema#Literal"/>
    <rdf:type rdf:resource="http://www.w3.org/2002/07/owl#DatatypeProperty"/>
    <owl:equivalentProperty rdf:resource="http://id.loc.gov/ontologies/bibframe/coordinates"/>
    <bffi-meta:exactMatch rdf:resource="http://rdaregistry.info/Elements/w/P10081"/>
    <skos:definition xml:lang="en">BIBFRAME definition: Mathematical system for identifying the area covered by the cartographic content of a resource, expressed either by means of longitude and latitude on the surface of planets or by the angles of right ascension and declination for celestial cartographic content.</skos:definition>
  </rdf:Description>
  <rdf:Description rdf:about="http://urn.fi/URN:NBN:fi:schema:bffi:coverArt">
    <dct:modified>2024-02-23 (New)</dct:modified>
    <rdfs:label xml:lang="en">cover art</rdfs:label>
    <rdfs:label xml:lang="fi">kansikuva</rdfs:label>
    <rdfs:domain rdf:resource="http://urn.fi/URN:NBN:fi:schema:bffi:Manifestation"/>
    <rdfs:range rdf:resource="http://urn.fi/URN:NBN:fi:schema:bffi:CoverArt"/>
    <rdf:type rdf:resource="http://www.w3.org/2002/07/owl#ObjectProperty"/>
    <owl:equivalentProperty rdf:resource="http://id.loc.gov/ontologies/bibframe/coverArt"/>
    <skos:definition xml:lang="en">BIBFRAME definition: Cover art image of a resource.</skos:definition>
  </rdf:Description>
  <rdf:Description rdf:about="http://urn.fi/URN:NBN:fi:schema:bffi:creditsPerformer">
    <dct:modified>2024-06-19 (New)</dct:modified>
    <rdfs:label xml:lang="en">participant or performer credits</rdfs:label>
    <rdfs:label xml:lang="fi">huomautus osallistujista tai esittäjistä</rdfs:label>
    <rdfs:domain rdf:resource="http://urn.fi/URN:NBN:fi:schema:bffi:Manifestation"/>
    <rdfs:range rdf:resource="http://www.w3.org/2000/01/rdf-schema#Literal"/>
    <rdf:type rdf:resource="http://www.w3.org/2002/07/owl#DatatypeProperty"/>
    <bffi-meta:broadMatch rdf:resource="http://id.loc.gov/ontologies/bibframe/credits"/>
    <bffi-meta:broadMatch rdf:resource="http://rdaregistry.info/Elements/m/P30057"/>
    <rdfs:subPropertyOf rdf:resource="http://urn.fi/URN:NBN:fi:schema:bffi:credits"/>
  </rdf:Description>
  <rdf:Description rdf:about="http://urn.fi/URN:NBN:fi:schema:bffi:AgeLimit">
    <dct:modified>2025-01-02 (New)</dct:modified>
    <rdfs:label xml:lang="en">Age limit</rdfs:label>
    <rdfs:label xml:lang="fi">Ikäraja</rdfs:label>
    <rdf:type rdf:resource="http://www.w3.org/2002/07/owl#Class"/>
    <bffi-meta:broadMatch rdf:resource="http://id.loc.gov/ontologies/bibframe/AccessPolicy"/>
    <bffi-meta:broadMatch rdf:resource="http://rdaregistry.info/Elements/m/P30145"/>
    <skos:definition xml:lang="en">Statutory age limits for access to resources.</skos:definition>
    <rdfs:subClassOf rdf:resource="http://urn.fi/URN:NBN:fi:schema:bffi:AccessPolicy"/>
  </rdf:Description>
  <rdf:Description rdf:about="http://urn.fi/URN:NBN:fi:schema:bffi:hasItem">
    <dct:modified>2024-02-23 (New)</dct:modified>
    <rdfs:label xml:lang="en">exemplar of manifestation</rdfs:label>
    <rdfs:label xml:lang="fi">manifestaation kappale</rdfs:label>
    <rdfs:domain rdf:resource="http://urn.fi/URN:NBN:fi:schema:bffi:Manifestation"/>
    <rdfs:range rdf:resource="http://urn.fi/URN:NBN:fi:schema:bffi:Item"/>
    <rdf:type rdf:resource="http://www.w3.org/2002/07/owl#ObjectProperty"/>
    <owl:equivalentProperty rdf:resource="http://id.loc.gov/ontologies/bibframe/hasItem"/>
    <bffi-meta:exactMatch rdf:resource="http://rdaregistry.info/Elements/m/P30103"/>
    <rdfs:subPropertyOf rdf:resource="http://urn.fi/URN:NBN:fi:schema:bffi:relatedTo"/>
    <owl:inverseOf rdf:resource="http://urn.fi/URN:NBN:fi:schema:bffi:itemOf"/>
    <skos:definition xml:lang="en">BIBFRAME definition: Item which is an example of the described Instance</skos:definition>
  </rdf:Description>
  <rdf:Description rdf:about="http://urn.fi/URN:NBN:fi:schema:bffi:Role">
    <dct:modified>2024-02-23 (New)</dct:modified>
    <rdfs:label xml:lang="en">Role</rdfs:label>
    <rdfs:label xml:lang="fi">Rooli</rdfs:label>
    <bffi-meta:relatedValueVocabulary rdf:resource="http://urn.fi/URN:NBN:fi:au:mts:m34"/>
    <bffi-meta:relatedValueVocabulary rdf:resource="http://urn.fi/URN:NBN:fi:au:mts:m153"/>
    <bffi-meta:relatedValueVocabulary rdf:resource="http://urn.fi/URN:NBN:fi:au:mts:m491"/>
    <bffi-meta:relatedValueVocabulary rdf:resource="http://urn.fi/URN:NBN:fi:au:mts:m1157"/>
    <rdf:type rdf:resource="http://www.w3.org/2002/07/owl#Class"/>
    <owl:equivalentClass rdf:resource="http://id.loc.gov/ontologies/bibframe/Role"/>
    <skos:definition xml:lang="en">BIBFRAME definition: Function played or provided by a contributor, e.g., author or illustrator</skos:definition>
  </rdf:Description>
  <rdf:Description rdf:about="http://urn.fi/URN:NBN:fi:schema:bffi:table">
    <dct:modified>2024-06-19 (New)</dct:modified>
    <rdfs:label xml:lang="en">classification table identification</rdfs:label>
    <rdfs:label xml:lang="fi">luokkataulun tunniste</rdfs:label>
    <rdfs:domain rdf:resource="http://urn.fi/URN:NBN:fi:schema:bffi:Classification"/>
    <rdfs:range rdf:resource="http://www.w3.org/2000/01/rdf-schema#Literal"/>
    <rdf:type rdf:resource="http://www.w3.org/2002/07/owl#DatatypeProperty"/>
    <owl:equivalentProperty rdf:resource="http://id.loc.gov/ontologies/bibframe/table"/>
    <skos:definition xml:lang="en">BIBFRAME definition: Number of the table from which the classification number in a subdivision entry is taken, e.g., a DDC table.</skos:definition>
  </rdf:Description>
  <rdf:Description rdf:about="http://urn.fi/URN:NBN:fi:schema:bffi:descriptionLanguage">
    <dct:modified>2024-06-19 (New)</dct:modified>
    <rdfs:label xml:lang="en">description language</rdfs:label>
    <rdfs:label xml:lang="fi">kuvailukieli</rdfs:label>
    <rdfs:domain rdf:resource="http://urn.fi/URN:NBN:fi:schema:bffi:AdminMetadata"/>
    <rdfs:range rdf:resource="http://urn.fi/URN:NBN:fi:schema:bffi:Language"/>
    <rdf:type rdf:resource="http://www.w3.org/2002/07/owl#ObjectProperty"/>
    <owl:equivalentProperty rdf:resource="http://id.loc.gov/ontologies/bibframe/descriptionLanguage"/>
    <skos:definition xml:lang="en">BIBFRAME definition: Language used for the metadata</skos:definition>
  </rdf:Description>
  <rdf:Description rdf:about="http://urn.fi/URN:NBN:fi:schema:bffi:Work">
    <owl:disjointWith rdf:resource="http://urn.fi/URN:NBN:fi:schema:bffi:Expression"/>
    <dct:modified>2024-02-23 (New)</dct:modified>
    <rdfs:label xml:lang="en">Work</rdfs:label>
    <rdfs:label xml:lang="fi">Teos</rdfs:label>
    <rdf:type rdf:resource="http://www.w3.org/2002/07/owl#Class"/>
    <bffi-meta:broadMatch rdf:resource="http://id.loc.gov/ontologies/bibframe/Work"/>
    <bffi-meta:broadMatch rdf:resource="http://rdaregistry.info/Elements/c/C10001"/>
    <rdfs:subClassOf rdf:resource="http://urn.fi/URN:NBN:fi:schema:bffi:BibframeWork"/>
  </rdf:Description>
  <rdf:Description rdf:about="http://urn.fi/URN:NBN:fi:schema:bffi:digitalCharacteristic">
    <dct:modified>2024-04-16 (New)</dct:modified>
    <rdfs:label xml:lang="en">digital characteristic</rdfs:label>
    <rdfs:label xml:lang="fi">digitaalisen tiedoston ominaisuudet</rdfs:label>
    <rdfs:domain rdf:resource="http://urn.fi/URN:NBN:fi:schema:bffi:Manifestation"/>
    <rdfs:range rdf:resource="http://urn.fi/URN:NBN:fi:schema:bffi:DigitalCharacteristic"/>
    <rdf:type rdf:resource="http://www.w3.org/2002/07/owl#ObjectProperty"/>
    <owl:equivalentProperty rdf:resource="http://id.loc.gov/ontologies/bibframe/digitalCharacteristic"/>
    <bffi-meta:exactMatch rdf:resource="http://rdaregistry.info/Elements/m/P30124"/>
    <skos:definition xml:lang="en">BIBFRAME definition: Technical specification relating to the digital encoding of text, image, audio, video, and other types of data in a resource.</skos:definition>
  </rdf:Description>
  <rdf:Description rdf:about="http://urn.fi/URN:NBN:fi:schema:bffi:musicOpusNumber">
    <dct:modified>2024-02-23 (New)</dct:modified>
    <rdfs:label xml:lang="en">music opus number</rdfs:label>
    <rdfs:label xml:lang="fi">opusnumero</rdfs:label>
    <rdfs:domain rdf:resource="http://urn.fi/URN:NBN:fi:schema:bffi:Work"/>
    <rdfs:range rdf:resource="http://www.w3.org/2000/01/rdf-schema#Literal"/>
    <rdf:type rdf:resource="http://www.w3.org/2002/07/owl#DatatypeProperty"/>
    <owl:equivalentProperty rdf:resource="http://id.loc.gov/ontologies/bibframe/musicOpusNumber"/>
    <bffi-meta:exactMatch rdf:resource="http://rdaregistry.info/Elements/w/P10333"/>
    <skos:definition xml:lang="en">BIBFRAME definition: Numeric designation of a musical work assigned by a composer, publisher, or a musicologist.</skos:definition>
  </rdf:Description>
  <rdf:Description rdf:about="http://urn.fi/URN:NBN:fi:schema:bffi:TrackConfig">
    <dct:modified>2024-11-22 (New)</dct:modified>
    <rdfs:label xml:lang="en">Track configuration</rdfs:label>
    <rdfs:label xml:lang="fi">Ääniraidan asemointi</rdfs:label>
    <bffi-meta:relatedValueVocabulary rdf:resource="http://urn.fi/URN:NBN:fi:au:mts:m1432"/>
    <rdf:type rdf:resource="http://www.w3.org/2002/07/owl#Class"/>
    <owl:equivalentClass rdf:resource="http://id.loc.gov/ontologies/bibframe/TrackConfig"/>
    <rdfs:seeAlso rdf:resource="http://rdaregistry.info/termList/trackConfig/"/>
    <rdfs:subClassOf rdf:resource="http://urn.fi/URN:NBN:fi:schema:bffi:SoundCharacteristic"/>
    <skos:definition xml:lang="en">BIBFRAME definition: Configuration of the audio track on a sound-track film, e.g., center track, edge track</skos:definition>
  </rdf:Description>
  <rdf:Description rdf:about="http://urn.fi/URN:NBN:fi:schema:bffi:Mount">
    <dct:modified>2024-09-16 (New)</dct:modified>
    <rdfs:label xml:lang="en">Mount</rdfs:label>
    <rdfs:label xml:lang="fi">Tukimateriaali</rdfs:label>
    <rdf:type rdf:resource="http://www.w3.org/2002/07/owl#Class"/>
    <owl:equivalentClass rdf:resource="http://id.loc.gov/ontologies/bibframe/Mount"/>
    <skos:definition xml:lang="en">BIBFRAME definition: Physical material or object used for the support or backing to which the base material of a resource has been attached</skos:definition>
  </rdf:Description>
  <rdf:Description rdf:about="http://urn.fi/URN:NBN:fi:schema:bffi:changeDate">
    <dct:modified>2024-06-19 (New)</dct:modified>
    <rdfs:label xml:lang="en">description change date</rdfs:label>
    <rdfs:label xml:lang="fi">kuvailun muokkausajankohta</rdfs:label>
    <rdfs:domain rdf:resource="http://urn.fi/URN:NBN:fi:schema:bffi:AdminMetadata"/>
    <rdfs:range rdf:resource="http://www.w3.org/2000/01/rdf-schema#Literal"/>
    <rdf:type rdf:resource="http://www.w3.org/2002/07/owl#DatatypeProperty"/>
    <owl:equivalentProperty rdf:resource="http://id.loc.gov/ontologies/bibframe/changeDate"/>
    <rdfs:subPropertyOf rdf:resource="http://urn.fi/URN:NBN:fi:schema:bffi:date"/>
    <skos:definition xml:lang="en">BIBFRAME definition: Date or date and time on which the metadata was modified</skos:definition>
  </rdf:Description>
  <rdf:Description rdf:about="http://urn.fi/URN:NBN:fi:schema:bffi:originPlace">
    <dct:modified>2024-02-23 (New)</dct:modified>
    <rdfs:label xml:lang="en">origin place</rdfs:label>
    <rdfs:label xml:lang="fi">teoksen alkuperään liittyvä paikka</rdfs:label>
    <rdfs:domain rdf:resource="http://urn.fi/URN:NBN:fi:schema:bffi:Work"/>
    <rdfs:range rdf:resource="http://urn.fi/URN:NBN:fi:schema:bffi:Place"/>
    <rdf:type rdf:resource="http://www.w3.org/2002/07/owl#ObjectProperty"/>
    <owl:equivalentProperty rdf:resource="http://id.loc.gov/ontologies/bibframe/originPlace"/>
    <bffi-meta:exactMatch rdf:resource="http://rdaregistry.info/Elements/w/P10218"/>
    <rdfs:subPropertyOf rdf:resource="http://urn.fi/URN:NBN:fi:schema:bffi:place"/>
    <skos:definition xml:lang="en">BIBFRAME definition: Place from which the creation of the resource originated.</skos:definition>
  </rdf:Description>
  <rdf:Description rdf:about="http://urn.fi/URN:NBN:fi:schema:bffi:NotatedMusic">
    <dct:modified>2024-02-23 (New)</dct:modified>
    <rdfs:label xml:lang="en">Notated music</rdfs:label>
    <rdfs:label xml:lang="fi">Nuottikirjoitus</rdfs:label>
    <rdf:type rdf:resource="http://www.w3.org/2002/07/owl#Class"/>
    <owl:equivalentClass rdf:resource="http://id.loc.gov/ontologies/bibframe/NotatedMusic"/>
    <rdfs:subClassOf rdf:resource="http://urn.fi/URN:NBN:fi:schema:bffi:Expression"/>
    <skos:definition xml:lang="en">BIBFRAME definition: Graphic, non-realized representations of musical works intended to be perceived visually</skos:definition>
  </rdf:Description>
  <rdf:Description rdf:about="http://urn.fi/URN:NBN:fi:schema:bffi:collectionArrangement">
    <dct:modified>2024-04-16 (New)</dct:modified>
    <rdfs:label xml:lang="en">collection organization and arrangement</rdfs:label>
    <rdfs:label xml:lang="fi">järjestämisperiaate</rdfs:label>
    <rdfs:domain rdf:resource="http://urn.fi/URN:NBN:fi:schema:bffi:CollectionWork"/>
    <rdfs:range rdf:resource="http://urn.fi/URN:NBN:fi:schema:bffi:CollectionArrangement"/>
    <rdf:type rdf:resource="http://www.w3.org/2002/07/owl#ObjectProperty"/>
    <owl:equivalentProperty rdf:resource="http://id.loc.gov/ontologies/bibframe/collectionArrangement"/>
    <bffi-meta:exactMatch rdf:resource="http://rdaregistry.info/Elements/w/P10084"/>
    <owl:inverseOf rdf:resource="http://urn.fi/URN:NBN:fi:schema:bffi:collectionArrangementOf"/>
    <skos:definition xml:lang="en">BIBFRAME definition: Information about the organization and arrangement of a collection of resources.</skos:definition>
  </rdf:Description>
  <rdf:Description rdf:about="http://urn.fi/URN:NBN:fi:schema:bffi:SoundContent">
    <dct:modified>2024-11-22 (New)</dct:modified>
    <rdfs:label xml:lang="en">Sound content</rdfs:label>
    <rdfs:label xml:lang="fi">Äänisisältö</rdfs:label>
    <bffi-meta:relatedValueVocabulary rdf:resource="http://urn.fi/URN:NBN:fi:au:mts:m2207"/>
    <rdf:type rdf:resource="http://www.w3.org/2002/07/owl#Class"/>
    <owl:equivalentClass rdf:resource="http://id.loc.gov/ontologies/bibframe/SoundContent"/>
    <rdfs:seeAlso rdf:resource="http://rdaregistry.info/termList/soundCont/"/>
    <skos:definition xml:lang="en">BIBFRAME definition: Indication of whether the production of sound is an integral part of the resource</skos:definition>
  </rdf:Description>
  <rdf:Description rdf:about="http://urn.fi/URN:NBN:fi:schema:bffi:expressionOf">
    <dct:modified>2024-02-23 (New)</dct:modified>
    <rdfs:label xml:lang="en">expression of</rdfs:label>
    <rdfs:label xml:lang="fi">ekspression toteuttama teos</rdfs:label>
    <rdfs:domain rdf:resource="http://urn.fi/URN:NBN:fi:schema:bffi:Expression"/>
    <rdfs:range rdf:resource="http://urn.fi/URN:NBN:fi:schema:bffi:Work"/>
    <rdf:type rdf:resource="http://www.w3.org/2002/07/owl#ObjectProperty"/>
    <owl:equivalentProperty rdf:resource="http://id.loc.gov/ontologies/bibframe/expressionOf"/>
    <bffi-meta:exactMatch rdf:resource="http://rdaregistry.info/Elements/e/P20231"/>
    <rdfs:subPropertyOf rdf:resource="http://urn.fi/URN:NBN:fi:schema:bffi:relatedTo"/>
    <owl:inverseOf rdf:resource="http://urn.fi/URN:NBN:fi:schema:bffi:hasExpression"/>
    <skos:definition xml:lang="en">BIBFRAME definition: Work or Hub that the described Work or Hub is an expression of; used to connect Works and/or Hubs under LRM/RDA guidelines or similar implementations</skos:definition>
  </rdf:Description>
  <rdf:Description rdf:about="http://urn.fi/URN:NBN:fi:schema:bffi:ChoreographicMedium">
    <dct:modified>2024-11-22 (New)</dct:modified>
    <rdfs:label xml:lang="en">Choreographic medium</rdfs:label>
    <rdfs:label xml:lang="fi">Koreografinen esityskokoonpano</rdfs:label>
    <rdf:type rdf:resource="http://www.w3.org/2002/07/owl#Class"/>
    <bffi-meta:closeMatch rdf:resource="http://id.loc.gov/ontologies/bibframe/MusicMedium"/>
    <skos:definition xml:lang="fi">Koreografiseen tai ei-musiikilliseen draamasisältöön osallistuvan tai osallistuvaksi tarkoitetun esittäjän tai esittäjien ryhmän tyyppi.</skos:definition>
    <skos:definition xml:lang="en">A type of performer or group of performers participating, or intended to participate, in a performance of choreographic or non-musical dramatic content.</skos:definition>
  </rdf:Description>
  <rdf:Description rdf:about="http://urn.fi/URN:NBN:fi:schema:bffi:Frequency">
    <dct:modified>2024-11-22 (New)</dct:modified>
    <rdfs:label xml:lang="en">Frequency</rdfs:label>
    <rdfs:label xml:lang="fi">Ilmestymistiheys</rdfs:label>
    <bffi-meta:relatedValueVocabulary rdf:resource="http://urn.fi/URN:NBN:fi:au:mts:m291"/>
    <rdf:type rdf:resource="http://www.w3.org/2002/07/owl#Class"/>
    <owl:equivalentClass rdf:resource="http://id.loc.gov/ontologies/bibframe/Frequency"/>
    <rdfs:seeAlso rdf:resource="http://rdaregistry.info/termList/frequency"/>
    <skos:definition xml:lang="en">BIBFRAME definition: Information about intervals at which the parts of a serially produced resource or the updates to an integrating resource are issued</skos:definition>
  </rdf:Description>
  <rdf:Description rdf:about="http://urn.fi/URN:NBN:fi:schema:bffi:genreForm">
    <dct:modified>2024-02-23 (New)</dct:modified>
    <rdfs:label xml:lang="en">category of work</rdfs:label>
    <rdfs:label xml:lang="fi">kategoria</rdfs:label>
    <rdfs:domain rdf:resource="http://urn.fi/URN:NBN:fi:schema:bffi:Work"/>
    <rdfs:range rdf:resource="http://www.w3.org/2000/01/rdf-schema#Resource"/>
    <rdf:type rdf:resource="http://www.w3.org/2002/07/owl#ObjectProperty"/>
    <owl:equivalentProperty rdf:resource="http://id.loc.gov/ontologies/bibframe/genreForm"/>
    <bffi-meta:narrowMatch rdf:resource="http://rdaregistry.info/Elements/w/P10004"/>
    <bffi-meta:narrowMatch rdf:resource="http://rdaregistry.info/Elements/e/P20331"/>
    <bffi-meta:narrowMatch rdf:resource="http://rdaregistry.info/Elements/m/P30335"/>
    <bffi-meta:narrowMatch rdf:resource="http://rdaregistry.info/Elements/i/P40096"/>
    <skos:definition xml:lang="en">BIBFRAME definition: Form category or genre to which a resource belongs</skos:definition>
  </rdf:Description>
  <rdf:Description rdf:about="http://urn.fi/URN:NBN:fi:schema:bffi:CollectionWork">
    <dct:modified>2024-02-23 (New)</dct:modified>
    <rdfs:label xml:lang="en">Collection work</rdfs:label>
    <rdfs:label xml:lang="fi">Kokoelmateos</rdfs:label>
    <rdf:type rdf:resource="http://www.w3.org/2002/07/owl#Class"/>
    <bffi-meta:broadMatch rdf:resource="http://id.loc.gov/ontologies/bibframe/Collection"/>
    <rdfs:subClassOf rdf:resource="http://urn.fi/URN:NBN:fi:schema:bffi:Work"/>
  </rdf:Description>
  <rdf:Description rdf:about="http://urn.fi/URN:NBN:fi:schema:bffi:MovementNotation">
    <dct:modified>2024-02-23 (New)</dct:modified>
    <rdfs:label xml:lang="en">Movement notation</rdfs:label>
    <rdfs:label xml:lang="fi">Liikenotaation tyyppi</rdfs:label>
    <bffi-meta:relatedValueVocabulary rdf:resource="http://urn.fi/URN:NBN:fi:au:mts:m1981"/>
    <rdf:type rdf:resource="http://www.w3.org/2002/07/owl#Class"/>
    <owl:equivalentClass rdf:resource="http://id.loc.gov/ontologies/bibframe/MovementNotation"/>
    <rdfs:seeAlso rdf:resource="https://www.rdaregistry.info/termList/noteMove/"/>
    <rdfs:subClassOf rdf:resource="http://urn.fi/URN:NBN:fi:schema:bffi:Notation"/>
    <skos:definition xml:lang="en">BIBFRAME definition: Information on the symbol system used to convey the content of a movement resource</skos:definition>
  </rdf:Description>
  <rdf:Description rdf:about="http://urn.fi/URN:NBN:fi:schema:bffi:status">
    <dct:modified>2024-02-23 (New)</dct:modified>
    <rdfs:label xml:lang="en">status</rdfs:label>
    <rdfs:label xml:lang="fi">status</rdfs:label>
    <rdfs:domain rdf:resource="http://www.w3.org/2000/01/rdf-schema#Resource"/>
    <rdfs:range rdf:resource="http://urn.fi/URN:NBN:fi:schema:bffi:Status"/>
    <rdf:type rdf:resource="http://www.w3.org/2002/07/owl#ObjectProperty"/>
    <owl:equivalentProperty rdf:resource="http://id.loc.gov/ontologies/bibframe/status"/>
    <bffi-meta:narrowMatch rdf:resource="http://rdaregistry.info/Elements/n/P80168"/>
    <skos:definition xml:lang="en">BIBFRAME definition: Designation of the validity or position of something, such as indication that the classification number is canceled or invalid, circulation availability of an item, indication of whether the identifier is canceled or invalid.</skos:definition>
  </rdf:Description>
  <rdf:Description rdf:about="http://urn.fi/URN:NBN:fi:schema:bffi:scaleDesignation">
    <dct:modified>2024-04-16 (New)</dct:modified>
    <rdfs:label xml:lang="en">scale designation</rdfs:label>
    <rdfs:label xml:lang="fi">mittakaavan määrite</rdfs:label>
    <rdfs:domain rdf:resource="http://urn.fi/URN:NBN:fi:schema:bffi:Scale"/>
    <rdfs:range rdf:resource="http://urn.fi/URN:NBN:fi:schema:bffi:ScaleDesignation"/>
    <rdf:type rdf:resource="http://www.w3.org/2002/07/owl#ObjectProperty"/>
    <bffi-meta:broadMatch rdf:resource="http://id.loc.gov/ontologies/bibframe/scale"/>
    <bffi-meta:exactMatch rdf:resource="http://rdaregistry.info/Elements/e/P20291"/>
  </rdf:Description>
  <rdf:Description rdf:about="http://urn.fi/URN:NBN:fi:schema:bffi:CartographicDataType">
    <dct:modified>2024-04-16 (New)</dct:modified>
    <rdfs:label xml:lang="en">Digital cartographic data type</rdfs:label>
    <rdfs:label xml:lang="fi">Kartografinen tietotyyppi</rdfs:label>
    <bffi-meta:relatedValueVocabulary rdf:resource="http://urn.fi/URN:NBN:fi:au:mts:m1509"/>
    <rdf:type rdf:resource="http://www.w3.org/2002/07/owl#Class"/>
    <owl:equivalentClass rdf:resource="http://id.loc.gov/ontologies/bibframe/CartographicDataType"/>
    <rdfs:seeAlso rdf:resource="http://rdaregistry.info/termList/RDACartoDT/"/>
    <rdfs:subClassOf rdf:resource="http://urn.fi/URN:NBN:fi:schema:bffi:DigitalCharacteristic"/>
    <skos:definition xml:lang="en">BIBFRAME definition: Data type for encoding of geospatial information in a cartographic resource, e.g., raster, vector, point</skos:definition>
  </rdf:Description>
  <rdf:Description rdf:about="http://urn.fi/URN:NBN:fi:schema:bffi:RecordingMedium">
    <dct:modified>2024-11-22 (New)</dct:modified>
    <rdfs:label xml:lang="en">Recording medium</rdfs:label>
    <rdfs:label xml:lang="fi">Äänen tallennusmenetelmä</rdfs:label>
    <bffi-meta:relatedValueVocabulary rdf:resource="http://urn.fi/URN:NBN:fi:au:mts:m1226"/>
    <rdf:type rdf:resource="http://www.w3.org/2002/07/owl#Class"/>
    <owl:equivalentClass rdf:resource="http://id.loc.gov/ontologies/bibframe/RecordingMedium"/>
    <rdfs:seeAlso rdf:resource="http://rdaregistry.info/termList/recMedium/"/>
    <rdfs:subClassOf rdf:resource="http://urn.fi/URN:NBN:fi:schema:bffi:SoundCharacteristic"/>
    <skos:definition xml:lang="en">BIBFRAME definition: Type of medium used to record sound on an audio carrier, e.g., magnetic, optical</skos:definition>
  </rdf:Description>
  <rdf:Description rdf:about="http://urn.fi/URN:NBN:fi:schema:bffi:sourceConsulted">
    <dct:modified>2024-02-23 (New)</dct:modified>
    <rdfs:label xml:lang="en">source consulted</rdfs:label>
    <rdfs:label xml:lang="fi">käytetty lähde</rdfs:label>
    <rdfs:domain rdf:resource="http://urn.fi/URN:NBN:fi:schema:bffi:AdminMetadata"/>
    <rdfs:range rdf:resource="http://urn.fi/URN:NBN:fi:schema:bffi:SourceConsulted"/>
    <rdf:type rdf:resource="http://www.w3.org/2002/07/owl#ObjectProperty"/>
    <bffi-meta:broadMatch rdf:resource="http://id.loc.gov/ontologies/bibframe/source"/>
    <bffi-meta:exactMatch rdf:resource="http://rdaregistry.info/Elements/w/P10406"/>
  </rdf:Description>
  <rdf:Description rdf:nodeID="n3340e60e05a148bda7f556ae223dde3ab3">
    <rdf:first rdf:resource="http://urn.fi/URN:NBN:fi:schema:bffi:Expression"/>
    <rdf:rest rdf:nodeID="n3340e60e05a148bda7f556ae223dde3ab4"/>
  </rdf:Description>
  <rdf:Description rdf:about="http://urn.fi/URN:NBN:fi:schema:bffi:dateOfRepresentativeExpression">
    <dct:modified>2025-01-02 (New)</dct:modified>
    <rdfs:label xml:lang="en">date of representative expression</rdfs:label>
    <rdfs:label xml:lang="fi">edustavan ekspression ajankohta</rdfs:label>
    <rdfs:domain rdf:resource="http://urn.fi/URN:NBN:fi:schema:bffi:Work"/>
    <rdfs:range rdf:resource="http://www.w3.org/2000/01/rdf-schema#Literal"/>
    <rdf:type rdf:resource="http://www.w3.org/2002/07/owl#DatatypeProperty"/>
    <bffi-meta:exactMatch rdf:resource="http://rdaregistry.info/Elements/w/P10398"/>
    <rdfs:subPropertyOf rdf:resource="http://id.loc.gov/ontologies/bibframe/date"/>
  </rdf:Description>
  <rdf:Description rdf:about="http://urn.fi/URN:NBN:fi:schema:bffi:carrier">
    <dct:modified>2024-02-23 (New)</dct:modified>
    <rdfs:label xml:lang="en">carrier type</rdfs:label>
    <rdfs:label xml:lang="fi">tallennetyyppi</rdfs:label>
    <rdfs:domain rdf:resource="http://urn.fi/URN:NBN:fi:schema:bffi:Manifestation"/>
    <rdfs:range rdf:resource="http://urn.fi/URN:NBN:fi:schema:bffi:Carrier"/>
    <rdf:type rdf:resource="http://www.w3.org/2002/07/owl#ObjectProperty"/>
    <bffi-meta:exactMatch rdf:resource="http://rdaregistry.info/Elements/m/P30001"/>
    <rdfs:subPropertyOf rdf:resource="http://id.loc.gov/ontologies/bibframe/carrier"/>
  </rdf:Description>
  <rdf:Description rdf:nodeID="n23d9c564949d4a53a71610ff1e9857f7b1">
    <rdf:type rdf:resource="http://www.w3.org/2002/07/owl#Class"/>
    <owl:unionOf rdf:nodeID="n23d9c564949d4a53a71610ff1e9857f7b2"/>
  </rdf:Description>
  <rdf:Description rdf:nodeID="n1e5b766c1bf94ff9812af7b852f48486b4">
    <rdf:first rdf:resource="http://urn.fi/URN:NBN:fi:schema:bffi:Manifestation"/>
    <rdf:rest rdf:nodeID="n1e5b766c1bf94ff9812af7b852f48486b5"/>
  </rdf:Description>
  <rdf:Description rdf:about="http://urn.fi/URN:NBN:fi:schema:bffi:CreatorCharacteristic">
    <dct:modified>2025-01-02 (New)</dct:modified>
    <rdfs:label xml:lang="en">Creator characteristic</rdfs:label>
    <rdfs:label xml:lang="fi">Tekijän ominaisuudet</rdfs:label>
    <rdf:type rdf:resource="http://www.w3.org/2002/07/owl#Class"/>
    <owl:equivalentClass rdf:resource="http://id.loc.gov/ontologies/bflc/CreatorCharacteristic"/>
    <skos:definition xml:lang="en">BFLC definition: Category to which the creators of the resource belong.</skos:definition>
  </rdf:Description>
  <rdf:Description rdf:about="http://urn.fi/URN:NBN:fi:schema:bffi:custodialHistory">
    <dct:modified>2024-04-16 (New)</dct:modified>
    <rdfs:label xml:lang="en">custodial history</rdfs:label>
    <rdfs:label xml:lang="fi">kappaleen omistushistoria</rdfs:label>
    <rdfs:domain rdf:resource="http://urn.fi/URN:NBN:fi:schema:bffi:Item"/>
    <rdfs:range rdf:resource="http://www.w3.org/2000/01/rdf-schema#Literal"/>
    <rdf:type rdf:resource="http://www.w3.org/2002/07/owl#DatatypeProperty"/>
    <owl:equivalentProperty rdf:resource="http://id.loc.gov/ontologies/bibframe/custodialHistory"/>
    <bffi-meta:exactMatch rdf:resource="http://rdaregistry.info/Elements/i/P40026"/>
    <skos:definition xml:lang="en">BIBFRAME definition: Information about the provenance, such as origin, ownership and custodial history (chain of custody), of a resource.</skos:definition>
  </rdf:Description>
  <rdf:Description rdf:about="http://urn.fi/URN:NBN:fi:schema:bffi:mediumOfChoreographicContentOfRepresentativeExpression">
    <dct:modified>2024-11-22 (New)</dct:modified>
    <rdfs:label xml:lang="en">medium of performance of choreographic content of representative expression</rdfs:label>
    <rdfs:label xml:lang="fi">edustavan ekspression koreografisen sisällön esityskokoonpano</rdfs:label>
    <rdfs:domain rdf:resource="http://urn.fi/URN:NBN:fi:schema:bffi:Work"/>
    <rdfs:range rdf:resource="http://urn.fi/URN:NBN:fi:schema:bffi:ChoreographicMedium"/>
    <rdf:type rdf:resource="http://www.w3.org/2002/07/owl#ObjectProperty"/>
    <bffi-meta:closeMatch rdf:resource="http://id.loc.gov/ontologies/bibframe/musicMedium"/>
    <bffi-meta:exactMatch rdf:resource="http://rdaregistry.info/Elements/w/P10603"/>
  </rdf:Description>
  <rdf:Description rdf:about="http://urn.fi/URN:NBN:fi:schema:bffi:summary">
    <dct:modified>2024-02-23 (New)</dct:modified>
    <rdfs:label xml:lang="en">summary content</rdfs:label>
    <rdfs:label xml:lang="fi">sisällön yhteenveto</rdfs:label>
    <rdfs:domain rdf:resource="http://urn.fi/URN:NBN:fi:schema:bffi:Expression"/>
    <rdfs:range rdf:resource="http://urn.fi/URN:NBN:fi:schema:bffi:Summary"/>
    <rdf:type rdf:resource="http://www.w3.org/2002/07/owl#ObjectProperty"/>
    <owl:equivalentProperty rdf:resource="http://id.loc.gov/ontologies/bibframe/summary"/>
    <skos:definition xml:lang="en">BIBFRAME definition: Summary or abstract of the resource described.</skos:definition>
  </rdf:Description>
  <rdf:Description rdf:about="http://urn.fi/URN:NBN:fi:schema:bffi:ClassificationNal">
    <dct:modified>2024-09-16 (New)</dct:modified>
    <rdfs:label xml:lang="en">NAL classification</rdfs:label>
    <rdfs:label xml:lang="fi">National Agricultural Library -luokitus</rdfs:label>
    <rdf:type rdf:resource="http://www.w3.org/2002/07/owl#Class"/>
    <owl:equivalentClass rdf:resource="http://id.loc.gov/ontologies/bibframe/ClassificationNal"/>
    <rdfs:subClassOf rdf:resource="http://urn.fi/URN:NBN:fi:schema:bffi:Classification"/>
    <skos:definition xml:lang="en">BIBFRAME definition: National Library of Agriculter number used for subject access</skos:definition>
  </rdf:Description>
  <rdf:Description rdf:about="http://urn.fi/URN:NBN:fi:schema:bffi:Resolution">
    <dct:modified>2024-11-22 (New)</dct:modified>
    <rdfs:label xml:lang="en">Resolution</rdfs:label>
    <rdfs:label xml:lang="fi">Resoluutio</rdfs:label>
    <rdf:type rdf:resource="http://www.w3.org/2002/07/owl#Class"/>
    <owl:equivalentClass rdf:resource="http://id.loc.gov/ontologies/bibframe/Resolution"/>
    <rdfs:subClassOf rdf:resource="http://urn.fi/URN:NBN:fi:schema:bffi:DigitalCharacteristic"/>
    <skos:definition xml:lang="en">BIBFRAME definition: Clarity or fineness of detail in a digital image, expressed by the measurement of the image in pixels, etc., e.g., 3.1 megapixels</skos:definition>
  </rdf:Description>
  <rdf:Description rdf:about="http://urn.fi/URN:NBN:fi:schema:bffi:Classification">
    <dct:modified>2024-02-23 (New)</dct:modified>
    <rdfs:label xml:lang="en">Classification entity</rdfs:label>
    <rdfs:label xml:lang="fi">Luokitus</rdfs:label>
    <rdf:type rdf:resource="http://www.w3.org/2002/07/owl#Class"/>
    <owl:equivalentClass rdf:resource="http://id.loc.gov/ontologies/bibframe/Classification"/>
    <bffi-meta:broadMatch rdf:resource="http://rdaregistry.info/Elements/c/C10013"/>
    <skos:definition xml:lang="en">BIBFRAME definition: System of coding and organizing materials according to their subject</skos:definition>
  </rdf:Description>
  <rdf:Description rdf:about="http://urn.fi/URN:NBN:fi:schema:bffi:identifiedBy">
    <dct:modified>2024-02-23 (New)</dct:modified>
    <rdfs:label xml:lang="en">identifier</rdfs:label>
    <rdfs:label xml:lang="fi">tunniste</rdfs:label>
    <rdfs:domain rdf:resource="http://www.w3.org/2000/01/rdf-schema#Resource"/>
    <rdfs:range rdf:resource="http://urn.fi/URN:NBN:fi:schema:bffi:Identifier"/>
    <rdf:type rdf:resource="http://www.w3.org/2002/07/owl#ObjectProperty"/>
    <owl:equivalentProperty rdf:resource="http://id.loc.gov/ontologies/bibframe/identifiedBy"/>
    <bffi-meta:narrowMatch rdf:resource="http://rdaregistry.info/Elements/w/P10002"/>
    <bffi-meta:narrowMatch rdf:resource="http://rdaregistry.info/Elements/e/P20002"/>
    <bffi-meta:narrowMatch rdf:resource="http://rdaregistry.info/Elements/m/P30004"/>
    <bffi-meta:narrowMatch rdf:resource="http://rdaregistry.info/Elements/i/P40001"/>
    <bffi-meta:narrowMatch rdf:resource="http://rdaregistry.info/Elements/t/P70018"/>
    <bffi-meta:narrowMatch rdf:resource="http://rdaregistry.info/Elements/p/P70020"/>
    <owl:inverseOf rdf:resource="http://urn.fi/URN:NBN:fi:schema:bffi:identifies"/>
    <skos:definition xml:lang="en">BIBFRAME definition: Character string associated with a resource that serves to differentiate that resource from other resources, i.e., that uniquely identifies an entity.</skos:definition>
  </rdf:Description>
  <rdf:Description rdf:about="http://urn.fi/URN:NBN:fi:schema:bffi:UsageAndAccessPolicy">
    <dct:modified>2024-02-23 (New)</dct:modified>
    <rdfs:label xml:lang="en">Use and access conditions</rdfs:label>
    <rdfs:label xml:lang="fi">Käyttö- ja pääsyrajoitukset</rdfs:label>
    <rdf:type rdf:resource="http://www.w3.org/2002/07/owl#Class"/>
    <owl:equivalentClass rdf:resource="http://id.loc.gov/ontologies/bibframe/UsageAndAccessPolicy"/>
    <skos:definition xml:lang="en">BIBFRAME definition: General statement of allowances and restrictions on access to a resource, including retention, reproduction, access, and lending</skos:definition>
  </rdf:Description>
  <rdf:Description rdf:about="http://urn.fi/URN:NBN:fi:schema:bffi:Modification">
    <dct:modified>2024-02-23 (New)</dct:modified>
    <rdfs:label xml:lang="en">Modification</rdfs:label>
    <rdfs:label xml:lang="fi">Muokkaus</rdfs:label>
    <rdf:type rdf:resource="http://www.w3.org/2002/07/owl#Class"/>
    <owl:equivalentClass rdf:resource="http://id.loc.gov/ontologies/bibframe/Modification"/>
    <rdfs:subClassOf rdf:resource="http://urn.fi/URN:NBN:fi:schema:bffi:ProvisionActivity"/>
    <skos:definition xml:lang="en">BIBFRAME definition: Information relating to modification of a resource</skos:definition>
  </rdf:Description>
  <rdf:Description rdf:about="http://urn.fi/URN:NBN:fi:schema:bffi:Agent">
    <dct:modified>2024-02-23 (New)</dct:modified>
    <rdfs:label xml:lang="en">Agent</rdfs:label>
    <rdfs:label xml:lang="fi">Toimija</rdfs:label>
    <rdf:type rdf:resource="http://www.w3.org/2002/07/owl#Class"/>
    <owl:equivalentClass rdf:resource="http://id.loc.gov/ontologies/bibframe/Agent"/>
    <bffi-meta:exactMatch rdf:resource="http://rdaregistry.info/Elements/c/C10002"/>
    <skos:definition xml:lang="en">BIBFRAME definition: Entity having a role in a resource, such as a person or organization</skos:definition>
  </rdf:Description>
  <rdf:Description rdf:about="http://urn.fi/URN:NBN:fi:schema:bffi:Multimedia">
    <dct:modified>2024-02-23 (New)</dct:modified>
    <rdfs:label xml:lang="en">Software</rdfs:label>
    <rdfs:label xml:lang="fi">Ohjelmisto</rdfs:label>
    <rdf:type rdf:resource="http://www.w3.org/2002/07/owl#Class"/>
    <owl:equivalentClass rdf:resource="http://id.loc.gov/ontologies/bibframe/Multimedia"/>
    <rdfs:subClassOf rdf:resource="http://urn.fi/URN:NBN:fi:schema:bffi:Expression"/>
    <skos:definition xml:lang="en">BIBFRAME definition: Electronic resource which is a computer program or consists of multiple media types that are software driven, such as videogames</skos:definition>
  </rdf:Description>
  <rdf:Description rdf:about="http://urn.fi/URN:NBN:fi:schema:bffi:serialPubType">
    <dct:modified>2024-11-22 (New)</dct:modified>
    <rdfs:label xml:lang="en">serial publication type</rdfs:label>
    <rdfs:label xml:lang="fi">jatkuvan julkaisun tyyppi</rdfs:label>
    <rdfs:domain rdf:resource="http://urn.fi/URN:NBN:fi:schema:bffi:SerialWork"/>
    <rdfs:range rdf:resource="http://urn.fi/URN:NBN:fi:schema:bffi:SerialPubType"/>
    <rdf:type rdf:resource="http://www.w3.org/2002/07/owl#ObjectProperty"/>
    <owl:equivalentProperty rdf:resource="http://id.loc.gov/ontologies/bflc/serialPubType"/>
    <skos:definition xml:lang="en">BFLC definition: Information recording the type of continuing resource.</skos:definition>
  </rdf:Description>
  <rdf:Description rdf:about="http://urn.fi/URN:NBN:fi:schema:bffi:seriesEnumeration">
    <dct:modified>2024-02-23 (New)</dct:modified>
    <rdfs:label xml:lang="en">series enumeration</rdfs:label>
    <rdfs:label xml:lang="fi">numerointijakson sisäinen numerointi</rdfs:label>
    <rdfs:domain rdf:resource="http://urn.fi/URN:NBN:fi:schema:bffi:Manifestation"/>
    <rdfs:range rdf:resource="http://www.w3.org/2000/01/rdf-schema#Literal"/>
    <rdf:type rdf:resource="http://www.w3.org/2002/07/owl#DatatypeProperty"/>
    <owl:equivalentProperty rdf:resource="http://id.loc.gov/ontologies/bibframe/seriesEnumeration"/>
    <bffi-meta:exactMatch rdf:resource="http://rdaregistry.info/Elements/m/P30014"/>
    <skos:definition xml:lang="en">BIBFRAME definition: Series enumeration of the resource; usually transcribed.</skos:definition>
  </rdf:Description>
  <rdf:Description rdf:about="http://urn.fi/URN:NBN:fi:schema:bffi:firstIssueEnumeration">
    <dct:modified>2024-02-23 (New)</dct:modified>
    <rdfs:label xml:lang="en">first alphanumeric designation of sequence</rdfs:label>
    <rdfs:label xml:lang="fi">numerointijakson ensimmäinen numero- ja/tai kirjainmäärite</rdfs:label>
    <rdfs:domain rdf:resource="http://urn.fi/URN:NBN:fi:schema:bffi:Manifestation"/>
    <rdfs:range rdf:resource="http://www.w3.org/2000/01/rdf-schema#Literal"/>
    <rdf:type rdf:resource="http://www.w3.org/2002/07/owl#DatatypeProperty"/>
    <bffi-meta:broadMatch rdf:resource="http://id.loc.gov/ontologies/bibframe/firstIssue"/>
    <bffi-meta:exactMatch rdf:resource="http://rdaregistry.info/Elements/m/P30147"/>
  </rdf:Description>
  <rdf:Description rdf:nodeID="n68bca78492684c1398be6f6d4f77765db1">
    <rdf:type rdf:resource="http://www.w3.org/2002/07/owl#Class"/>
    <owl:unionOf rdf:nodeID="n68bca78492684c1398be6f6d4f77765db2"/>
  </rdf:Description>
  <rdf:Description rdf:about="http://urn.fi/URN:NBN:fi:schema:bffi:Integrating">
    <dct:modified>2024-02-23 (New)</dct:modified>
    <rdfs:label xml:lang="en">Integrating work</rdfs:label>
    <rdfs:label xml:lang="fi">Päivittyvä teos</rdfs:label>
    <rdf:type rdf:resource="http://www.w3.org/2002/07/owl#Class"/>
    <owl:equivalentClass rdf:resource="http://id.loc.gov/ontologies/bibframe/Integrating"/>
    <bffi-meta:broadMatch rdf:resource="http://rdaregistry.info/Elements/c/C10001"/>
    <rdfs:subClassOf rdf:resource="http://urn.fi/URN:NBN:fi:schema:bffi:Work"/>
    <skos:definition xml:lang="en">BIBFRAME definition: Resource that is added to or changed by updates that do not remain discrete but are integrated into the whole</skos:definition>
  </rdf:Description>
  <rdf:Description rdf:about="http://urn.fi/URN:NBN:fi:schema:bffi:electronicLocator">
    <dct:modified>2024-11-22 (New)</dct:modified>
    <rdfs:label xml:lang="en">electronic location</rdfs:label>
    <rdfs:label xml:lang="fi">elektronisen aineiston sijainti</rdfs:label>
    <rdfs:domain rdf:resource="http://www.w3.org/2000/01/rdf-schema#Resource"/>
    <rdfs:range rdf:resource="http://www.w3.org/2000/01/rdf-schema#Resource"/>
    <rdf:type rdf:resource="http://www.w3.org/2002/07/owl#ObjectProperty"/>
    <owl:equivalentProperty rdf:resource="http://id.loc.gov/ontologies/bibframe/electronicLocator"/>
    <bffi-meta:narrowMatch rdf:resource="http://rdaregistry.info/Elements/m/P30154"/>
    <skos:definition xml:lang="en">BIBFRAME definition: Electronic location from which the resource is available.</skos:definition>
  </rdf:Description>
  <rdf:Description rdf:about="http://urn.fi/URN:NBN:fi:schema:bffi:identifies">
    <dct:modified>2024-02-23 (New)</dct:modified>
    <rdfs:label xml:lang="en">resource identified</rdfs:label>
    <rdfs:label xml:lang="fi">tunniste entiteetille</rdfs:label>
    <rdfs:domain rdf:resource="http://urn.fi/URN:NBN:fi:schema:bffi:Identifier"/>
    <rdfs:range rdf:resource="http://www.w3.org/2000/01/rdf-schema#Resource"/>
    <rdf:type rdf:resource="http://www.w3.org/2002/07/owl#ObjectProperty"/>
    <owl:equivalentProperty rdf:resource="http://id.loc.gov/ontologies/bibframe/identifies"/>
    <rdfs:seeAlso rdf:resource="http://rdaregistry.info/Elements/n/P80160"/>
    <owl:inverseOf rdf:resource="http://urn.fi/URN:NBN:fi:schema:bffi:identifiedBy"/>
    <skos:definition xml:lang="en">BIBFRAME definition: Resource that is associated with a character string that serves to differentiate one resource from another.</skos:definition>
  </rdf:Description>
  <rdf:Description rdf:about="http://urn.fi/URN:NBN:fi:schema:bffi:EncodingLevel">
    <dct:modified>2024-11-22 (New)</dct:modified>
    <rdfs:label xml:lang="en">Encoding level</rdfs:label>
    <rdfs:label xml:lang="fi">Kuvailutaso</rdfs:label>
    <rdf:type rdf:resource="http://www.w3.org/2002/07/owl#Class"/>
    <owl:equivalentClass rdf:resource="http://id.loc.gov/ontologies/bflc/EncodingLevel"/>
    <skos:definition xml:lang="en">BFLC definition: Designation of the fullness of the bibliographic description.</skos:definition>
  </rdf:Description>
  <rdf:Description rdf:about="http://urn.fi/URN:NBN:fi:schema:bffi:simpleAgent">
    <dct:modified>2024-02-23 (New)</dct:modified>
    <rdfs:label xml:lang="en">agent</rdfs:label>
    <rdfs:label xml:lang="fi">auktorisoimaton liittyvä toimija</rdfs:label>
    <rdfs:domain rdf:resource="http://urn.fi/URN:NBN:fi:schema:bffi:ProvisionActivity"/>
    <rdfs:range rdf:resource="http://www.w3.org/2000/01/rdf-schema#Literal"/>
    <rdf:type rdf:resource="http://www.w3.org/2002/07/owl#DatatypeProperty"/>
    <owl:equivalentProperty rdf:resource="http://id.loc.gov/ontologies/bflc/simpleAgent"/>
    <skos:definition xml:lang="en">BFLC definition: Name of publisher, distributor, manufacturer or producer as transcribed from the resource</skos:definition>
  </rdf:Description>
  <rdf:Description rdf:about="http://urn.fi/URN:NBN:fi:schema:bffi:GrooveCharacteristic">
    <dct:modified>2024-11-22 (New)</dct:modified>
    <rdfs:label xml:lang="en">Groove characteristic</rdfs:label>
    <rdfs:label xml:lang="fi">Uran ominaisuudet</rdfs:label>
    <rdf:type rdf:resource="http://www.w3.org/2002/07/owl#Class"/>
    <owl:equivalentProperty rdf:resource="http://id.loc.gov/ontologies/bibframe/GrooveCharacteristic"/>
    <rdfs:seeAlso rdf:resource="http://rdaregistry.info/termList/grooveWidth/"/>
    <rdfs:subClassOf rdf:resource="http://urn.fi/URN:NBN:fi:schema:bffi:SoundCharacteristic"/>
    <skos:definition xml:lang="en">BIBFRAME definition: Groove width of an analog disc or the groove pitch of an analog cylinder, e.g., coarse groove, microgroove</skos:definition>
  </rdf:Description>
  <rdf:Description rdf:about="http://urn.fi/URN:NBN:fi:schema:bffi:pubFrequency">
    <dct:modified>2024-11-22 (New)</dct:modified>
    <rdfs:label xml:lang="en">publication frequency</rdfs:label>
    <rdfs:label xml:lang="fi">aiemmat ilmestymistiedot</rdfs:label>
    <rdfs:domain rdf:nodeID="n26a54bed81f14ec98f0dfd0d8091fc72b1"/>
    <rdfs:range rdf:resource="http://urn.fi/URN:NBN:fi:schema:bffi:PubFrequency"/>
    <rdf:type rdf:resource="http://www.w3.org/2002/07/owl#ObjectProperty"/>
    <owl:equivalentProperty rdf:resource="http://id.loc.gov/ontologies/bibframe/pubFrequency"/>
    <bffi-meta:exactMatch rdf:resource="http://rdaregistry.info/Elements/m/P30285"/>
    <skos:definition xml:lang="en">BIBFRAME definition: Relates a resource to a publication frequency resource to capture such details as first issue, last issue, status, etc.</skos:definition>
  </rdf:Description>
  <rdf:Description rdf:about="http://urn.fi/URN:NBN:fi:schema:bffi:editionEnumeration">
    <dct:modified>2024-11-22 (New)</dct:modified>
    <rdfs:label xml:lang="en">edition enumeration</rdfs:label>
    <rdfs:label xml:lang="fi">painosmäärite</rdfs:label>
    <rdfs:domain rdf:resource="http://urn.fi/URN:NBN:fi:schema:bffi:Manifestation"/>
    <rdfs:range rdf:resource="http://www.w3.org/2000/01/rdf-schema#Literal"/>
    <rdf:type rdf:resource="http://www.w3.org/2002/07/owl#DatatypeProperty"/>
    <owl:equivalentProperty rdf:resource="http://id.loc.gov/ontologies/bibframe/editionEnumeration"/>
    <bffi-meta:narrowMatch rdf:resource="http://rdaregistry.info/Elements/m/P30133"/>
    <bffi-meta:narrowMatch rdf:resource="http://rdaregistry.info/Elements/m/P30013"/>
    <bffi-meta:narrowMatch rdf:resource="http://rdaregistry.info/Elements/m/P30132"/>
    <bffi-meta:narrowMatch rdf:resource="http://rdaregistry.info/Elements/m/P30012"/>
    <skos:definition xml:lang="en">BIBFRAME definition: Enumeration of the edition; usually transcribed.</skos:definition>
  </rdf:Description>
  <rdf:Description rdf:about="http://urn.fi/URN:NBN:fi:schema:bffi:contribution">
    <dct:modified>2024-02-23 (New)</dct:modified>
    <rdfs:label xml:lang="en">contribution</rdfs:label>
    <rdfs:label xml:lang="fi">kontribuutio</rdfs:label>
    <rdfs:domain rdf:nodeID="n5cd48ce8767a480c888bcf43bfaa8780b1"/>
    <rdfs:range rdf:resource="http://urn.fi/URN:NBN:fi:schema:bffi:Contribution"/>
    <rdf:type rdf:resource="http://www.w3.org/2002/07/owl#ObjectProperty"/>
    <owl:equivalentProperty rdf:resource="http://id.loc.gov/ontologies/bibframe/contribution"/>
    <bffi-meta:narrowMatch rdf:resource="http://rdaregistry.info/Elements/w/P10311"/>
    <bffi-meta:narrowMatch rdf:resource="http://rdaregistry.info/Elements/e/P20301"/>
    <bffi-meta:narrowMatch rdf:resource="http://rdaregistry.info/Elements/m/P30267"/>
    <bffi-meta:narrowMatch rdf:resource="http://rdaregistry.info/Elements/m/P30327"/>
    <skos:definition xml:lang="en">BIBFRAME definition: Agent and its role in relation to the resource</skos:definition>
  </rdf:Description>
  <rdf:Description rdf:about="http://urn.fi/URN:NBN:fi:schema:bffi:CollectionExpression">
    <dct:modified>2024-02-23 (New)</dct:modified>
    <rdfs:label xml:lang="en">Collection expression</rdfs:label>
    <rdfs:label xml:lang="fi">Kokoelmaekspressio</rdfs:label>
    <rdf:type rdf:resource="http://www.w3.org/2002/07/owl#Class"/>
    <bffi-meta:broadMatch rdf:resource="http://id.loc.gov/ontologies/bibframe/Collection"/>
    <rdfs:subClassOf rdf:resource="http://urn.fi/URN:NBN:fi:schema:bffi:Expression"/>
  </rdf:Description>
  <rdf:Description rdf:about="http://urn.fi/URN:NBN:fi:schema:bffi:equinox">
    <dct:modified>2024-04-16 (New)</dct:modified>
    <rdfs:label xml:lang="en">cartographic equinox</rdfs:label>
    <rdfs:label xml:lang="fi">ekvinokti</rdfs:label>
    <rdfs:domain rdf:resource="http://urn.fi/URN:NBN:fi:schema:bffi:Cartographic"/>
    <rdfs:range rdf:resource="http://www.w3.org/2000/01/rdf-schema#Literal"/>
    <rdf:type rdf:resource="http://www.w3.org/2002/07/owl#DatatypeProperty"/>
    <owl:equivalentProperty rdf:resource="http://id.loc.gov/ontologies/bibframe/equinox"/>
    <skos:definition xml:lang="en">BIBFRAME definition: One of two points of intersection of the ecliptic and the celestial equator, occupied by the sun when its declination is 0 degrees.</skos:definition>
  </rdf:Description>
  <rdf:Description rdf:about="http://urn.fi/URN:NBN:fi:schema:bffi:acquisitionSource">
    <dct:modified>2024-04-16 (New)</dct:modified>
    <rdfs:label xml:lang="en">source of acquisition</rdfs:label>
    <rdfs:label xml:lang="fi">hankintalähde</rdfs:label>
    <rdfs:domain rdf:resource="http://urn.fi/URN:NBN:fi:schema:bffi:Manifestation"/>
    <rdfs:range rdf:resource="http://urn.fi/URN:NBN:fi:schema:bffi:AcquisitionSource"/>
    <rdf:type rdf:resource="http://www.w3.org/2002/07/owl#ObjectProperty"/>
    <owl:equivalentProperty rdf:resource="http://id.loc.gov/ontologies/bibframe/acquisitionSource"/>
    <bffi-meta:broadMatch rdf:resource="http://rdaregistry.info/Elements/m/P30141"/>
    <skos:definition xml:lang="en">BIBFRAME definition: Information about an organization, person, etc., from which a resource may be obtained.</skos:definition>
  </rdf:Description>
  <rdf:Description rdf:about="http://urn.fi/URN:NBN:fi:schema:bffi:Cartographic">
    <dct:modified>2024-02-23 (New)</dct:modified>
    <rdfs:label xml:lang="en">Cartographic information</rdfs:label>
    <rdfs:label xml:lang="fi">Kartografinen tieto</rdfs:label>
    <rdf:type rdf:resource="http://www.w3.org/2002/07/owl#Class"/>
    <owl:equivalentClass rdf:resource="http://id.loc.gov/ontologies/bibframe/Cartographic"/>
    <skos:definition xml:lang="en">BIBFRAME definition: Content that represents the whole or part of the earth, any celestial body, or imaginary place at any scale</skos:definition>
  </rdf:Description>
  <rdf:Description rdf:nodeID="n1e5b766c1bf94ff9812af7b852f48486b1">
    <rdf:type rdf:resource="http://www.w3.org/2002/07/owl#Class"/>
    <owl:unionOf rdf:nodeID="n1e5b766c1bf94ff9812af7b852f48486b2"/>
  </rdf:Description>
  <rdf:Description rdf:about="http://urn.fi/URN:NBN:fi:schema:bffi:applicableInstitution">
    <dct:modified>2025-01-02 (New)</dct:modified>
    <rdfs:label xml:lang="en">applicable institution</rdfs:label>
    <rdfs:label xml:lang="fi">organisaatio, jota tiedot koskevat</rdfs:label>
    <rdfs:domain rdf:nodeID="n42dc8c45022c4e7c8886fe842cc1e72fb1"/>
    <rdfs:range rdf:resource="http://urn.fi/URN:NBN:fi:schema:bffi:Organization"/>
    <rdf:type rdf:resource="http://www.w3.org/2002/07/owl#ObjectProperty"/>
    <owl:equivalentProperty rdf:resource="http://id.loc.gov/ontologies/bflc/applicableInstitution"/>
    <skos:definition xml:lang="en">BFLC definition: Institutional location of a resource to which a particular piece of description applies.</skos:definition>
  </rdf:Description>
  <rdf:Description rdf:about="http://urn.fi/URN:NBN:fi:schema:bffi:frequency">
    <dct:modified>2024-11-22 (New)</dct:modified>
    <rdfs:label xml:lang="en">frequency</rdfs:label>
    <rdfs:label xml:lang="fi">ilmestymistiheys</rdfs:label>
    <rdfs:domain rdf:resource="http://www.w3.org/2000/01/rdf-schema#Resource"/>
    <rdfs:range rdf:resource="http://urn.fi/URN:NBN:fi:schema:bffi:Frequency"/>
    <rdf:type rdf:resource="http://www.w3.org/2002/07/owl#ObjectProperty"/>
    <owl:equivalentProperty rdf:resource="http://id.loc.gov/ontologies/bibframe/frequency"/>
    <bffi-meta:closeMatch rdf:resource="http://rdaregistry.info/Elements/w/P10368"/>
    <skos:definition xml:lang="en">BIBFRAME definition: Intervals at which the parts of a serially produced resource or the updates to an integrating resource are issued.</skos:definition>
  </rdf:Description>
  <rdf:Description rdf:about="http://urn.fi/URN:NBN:fi:schema:bffi:DigitalCharacteristic">
    <dct:modified>2024-04-16 (New)</dct:modified>
    <rdfs:label xml:lang="en">Digital characteristic</rdfs:label>
    <rdfs:label xml:lang="fi">Digitaalisen tiedoston ominaisuus</rdfs:label>
    <rdf:type rdf:resource="http://www.w3.org/2002/07/owl#Class"/>
    <owl:equivalentClass rdf:resource="http://id.loc.gov/ontologies/bibframe/DigitalCharacteristic"/>
    <skos:definition xml:lang="en">BIBFRAME definition: Technical specification relating to the digital encoding of text, image, audio, video, and other types of data in a resource</skos:definition>
  </rdf:Description>
  <rdf:Description rdf:about="http://urn.fi/URN:NBN:fi:schema:bffi:AdminMetadata">
    <dct:modified>2024-02-23 (New)</dct:modified>
    <rdfs:label xml:lang="en">Administrative metadata</rdfs:label>
    <rdfs:label xml:lang="fi">Hallinnolliset metatiedot</rdfs:label>
    <rdf:type rdf:resource="http://www.w3.org/2002/07/owl#Class"/>
    <owl:equivalentClass rdf:resource="http://id.loc.gov/ontologies/bibframe/AdminMetadata"/>
    <skos:definition xml:lang="en">BIBFRAME definition: Metadata about the metadata, especially provenance information</skos:definition>
  </rdf:Description>
  <rdf:Description rdf:about="http://urn.fi/URN:NBN:fi:schema:bffi:recordingSource">
    <dct:modified>2024-02-23 (New)</dct:modified>
    <rdfs:label xml:lang="en">recording source</rdfs:label>
    <rdfs:label xml:lang="fi">merkintälähde</rdfs:label>
    <rdfs:domain rdf:resource="http://urn.fi/URN:NBN:fi:schema:bffi:AdminMetadata"/>
    <rdfs:range rdf:resource="http://urn.fi/URN:NBN:fi:schema:bffi:RecordingSource"/>
    <rdf:type rdf:resource="http://www.w3.org/2002/07/owl#ObjectProperty"/>
    <bffi-meta:broadMatch rdf:resource="http://id.loc.gov/ontologies/bibframe/derivedFrom"/>
    <bffi-meta:exactMatch rdf:resource="http://rdaregistry.info/Elements/w/P10404"/>
  </rdf:Description>
  <rdf:Description rdf:about="http://urn.fi/URN:NBN:fi:schema:bffi:">
    <dct:relation rdf:resource="http://www.rdaregistry.info/Elements/"/>
    <dct:relation rdf:resource="http://id.loc.gov/ontologies/bibframe-2-4-0/"/>
    <dct:relation rdf:resource="http://id.loc.gov/ontologies/bflc-2-4-0/"/>
    <dct:description xml:lang="fi">Tämä BIBFRAME-tietomalli perustuu Kongressin kirjaston julkaisemaan BIBFRAME-tietomallin 2.4.0 versioon. Mallia on täydennetty RDA-tietomallin luokilla ja ominaisuuksilla sekä suomalaisiin kansallisiin kuvailuohjeisiin perustuvilla täydennyksillä. Versio 1.0.0 suomalaisesta linkitetyn kirjastodatan tietomallista sisältää kaikki suomalaisessa kuvailussa tarvittavat BIBFRAME-luokat ja -ominaisuudet.</dct:description>
    <dct:description xml:lang="en">This BIBFRAME data model is based on the BIBFRAME 2.4.0 model published by the Library of Congress. The model has been supplemented with classes and properties from the RDA element sets, as well as the Finnish national cataloguing guidelines. Version 1.0.0 of the Finnish linked library data model includes all the BIBFRAME classes and properties required in Finnish cataloguing.</dct:description>
    <dct:title xml:lang="fi">LKD-tietomalli -- BIBFRAME 2.4.0 -tietomallin kansallinen sovellus</dct:title>
    <dct:title xml:lang="en">LKD data model -- BIBFRAME 2.4.0 data model Finnish implementation</dct:title>
    <rdf:type rdf:resource="http://www.w3.org/2002/07/owl#Ontology"/>
    <dct:publisher rdf:resource="http://urn.fi/URN:NBN:fi:au:finaf:000034269"/>
    <dct:license rdf:resource="http://creativecommons.org/publicdomain/zero/1.0/"/>
    <dct:contributor rdf:resource="http://www.wikidata.org/entity/Q124635303"/>
    <dct:issued rdf:datatype="http://www.w3.org/2001/XMLSchema#date">2025-01-02</dct:issued>
    <owl:versionIRI rdf:resource="http://schema.finto.fi/bffi/1-0-0/"/>
    <owl:versionInfo>1.0.0</owl:versionInfo>
    <owl:priorVersion rdf:resource="http://schema.finto.fi/bffi/0-8-0/"/>
    <dct:modified rdf:datatype="http://www.w3.org/2001/XMLSchema#dateTime">2025-01-02T11:49:20+00:00</dct:modified>
  </rdf:Description>
  <rdf:Description rdf:about="http://urn.fi/URN:NBN:fi:schema:bffi:aggregates">
    <dct:modified>2024-02-23 (New)</dct:modified>
    <rdfs:label xml:lang="en">aggregates expression</rdfs:label>
    <rdfs:label xml:lang="fi">aggregoi ekspression</rdfs:label>
    <rdfs:domain rdf:resource="http://urn.fi/URN:NBN:fi:schema:bffi:AggregatingExpression"/>
    <rdfs:range rdf:resource="http://urn.fi/URN:NBN:fi:schema:bffi:Expression"/>
    <rdf:type rdf:resource="http://www.w3.org/2002/07/owl#ObjectProperty"/>
    <bffi-meta:broadMatch rdf:resource="http://id.loc.gov/ontologies/bibframe/relatedTo"/>
    <bffi-meta:exactMatch rdf:resource="http://rdaregistry.info/Elements/e/P20319"/>
    <rdfs:subPropertyOf rdf:resource="http://urn.fi/URN:NBN:fi:schema:bffi:relatedTo"/>
    <owl:inverseOf rdf:resource="http://urn.fi/URN:NBN:fi:schema:bffi:aggregatedBy"/>
  </rdf:Description>
  <rdf:Description rdf:about="http://urn.fi/URN:NBN:fi:schema:bffi:itemPortion">
    <dct:modified>2024-06-19 (New)</dct:modified>
    <rdfs:label xml:lang="en">classification item number</rdfs:label>
    <rdfs:label xml:lang="fi">kappalenumero</rdfs:label>
    <rdfs:domain rdf:resource="http://urn.fi/URN:NBN:fi:schema:bffi:Classification"/>
    <rdfs:range rdf:resource="http://www.w3.org/2000/01/rdf-schema#Literal"/>
    <rdf:type rdf:resource="http://www.w3.org/2002/07/owl#DatatypeProperty"/>
    <owl:equivalentProperty rdf:resource="http://id.loc.gov/ontologies/bibframe/itemPortion"/>
    <skos:definition xml:lang="en">BIBFRAME definition: Number attached to a classification string that indicates a particular item.</skos:definition>
  </rdf:Description>
  <rdf:Description rdf:about="http://urn.fi/URN:NBN:fi:schema:bffi:Sublocation">
    <dct:modified>2024-04-16 (New)</dct:modified>
    <rdfs:label xml:lang="en">Sublocation</rdfs:label>
    <rdfs:label xml:lang="fi">Alayksikkö tai alakokoelma</rdfs:label>
    <rdf:type rdf:resource="http://www.w3.org/2002/07/owl#Class"/>
    <owl:equivalentClass rdf:resource="http://id.loc.gov/ontologies/bibframe/Sublocation"/>
    <skos:definition xml:lang="en">BIBFRAME definition: Specific place within the holding entity where the item is located or made available</skos:definition>
  </rdf:Description>
  <rdf:Description rdf:about="http://urn.fi/URN:NBN:fi:schema:bffi:catalogerId">
    <dct:modified>2024-06-19 (New)</dct:modified>
    <rdfs:label xml:lang="en">cataloger ID</rdfs:label>
    <rdfs:label xml:lang="fi">kuvailijan tunnus</rdfs:label>
    <rdfs:domain rdf:resource="http://urn.fi/URN:NBN:fi:schema:bffi:AdminMetadata"/>
    <rdfs:range rdf:resource="http://www.w3.org/2000/01/rdf-schema#Literal"/>
    <rdf:type rdf:resource="http://www.w3.org/2002/07/owl#DatatypeProperty"/>
    <owl:equivalentProperty rdf:resource="http://id.loc.gov/ontologies/bflc/catalogerId"/>
    <skos:definition xml:lang="en">BFLC definition: ID of the cataloger who created or edited the description.</skos:definition>
  </rdf:Description>
  <rdf:Description rdf:about="http://urn.fi/URN:NBN:fi:schema:bffi-meta:relatedValueVocabulary">
    <dct:modified>2024-02-23 (New)</dct:modified>
    <rdf:type rdf:resource="http://www.w3.org/2002/07/owl#AnnotationProperty"/>
    <rdfs:label xml:lang="fi">liittyvä arvosanasto</rdfs:label>
    <rdfs:label xml:lang="en">related value vocabulary</rdfs:label>
    <rdfs:subPropertyOf rdf:resource="http://purl.org/dc/terms/relation"/>
    <skos:definition xml:lang="fi">Liittyvän luokan edustajia sisältävä arvosanasto.</skos:definition>
    <skos:definition xml:lang="en">Value vocabulary containing values of the related class.</skos:definition>
  </rdf:Description>
  <rdf:Description rdf:about="http://urn.fi/URN:NBN:fi:schema:bffi:classificationPortion">
    <dct:modified>2024-06-19 (New)</dct:modified>
    <rdfs:label xml:lang="en">classification number</rdfs:label>
    <rdfs:label xml:lang="fi">luokka</rdfs:label>
    <rdfs:domain rdf:resource="http://urn.fi/URN:NBN:fi:schema:bffi:Classification"/>
    <rdfs:range rdf:resource="http://www.w3.org/2000/01/rdf-schema#Literal"/>
    <rdf:type rdf:resource="http://www.w3.org/2002/07/owl#DatatypeProperty"/>
    <owl:equivalentProperty rdf:resource="http://id.loc.gov/ontologies/bibframe/classificationPortion"/>
    <skos:definition xml:lang="en">BIBFRAME definition: Classification number (single class number or beginning number of a span) that indicates the subject by applying a formal system of coding and organizing resources.</skos:definition>
  </rdf:Description>
  <rdf:Description rdf:about="http://urn.fi/URN:NBN:fi:schema:bffi:demographicGroup">
    <dct:modified>2025-01-02 (New)</dct:modified>
    <rdfs:label xml:lang="en">demographic group</rdfs:label>
    <rdfs:label xml:lang="fi">väestöryhmä</rdfs:label>
    <rdfs:domain rdf:nodeID="n14ff77a0080346dbb0cd2218439611d1b1"/>
    <rdfs:range rdf:resource="http://urn.fi/URN:NBN:fi:schema:bffi:DemographicGroup"/>
    <rdf:type rdf:resource="http://www.w3.org/2002/07/owl#ObjectProperty"/>
    <owl:equivalentProperty rdf:resource="http://id.loc.gov/ontologies/bflc/demographicGroup"/>
    <skos:definition xml:lang="en">BFLC definition: Characteristics of a group of agents.</skos:definition>
  </rdf:Description>
  <rdf:Description rdf:about="http://urn.fi/URN:NBN:fi:schema:bffi:creatorCharacteristic">
    <dct:modified>2025-01-02 (New)</dct:modified>
    <rdfs:label xml:lang="en">creator characteristic</rdfs:label>
    <rdfs:label xml:lang="fi">tekijän ominaisuudet</rdfs:label>
    <rdfs:domain rdf:nodeID="ne27b8fc3c7014a3a99b60051d23322e1b1"/>
    <rdfs:range rdf:resource="http://urn.fi/URN:NBN:fi:schema:bffi:CreatorCharacteristic"/>
    <rdf:type rdf:resource="http://www.w3.org/2002/07/owl#ObjectProperty"/>
    <owl:equivalentProperty rdf:resource="http://id.loc.gov/ontologies/bflc/creatorCharacteristic"/>
    <skos:definition xml:lang="en">BFLC definition: Category to which the creators of the resource belong.</skos:definition>
  </rdf:Description>
  <rdf:Description rdf:about="http://urn.fi/URN:NBN:fi:schema:bffi:edition">
    <dct:modified>2024-06-19 (New)</dct:modified>
    <rdfs:label xml:lang="en">classification scheme edition</rdfs:label>
    <rdfs:label xml:lang="fi">luokituksen painos</rdfs:label>
    <rdfs:domain rdf:resource="http://urn.fi/URN:NBN:fi:schema:bffi:Classification"/>
    <rdfs:range rdf:resource="http://www.w3.org/2000/01/rdf-schema#Literal"/>
    <rdf:type rdf:resource="http://www.w3.org/2002/07/owl#DatatypeProperty"/>
    <owl:equivalentProperty rdf:resource="http://id.loc.gov/ontologies/bibframe/edition"/>
    <skos:definition xml:lang="en">BIBFRAME definition: Edition of the classification scheme, such as full, abridged or a number, when a classification scheme designates editions.</skos:definition>
  </rdf:Description>
  <rdf:Description rdf:about="http://urn.fi/URN:NBN:fi:schema:bffi:Organization">
    <dct:modified>2024-02-23 (New)</dct:modified>
    <rdfs:label xml:lang="en">Organization</rdfs:label>
    <rdfs:label xml:lang="fi">Yhteisö</rdfs:label>
    <rdf:type rdf:resource="http://www.w3.org/2002/07/owl#Class"/>
    <owl:equivalentClass rdf:resource="http://id.loc.gov/ontologies/bibframe/Organization"/>
    <bffi-meta:closeMatch rdf:resource="http://rdaregistry.info/Elements/c/C10005"/>
    <rdfs:subClassOf rdf:resource="http://urn.fi/URN:NBN:fi:schema:bffi:Agent"/>
    <skos:definition xml:lang="en">BIBFRAME definition: Corporation or group of persons and/or organizations that acts, or may act, as a unit</skos:definition>
  </rdf:Description>
  <rdf:Description rdf:about="http://urn.fi/URN:NBN:fi:schema:bffi:Dataset">
    <dct:modified>2024-02-23 (New)</dct:modified>
    <rdfs:label xml:lang="en">Dataset</rdfs:label>
    <rdfs:label xml:lang="fi">Datasetti</rdfs:label>
    <rdf:type rdf:resource="http://www.w3.org/2002/07/owl#Class"/>
    <owl:equivalentClass rdf:resource="http://id.loc.gov/ontologies/bibframe/Dataset"/>
    <rdfs:subClassOf rdf:resource="http://urn.fi/URN:NBN:fi:schema:bffi:Expression"/>
    <skos:definition xml:lang="en">BIBFRAME definition: Data encoded in a defined structure, including numeric data, environmental data, etc., used by applications software</skos:definition>
  </rdf:Description>
  <rdf:Description rdf:about="http://urn.fi/URN:NBN:fi:schema:bffi:mediumOfChoreographicContent">
    <dct:modified>2024-11-22 (New)</dct:modified>
    <rdfs:label xml:lang="en">medium of performance of choreographic content</rdfs:label>
    <rdfs:label xml:lang="fi">koreografisen sisällön esityskokoonpano</rdfs:label>
    <rdfs:domain rdf:resource="http://urn.fi/URN:NBN:fi:schema:bffi:Expression"/>
    <rdfs:range rdf:resource="http://urn.fi/URN:NBN:fi:schema:bffi:ChoreographicMedium"/>
    <rdf:type rdf:resource="http://www.w3.org/2002/07/owl#ObjectProperty"/>
    <bffi-meta:closeMatch rdf:resource="http://id.loc.gov/ontologies/bibframe/musicMedium"/>
    <bffi-meta:exactMatch rdf:resource="http://rdaregistry.info/Elements/e/P20324"/>
  </rdf:Description>
  <rdf:Description rdf:about="http://urn.fi/URN:NBN:fi:schema:bffi:Extent">
    <dct:modified>2024-02-23 (New)</dct:modified>
    <rdfs:label xml:lang="en">Extent</rdfs:label>
    <rdfs:label xml:lang="fi">Laajuus</rdfs:label>
    <bffi-meta:relatedValueVocabulary rdf:resource="http://urn.fi/URN:NBN:fi:au:mts:m8"/>
    <rdf:type rdf:resource="http://www.w3.org/2002/07/owl#Class"/>
    <owl:equivalentClass rdf:resource="http://id.loc.gov/ontologies/bibframe/Extent"/>
    <rdfs:seeAlso rdf:resource="http://www.rdaregistry.info/termList/RDACarrierEU/"/>
    <skos:definition xml:lang="en">BIBFRAME definition: Number and type of units and/or subunits making up a resource</skos:definition>
  </rdf:Description>
  <rdf:Description rdf:nodeID="n0d5ef643a16a443a8864901b85eb32dbb1">
    <rdf:type rdf:resource="http://www.w3.org/2002/07/owl#Class"/>
    <owl:unionOf rdf:nodeID="n0d5ef643a16a443a8864901b85eb32dbb2"/>
  </rdf:Description>
  <rdf:Description rdf:about="http://urn.fi/URN:NBN:fi:schema:bffi:PubFrequency">
    <dct:modified>2024-11-22 (New)</dct:modified>
    <rdfs:label xml:lang="en">Publication Frequency</rdfs:label>
    <rdfs:label xml:lang="fi">Aiemmat ilmestymistiedot</rdfs:label>
    <rdf:type rdf:resource="http://www.w3.org/2002/07/owl#Class"/>
    <owl:equivalentClass rdf:resource="http://id.loc.gov/ontologies/bibframe/PubFrequency"/>
    <rdfs:seeAlso rdf:resource="http://rdaregistry.info/termList/frequency/"/>
    <skos:definition xml:lang="en">BIBFRAME definition: Information about the publication frequency of a resource</skos:definition>
  </rdf:Description>
  <rdf:Description rdf:about="http://urn.fi/URN:NBN:fi:schema:bffi:musicMedium">
    <dct:modified>2024-02-23 (New)</dct:modified>
    <rdfs:label xml:lang="en">music medium of performance</rdfs:label>
    <rdfs:label xml:lang="fi">musiikin esityskokoonpano</rdfs:label>
    <rdfs:domain rdf:nodeID="n2d6ab2e53ad74c4b81628c947ca3da20b1"/>
    <rdfs:range rdf:resource="http://urn.fi/URN:NBN:fi:schema:bffi:MusicMedium"/>
    <rdf:type rdf:resource="http://www.w3.org/2002/07/owl#ObjectProperty"/>
    <bffi-meta:exactMatch rdf:resource="http://rdaregistry.info/Elements/e/P20215"/>
    <rdfs:subPropertyOf rdf:resource="http://id.loc.gov/ontologies/bibframe/musicMedium"/>
  </rdf:Description>
  <rdf:Description rdf:about="http://urn.fi/URN:NBN:fi:schema:bffi:capture">
    <dct:modified>2024-02-23 (New)</dct:modified>
    <rdfs:label xml:lang="en">capture of content</rdfs:label>
    <rdfs:label xml:lang="fi">taltiointitiedot</rdfs:label>
    <rdfs:domain rdf:nodeID="n096c0702f8c64e3bbe53573a59499c9ab1"/>
    <rdfs:range rdf:resource="http://urn.fi/URN:NBN:fi:schema:bffi:Capture"/>
    <rdf:type rdf:resource="http://www.w3.org/2002/07/owl#ObjectProperty"/>
    <bffi-meta:exactMatch rdf:resource="http://rdaregistry.info/Elements/e/P20217"/>
    <rdfs:subPropertyOf rdf:resource="http://id.loc.gov/ontologies/bibframe/capture"/>
  </rdf:Description>
  <rdf:Description rdf:about="http://urn.fi/URN:NBN:fi:schema:bffi:GenreForm">
    <dct:modified>2024-02-23 (New)</dct:modified>
    <rdfs:label xml:lang="en">Category of work</rdfs:label>
    <rdfs:label xml:lang="fi">Kategoria</rdfs:label>
    <bffi-meta:relatedValueVocabulary rdf:resource="http://urn.fi/URN:NBN:fi:au:mts:m991"/>
    <bffi-meta:relatedValueVocabulary rdf:resource="http://urn.fi/URN:NBN:fi:au:mts:m5072"/>
    <rdf:type rdf:resource="http://www.w3.org/2002/07/owl#Class"/>
    <owl:equivalentClass rdf:resource="http://id.loc.gov/ontologies/bibframe/GenreForm"/>
    <skos:definition xml:lang="en">BIBFRAME definition: Form category or genre to which a resource belongs</skos:definition>
  </rdf:Description>
  <rdf:Description rdf:about="http://urn.fi/URN:NBN:fi:schema:bffi:dimensions">
    <dct:modified>2024-06-19 (New)</dct:modified>
    <rdfs:label xml:lang="en">dimensions</rdfs:label>
    <rdfs:label xml:lang="fi">koko</rdfs:label>
    <rdfs:domain rdf:resource="http://urn.fi/URN:NBN:fi:schema:bffi:Manifestation"/>
    <rdfs:range rdf:resource="http://www.w3.org/2000/01/rdf-schema#Literal"/>
    <rdf:type rdf:resource="http://www.w3.org/2002/07/owl#DatatypeProperty"/>
    <owl:equivalentProperty rdf:resource="http://id.loc.gov/ontologies/bibframe/dimensions"/>
    <bffi-meta:exactMatch rdf:resource="http://rdaregistry.info/Elements/m/P30169"/>
    <skos:definition xml:lang="en">BIBFRAME definition: Measurements of the carrier or carriers and/or the container of a resource.</skos:definition>
  </rdf:Description>
  <rdf:Description rdf:about="http://urn.fi/URN:NBN:fi:schema:bffi:MusicFormat">
    <dct:modified>2024-02-23 (New)</dct:modified>
    <rdfs:label xml:lang="en">Notated music format</rdfs:label>
    <rdfs:label xml:lang="fi">Nuottiaineiston muoto</rdfs:label>
    <bffi-meta:relatedValueVocabulary rdf:resource="http://urn.fi/URN:NBN:fi:au:mts:m2002"/>
    <rdf:type rdf:resource="http://www.w3.org/2002/07/owl#Class"/>
    <owl:equivalentClass rdf:resource="http://id.loc.gov/ontologies/bibframe/MusicFormat"/>
    <rdfs:seeAlso rdf:resource="http://rdaregistry.info/termList/formatNoteMus/"/>
    <skos:definition xml:lang="en">BIBFRAME definition: Layout for content of a resource that is presented in the form of musical notation</skos:definition>
  </rdf:Description>
  <rdf:Description rdf:about="http://urn.fi/URN:NBN:fi:schema:bffi:RecordingMethod">
    <dct:modified>2024-11-22 (New)</dct:modified>
    <rdfs:label xml:lang="en">Type of recording</rdfs:label>
    <rdfs:label xml:lang="fi">Äänen tallennustapa</rdfs:label>
    <bffi-meta:relatedValueVocabulary rdf:resource="http://urn.fi/URN:NBN:fi:au:mts:m645"/>
    <rdf:type rdf:resource="http://www.w3.org/2002/07/owl#Class"/>
    <owl:equivalentClass rdf:resource="http://id.loc.gov/ontologies/bibframe/RecordingMethod"/>
    <rdfs:subClassOf rdf:resource="http://urn.fi/URN:NBN:fi:schema:bffi:SoundCharacteristic"/>
    <skos:definition xml:lang="en">BIBFRAME definition: Method used to encode audio content for playback, e.g., analog, digital</skos:definition>
  </rdf:Description>
  <rdf:Description rdf:about="http://urn.fi/URN:NBN:fi:schema:bffi:systemRequirement">
    <dct:modified>2024-11-22 (New)</dct:modified>
    <rdfs:label xml:lang="en">equipment or system requirement</rdfs:label>
    <rdfs:label xml:lang="fi">laitteisto- tai järjestelmävaatimukset</rdfs:label>
    <rdfs:domain rdf:resource="http://urn.fi/URN:NBN:fi:schema:bffi:Manifestation"/>
    <rdfs:range rdf:resource="http://urn.fi/URN:NBN:fi:schema:bffi:SystemRequirement"/>
    <rdf:type rdf:resource="http://www.w3.org/2002/07/owl#ObjectProperty"/>
    <owl:equivalentProperty rdf:resource="http://id.loc.gov/ontologies/bibframe/systemRequirement"/>
    <skos:definition xml:lang="en">BIBFRAME definition: Equipment or system requirement beyond what is normal and obvious for the type of carrier or type of file, such as make and model of equipment or hardware, operating system, amount of memory, programming language, other necessary software, any plug-ins or peripherals required to play, view, or run the resource, etc.</skos:definition>
  </rdf:Description>
  <rdf:Description rdf:about="http://urn.fi/URN:NBN:fi:schema:bffi:TactileNotation">
    <dct:modified>2024-02-23 (New)</dct:modified>
    <rdfs:label xml:lang="en">Tactile notation</rdfs:label>
    <rdfs:label xml:lang="fi">Taktiili notaatio</rdfs:label>
    <bffi-meta:relatedValueVocabulary rdf:resource="http://urn.fi/URN:NBN:fi:au:mts:m2003"/>
    <rdf:type rdf:resource="http://www.w3.org/2002/07/owl#Class"/>
    <owl:equivalentClass rdf:resource="http://id.loc.gov/ontologies/bibframe/TactileNotation"/>
    <rdfs:seeAlso rdf:resource="http://rdaregistry.info/termList/TacNotation"/>
    <rdfs:subClassOf rdf:resource="http://urn.fi/URN:NBN:fi:schema:bffi:Notation"/>
    <skos:definition xml:lang="en">BIBFRAME definition: Information on the symbol system used to convey the content of a tactile resource</skos:definition>
  </rdf:Description>
  <rdf:Description rdf:about="http://urn.fi/URN:NBN:fi:schema:bffi:PlaybackChannels">
    <dct:modified>2024-11-22 (New)</dct:modified>
    <rdfs:label xml:lang="en">Configuration of playback channels</rdfs:label>
    <rdfs:label xml:lang="fi">Toistokanavien määrä</rdfs:label>
    <bffi-meta:relatedValueVocabulary rdf:resource="http://urn.fi/URN:NBN:fi:au:mts:m4574"/>
    <rdf:type rdf:resource="http://www.w3.org/2002/07/owl#Class"/>
    <owl:equivalentClass rdf:resource="http://id.loc.gov/ontologies/bibframe/PlaybackChannels"/>
    <rdfs:seeAlso rdf:resource="http://rdaregistry.info/termList/configPlayback/"/>
    <rdfs:subClassOf rdf:resource="http://urn.fi/URN:NBN:fi:schema:bffi:SoundCharacteristic"/>
    <skos:definition xml:lang="en">BIBFRAME definition: Configuration/number of sound channels used to make a recording, such as one channel for a monophonic recording, e.g., mono, stereo, quadraphonic, surround</skos:definition>
  </rdf:Description>
  <rdf:Description rdf:about="http://urn.fi/URN:NBN:fi:schema:bffi:ExtensionPlan">
    <dct:modified>2024-04-16 (New)</dct:modified>
    <rdfs:label xml:lang="en">Extension plan</rdfs:label>
    <rdfs:label xml:lang="fi">Laajennussuunnitelma</rdfs:label>
    <bffi-meta:relatedValueVocabulary rdf:resource="http://urn.fi/URN:NBN:fi:au:mts:m5119"/>
    <rdf:type rdf:resource="http://www.w3.org/2002/07/owl#Class"/>
    <bffi-meta:broadMatch rdf:resource="http://id.loc.gov/ontologies/bibframe/Issuance"/>
    <rdfs:seeAlso rdf:resource="http://rdaregistry.info/termList/RDAExtensionPlan"/>
  </rdf:Description>
  <rdf:Description rdf:nodeID="n3340e60e05a148bda7f556ae223dde3ab2">
    <rdf:first rdf:resource="http://urn.fi/URN:NBN:fi:schema:bffi:Work"/>
    <rdf:rest rdf:nodeID="n3340e60e05a148bda7f556ae223dde3ab3"/>
  </rdf:Description>
  <rdf:Description rdf:about="http://urn.fi/URN:NBN:fi:schema:bffi:RecordingSource">
    <dct:modified>2024-02-23 (New)</dct:modified>
    <rdfs:label xml:lang="en">Recording source</rdfs:label>
    <rdfs:label xml:lang="fi">Merkintälähde</rdfs:label>
    <bffi-meta:relatedValueVocabulary rdf:resource="http://urn.fi/URN:NBN:fi:au:mts:m5137"/>
    <rdf:type rdf:resource="http://www.w3.org/2002/07/owl#Class"/>
    <bffi-meta:broadMatch rdf:resource="http://id.loc.gov/ontologies/bibframe/Source"/>
    <rdfs:seeAlso rdf:resource="http://rdaregistry.info/termList/RDARecordingSources"/>
    <rdfs:subClassOf rdf:resource="http://urn.fi/URN:NBN:fi:schema:bffi:Source"/>
  </rdf:Description>
  <rdf:Description rdf:about="http://urn.fi/URN:NBN:fi:schema:bffi:creationDate">
    <dct:modified>2024-06-19 (New)</dct:modified>
    <rdfs:label xml:lang="en">description creation date</rdfs:label>
    <rdfs:label xml:lang="fi">kuvailun luontiajankohta</rdfs:label>
    <rdfs:domain rdf:resource="http://urn.fi/URN:NBN:fi:schema:bffi:AdminMetadata"/>
    <rdfs:range rdf:resource="http://www.w3.org/2000/01/rdf-schema#Literal"/>
    <rdf:type rdf:resource="http://www.w3.org/2002/07/owl#DatatypeProperty"/>
    <owl:equivalentProperty rdf:resource="http://id.loc.gov/ontologies/bibframe/creationDate"/>
    <bffi-meta:closeMatch rdf:resource="http://rdaregistry.info/Elements/m/P30011"/>
    <rdfs:subPropertyOf rdf:resource="http://urn.fi/URN:NBN:fi:schema:bffi:date"/>
    <skos:definition xml:lang="en">BIBFRAME definition: Date or date and time on which the original metadata first created</skos:definition>
  </rdf:Description>
  <rdf:Description rdf:about="http://urn.fi/URN:NBN:fi:schema:bffi:GenerationProcess">
    <dct:modified>2024-06-19 (New)</dct:modified>
    <rdfs:label xml:lang="en">Generation process</rdfs:label>
    <rdfs:label xml:lang="fi">Konversioprosessi</rdfs:label>
    <rdf:type rdf:resource="http://www.w3.org/2002/07/owl#Class"/>
    <owl:equivalentClass rdf:resource="http://id.loc.gov/ontologies/bibframe/GenerationProcess"/>
    <skos:definition xml:lang="en">BIBFRAME definition: Indication of the program or process used to generate the description by application of a particular transformation</skos:definition>
  </rdf:Description>
  <rdf:Description rdf:about="http://urn.fi/URN:NBN:fi:schema:bffi:adminMetadataFor">
    <dct:modified>2024-06-19 (New)</dct:modified>
    <rdfs:label xml:lang="en">administrative metadata for</rdfs:label>
    <rdfs:label xml:lang="fi">hallinnolliset metatiedot kohteelle</rdfs:label>
    <rdfs:domain rdf:resource="http://urn.fi/URN:NBN:fi:schema:bffi:AdminMetadata"/>
    <rdfs:range rdf:resource="http://www.w3.org/2000/01/rdf-schema#Resource"/>
    <rdf:type rdf:resource="http://www.w3.org/2002/07/owl#ObjectProperty"/>
    <owl:equivalentProperty rdf:resource="http://id.loc.gov/ontologies/bibframe/adminMetadataFor"/>
    <bffi-meta:closeMatch rdf:resource="http://rdaregistry.info/Elements/w/P10403"/>
    <skos:definition xml:lang="en">BIBFRAME definition: Relates an Administrative metadata resource to the resource it captures information about.</skos:definition>
  </rdf:Description>
  <rdf:Description rdf:nodeID="n096c0702f8c64e3bbe53573a59499c9ab3">
    <rdf:first rdf:resource="http://urn.fi/URN:NBN:fi:schema:bffi:NonMusicAudioExpression"/>
    <rdf:rest rdf:nodeID="n096c0702f8c64e3bbe53573a59499c9ab4"/>
  </rdf:Description>
  <rdf:Description rdf:about="http://urn.fi/URN:NBN:fi:schema:bffi:extent">
    <dct:modified>2024-02-23 (New)</dct:modified>
    <rdfs:label xml:lang="en">extent</rdfs:label>
    <rdfs:label xml:lang="fi">laajuus</rdfs:label>
    <rdfs:domain rdf:resource="http://www.w3.org/2000/01/rdf-schema#Resource"/>
    <rdfs:range rdf:resource="http://urn.fi/URN:NBN:fi:schema:bffi:Extent"/>
    <rdf:type rdf:resource="http://www.w3.org/2002/07/owl#ObjectProperty"/>
    <owl:equivalentProperty rdf:resource="http://id.loc.gov/ontologies/bibframe/extent"/>
    <bffi-meta:narrowMatch rdf:resource="http://rdaregistry.info/Elements/e/P20321"/>
    <bffi-meta:narrowMatch rdf:resource="http://rdaregistry.info/Elements/m/P30182"/>
    <skos:definition xml:lang="en">BIBFRAME definition: Number and type of units and/or subunits making up a resource.</skos:definition>
  </rdf:Description>
  <rdf:Description rdf:about="http://urn.fi/URN:NBN:fi:schema:bffi:note">
    <dct:modified>2024-02-23 (New)</dct:modified>
    <rdfs:label xml:lang="en">note</rdfs:label>
    <rdfs:label xml:lang="fi">huomautus</rdfs:label>
    <rdfs:domain rdf:resource="http://www.w3.org/2000/01/rdf-schema#Resource"/>
    <rdfs:range rdf:resource="http://urn.fi/URN:NBN:fi:schema:bffi:Note"/>
    <rdf:type rdf:resource="http://www.w3.org/2002/07/owl#ObjectProperty"/>
    <bffi-meta:narrowMatch rdf:resource="http://rdaregistry.info/Elements/w/P10330"/>
    <bffi-meta:narrowMatch rdf:resource="http://rdaregistry.info/Elements/w/P10402"/>
    <bffi-meta:narrowMatch rdf:resource="http://rdaregistry.info/Elements/e/P20071"/>
    <bffi-meta:narrowMatch rdf:resource="http://rdaregistry.info/Elements/m/P30137"/>
    <bffi-meta:narrowMatch rdf:resource="http://rdaregistry.info/Elements/i/P40028"/>
    <rdfs:subPropertyOf rdf:resource="http://id.loc.gov/ontologies/bibframe/note"/>
  </rdf:Description>
  <rdf:Description rdf:about="http://urn.fi/URN:NBN:fi:schema:bffi:titleOf">
    <owl:inverseOf rdf:resource="http://urn.fi/URN:NBN:fi:schema:bffi:title"/>
    <dct:modified>2024-02-23 (New)</dct:modified>
    <rdfs:label xml:lang="en">title of</rdfs:label>
    <rdfs:label xml:lang="fi">nimekkeenä</rdfs:label>
    <rdfs:domain rdf:resource="http://urn.fi/URN:NBN:fi:schema:bffi:Title"/>
    <rdfs:range rdf:nodeID="n0d5ef643a16a443a8864901b85eb32dbb1"/>
    <rdf:type rdf:resource="http://www.w3.org/2002/07/owl#ObjectProperty"/>
    <owl:equivalentProperty rdf:resource="http://id.loc.gov/ontologies/bibframe/titleOf"/>
    <bffi-meta:narrowMatch rdf:resource="http://rdaregistry.info/Elements/n/P80064"/>
    <bffi-meta:narrowMatch rdf:resource="http://rdaregistry.info/Elements/n/P80039"/>
    <bffi-meta:narrowMatch rdf:resource="http://rdaregistry.info/Elements/n/P80062"/>
    <bffi-meta:narrowMatch rdf:resource="http://rdaregistry.info/Elements/n/P80017"/>
    <skos:definition xml:lang="en">BIBFRAME definition: Relates a title resource to that which it is the title of.</skos:definition>
  </rdf:Description>
  <rdf:Description rdf:about="http://urn.fi/URN:NBN:fi:schema:bffi:Generation">
    <dct:modified>2024-09-16 (New)</dct:modified>
    <rdfs:label xml:lang="en">Generation</rdfs:label>
    <rdfs:label xml:lang="fi">Sukupolvi</rdfs:label>
    <bffi-meta:relatedValueVocabulary rdf:resource="http://urn.fi/URN:NBN:fi:au:mts:m245"/>
    <rdf:type rdf:resource="http://www.w3.org/2002/07/owl#Class"/>
    <owl:equivalentClass rdf:resource="http://id.loc.gov/ontologies/bibframe/Generation"/>
    <rdfs:seeAlso rdf:resource="http://rdaregistry.info/termList/RDAGeneration/"/>
    <skos:definition xml:lang="en">BIBFRAME definition: Relationship between an original carrier and the carrier of a reproduction made from the original</skos:definition>
  </rdf:Description>
  <rdf:Description rdf:nodeID="n9f671517b9dd4b7c955826691e2215f4b3">
    <rdf:first rdf:resource="http://urn.fi/URN:NBN:fi:schema:bffi:Expression"/>
    <rdf:rest rdf:nodeID="n9f671517b9dd4b7c955826691e2215f4b4"/>
  </rdf:Description>
  <rdf:Description rdf:about="http://urn.fi/URN:NBN:fi:schema:bffi:media">
    <dct:modified>2024-02-23 (New)</dct:modified>
    <rdfs:label xml:lang="en">media type</rdfs:label>
    <rdfs:label xml:lang="fi">mediatyyppi</rdfs:label>
    <rdfs:domain rdf:resource="http://urn.fi/URN:NBN:fi:schema:bffi:Manifestation"/>
    <rdfs:range rdf:resource="http://urn.fi/URN:NBN:fi:schema:bffi:Media"/>
    <rdf:type rdf:resource="http://www.w3.org/2002/07/owl#ObjectProperty"/>
    <owl:equivalentProperty rdf:resource="http://id.loc.gov/ontologies/bibframe/media"/>
    <bffi-meta:exactMatch rdf:resource="http://rdaregistry.info/Elements/m/P30002"/>
    <skos:definition xml:lang="en">BIBFRAME definition: Categorization reflecting the general type of intermediation device required to view, play, run, etc., the content of a resource.</skos:definition>
  </rdf:Description>
  <rdf:Description rdf:about="http://urn.fi/URN:NBN:fi:schema:bffi:timePeriodOfCreation">
    <dct:modified>2025-01-02 (New)</dct:modified>
    <rdfs:label xml:lang="en">time period of creation</rdfs:label>
    <rdfs:label xml:lang="fi">teoksen luomisaika</rdfs:label>
    <rdfs:domain rdf:resource="http://urn.fi/URN:NBN:fi:schema:bffi:Work"/>
    <rdfs:range rdf:resource="http://urn.fi/URN:NBN:fi:schema:bffi:Temporal"/>
    <rdf:type rdf:resource="http://www.w3.org/2002/07/owl#ObjectProperty"/>
    <bffi-meta:closeMatch rdf:resource="http://id.loc.gov/ontologies/bibframe/originDate"/>
    <bffi-meta:closeMatch rdf:resource="http://rdaregistry.info/Elements/w/P10219"/>
  </rdf:Description>
  <rdf:Description rdf:about="http://urn.fi/URN:NBN:fi:schema:bffi:historyOfWork">
    <dct:modified>2024-02-23 (New)</dct:modified>
    <rdfs:label xml:lang="en">history of the work</rdfs:label>
    <rdfs:label xml:lang="fi">teoksen historia</rdfs:label>
    <rdfs:domain rdf:resource="http://urn.fi/URN:NBN:fi:schema:bffi:Work"/>
    <rdfs:range rdf:resource="http://www.w3.org/2000/01/rdf-schema#Literal"/>
    <rdf:type rdf:resource="http://www.w3.org/2002/07/owl#DatatypeProperty"/>
    <owl:equivalentProperty rdf:resource="http://id.loc.gov/ontologies/bibframe/historyOfWork"/>
    <bffi-meta:exactMatch rdf:resource="http://rdaregistry.info/Elements/w/P10210"/>
    <skos:definition xml:lang="en">BIBFRAME definition: Information about the history of a Work.</skos:definition>
  </rdf:Description>
  <rdf:Description rdf:about="http://urn.fi/URN:NBN:fi:schema:bffi:DescriptionLevel">
    <dct:modified>2024-06-19 (New)</dct:modified>
    <rdfs:label xml:lang="en">Description level</rdfs:label>
    <rdfs:label xml:lang="fi">Kuvailun tietomalli</rdfs:label>
    <rdf:type rdf:resource="http://www.w3.org/2002/07/owl#Class"/>
    <owl:equivalentClass rdf:resource="http://id.loc.gov/ontologies/bibframe/DescriptionLevel"/>
    <skos:definition xml:lang="en">BIBFRAME definition: Designation of the descriptive content of the metadata</skos:definition>
  </rdf:Description>
  <rdf:Description rdf:about="http://urn.fi/URN:NBN:fi:schema:bffi:partName">
    <dct:modified>2024-02-23 (New)</dct:modified>
    <rdfs:label xml:lang="en">part title</rdfs:label>
    <rdfs:label xml:lang="fi">osan nimeke</rdfs:label>
    <rdfs:domain rdf:resource="http://urn.fi/URN:NBN:fi:schema:bffi:Title"/>
    <rdfs:range rdf:resource="http://www.w3.org/2000/01/rdf-schema#Literal"/>
    <rdf:type rdf:resource="http://www.w3.org/2002/07/owl#DatatypeProperty"/>
    <owl:equivalentProperty rdf:resource="http://id.loc.gov/ontologies/bibframe/partName"/>
    <skos:definition xml:lang="en">BIBFRAME definition: Part or section name of a title. Possible title component.</skos:definition>
  </rdf:Description>
  <rdf:Description rdf:about="http://urn.fi/URN:NBN:fi:schema:bffi:spanEnd">
    <dct:modified>2024-06-19 (New)</dct:modified>
    <rdfs:label xml:lang="en">classification number span end</rdfs:label>
    <rdfs:label xml:lang="fi">luokan loppunumero</rdfs:label>
    <rdfs:domain rdf:resource="http://urn.fi/URN:NBN:fi:schema:bffi:Classification"/>
    <rdfs:range rdf:resource="http://www.w3.org/2000/01/rdf-schema#Literal"/>
    <rdf:type rdf:resource="http://www.w3.org/2002/07/owl#DatatypeProperty"/>
    <owl:equivalentProperty rdf:resource="http://id.loc.gov/ontologies/bibframe/spanEnd"/>
    <skos:definition xml:lang="en">BIBFRAME definition: Ending number of classification number span.</skos:definition>
  </rdf:Description>
  <rdf:Description rdf:about="http://urn.fi/URN:NBN:fi:schema:bffi:AggregatingExpression">
    <dct:modified>2024-02-23 (New)</dct:modified>
    <rdfs:label xml:lang="en">Aggregating expression</rdfs:label>
    <rdfs:label xml:lang="fi">Aggregoiva ekspressio</rdfs:label>
    <rdf:type rdf:resource="http://www.w3.org/2002/07/owl#Class"/>
    <bffi-meta:broadMatch rdf:resource="http://id.loc.gov/ontologies/bibframe/Work"/>
    <rdfs:subClassOf rdf:resource="http://urn.fi/URN:NBN:fi:schema:bffi:Expression"/>
  </rdf:Description>
  <rdf:Description rdf:nodeID="n0d5ef643a16a443a8864901b85eb32dbb5">
    <rdf:first rdf:resource="http://urn.fi/URN:NBN:fi:schema:bffi:Item"/>
    <rdf:rest rdf:resource="http://www.w3.org/1999/02/22-rdf-syntax-ns#nil"/>
  </rdf:Description>
  <rdf:Description rdf:about="http://urn.fi/URN:NBN:fi:schema:bffi:Tactile">
    <dct:modified>2024-09-16 (New)</dct:modified>
    <rdfs:label xml:lang="en">Tactile material</rdfs:label>
    <rdfs:label xml:lang="fi">Taktiili</rdfs:label>
    <rdf:type rdf:resource="http://www.w3.org/2002/07/owl#Class"/>
    <owl:equivalentClass rdf:resource="http://id.loc.gov/ontologies/bibframe/Tactile"/>
    <rdfs:subClassOf rdf:resource="http://urn.fi/URN:NBN:fi:schema:bffi:Manifestation"/>
    <skos:definition xml:lang="en">BIBFRAME definition: Resource that is intended to be perceived by touch</skos:definition>
  </rdf:Description>
  <rdf:Description rdf:about="http://urn.fi/URN:NBN:fi:schema:bffi:descriptionAuthentication">
    <dct:modified>2024-06-19 (New)</dct:modified>
    <rdfs:label xml:lang="en">description authentication</rdfs:label>
    <rdfs:label xml:lang="fi">autentikointikoodi</rdfs:label>
    <rdfs:domain rdf:resource="http://urn.fi/URN:NBN:fi:schema:bffi:AdminMetadata"/>
    <rdfs:range rdf:resource="http://urn.fi/URN:NBN:fi:schema:bffi:DescriptionAuthentication"/>
    <rdf:type rdf:resource="http://www.w3.org/2002/07/owl#ObjectProperty"/>
    <owl:equivalentProperty rdf:resource="http://id.loc.gov/ontologies/bibframe/descriptionAuthentication"/>
    <skos:definition xml:lang="en">BIBFRAME definition: Indication of specific types of reviews that have been carried out on the description information</skos:definition>
  </rdf:Description>
  <rdf:Description rdf:about="http://urn.fi/URN:NBN:fi:schema:bffi:source">
    <dct:modified>2024-02-23 (New)</dct:modified>
    <rdfs:label xml:lang="en">source</rdfs:label>
    <rdfs:label xml:lang="fi">lähde</rdfs:label>
    <rdfs:domain rdf:resource="http://www.w3.org/2000/01/rdf-schema#Resource"/>
    <rdfs:range rdf:resource="http://urn.fi/URN:NBN:fi:schema:bffi:Source"/>
    <rdf:type rdf:resource="http://www.w3.org/2002/07/owl#ObjectProperty"/>
    <bffi-meta:narrowMatch rdf:resource="http://rdaregistry.info/Elements/n/P80139"/>
    <rdfs:subPropertyOf rdf:resource="http://id.loc.gov/ontologies/bibframe/source"/>
  </rdf:Description>
  <rdf:Description rdf:about="http://urn.fi/URN:NBN:fi:schema:bffi:Text">
    <dct:modified>2024-02-23 (New)</dct:modified>
    <rdfs:label xml:lang="en">Text</rdfs:label>
    <rdfs:label xml:lang="fi">Teksti</rdfs:label>
    <rdf:type rdf:resource="http://www.w3.org/2002/07/owl#Class"/>
    <owl:equivalentClass rdf:resource="http://id.loc.gov/ontologies/bibframe/Text"/>
    <rdfs:seeAlso rdf:resource="http://rdaregistry.info/termList/RDAContentType/1020"/>
    <rdfs:subClassOf rdf:resource="http://urn.fi/URN:NBN:fi:schema:bffi:Expression"/>
    <skos:definition xml:lang="en">BIBFRAME definition: Resource intended to be perceived visually and understood through the use of language in written or spoken form</skos:definition>
  </rdf:Description>
  <rdf:Description rdf:about="http://urn.fi/URN:NBN:fi:schema:bffi:Title">
    <dct:modified>2024-02-23 (New)</dct:modified>
    <rdfs:label xml:lang="en">Title entity</rdfs:label>
    <rdfs:label xml:lang="fi">Nimeke</rdfs:label>
    <rdf:type rdf:resource="http://www.w3.org/2002/07/owl#Class"/>
    <owl:equivalentClass rdf:resource="http://id.loc.gov/ontologies/bibframe/Title"/>
    <skos:definition xml:lang="en">BIBFRAME definition: Title information relating to a resource: work title, preferred title, instance title, transcribed title, translated title, variant form of title, etc.</skos:definition>
  </rdf:Description>
  <rdf:Description rdf:about="http://urn.fi/URN:NBN:fi:schema:bffi:firstIssue">
    <dct:modified>2024-02-23 (New)</dct:modified>
    <rdfs:label xml:lang="en">multipart first issue</rdfs:label>
    <rdfs:label xml:lang="fi">ensimmäinen numero</rdfs:label>
    <rdfs:domain rdf:resource="http://urn.fi/URN:NBN:fi:schema:bffi:Manifestation"/>
    <rdfs:range rdf:resource="http://www.w3.org/2000/01/rdf-schema#Literal"/>
    <rdf:type rdf:resource="http://www.w3.org/2002/07/owl#DatatypeProperty"/>
    <owl:equivalentProperty rdf:resource="http://id.loc.gov/ontologies/bibframe/firstIssue"/>
    <skos:definition xml:lang="en">BIBFRAME definition: Beginning date of a resource and/or the sequential designations.</skos:definition>
  </rdf:Description>
  <rdf:Description rdf:about="http://urn.fi/URN:NBN:fi:schema:bffi:FileType">
    <dct:modified>2024-09-16 (New)</dct:modified>
    <rdfs:label xml:lang="en">File type</rdfs:label>
    <rdfs:label xml:lang="fi">Tiedostotyyppi</rdfs:label>
    <bffi-meta:relatedValueVocabulary rdf:resource="http://urn.fi/URN:NBN:fi:au:mts:m537"/>
    <rdf:type rdf:resource="http://www.w3.org/2002/07/owl#Class"/>
    <owl:equivalentClass rdf:resource="http://id.loc.gov/ontologies/bibframe/FileType"/>
    <rdfs:seeAlso rdf:resource="http://rdaregistry.info/termList/fileType/"/>
    <rdfs:subClassOf rdf:resource="http://urn.fi/URN:NBN:fi:schema:bffi:DigitalCharacteristic"/>
    <skos:definition xml:lang="en">BIBFRAME definition: General type of data content encoded in a computer file, e.g., text file, audio file</skos:definition>
  </rdf:Description>
  <rdf:Description rdf:about="http://urn.fi/URN:NBN:fi:schema:bffi:adminMetadata">
    <dct:modified>2024-06-19 (New)</dct:modified>
    <rdfs:label xml:lang="en">administrative metadata</rdfs:label>
    <rdfs:label xml:lang="fi">hallinnolliset metatiedot</rdfs:label>
    <rdfs:domain rdf:resource="http://www.w3.org/2000/01/rdf-schema#Resource"/>
    <rdfs:range rdf:resource="http://urn.fi/URN:NBN:fi:schema:bffi:AdminMetadata"/>
    <rdf:type rdf:resource="http://www.w3.org/2002/07/owl#ObjectProperty"/>
    <owl:equivalentProperty rdf:resource="http://id.loc.gov/ontologies/bibframe/adminMetadata"/>
    <skos:definition xml:lang="en">BIBFRAME definition: Metadata about the metadata, especially provenance information.</skos:definition>
  </rdf:Description>
  <rdf:Description rdf:about="http://urn.fi/URN:NBN:fi:schema:bffi:locationOfCollection">
    <dct:modified>2024-04-16 (New)</dct:modified>
    <rdfs:label xml:lang="en">location of collection</rdfs:label>
    <rdfs:label xml:lang="fi">kokoelman sijainti</rdfs:label>
    <rdfs:domain rdf:resource="http://urn.fi/URN:NBN:fi:schema:bffi:CollectionManifestation"/>
    <rdfs:range rdf:resource="http://urn.fi/URN:NBN:fi:schema:bffi:Place"/>
    <rdf:type rdf:resource="http://www.w3.org/2002/07/owl#ObjectProperty"/>
    <bffi-meta:broadMatch rdf:resource="http://id.loc.gov/ontologies/bibframe/place"/>
    <bffi-meta:exactMatch rdf:resource="http://rdaregistry.info/Elements/m/P30461"/>
    <rdfs:subPropertyOf rdf:resource="http://urn.fi/URN:NBN:fi:schema:bffi:place"/>
  </rdf:Description>
  <rdf:Description rdf:about="http://urn.fi/URN:NBN:fi:schema:bffi:ContentAccessibility">
    <dct:modified>2024-09-16 (New)</dct:modified>
    <rdfs:label xml:lang="en">Content accessibility information</rdfs:label>
    <rdfs:label xml:lang="fi">Saavutettavuussisältö</rdfs:label>
    <rdf:type rdf:resource="http://www.w3.org/2002/07/owl#Class"/>
    <owl:equivalentClass rdf:resource="http://id.loc.gov/ontologies/bibframe/ContentAccessibility"/>
    <skos:definition xml:lang="en">BIBFRAME definition: Information that assists those with a sensory impairment for greater understanding of content, e.g., captions</skos:definition>
  </rdf:Description>
  <rdf:Description rdf:about="http://urn.fi/URN:NBN:fi:schema:bffi:distributionStatement">
    <dct:modified>2024-09-16 (New)</dct:modified>
    <rdfs:label xml:lang="en">distribution statement</rdfs:label>
    <rdfs:label xml:lang="fi">jakelumerkintö</rdfs:label>
    <rdfs:domain rdf:resource="http://urn.fi/URN:NBN:fi:schema:bffi:Manifestation"/>
    <rdfs:range rdf:resource="http://www.w3.org/2000/01/rdf-schema#Literal"/>
    <rdf:type rdf:resource="http://www.w3.org/2002/07/owl#DatatypeProperty"/>
    <owl:equivalentProperty rdf:resource="http://id.loc.gov/ontologies/bibframe/distributionStatement"/>
    <bffi-meta:exactMatch rdf:resource="http://rdaregistry.info/Elements/m/P30108"/>
    <skos:definition xml:lang="en">BIBFRAME definition: Statement related to the distribution of the resources; usually transcribed.</skos:definition>
  </rdf:Description>
  <rdf:Description rdf:about="http://urn.fi/URN:NBN:fi:schema:bffi:aspectRatioOfRepresentativeExpression">
    <dct:modified>2024-11-22 (New)</dct:modified>
    <rdfs:label xml:lang="en">aspect ratio of representative expression</rdfs:label>
    <rdfs:label xml:lang="fi">edustavan ekspression kuvasuhde</rdfs:label>
    <rdfs:domain rdf:resource="http://urn.fi/URN:NBN:fi:schema:bffi:MovingImageWork"/>
    <rdfs:range rdf:resource="http://urn.fi/URN:NBN:fi:schema:bffi:AspectRatio"/>
    <rdf:type rdf:resource="http://www.w3.org/2002/07/owl#ObjectProperty"/>
    <bffi-meta:exactMatch rdf:resource="http://rdaregistry.info/Elements/w/P10347"/>
    <rdfs:subPropertyOf rdf:resource="http://id.loc.gov/ontologies/bibframe/aspectRatio"/>
  </rdf:Description>
  <rdf:Description rdf:about="http://urn.fi/URN:NBN:fi:schema:bffi:Summary">
    <dct:modified>2024-02-23 (New)</dct:modified>
    <rdfs:label xml:lang="en">Summary</rdfs:label>
    <rdfs:label xml:lang="fi">Sisällön yhteenveto</rdfs:label>
    <rdf:type rdf:resource="http://www.w3.org/2002/07/owl#Class"/>
    <owl:equivalentClass rdf:resource="http://id.loc.gov/ontologies/bibframe/Summary"/>
    <skos:definition xml:lang="en">BIBFRAME definition: Description of the content of a resource, such as an abstract, summary, etc.</skos:definition>
  </rdf:Description>
  <rdf:Description rdf:about="http://urn.fi/URN:NBN:fi:schema:bffi:CoverArt">
    <dct:modified>2024-02-23 (New)</dct:modified>
    <rdfs:label xml:lang="en">Cover art</rdfs:label>
    <rdfs:label xml:lang="fi">Kansikuva</rdfs:label>
    <rdf:type rdf:resource="http://www.w3.org/2002/07/owl#Class"/>
    <owl:equivalentClass rdf:resource="http://id.loc.gov/ontologies/bibframe/CoverArt"/>
    <skos:definition xml:lang="en">BIBFRAME definition: Cover illustration of a resource</skos:definition>
  </rdf:Description>
  <rdf:Description rdf:about="http://urn.fi/URN:NBN:fi:schema:bffi:generationProcess">
    <dct:modified>2024-06-19 (New)</dct:modified>
    <rdfs:label xml:lang="en">generation process</rdfs:label>
    <rdfs:label xml:lang="fi">konversioprosessi</rdfs:label>
    <rdfs:domain rdf:resource="http://urn.fi/URN:NBN:fi:schema:bffi:AdminMetadata"/>
    <rdfs:range rdf:resource="http://urn.fi/URN:NBN:fi:schema:bffi:GenerationProcess"/>
    <rdf:type rdf:resource="http://www.w3.org/2002/07/owl#ObjectProperty"/>
    <owl:equivalentProperty rdf:resource="http://id.loc.gov/ontologies/bibframe/generationProcess"/>
    <skos:definition xml:lang="en">BIBFRAME definition: Indication of the program or process used to generate the description by application of a particular transformation</skos:definition>
  </rdf:Description>
  <rdf:Description rdf:about="http://urn.fi/URN:NBN:fi:schema:bffi:TapeConfig">
    <dct:modified>2024-11-22 (New)</dct:modified>
    <rdfs:label xml:lang="en">Tape configuration</rdfs:label>
    <rdfs:label xml:lang="fi">Ääninauhan raitojen määrä</rdfs:label>
    <bffi-meta:relatedValueVocabulary rdf:resource="http://urn.fi/URN:NBN:fi:au:mts:m1079"/>
    <rdf:type rdf:resource="http://www.w3.org/2002/07/owl#Class"/>
    <owl:equivalentClass rdf:resource="http://id.loc.gov/ontologies/bibframe/TapeConfig"/>
    <rdfs:subClassOf rdf:resource="http://urn.fi/URN:NBN:fi:schema:bffi:SoundCharacteristic"/>
    <skos:definition xml:lang="en">BIBFRAME definition: Number of tracks on an audiotape, e.g., 12 track</skos:definition>
  </rdf:Description>
  <rdf:Description rdf:about="http://urn.fi/URN:NBN:fi:schema:bffi:Relation">
    <dct:modified>2024-09-16 (New)</dct:modified>
    <rdfs:label xml:lang="en">Relation</rdfs:label>
    <rdfs:label xml:lang="fi">Suhde</rdfs:label>
    <rdf:type rdf:resource="http://www.w3.org/2002/07/owl#Class"/>
    <owl:equivalentClass rdf:resource="http://id.loc.gov/ontologies/bibframe/Relation"/>
    <skos:definition xml:lang="en">BIBFRAME definition: Associated resource and its relationship to the resource being described</skos:definition>
  </rdf:Description>
  <rdf:Description rdf:about="http://urn.fi/URN:NBN:fi:schema:bffi:Manufacture">
    <dct:modified>2024-02-23 (New)</dct:modified>
    <rdfs:label xml:lang="en">Manufacturer</rdfs:label>
    <rdfs:label xml:lang="fi">Valmistaja</rdfs:label>
    <rdf:type rdf:resource="http://www.w3.org/2002/07/owl#Class"/>
    <owl:equivalentClass rdf:resource="http://id.loc.gov/ontologies/bibframe/Manufacture"/>
    <bffi-meta:broadMatch rdf:resource="http://rdaregistry.info/Elements/c/C10005"/>
    <rdfs:subClassOf rdf:resource="http://urn.fi/URN:NBN:fi:schema:bffi:ProvisionActivity"/>
    <skos:definition xml:lang="en">BIBFRAME definition: Information relating to manufacture of a resource</skos:definition>
  </rdf:Description>
  <rdf:Description rdf:about="http://urn.fi/URN:NBN:fi:schema:bffi:collectionOrganization">
    <dct:modified>2024-04-16 (New)</dct:modified>
    <rdfs:label xml:lang="en">organization of material</rdfs:label>
    <rdfs:label xml:lang="fi">aineiston ryhmittely</rdfs:label>
    <rdfs:domain rdf:resource="http://urn.fi/URN:NBN:fi:schema:bffi:CollectionArrangement"/>
    <rdfs:range rdf:resource="http://www.w3.org/2000/01/rdf-schema#Literal"/>
    <rdf:type rdf:resource="http://www.w3.org/2002/07/owl#DatatypeProperty"/>
    <owl:equivalentProperty rdf:resource="http://id.loc.gov/ontologies/bibframe/collectionOrganization"/>
    <skos:definition xml:lang="en">BIBFRAME definition: Manner in which the resource is divided into smaller units.</skos:definition>
  </rdf:Description>
  <rdf:Description rdf:about="http://urn.fi/URN:NBN:fi:schema:bffi:Manifestation">
    <dct:modified>2024-02-23 (New)</dct:modified>
    <rdfs:label xml:lang="en">Manifestation</rdfs:label>
    <rdfs:label xml:lang="fi">Manifestaatio</rdfs:label>
    <rdf:type rdf:resource="http://www.w3.org/2002/07/owl#Class"/>
    <owl:equivalentClass rdf:resource="http://id.loc.gov/ontologies/bibframe/Instance"/>
    <bffi-meta:exactMatch rdf:resource="http://rdaregistry.info/Elements/c/C10007"/>
    <skos:definition xml:lang="en">BIBFRAME definition: Resource reflecting an individual, material embodiment of a Work</skos:definition>
  </rdf:Description>
  <rdf:Description rdf:about="http://urn.fi/URN:NBN:fi:schema:bffi:MovingImageWork">
    <owl:disjointWith rdf:resource="http://urn.fi/URN:NBN:fi:schema:bffi:MovingImageExpression"/>
    <dct:modified>2024-02-23 (New)</dct:modified>
    <rdfs:label xml:lang="en">Moving image work</rdfs:label>
    <rdfs:label xml:lang="fi">Liikkuvan kuvan teos</rdfs:label>
    <rdf:type rdf:resource="http://www.w3.org/2002/07/owl#Class"/>
    <bffi-meta:broadMatch rdf:resource="http://id.loc.gov/ontologies/bibframe/MovingImage"/>
    <rdfs:subClassOf rdf:resource="http://urn.fi/URN:NBN:fi:schema:bffi:Work"/>
  </rdf:Description>
  <rdf:Description rdf:about="http://urn.fi/URN:NBN:fi:schema:bffi:Topic">
    <dct:modified>2024-02-23 (New)</dct:modified>
    <rdfs:label xml:lang="en">Topic</rdfs:label>
    <rdfs:label xml:lang="fi">Aihe</rdfs:label>
    <rdf:type rdf:resource="http://www.w3.org/2002/07/owl#Class"/>
    <owl:equivalentClass rdf:resource="http://id.loc.gov/ontologies/bibframe/Topic"/>
    <skos:definition xml:lang="en">BIBFRAME definition: Concept or area of knowledge</skos:definition>
  </rdf:Description>
  <rdf:Description rdf:about="http://urn.fi/URN:NBN:fi:schema:bffi:content">
    <dct:modified>2024-02-23 (New)</dct:modified>
    <rdfs:label xml:lang="en">content type</rdfs:label>
    <rdfs:label xml:lang="fi">sisältötyyppi</rdfs:label>
    <rdfs:domain rdf:resource="http://urn.fi/URN:NBN:fi:schema:bffi:Expression"/>
    <rdfs:range rdf:resource="http://urn.fi/URN:NBN:fi:schema:bffi:Content"/>
    <bffi-meta:relatedValueVocabulary rdf:resource="http://urn.fi/URN:NBN:fi:au:mts:m346"/>
    <rdf:type rdf:resource="http://www.w3.org/2002/07/owl#ObjectProperty"/>
    <bffi-meta:exactMatch rdf:resource="http://rdaregistry.info/Elements/e/P20001"/>
    <rdfs:subPropertyOf rdf:resource="http://id.loc.gov/ontologies/bibframe/content"/>
  </rdf:Description>
  <rdf:Description rdf:about="http://urn.fi/URN:NBN:fi:schema:bffi:immediateAcquisition">
    <dct:modified>2024-04-16 (New)</dct:modified>
    <rdfs:label xml:lang="en">immediate acquisition</rdfs:label>
    <rdfs:label xml:lang="fi">kokoelman kartuttamisen menetelmä</rdfs:label>
    <rdfs:domain rdf:resource="http://urn.fi/URN:NBN:fi:schema:bffi:Item"/>
    <rdfs:range rdf:resource="http://urn.fi/URN:NBN:fi:schema:bffi:ImmediateAcquisition"/>
    <rdf:type rdf:resource="http://www.w3.org/2002/07/owl#ObjectProperty"/>
    <owl:equivalentProperty rdf:resource="http://id.loc.gov/ontologies/bibframe/immediateAcquisition"/>
    <bffi-meta:exactMatch rdf:resource="http://rdaregistry.info/Elements/i/P40050"/>
    <skos:definition xml:lang="en">BIBFRAME definition: Information about the circumstances, e.g., source, date, method, under which the resource was directly acquired.</skos:definition>
  </rdf:Description>
  <rdf:Description rdf:about="http://urn.fi/URN:NBN:fi:schema:bffi:credits">
    <dct:modified>2024-06-19 (New)</dct:modified>
    <rdfs:label xml:lang="en">credits note</rdfs:label>
    <rdfs:label xml:lang="fi">huomautus esittäjistä ja tuotantoon osallistujista</rdfs:label>
    <rdfs:domain rdf:resource="http://urn.fi/URN:NBN:fi:schema:bffi:Manifestation"/>
    <rdfs:range rdf:resource="http://www.w3.org/2000/01/rdf-schema#Literal"/>
    <rdf:type rdf:resource="http://www.w3.org/2002/07/owl#DatatypeProperty"/>
    <bffi-meta:closeMatch rdf:resource="http://rdaregistry.info/Elements/m/P30057"/>
    <rdfs:subPropertyOf rdf:resource="http://id.loc.gov/ontologies/bibframe/credits"/>
  </rdf:Description>
  <rdf:Description rdf:about="http://urn.fi/URN:NBN:fi:schema:bffi:count">
    <dct:modified>2025-01-02 (New)</dct:modified>
    <rdfs:label xml:lang="en">number of units</rdfs:label>
    <rdfs:label xml:lang="fi">lukumäärä</rdfs:label>
    <rdfs:domain rdf:resource="http://www.w3.org/2000/01/rdf-schema#Resource"/>
    <rdfs:range rdf:resource="http://www.w3.org/2000/01/rdf-schema#Literal"/>
    <rdf:type rdf:resource="http://www.w3.org/2002/07/owl#DatatypeProperty"/>
    <owl:equivalentProperty rdf:resource="http://id.loc.gov/ontologies/bibframe/count"/>
    <skos:definition xml:lang="en">BIBFRAME definition: Number associated with a measure of units, such as the number of units and/or subunits making up a resource.</skos:definition>
  </rdf:Description>
  <rdf:Description rdf:about="http://urn.fi/URN:NBN:fi:schema:bffi:generationDate">
    <dct:modified>2024-06-19 (New)</dct:modified>
    <rdfs:label xml:lang="en">date generated</rdfs:label>
    <rdfs:label xml:lang="fi">konversioajankohta</rdfs:label>
    <rdfs:domain rdf:resource="http://urn.fi/URN:NBN:fi:schema:bffi:AdminMetadata"/>
    <rdfs:range rdf:resource="http://www.w3.org/2000/01/rdf-schema#Literal"/>
    <rdf:type rdf:resource="http://www.w3.org/2002/07/owl#DatatypeProperty"/>
    <owl:equivalentProperty rdf:resource="http://id.loc.gov/ontologies/bibframe/generationDate"/>
    <rdfs:subPropertyOf rdf:resource="http://urn.fi/URN:NBN:fi:schema:bffi:date"/>
    <skos:definition xml:lang="en">BIBFRAME definition: Date of conversion of the metadata from another format</skos:definition>
  </rdf:Description>
  <rdf:Description rdf:about="http://urn.fi/URN:NBN:fi:schema:bffi:GeographicCoverage">
    <dct:modified>2025-01-02 (New)</dct:modified>
    <rdfs:label xml:lang="en">Geographic coverage</rdfs:label>
    <rdfs:label xml:lang="fi">Maantieteellinen kattavuus</rdfs:label>
    <rdf:type rdf:resource="http://www.w3.org/2002/07/owl#Class"/>
    <owl:equivalentClass rdf:resource="http://id.loc.gov/ontologies/bibframe/GeographicCoverage"/>
    <skos:definition xml:lang="en">BIBFRAME definition: Geographic coverage of the content of the resource</skos:definition>
  </rdf:Description>
  <rdf:Description rdf:about="http://urn.fi/URN:NBN:fi:schema:bffi:polarity">
    <dct:modified>2024-09-16 (New)</dct:modified>
    <rdfs:label xml:lang="en">polarity</rdfs:label>
    <rdfs:label xml:lang="fi">polariteetti</rdfs:label>
    <rdfs:domain rdf:resource="http://urn.fi/URN:NBN:fi:schema:bffi:Manifestation"/>
    <rdfs:range rdf:resource="http://urn.fi/URN:NBN:fi:schema:bffi:Polarity"/>
    <rdf:type rdf:resource="http://www.w3.org/2002/07/owl#ObjectProperty"/>
    <owl:equivalentProperty rdf:resource="http://id.loc.gov/ontologies/bibframe/polarity"/>
    <bffi-meta:exactMatch rdf:resource="http://rdaregistry.info/Elements/m/P30196"/>
    <skos:definition xml:lang="en">BIBFRAME definition: Relationship of the colors and tones in an image to the colors and tones of the object reproduced.</skos:definition>
  </rdf:Description>
  <rdf:Description rdf:about="http://urn.fi/URN:NBN:fi:schema:bffi:FileSize">
    <dct:modified>2024-09-16 (New)</dct:modified>
    <rdfs:label xml:lang="en">File size</rdfs:label>
    <rdfs:label xml:lang="fi">Tiedostokoko</rdfs:label>
    <rdf:type rdf:resource="http://www.w3.org/2002/07/owl#Class"/>
    <owl:equivalentClass rdf:resource="http://id.loc.gov/ontologies/bibframe/FileSize"/>
    <rdfs:subClassOf rdf:resource="http://urn.fi/URN:NBN:fi:schema:bffi:DigitalCharacteristic"/>
    <skos:definition xml:lang="en">BIBFRAME definition: Number of bytes in a digital file, e.g., 162 KB</skos:definition>
  </rdf:Description>
  <rdf:Description rdf:about="http://urn.fi/URN:NBN:fi:schema:bffi:additionalScaleInformation">
    <dct:modified>2024-04-16 (New)</dct:modified>
    <rdfs:label xml:lang="en">additional scale information</rdfs:label>
    <rdfs:label xml:lang="fi">lisätieto mittakaavasta</rdfs:label>
    <rdfs:domain rdf:resource="http://urn.fi/URN:NBN:fi:schema:bffi:Scale"/>
    <rdfs:range rdf:resource="http://www.w3.org/2000/01/rdf-schema#Literal"/>
    <rdf:type rdf:resource="http://www.w3.org/2002/07/owl#DatatypeProperty"/>
    <bffi-meta:exactMatch rdf:resource="http://rdaregistry.info/Elements/e/P20213"/>
  </rdf:Description>
  <rdf:Description rdf:about="http://urn.fi/URN:NBN:fi:schema:bffi:unit">
    <dct:modified>2025-01-02 (New)</dct:modified>
    <rdfs:label xml:lang="en">type of unit</rdfs:label>
    <rdfs:label xml:lang="fi">yksikön tyyppi</rdfs:label>
    <rdfs:domain rdf:resource="http://www.w3.org/2000/01/rdf-schema#Resource"/>
    <rdfs:range rdf:resource="http://urn.fi/URN:NBN:fi:schema:bffi:Unit"/>
    <rdf:type rdf:resource="http://www.w3.org/2002/07/owl#ObjectProperty"/>
    <owl:equivalentProperty rdf:resource="http://id.loc.gov/ontologies/bibframe/unit"/>
    <skos:definition xml:lang="en">BIBFRAME definition: Units in which a value is expressed, such as the physical or logical constituent of a resource (e.g., a volume, audiocassette, film reel, a map, a digital file).</skos:definition>
  </rdf:Description>
  <rdf:Description rdf:about="http://urn.fi/URN:NBN:fi:schema:bffi:Capture">
    <dct:modified>2024-02-23 (New)</dct:modified>
    <rdfs:label xml:lang="en">Capture of content</rdfs:label>
    <rdfs:label xml:lang="fi">Taltiointitiedot</rdfs:label>
    <rdf:type rdf:resource="http://www.w3.org/2002/07/owl#Class"/>
    <owl:equivalentClass rdf:resource="http://id.loc.gov/ontologies/bibframe/Capture"/>
    <skos:definition xml:lang="en">BIBFRAME definition: Information about place and date associated with the capture (i.e., recording, filming, etc.) of the content of a resource</skos:definition>
  </rdf:Description>
  <rdf:Description rdf:about="http://urn.fi/URN:NBN:fi:schema:bffi:Unit">
    <dct:modified>2025-01-02 (New)</dct:modified>
    <rdfs:label xml:lang="en">Unit</rdfs:label>
    <rdfs:label xml:lang="fi">Yksikkö</rdfs:label>
    <rdf:type rdf:resource="http://www.w3.org/2002/07/owl#Class"/>
    <owl:equivalentClass rdf:resource="http://id.loc.gov/ontologies/bibframe/Unit"/>
    <skos:definition xml:lang="en">BIBFRAME definition: Units in which a value is expressed</skos:definition>
  </rdf:Description>
  <rdf:Description rdf:about="http://urn.fi/URN:NBN:fi:schema:bffi:natureOfContent">
    <dct:modified>2024-02-23 (New)</dct:modified>
    <rdfs:label xml:lang="en">content nature</rdfs:label>
    <rdfs:label xml:lang="fi">sisällön luonne</rdfs:label>
    <rdfs:domain rdf:resource="http://urn.fi/URN:NBN:fi:schema:bffi:Work"/>
    <rdfs:range rdf:resource="http://www.w3.org/2000/01/rdf-schema#Literal"/>
    <rdf:type rdf:resource="http://www.w3.org/2002/07/owl#DatatypeProperty"/>
    <owl:equivalentProperty rdf:resource="http://id.loc.gov/ontologies/bibframe/natureOfContent"/>
    <bffi-meta:exactMatch rdf:resource="http://rdaregistry.info/Elements/w/P10222"/>
    <skos:definition xml:lang="en">BIBFRAME definition: Characterization that epitomizes the primary content of a resource, e.g., field recording of birdsong; combined time series analysis and graph plotting system.</skos:definition>
  </rdf:Description>
  <rdf:Description rdf:about="http://urn.fi/URN:NBN:fi:schema:bffi:Object">
    <dct:modified>2024-02-23 (New)</dct:modified>
    <rdfs:label xml:lang="en">Three-dimensional form</rdfs:label>
    <rdfs:label xml:lang="fi">Kolmiulotteinen muoto</rdfs:label>
    <rdf:type rdf:resource="http://www.w3.org/2002/07/owl#Class"/>
    <owl:equivalentClass rdf:resource="http://id.loc.gov/ontologies/bibframe/Object"/>
    <rdfs:seeAlso rdf:resource="http://rdaregistry.info/termList/RDAContentType/1021"/>
    <rdfs:subClassOf rdf:resource="http://urn.fi/URN:NBN:fi:schema:bffi:Expression"/>
    <skos:definition xml:lang="en">BIBFRAME definition: Resource in a form intended to be perceived visually in three-dimensions, including man-made objects such as models, sculptures, clothing, and toys, as well as naturally occurring objects such as specimens mounted for viewing</skos:definition>
  </rdf:Description>
  <rdf:Description rdf:about="http://urn.fi/URN:NBN:fi:schema:bffi:RetentionPolicy">
    <dct:modified>2024-04-16 (New)</dct:modified>
    <rdfs:label xml:lang="en">Retention policy</rdfs:label>
    <rdfs:label xml:lang="fi">Säilytyskäytäntö</rdfs:label>
    <rdf:type rdf:resource="http://www.w3.org/2002/07/owl#Class"/>
    <owl:equivalentClass rdf:resource="http://id.loc.gov/ontologies/bibframe/RetentionPolicy"/>
    <rdfs:subClassOf rdf:resource="http://urn.fi/URN:NBN:fi:schema:bffi:UsageAndAccessPolicy"/>
    <skos:definition xml:lang="en">BIBFRAME definition: Policy of holding institution for retaining resource</skos:definition>
  </rdf:Description>
  <rdf:Description rdf:about="http://urn.fi/URN:NBN:fi:schema:bffi:publicationStatement">
    <dct:modified>2024-09-16 (New)</dct:modified>
    <rdfs:label xml:lang="en">publication statement</rdfs:label>
    <rdfs:label xml:lang="fi">julkaisumerkintö</rdfs:label>
    <rdfs:domain rdf:resource="http://urn.fi/URN:NBN:fi:schema:bffi:Manifestation"/>
    <rdfs:range rdf:resource="http://www.w3.org/2000/01/rdf-schema#Literal"/>
    <rdf:type rdf:resource="http://www.w3.org/2002/07/owl#DatatypeProperty"/>
    <owl:equivalentProperty rdf:resource="http://id.loc.gov/ontologies/bibframe/publicationStatement"/>
    <bffi-meta:exactMatch rdf:resource="http://rdaregistry.info/Elements/m/P30111"/>
    <skos:definition xml:lang="en">BIBFRAME definition: Statement related to the publication of the resources; usually transcribed.</skos:definition>
  </rdf:Description>
  <rdf:Description rdf:about="http://urn.fi/URN:NBN:fi:schema:bffi:Distribution">
    <dct:modified>2024-02-23 (New)</dct:modified>
    <rdfs:label xml:lang="en">Distributor</rdfs:label>
    <rdfs:label xml:lang="fi">Jakelija</rdfs:label>
    <rdf:type rdf:resource="http://www.w3.org/2002/07/owl#Class"/>
    <owl:equivalentClass rdf:resource="http://id.loc.gov/ontologies/bibframe/Distribution"/>
    <rdfs:subClassOf rdf:resource="http://urn.fi/URN:NBN:fi:schema:bffi:ProvisionActivity"/>
    <skos:definition xml:lang="en">BIBFRAME definition: Information relating to distribution of a resource</skos:definition>
  </rdf:Description>
  <rdf:Description rdf:about="http://urn.fi/URN:NBN:fi:schema:bffi:Dissertation">
    <dct:modified>2024-02-23 (New)</dct:modified>
    <rdfs:label xml:lang="en">Dissertation information</rdfs:label>
    <rdfs:label xml:lang="fi">Tieto väitöskirjasta tai muusta opinnäytteestä</rdfs:label>
    <rdf:type rdf:resource="http://www.w3.org/2002/07/owl#Class"/>
    <owl:equivalentClass rdf:resource="http://id.loc.gov/ontologies/bibframe/Dissertation"/>
    <skos:definition xml:lang="en">BIBFRAME definition: Information about a work presented as part of the formal requirements for an academic degree</skos:definition>
  </rdf:Description>
  <rdf:Description rdf:about="http://urn.fi/URN:NBN:fi:schema:bffi:emulsion">
    <dct:modified>2024-09-16 (New)</dct:modified>
    <rdfs:label xml:lang="en">emulsion</rdfs:label>
    <rdfs:label xml:lang="fi">mikrofilmin ja mikrokortin emulsio</rdfs:label>
    <rdfs:domain rdf:resource="http://urn.fi/URN:NBN:fi:schema:bffi:Manifestation"/>
    <rdfs:range rdf:resource="http://urn.fi/URN:NBN:fi:schema:bffi:Emulsion"/>
    <rdf:type rdf:resource="http://www.w3.org/2002/07/owl#ObjectProperty"/>
    <owl:equivalentProperty rdf:resource="http://id.loc.gov/ontologies/bibframe/emulsion"/>
    <bffi-meta:exactMatch rdf:resource="http://rdaregistry.info/Elements/m/P30122"/>
    <skos:definition xml:lang="en">BIBFRAME definition: Suspension of light-sensitive chemicals used as a coating on a microfilm or microfiche, e.g., silver halide.</skos:definition>
  </rdf:Description>
  <rdf:Description rdf:about="http://urn.fi/URN:NBN:fi:schema:bffi:schedulePart">
    <dct:modified>2025-01-02 (New)</dct:modified>
    <rdfs:label xml:lang="en">classification designation</rdfs:label>
    <rdfs:label xml:lang="fi">luokituksen määre</rdfs:label>
    <rdfs:domain rdf:resource="http://urn.fi/URN:NBN:fi:schema:bffi:Classification"/>
    <rdfs:range rdf:resource="http://www.w3.org/2000/01/rdf-schema#Literal"/>
    <rdf:type rdf:resource="http://www.w3.org/2002/07/owl#DatatypeProperty"/>
    <owl:equivalentProperty rdf:resource="http://id.loc.gov/ontologies/bibframe/schedulePart"/>
    <skos:definition xml:lang="en">BIBFRAME definition: Designates whether the classification number is from the standard or optional part of a schedule or table.</skos:definition>
  </rdf:Description>
  <rdf:Description rdf:about="http://urn.fi/URN:NBN:fi:schema:bffi:part">
    <dct:modified>2025-01-02 (New)</dct:modified>
    <rdfs:label xml:lang="en">part</rdfs:label>
    <rdfs:label xml:lang="fi">osa</rdfs:label>
    <rdfs:domain rdf:resource="http://www.w3.org/2000/01/rdf-schema#Resource"/>
    <rdfs:range rdf:resource="http://www.w3.org/2000/01/rdf-schema#Literal"/>
    <rdf:type rdf:resource="http://www.w3.org/2002/07/owl#DatatypeProperty"/>
    <owl:equivalentProperty rdf:resource="http://id.loc.gov/ontologies/bibframe/part"/>
    <skos:definition xml:lang="en">BIBFRAME definition: Part of a resource to which information applies.</skos:definition>
  </rdf:Description>
  <rdf:Description rdf:about="http://urn.fi/URN:NBN:fi:schema:bffi:material">
    <dct:modified>2024-09-16 (New)</dct:modified>
    <rdfs:label xml:lang="en">material</rdfs:label>
    <rdfs:label xml:lang="fi">materiaali</rdfs:label>
    <rdfs:domain rdf:nodeID="n23d9c564949d4a53a71610ff1e9857f7b1"/>
    <rdfs:range rdf:resource="http://urn.fi/URN:NBN:fi:schema:bffi:Material"/>
    <rdf:type rdf:resource="http://www.w3.org/2002/07/owl#ObjectProperty"/>
    <owl:equivalentProperty rdf:resource="http://id.loc.gov/ontologies/bibframe/material"/>
    <bffi-meta:exactMatch rdf:resource="http://rdaregistry.info/Elements/m/P30304"/>
    <skos:definition xml:lang="en">BIBFRAME definition: Resource uses, is composed of, integrates, etc. the related material.</skos:definition>
  </rdf:Description>
  <rdf:Description rdf:about="http://urn.fi/URN:NBN:fi:schema:bffi:relation">
    <dct:modified>2024-09-16 (New)</dct:modified>
    <rdfs:label xml:lang="en">relation</rdfs:label>
    <rdfs:label xml:lang="fi">suhde</rdfs:label>
    <rdfs:domain rdf:nodeID="n1e5b766c1bf94ff9812af7b852f48486b1"/>
    <rdfs:range rdf:resource="http://urn.fi/URN:NBN:fi:schema:bffi:Relation"/>
    <rdf:type rdf:resource="http://www.w3.org/2002/07/owl#ObjectProperty"/>
    <owl:equivalentProperty rdf:resource="http://id.loc.gov/ontologies/bibframe/relation"/>
    <skos:definition xml:lang="en">BIBFRAME definition: Associated resource and its relationship to the resource being described</skos:definition>
  </rdf:Description>
  <rdf:Description rdf:about="http://urn.fi/URN:NBN:fi:schema:bffi:Manuscript">
    <dct:modified>2024-04-16 (New)</dct:modified>
    <rdfs:label xml:lang="en">Manuscript</rdfs:label>
    <rdfs:label xml:lang="fi">Käsikirjoitus</rdfs:label>
    <rdf:type rdf:resource="http://www.w3.org/2002/07/owl#Class"/>
    <owl:equivalentClass rdf:resource="http://id.loc.gov/ontologies/bibframe/Manuscript"/>
    <rdfs:subClassOf rdf:resource="http://urn.fi/URN:NBN:fi:schema:bffi:Work"/>
    <skos:definition xml:lang="en">BIBFRAME definition: Resource which is written in handwriting or typescript</skos:definition>
  </rdf:Description>
  <rdf:Description rdf:nodeID="n7333c8087d784d019f2d09a8a88483c5b5">
    <rdf:first rdf:resource="http://urn.fi/URN:NBN:fi:schema:bffi:Item"/>
    <rdf:rest rdf:resource="http://www.w3.org/1999/02/22-rdf-syntax-ns#nil"/>
  </rdf:Description>
  <rdf:Description rdf:about="http://urn.fi/URN:NBN:fi:schema:bffi:manufactureStatement">
    <dct:modified>2024-02-23 (New)</dct:modified>
    <rdfs:label xml:lang="en">manufacture statement</rdfs:label>
    <rdfs:label xml:lang="fi">valmistusmerkintö</rdfs:label>
    <rdfs:domain rdf:resource="http://urn.fi/URN:NBN:fi:schema:bffi:Manifestation"/>
    <rdfs:range rdf:resource="http://www.w3.org/2000/01/rdf-schema#Literal"/>
    <rdf:type rdf:resource="http://www.w3.org/2002/07/owl#DatatypeProperty"/>
    <owl:equivalentProperty rdf:resource="http://id.loc.gov/ontologies/bibframe/manufactureStatement"/>
    <bffi-meta:exactMatch rdf:resource="http://rdaregistry.info/Elements/m/P30109"/>
    <skos:definition xml:lang="en">BIBFRAME definition: Statement related to the manufacture of the resources; usually transcribed.</skos:definition>
  </rdf:Description>
  <rdf:Description rdf:about="http://urn.fi/URN:NBN:fi:schema:bffi:Chronology">
    <dct:modified>2024-02-23 (New)</dct:modified>
    <rdfs:label xml:lang="en">Chronology</rdfs:label>
    <rdfs:label xml:lang="fi">Julkaisuaikatiedot</rdfs:label>
    <rdf:type rdf:resource="http://www.w3.org/2002/07/owl#Class"/>
    <owl:equivalentClass rdf:resource="http://id.loc.gov/ontologies/bibframe/Chronology"/>
    <rdfs:subClassOf rdf:resource="http://urn.fi/URN:NBN:fi:schema:bffi:EnumerationAndChronology"/>
    <skos:definition xml:lang="en">BIBFRAME definition: Dates associated with issues or items held</skos:definition>
  </rdf:Description>
  <rdf:Description rdf:about="http://urn.fi/URN:NBN:fi:schema:bffi:SystemRequirement">
    <dct:modified>2024-11-22 (New)</dct:modified>
    <rdfs:label xml:lang="en">Equipment or system requirement</rdfs:label>
    <rdfs:label xml:lang="fi">Laitteisto- tai järjestelmävaatimukset</rdfs:label>
    <rdf:type rdf:resource="http://www.w3.org/2002/07/owl#Class"/>
    <owl:equivalentClass rdf:resource="http://id.loc.gov/ontologies/bibframe/SystemRequirement"/>
    <skos:definition xml:lang="en">BIBFRAME definition: Equipment or system requirements beyond what is normal and obvious for the type of carrier or type of file, such as make and model of equipment or hardware, operating system, amount of memory, programming language, other necessary software, any plug-ins or peripherals required to play, view, or run the resource</skos:definition>
  </rdf:Description>
  <rdf:Description rdf:nodeID="n2d6ab2e53ad74c4b81628c947ca3da20b2">
    <rdf:first rdf:resource="http://urn.fi/URN:NBN:fi:schema:bffi:MusicAudioExpression"/>
    <rdf:rest rdf:nodeID="n2d6ab2e53ad74c4b81628c947ca3da20b3"/>
  </rdf:Description>
  <rdf:Description rdf:about="http://urn.fi/URN:NBN:fi:schema:bffi:AcquisitionSource">
    <dct:modified>2024-04-16 (New)</dct:modified>
    <rdfs:label xml:lang="en">Acquisition source</rdfs:label>
    <rdfs:label xml:lang="fi">Hankintalähde</rdfs:label>
    <bffi-meta:relatedValueVocabulary rdf:resource="http://urn.fi/URN:NBN:fi:au:mts:m110"/>
    <rdf:type rdf:resource="http://www.w3.org/2002/07/owl#Class"/>
    <owl:equivalentClass rdf:resource="http://id.loc.gov/ontologies/bibframe/AcquisitionSource"/>
    <skos:definition xml:lang="en">BIBFRAME definition: Information about an organization, person, etc., from which a resource may be obtained</skos:definition>
  </rdf:Description>
  <rdf:Description rdf:about="http://urn.fi/URN:NBN:fi:schema:bffi:Layout">
    <dct:modified>2024-06-19 (New)</dct:modified>
    <rdfs:label xml:lang="en">Layout</rdfs:label>
    <rdfs:label xml:lang="fi">Layout</rdfs:label>
    <bffi-meta:relatedValueVocabulary rdf:resource="http://urn.fi/URN:NBN:fi:au:mts:m58"/>
    <rdf:type rdf:resource="http://www.w3.org/2002/07/owl#Class"/>
    <owl:equivalentClass rdf:resource="http://id.loc.gov/ontologies/bibframe/Layout"/>
    <rdfs:seeAlso rdf:resource="http://rdaregistry.info/termList/layout/"/>
    <skos:definition xml:lang="en">BIBFRAME definition: Arrangement of text, images, tactile notation, etc., in a resource</skos:definition>
  </rdf:Description>
  <rdf:Description rdf:about="http://urn.fi/URN:NBN:fi:schema:bffi:Polarity">
    <dct:modified>2024-09-16 (New)</dct:modified>
    <rdfs:label xml:lang="en">Polarity</rdfs:label>
    <rdfs:label xml:lang="fi">Polariteetti</rdfs:label>
    <bffi-meta:relatedValueVocabulary rdf:resource="http://urn.fi/URN:NBN:fi:au:mts:m558"/>
    <rdf:type rdf:resource="http://www.w3.org/2002/07/owl#Class"/>
    <owl:equivalentClass rdf:resource="http://id.loc.gov/ontologies/bibframe/Polarity"/>
    <rdfs:seeAlso rdf:resource="http://rdaregistry.info/termList/RDAPolarity/"/>
    <skos:definition xml:lang="en">BIBFRAME definition: Relationship of the colors and tones in an image to the colors and tones of the object reproduced</skos:definition>
  </rdf:Description>
  <rdf:Description rdf:about="http://urn.fi/URN:NBN:fi:schema:bffi:qualifier">
    <dct:modified>2024-02-23 (New)</dct:modified>
    <rdfs:label xml:lang="en">qualifier</rdfs:label>
    <rdfs:label xml:lang="fi">tarkenne</rdfs:label>
    <rdfs:domain rdf:resource="http://www.w3.org/2000/01/rdf-schema#Resource"/>
    <rdfs:range rdf:resource="http://www.w3.org/2000/01/rdf-schema#Literal"/>
    <rdf:type rdf:resource="http://www.w3.org/2002/07/owl#DatatypeProperty"/>
    <owl:equivalentProperty rdf:resource="http://id.loc.gov/ontologies/bibframe/qualifier"/>
    <bffi-meta:closeMatch rdf:resource="http://rdaregistry.info/Elements/x/P00015"/>
    <skos:definition xml:lang="en">BIBFRAME definition: Qualifier of information, such as an addition to a title to make it unique or qualifying information associated with an identifier.</skos:definition>
  </rdf:Description>
  <rdf:Description rdf:about="http://urn.fi/URN:NBN:fi:schema:bffi:manifestationOfWork">
    <dct:modified>2024-02-23 (New)</dct:modified>
    <rdfs:label xml:lang="en">manifestation of work</rdfs:label>
    <rdfs:label xml:lang="fi">teoksen manifestaatio</rdfs:label>
    <rdfs:domain rdf:resource="http://urn.fi/URN:NBN:fi:schema:bffi:Work"/>
    <rdfs:range rdf:resource="http://urn.fi/URN:NBN:fi:schema:bffi:Manifestation"/>
    <rdf:type rdf:resource="http://www.w3.org/2002/07/owl#ObjectProperty"/>
    <bffi-meta:broadMatch rdf:resource="http://id.loc.gov/ontologies/bibframe/hasInstance"/>
    <bffi-meta:exactMatch rdf:resource="http://rdaregistry.info/Elements/w/P10072"/>
    <rdfs:subPropertyOf rdf:resource="http://urn.fi/URN:NBN:fi:schema:bffi:relatedTo"/>
    <owl:inverseOf rdf:resource="http://urn.fi/URN:NBN:fi:schema:bffi:workManifested"/>
  </rdf:Description>
  <rdf:Description rdf:about="http://urn.fi/URN:NBN:fi:schema:bffi:hasExpression">
    <owl:inverseOf rdf:resource="http://urn.fi/URN:NBN:fi:schema:bffi:expressionOf"/>
    <dct:modified>2024-02-23 (New)</dct:modified>
    <rdfs:label xml:lang="en">expressed as</rdfs:label>
    <rdfs:label xml:lang="fi">teoksen ekspressio</rdfs:label>
    <rdfs:domain rdf:resource="http://urn.fi/URN:NBN:fi:schema:bffi:Work"/>
    <rdfs:range rdf:resource="http://urn.fi/URN:NBN:fi:schema:bffi:Expression"/>
    <rdf:type rdf:resource="http://www.w3.org/2002/07/owl#ObjectProperty"/>
    <bffi-meta:closeMatch rdf:resource="http://id.loc.gov/ontologies/bibframe/hasExpression"/>
    <bffi-meta:exactMatch rdf:resource="http://rdaregistry.info/Elements/w/P10078"/>
    <rdfs:subPropertyOf rdf:resource="http://urn.fi/URN:NBN:fi:schema:bffi:relatedTo"/>
  </rdf:Description>
  <rdf:Description rdf:about="http://urn.fi/URN:NBN:fi:schema:bffi:soundContent">
    <dct:modified>2024-11-22 (New)</dct:modified>
    <rdfs:label xml:lang="en">sound content</rdfs:label>
    <rdfs:label xml:lang="fi">äänisisältö</rdfs:label>
    <rdfs:domain rdf:resource="http://urn.fi/URN:NBN:fi:schema:bffi:Manifestation"/>
    <rdfs:range rdf:resource="http://urn.fi/URN:NBN:fi:schema:bffi:SoundContent"/>
    <rdf:type rdf:resource="http://www.w3.org/2002/07/owl#ObjectProperty"/>
    <owl:equivalentProperty rdf:resource="http://id.loc.gov/ontologies/bibframe/soundContent"/>
    <bffi-meta:exactMatch rdf:resource="http://rdaregistry.info/Elements/m/P30454"/>
    <skos:definition xml:lang="en">BIBFRAME definition: Indication of whether the production of sound is an integral part of the resource.</skos:definition>
  </rdf:Description>
  <rdf:Description rdf:about="http://urn.fi/URN:NBN:fi:schema:bffi:layout">
    <dct:modified>2024-06-19 (New)</dct:modified>
    <rdfs:label xml:lang="en">layout</rdfs:label>
    <rdfs:label xml:lang="fi">layout</rdfs:label>
    <rdfs:domain rdf:resource="http://urn.fi/URN:NBN:fi:schema:bffi:Manifestation"/>
    <rdfs:range rdf:resource="http://urn.fi/URN:NBN:fi:schema:bffi:Layout"/>
    <rdf:type rdf:resource="http://www.w3.org/2002/07/owl#ObjectProperty"/>
    <owl:equivalentProperty rdf:resource="http://id.loc.gov/ontologies/bibframe/layout"/>
    <bffi-meta:exactMatch rdf:resource="http://rdaregistry.info/Elements/m/P30155"/>
    <skos:definition xml:lang="en">BIBFRAME definition: Arrangement of text, images, tactile notation, etc., in a resource.</skos:definition>
  </rdf:Description>
  <rdf:Description rdf:about="http://urn.fi/URN:NBN:fi:schema:bffi:relief">
    <dct:modified>2024-04-16 (New)</dct:modified>
    <rdfs:label xml:lang="en">relief</rdfs:label>
    <rdfs:label xml:lang="fi">korkeuserojen esitystapa</rdfs:label>
    <rdfs:domain rdf:resource="http://urn.fi/URN:NBN:fi:schema:bffi:Cartographic"/>
    <rdfs:range rdf:resource="http://urn.fi/URN:NBN:fi:schema:bffi:Relief"/>
    <rdf:type rdf:resource="http://www.w3.org/2002/07/owl#ObjectProperty"/>
    <owl:equivalentProperty rdf:resource="http://id.loc.gov/ontologies/bibframe/relief"/>
    <bffi-meta:exactMatch rdf:resource="http://rdaregistry.info/Elements/e/P20318"/>
    <skos:definition xml:lang="en">BIBFRAME definition: Relief term specified on a cartographic resource</skos:definition>
  </rdf:Description>
  <rdf:Description rdf:about="http://urn.fi/URN:NBN:fi:schema:bffi:languageOfExpression">
    <dct:modified>2024-02-23 (New)</dct:modified>
    <rdfs:label xml:lang="en">language of expression</rdfs:label>
    <rdfs:label xml:lang="fi">ekspression kieli</rdfs:label>
    <rdfs:domain rdf:resource="http://urn.fi/URN:NBN:fi:schema:bffi:Expression"/>
    <rdfs:range rdf:resource="http://www.w3.org/2000/01/rdf-schema#Resource"/>
    <rdf:type rdf:resource="http://www.w3.org/2002/07/owl#ObjectProperty"/>
    <bffi-meta:broadMatch rdf:resource="http://id.loc.gov/ontologies/bibframe/language"/>
    <bffi-meta:exactMatch rdf:resource="http://rdaregistry.info/Elements/e/P20006"/>
    <rdfs:subPropertyOf rdf:resource="http://urn.fi/URN:NBN:fi:schema:bffi:language"/>
  </rdf:Description>
  <rdf:Description rdf:about="http://urn.fi/URN:NBN:fi:schema:bffi:CartographicObjectType">
    <dct:modified>2024-04-16 (New)</dct:modified>
    <rdfs:label xml:lang="en">Digital cartographic object type</rdfs:label>
    <rdfs:label xml:lang="fi">Kartografisen sisällön digitaalinen esitysmuoto</rdfs:label>
    <rdf:type rdf:resource="http://www.w3.org/2002/07/owl#Class"/>
    <owl:equivalentClass rdf:resource="http://id.loc.gov/ontologies/bibframe/CartographicObjectType"/>
    <rdfs:subClassOf rdf:resource="http://urn.fi/URN:NBN:fi:schema:bffi:DigitalCharacteristic"/>
    <skos:definition xml:lang="en">BIBFRAME definition: Object type for encoding of geospatial information in a cartographic resource, e.g., point, line, polygon</skos:definition>
  </rdf:Description>
  <rdf:Description rdf:about="http://urn.fi/URN:NBN:fi:schema:bffi:Issuance">
    <dct:modified>2024-02-23 (New)</dct:modified>
    <rdfs:label xml:lang="en">Mode of issuance</rdfs:label>
    <rdfs:label xml:lang="fi">Julkaisutapa</rdfs:label>
    <bffi-meta:relatedValueVocabulary rdf:resource="http://urn.fi/URN:NBN:fi:au:mts:m4372"/>
    <rdf:type rdf:resource="http://www.w3.org/2002/07/owl#Class"/>
    <bffi-meta:broadMatch rdf:resource="http://id.loc.gov/ontologies/bibframe/Issuance"/>
    <rdfs:seeAlso rdf:resource="http://www.rdaregistry.info/termList/ModeIssue/"/>
  </rdf:Description>
  <rdf:Description rdf:about="http://urn.fi/URN:NBN:fi:schema:bffi:MusicNotation">
    <dct:modified>2024-02-23 (New)</dct:modified>
    <rdfs:label xml:lang="en">Music notation</rdfs:label>
    <rdfs:label xml:lang="fi">Nuottikirjoituksen tyyppi</rdfs:label>
    <bffi-meta:relatedValueVocabulary rdf:resource="http://urn.fi/URN:NBN:fi:au:mts:m1990"/>
    <rdf:type rdf:resource="http://www.w3.org/2002/07/owl#Class"/>
    <owl:equivalentClass rdf:resource="http://id.loc.gov/ontologies/bibframe/MusicNotation"/>
    <rdfs:seeAlso rdf:resource="http://rdaregistry.info/termList/MusNotation"/>
    <rdfs:subClassOf rdf:resource="http://urn.fi/URN:NBN:fi:schema:bffi:Notation"/>
    <skos:definition xml:lang="en">BIBFRAME definition: Information on the symbol system used to convey the content of a music resource</skos:definition>
  </rdf:Description>
  <rdf:Description rdf:about="http://urn.fi/URN:NBN:fi:schema:bffi:relatedTo">
    <dct:modified>2024-02-23 (New)</dct:modified>
    <rdfs:label xml:lang="en">related resource</rdfs:label>
    <rdfs:label xml:lang="fi">liittyvä resurssi</rdfs:label>
    <rdfs:domain rdf:resource="http://www.w3.org/2000/01/rdf-schema#Resource"/>
    <rdfs:range rdf:resource="http://www.w3.org/2000/01/rdf-schema#Resource"/>
    <rdf:type rdf:resource="http://www.w3.org/2002/07/owl#SymmetricProperty"/>
    <rdf:type rdf:resource="http://www.w3.org/2002/07/owl#ObjectProperty"/>
    <owl:equivalentProperty rdf:resource="http://id.loc.gov/ontologies/bibframe/relatedTo"/>
    <bffi-meta:exactMatch rdf:resource="http://rdaregistry.info/Elements/x/P00001"/>
    <skos:definition xml:lang="en">BIBFRAME definition: Any relationship between Work, Instance, Item, and Event resources</skos:definition>
  </rdf:Description>
  <rdf:Description rdf:about="http://urn.fi/URN:NBN:fi:schema:bffi:Person">
    <dct:modified>2024-02-23 (New)</dct:modified>
    <rdfs:label xml:lang="en">Person</rdfs:label>
    <rdfs:label xml:lang="fi">Henkilö</rdfs:label>
    <rdf:type rdf:resource="http://www.w3.org/2002/07/owl#Class"/>
    <owl:equivalentClass rdf:resource="http://id.loc.gov/ontologies/bibframe/Person"/>
    <bffi-meta:exactMatch rdf:resource="http://rdaregistry.info/Elements/c/C10004"/>
    <rdfs:subClassOf rdf:resource="http://urn.fi/URN:NBN:fi:schema:bffi:Agent"/>
    <skos:definition xml:lang="en">BIBFRAME definition: Individual or identity established by an individual (either alone or in collaboration with one or more other individuals)</skos:definition>
  </rdf:Description>
  <rdf:Description rdf:nodeID="n2d6ab2e53ad74c4b81628c947ca3da20b3">
    <rdf:first rdf:resource="http://urn.fi/URN:NBN:fi:schema:bffi:NotatedMusic"/>
    <rdf:rest rdf:resource="http://www.w3.org/1999/02/22-rdf-syntax-ns#nil"/>
  </rdf:Description>
  <rdf:Description rdf:nodeID="nbf7db4a78c624ed983d40041e8bb0721b3">
    <rdf:first rdf:resource="http://urn.fi/URN:NBN:fi:schema:bffi:Item"/>
    <rdf:rest rdf:resource="http://www.w3.org/1999/02/22-rdf-syntax-ns#nil"/>
  </rdf:Description>
  <rdf:Description rdf:about="http://urn.fi/URN:NBN:fi:schema:bffi:StillImage">
    <dct:modified>2024-02-23 (New)</dct:modified>
    <rdfs:label xml:lang="en">Still image</rdfs:label>
    <rdfs:label xml:lang="fi">Stillkuva</rdfs:label>
    <rdf:type rdf:resource="http://www.w3.org/2002/07/owl#Class"/>
    <owl:equivalentClass rdf:resource="http://id.loc.gov/ontologies/bibframe/StillImage"/>
    <rdfs:seeAlso rdf:resource="http://rdaregistry.info/termList/RDAContentType/1014"/>
    <rdfs:subClassOf rdf:resource="http://urn.fi/URN:NBN:fi:schema:bffi:Expression"/>
    <skos:definition xml:lang="en">BIBFRAME definition: Resource expressed through line, shape, shading, etc., intended to be perceived visually as a still image or images in two dimensions, including two-dimensional images and slides and transparencies</skos:definition>
  </rdf:Description>
  <rdf:Description rdf:nodeID="n30938fe99dde46599fe6796e2af454deb3">
    <rdf:first rdf:resource="http://urn.fi/URN:NBN:fi:schema:bffi:Expression"/>
    <rdf:rest rdf:nodeID="n30938fe99dde46599fe6796e2af454deb4"/>
  </rdf:Description>
  <rdf:Description rdf:nodeID="n2d6ab2e53ad74c4b81628c947ca3da20b1">
    <rdf:type rdf:resource="http://www.w3.org/2002/07/owl#Class"/>
    <owl:unionOf rdf:nodeID="n2d6ab2e53ad74c4b81628c947ca3da20b2"/>
  </rdf:Description>
  <rdf:Description rdf:about="http://urn.fi/URN:NBN:fi:schema:bffi:scriptOfRepresentativeExpression">
    <dct:modified>2025-01-02 (New)</dct:modified>
    <rdfs:label xml:lang="en">script of representative expression</rdfs:label>
    <rdfs:label xml:lang="fi">edustavan ekspression kirjoitusjärjestelmä</rdfs:label>
    <rdfs:domain rdf:resource="http://urn.fi/URN:NBN:fi:schema:bffi:Work"/>
    <rdfs:range rdf:resource="http://urn.fi/URN:NBN:fi:schema:bffi:Script"/>
    <rdf:type rdf:resource="http://www.w3.org/2002/07/owl#ObjectProperty"/>
    <bffi-meta:broadMatch rdf:resource="http://id.loc.gov/ontologies/bibframe/notation"/>
    <bffi-meta:exactMatch rdf:resource="http://rdaregistry.info/Elements/w/P10357"/>
  </rdf:Description>
  <rdf:Description rdf:about="http://urn.fi/URN:NBN:fi:schema:bffi:version">
    <dct:modified>2024-11-22 (New)</dct:modified>
    <rdfs:label xml:lang="en">version</rdfs:label>
    <rdfs:label xml:lang="fi">versio</rdfs:label>
    <rdfs:domain rdf:resource="http://urn.fi/URN:NBN:fi:schema:bffi:Work"/>
    <rdfs:range rdf:resource="http://www.w3.org/2000/01/rdf-schema#Literal"/>
    <rdf:type rdf:resource="http://www.w3.org/2002/07/owl#DatatypeProperty"/>
    <owl:equivalentProperty rdf:resource="http://id.loc.gov/ontologies/bibframe/version"/>
    <skos:definition xml:lang="en">BIBFRAME definition: Term or terms that identify works such as arranged for music, vulgate for religious work, etc.</skos:definition>
  </rdf:Description>
  <rdf:Description rdf:about="http://urn.fi/URN:NBN:fi:schema:bffi:provisionActivity">
    <dct:modified>2024-02-23 (New)</dct:modified>
    <rdfs:label xml:lang="en">provision activity</rdfs:label>
    <rdfs:label xml:lang="fi">tuottamistiedot</rdfs:label>
    <rdfs:domain rdf:resource="http://urn.fi/URN:NBN:fi:schema:bffi:Manifestation"/>
    <rdfs:range rdf:resource="http://urn.fi/URN:NBN:fi:schema:bffi:ProvisionActivity"/>
    <rdf:type rdf:resource="http://www.w3.org/2002/07/owl#ObjectProperty"/>
    <owl:equivalentProperty rdf:resource="http://id.loc.gov/ontologies/bibframe/provisionActivity"/>
    <rdfs:seeAlso rdf:resource="http://rdaregistry.info/Elements/m/P30173"/>
    <rdfs:seeAlso rdf:resource="http://rdaregistry.info/Elements/m/P30176"/>
    <rdfs:seeAlso rdf:resource="http://rdaregistry.info/Elements/m/P30009"/>
    <rdfs:seeAlso rdf:resource="http://rdaregistry.info/Elements/m/P30175"/>
    <rdfs:seeAlso rdf:resource="http://rdaregistry.info/Elements/m/P30087"/>
    <rdfs:seeAlso rdf:resource="http://rdaregistry.info/Elements/m/P30088"/>
    <rdfs:seeAlso rdf:resource="http://rdaregistry.info/Elements/m/P30085"/>
    <rdfs:seeAlso rdf:resource="http://rdaregistry.info/Elements/m/P30086"/>
    <rdfs:seeAlso rdf:resource="http://rdaregistry.info/Elements/m/P30008"/>
    <rdfs:seeAlso rdf:resource="http://rdaregistry.info/Elements/m/P30010"/>
    <rdfs:seeAlso rdf:resource="http://rdaregistry.info/Elements/m/P30011"/>
    <rdfs:seeAlso rdf:resource="http://rdaregistry.info/Elements/m/P30174"/>
    <skos:definition xml:lang="en">BIBFRAME definition: Place, name, and/or date information relating to the publication, printing, distribution, issue, release, production, etc. of a resource.</skos:definition>
  </rdf:Description>
  <rdf:Description rdf:nodeID="n096c0702f8c64e3bbe53573a59499c9ab1">
    <rdf:type rdf:resource="http://www.w3.org/2002/07/owl#Class"/>
    <owl:unionOf rdf:nodeID="n096c0702f8c64e3bbe53573a59499c9ab2"/>
  </rdf:Description>
  <rdf:Description rdf:about="http://urn.fi/URN:NBN:fi:schema:bffi:Microform">
    <dct:modified>2024-09-16 (New)</dct:modified>
    <rdfs:label xml:lang="en">Microform</rdfs:label>
    <rdfs:label xml:lang="fi">Mikromuoto</rdfs:label>
    <rdf:type rdf:resource="http://www.w3.org/2002/07/owl#Class"/>
    <owl:equivalentClass rdf:resource="http://id.loc.gov/ontologies/bibframe/Microform"/>
    <bffi-meta:broadMatch rdf:resource="http://rdaregistry.info/Elements/c/C10007"/>
    <rdfs:subClassOf rdf:resource="http://urn.fi/URN:NBN:fi:schema:bffi:Manifestation"/>
    <skos:definition xml:lang="en">BIBFRAME definition: Resource that contains microimages, either transparent or opaque, that may be reproductions of existing textual or graphic materials or may be original publications</skos:definition>
  </rdf:Description>
  <rdf:Description rdf:about="http://urn.fi/URN:NBN:fi:schema:bffi:SeriesExpression">
    <owl:disjointWith rdf:resource="http://urn.fi/URN:NBN:fi:schema:bffi:SerialExpression"/>
    <dct:modified>2024-02-23 (New)</dct:modified>
    <rdfs:label xml:lang="en">Series expression</rdfs:label>
    <rdfs:label xml:lang="fi">Moniosainen ekspressio ekspressio</rdfs:label>
    <rdf:type rdf:resource="http://www.w3.org/2002/07/owl#Class"/>
    <bffi-meta:broadMatch rdf:resource="http://id.loc.gov/ontologies/bibframe/Series"/>
    <rdfs:subClassOf rdf:resource="http://urn.fi/URN:NBN:fi:schema:bffi:Expression"/>
  </rdf:Description>
  <rdf:Description rdf:about="http://urn.fi/URN:NBN:fi:schema:bffi:title">
    <dct:modified>2024-02-23 (New)</dct:modified>
    <rdfs:label xml:lang="en">title resource</rdfs:label>
    <rdfs:label xml:lang="fi">nimeke</rdfs:label>
    <rdfs:domain rdf:nodeID="n9f671517b9dd4b7c955826691e2215f4b1"/>
    <rdfs:range rdf:resource="http://urn.fi/URN:NBN:fi:schema:bffi:Title"/>
    <rdf:type rdf:resource="http://www.w3.org/2002/07/owl#ObjectProperty"/>
    <owl:equivalentProperty rdf:resource="http://id.loc.gov/ontologies/bibframe/title"/>
    <bffi-meta:narrowMatch rdf:resource="http://rdaregistry.info/Elements/w/P10088"/>
    <bffi-meta:narrowMatch rdf:resource="http://rdaregistry.info/Elements/e/P20312"/>
    <bffi-meta:narrowMatch rdf:resource="http://rdaregistry.info/Elements/m/P30134"/>
    <bffi-meta:narrowMatch rdf:resource="http://rdaregistry.info/Elements/i/P40082"/>
    <owl:inverseOf rdf:resource="http://urn.fi/URN:NBN:fi:schema:bffi:titleOf"/>
    <skos:definition xml:lang="en">BIBFRAME definition: Name given to a resource.</skos:definition>
  </rdf:Description>
  <rdf:Description rdf:about="http://urn.fi/URN:NBN:fi:schema:bffi:CollectionAccrualMethod">
    <dct:modified>2024-04-16 (New)</dct:modified>
    <rdfs:label xml:lang="en">Collection accrual method</rdfs:label>
    <rdfs:label xml:lang="fi">Kokoelman kartuntamenetelmä</rdfs:label>
    <bffi-meta:relatedValueVocabulary rdf:resource="http://urn.fi/URN:NBN:fi:au:mts:m5110"/>
    <rdf:type rdf:resource="http://www.w3.org/2002/07/owl#Class"/>
    <bffi-meta:broadMatch rdf:resource="http://id.loc.gov/ontologies/bibframe/UsageAndAccessPolicy"/>
    <rdfs:seeAlso rdf:resource="http://rdaregistry.info/termList/RDACollectionAccrualMethod/"/>
  </rdf:Description>
  <rdf:Description rdf:about="http://urn.fi/URN:NBN:fi:schema:bffi:illustrativeContent">
    <dct:modified>2024-02-23 (New)</dct:modified>
    <rdfs:label xml:lang="en">illustrative content</rdfs:label>
    <rdfs:label xml:lang="fi">kuvasisältö</rdfs:label>
    <rdfs:domain rdf:resource="http://urn.fi/URN:NBN:fi:schema:bffi:Manifestation"/>
    <rdfs:range rdf:resource="http://urn.fi/URN:NBN:fi:schema:bffi:Illustration"/>
    <rdf:type rdf:resource="http://www.w3.org/2002/07/owl#ObjectProperty"/>
    <owl:equivalentProperty rdf:resource="http://id.loc.gov/ontologies/bibframe/illustrativeContent"/>
    <bffi-meta:exactMatch rdf:resource="http://rdaregistry.info/Elements/m/P30453"/>
    <skos:definition xml:lang="en">BIBFRAME definition: Information about content intended to illustrate a resource.</skos:definition>
  </rdf:Description>
  <rdf:Description rdf:about="http://urn.fi/URN:NBN:fi:schema:bffi:ScaleDesignation">
    <dct:modified>2024-04-16 (New)</dct:modified>
    <rdfs:label xml:lang="en">Scale designation</rdfs:label>
    <rdfs:label xml:lang="fi">Mittakaavan määrite</rdfs:label>
    <bffi-meta:relatedValueVocabulary rdf:resource="http://urn.fi/URN:NBN:fi:au:mts:m4396"/>
    <rdf:type rdf:resource="http://www.w3.org/2002/07/owl#Class"/>
    <bffi-meta:broadMatch rdf:resource="http://id.loc.gov/ontologies/bibframe/Scale"/>
    <rdfs:seeAlso rdf:resource="http://rdaregistry.info/termList/scale/"/>
    <rdfs:subClassOf rdf:resource="http://urn.fi/URN:NBN:fi:schema:bffi:Scale"/>
  </rdf:Description>
  <rdf:Description rdf:about="http://urn.fi/URN:NBN:fi:schema:bffi:FontSize">
    <dct:modified>2024-09-16 (New)</dct:modified>
    <rdfs:label xml:lang="en">Font size</rdfs:label>
    <rdfs:label xml:lang="fi">Kirjasinkoko</rdfs:label>
    <bffi-meta:relatedValueVocabulary rdf:resource="http://urn.fi/URN:NBN:fi:au:mts:m1239"/>
    <rdf:type rdf:resource="http://www.w3.org/2002/07/owl#Class"/>
    <owl:equivalentClass rdf:resource="http://id.loc.gov/ontologies/bibframe/FontSize"/>
    <rdfs:seeAlso rdf:resource="http://rdaregistry.info/termList/fontSize/"/>
    <skos:definition xml:lang="en">BIBFRAME definition: Size of the type used to represent the characters and symbols in a resource</skos:definition>
  </rdf:Description>
  <rdf:Description rdf:about="http://urn.fi/URN:NBN:fi:schema:bffi:languageOfRepresentativeExpression">
    <dct:modified>2024-02-23 (New)</dct:modified>
    <rdfs:label xml:lang="en">language of representative expression</rdfs:label>
    <rdfs:label xml:lang="fi">edustavan ekspression kieli</rdfs:label>
    <rdfs:domain rdf:resource="http://urn.fi/URN:NBN:fi:schema:bffi:Work"/>
    <rdfs:range rdf:resource="http://www.w3.org/2000/01/rdf-schema#Resource"/>
    <rdf:type rdf:resource="http://www.w3.org/2002/07/owl#ObjectProperty"/>
    <bffi-meta:closeMatch rdf:resource="http://id.loc.gov/ontologies/bibframe/language"/>
    <bffi-meta:exactMatch rdf:resource="http://rdaregistry.info/Elements/w/P10353"/>
  </rdf:Description>
  <rdf:Description rdf:about="http://urn.fi/URN:NBN:fi:schema:bffi:usageAndAccessPolicy">
    <dct:modified>2024-02-23 (New)</dct:modified>
    <rdfs:label xml:lang="en">use and access condition</rdfs:label>
    <rdfs:label xml:lang="fi">käyttö- ja pääsyrajoitukset</rdfs:label>
    <rdfs:domain rdf:nodeID="naa57803e9b8e45bda2faf492b90c6d13b1"/>
    <rdfs:range rdf:resource="http://urn.fi/URN:NBN:fi:schema:bffi:UsageAndAccessPolicy"/>
    <rdf:type rdf:resource="http://www.w3.org/2002/07/owl#ObjectProperty"/>
    <bffi-meta:narrowMatch rdf:resource="http://rdaregistry.info/Elements/i/P40047"/>
    <bffi-meta:narrowMatch rdf:resource="http://rdaregistry.info/Elements/m/P30145"/>
    <bffi-meta:narrowMatch rdf:resource="http://rdaregistry.info/Elements/i/P40048"/>
    <bffi-meta:narrowMatch rdf:resource="http://rdaregistry.info/Elements/m/P30146"/>
    <rdfs:subPropertyOf rdf:resource="http://id.loc.gov/ontologies/bibframe/usageAndAccessPolicy"/>
  </rdf:Description>
  <rdf:Description rdf:about="http://urn.fi/URN:NBN:fi:schema:bffi:pattern">
    <dct:modified>2024-04-16 (New)</dct:modified>
    <rdfs:label xml:lang="en">arrangement of material</rdfs:label>
    <rdfs:label xml:lang="fi">järjestys</rdfs:label>
    <rdfs:domain rdf:resource="http://urn.fi/URN:NBN:fi:schema:bffi:CollectionArrangement"/>
    <rdfs:range rdf:resource="http://www.w3.org/2000/01/rdf-schema#Literal"/>
    <rdf:type rdf:resource="http://www.w3.org/2002/07/owl#DatatypeProperty"/>
    <owl:equivalentProperty rdf:resource="http://id.loc.gov/ontologies/bibframe/pattern"/>
    <skos:definition xml:lang="en">BIBFRAME definition: Pattern of arrangement of materials within a unit.</skos:definition>
  </rdf:Description>
  <rdf:Description rdf:nodeID="n23d9c564949d4a53a71610ff1e9857f7b3">
    <rdf:first rdf:resource="http://urn.fi/URN:NBN:fi:schema:bffi:Item"/>
    <rdf:rest rdf:resource="http://www.w3.org/1999/02/22-rdf-syntax-ns#nil"/>
  </rdf:Description>
  <rdf:Description rdf:about="http://urn.fi/URN:NBN:fi:schema:bffi:subjectOf">
    <dct:modified>2024-02-23 (New)</dct:modified>
    <rdfs:label xml:lang="en">subject of</rdfs:label>
    <rdfs:label xml:lang="fi">aiheena teoksessa</rdfs:label>
    <rdfs:domain rdf:resource="http://www.w3.org/2000/01/rdf-schema#Resource"/>
    <rdfs:range rdf:resource="http://urn.fi/URN:NBN:fi:schema:bffi:Work"/>
    <rdf:type rdf:resource="http://www.w3.org/2002/07/owl#ObjectProperty"/>
    <owl:equivalentProperty rdf:resource="http://id.loc.gov/ontologies/bibframe/subjectOf"/>
    <owl:inverseOf rdf:resource="http://urn.fi/URN:NBN:fi:schema:bffi:subject"/>
    <skos:definition xml:lang="en">BIBFRAME definition: Relates a subject to that which it describes.</skos:definition>
  </rdf:Description>
  <rdf:Description rdf:about="http://urn.fi/URN:NBN:fi:schema:bffi:ImmediateAcquisition">
    <dct:modified>2024-04-16 (New)</dct:modified>
    <rdfs:label xml:lang="en">Immediate acquisition</rdfs:label>
    <rdfs:label xml:lang="fi">Kokoelman kartuttamisen menetelmä</rdfs:label>
    <bffi-meta:relatedValueVocabulary rdf:resource="http://urn.fi/URN:NBN:fi:au:mts:m5110"/>
    <rdf:type rdf:resource="http://www.w3.org/2002/07/owl#Class"/>
    <owl:equivalentClass rdf:resource="http://id.loc.gov/ontologies/bibframe/ImmediateAcquisition"/>
    <skos:definition xml:lang="en">BIBFRAME definition: Information about the circumstances, e.g., source, date, method, under which the resource was directly acquired</skos:definition>
  </rdf:Description>
  <rdf:Description rdf:nodeID="n3fb00cccae3f45e2923b7c06d0716eb2b3">
    <rdf:first rdf:resource="http://urn.fi/URN:NBN:fi:schema:bffi:AggregatingWork"/>
    <rdf:rest rdf:resource="http://www.w3.org/1999/02/22-rdf-syntax-ns#nil"/>
  </rdf:Description>
  <rdf:Description rdf:about="http://urn.fi/URN:NBN:fi:schema:bffi:TitleSource">
    <dct:modified>2024-06-19 (New)</dct:modified>
    <rdfs:label xml:lang="en">Source of title proper</rdfs:label>
    <rdfs:label xml:lang="fi">Päänimekkeen tiedonlähde</rdfs:label>
    <bffi-meta:relatedValueVocabulary rdf:resource="http://urn.fi/URN:NBN:fi:au:mts:m1685"/>
    <rdf:type rdf:resource="http://www.w3.org/2002/07/owl#Class"/>
    <bffi-meta:broadMatch rdf:resource="http://id.loc.gov/ontologies/bibframe/Source"/>
    <rdfs:subClassOf rdf:resource="http://urn.fi/URN:NBN:fi:schema:bffi:RecordingSource"/>
  </rdf:Description>
  <rdf:Description rdf:about="http://urn.fi/URN:NBN:fi:schema:bffi:ProgrammingLanguage">
    <dct:modified>2024-11-22 (New)</dct:modified>
    <rdfs:label xml:lang="en">Programming language</rdfs:label>
    <rdfs:label xml:lang="fi">Ohjelmointikieli</rdfs:label>
    <rdf:type rdf:resource="http://www.w3.org/2002/07/owl#Class"/>
    <owl:equivalentClass rdf:resource="http://id.loc.gov/ontologies/bflc/ProgrammingLanguage"/>
    <rdfs:subClassOf rdf:resource="http://urn.fi/URN:NBN:fi:schema:bffi:SystemRequirement"/>
    <skos:definition xml:lang="en">BFLC definition: Name of the programming language associated with the data comprising the resource.</skos:definition>
  </rdf:Description>
  <rdf:Description rdf:about="http://urn.fi/URN:NBN:fi:schema:bffi:DescriptionAuthentication">
    <dct:modified>2024-06-19 (New)</dct:modified>
    <rdfs:label xml:lang="en">Description authentication</rdfs:label>
    <rdfs:label xml:lang="fi">Autentikointikoodi</rdfs:label>
    <rdf:type rdf:resource="http://www.w3.org/2002/07/owl#Class"/>
    <owl:equivalentClass rdf:resource="http://id.loc.gov/ontologies/bibframe/DescriptionAuthentication"/>
    <skos:definition xml:lang="en">BIBFRAME definition: Indication of specific types of reviews that have been carried out on the description information</skos:definition>
  </rdf:Description>
  <rdf:Description rdf:about="http://urn.fi/URN:NBN:fi:schema:bffi:NonMusicAudioExpression">
    <dct:modified>2024-02-23 (New)</dct:modified>
    <rdfs:label xml:lang="en">Non-music audio expression</rdfs:label>
    <rdfs:label xml:lang="fi">Musiikiton audioekspressio</rdfs:label>
    <rdf:type rdf:resource="http://www.w3.org/2002/07/owl#Class"/>
    <bffi-meta:broadMatch rdf:resource="http://id.loc.gov/ontologies/bibframe/NonMusicAudio"/>
    <bffi-meta:broadMatch rdf:resource="http://rdaregistry.info/Elements/c/C10006"/>
    <rdfs:subClassOf rdf:resource="http://urn.fi/URN:NBN:fi:schema:bffi:Expression"/>
  </rdf:Description>
  <rdf:Description rdf:about="http://urn.fi/URN:NBN:fi:schema:bffi:itemOf">
    <owl:inverseOf rdf:resource="http://urn.fi/URN:NBN:fi:schema:bffi:hasItem"/>
    <dct:modified>2024-02-23 (New)</dct:modified>
    <rdfs:label xml:lang="en">manifestation exemplified</rdfs:label>
    <rdfs:label xml:lang="fi">kappaleen edustama manifestaatio</rdfs:label>
    <rdfs:domain rdf:resource="http://urn.fi/URN:NBN:fi:schema:bffi:Item"/>
    <rdfs:range rdf:resource="http://urn.fi/URN:NBN:fi:schema:bffi:Manifestation"/>
    <rdf:type rdf:resource="http://www.w3.org/2002/07/owl#ObjectProperty"/>
    <owl:equivalentProperty rdf:resource="http://id.loc.gov/ontologies/bibframe/itemOf"/>
    <bffi-meta:exactMatch rdf:resource="http://rdaregistry.info/Elements/i/P40049"/>
    <rdfs:subPropertyOf rdf:resource="http://urn.fi/URN:NBN:fi:schema:bffi:relatedTo"/>
    <skos:definition xml:lang="en">BIBFRAME definition: Instance for which the described Item is an example</skos:definition>
  </rdf:Description>
  <rdf:Description rdf:about="http://urn.fi/URN:NBN:fi:schema:bffi:duration">
    <dct:modified>2024-02-23 (New)</dct:modified>
    <rdfs:label xml:lang="en">duration</rdfs:label>
    <rdfs:label xml:lang="fi">kesto</rdfs:label>
    <rdfs:domain rdf:nodeID="nd5a8377479bd46e890352259af2eb06cb1"/>
    <rdfs:range rdf:resource="http://www.w3.org/2000/01/rdf-schema#Literal"/>
    <rdf:type rdf:resource="http://www.w3.org/2002/07/owl#DatatypeProperty"/>
    <bffi-meta:exactMatch rdf:resource="http://rdaregistry.info/Elements/e/P20219"/>
    <rdfs:subPropertyOf rdf:resource="http://id.loc.gov/ontologies/bibframe/duration"/>
  </rdf:Description>
  <rdf:Description rdf:about="http://urn.fi/URN:NBN:fi:schema:bffi:collectionAccrualMethod">
    <dct:modified>2024-04-16 (New)</dct:modified>
    <rdfs:label xml:lang="en">collection accrual method</rdfs:label>
    <rdfs:label xml:lang="fi">kokoelman kartuntamenetelmä</rdfs:label>
    <rdfs:domain rdf:resource="http://urn.fi/URN:NBN:fi:schema:bffi:CollectionWork"/>
    <rdfs:range rdf:resource="http://urn.fi/URN:NBN:fi:schema:bffi:CollectionAccrualMethod"/>
    <rdf:type rdf:resource="http://www.w3.org/2002/07/owl#ObjectProperty"/>
    <bffi-meta:broadMatch rdf:resource="http://id.loc.gov/ontologies/bibframe/usageAndAccessPolicy"/>
    <bffi-meta:exactMatch rdf:resource="http://rdaregistry.info/Elements/w/P10608"/>
  </rdf:Description>
  <rdf:Description rdf:about="http://urn.fi/URN:NBN:fi:schema:bffi:Temporal">
    <dct:modified>2024-02-23 (New)</dct:modified>
    <rdfs:label xml:lang="en">Temporal concept</rdfs:label>
    <rdfs:label xml:lang="fi">Ajanjakso</rdfs:label>
    <rdf:type rdf:resource="http://www.w3.org/2002/07/owl#Class"/>
    <owl:equivalentClass rdf:resource="http://id.loc.gov/ontologies/bibframe/Temporal"/>
    <bffi-meta:closeMatch rdf:resource="http://rdaregistry.info/Elements/c/C10010"/>
    <skos:definition xml:lang="en">BIBFRAME definition: Chronological period</skos:definition>
  </rdf:Description>
  <rdf:Description rdf:about="http://urn.fi/URN:NBN:fi:schema:bffi:classification">
    <dct:modified>2024-02-23 (New)</dct:modified>
    <rdfs:label xml:lang="en">classification</rdfs:label>
    <rdfs:label xml:lang="fi">luokitus</rdfs:label>
    <rdfs:domain rdf:resource="http://urn.fi/URN:NBN:fi:schema:bffi:Work"/>
    <rdfs:range rdf:resource="http://urn.fi/URN:NBN:fi:schema:bffi:Classification"/>
    <rdf:type rdf:resource="http://www.w3.org/2002/07/owl#ObjectProperty"/>
    <owl:equivalentProperty rdf:resource="http://id.loc.gov/ontologies/bibframe/classification"/>
    <bffi-meta:closeMatch rdf:resource="http://rdaregistry.info/Elements/w/P10256"/>
    <skos:definition xml:lang="en">BIBFRAME definition: Classification number in any scheme.</skos:definition>
  </rdf:Description>
  <rdf:Description rdf:about="http://urn.fi/URN:NBN:fi:schema:bffi:lastIssue">
    <dct:modified>2024-02-23 (New)</dct:modified>
    <rdfs:label xml:lang="en">multipart last issue</rdfs:label>
    <rdfs:label xml:lang="fi">viimeinen numero</rdfs:label>
    <rdfs:domain rdf:resource="http://urn.fi/URN:NBN:fi:schema:bffi:Manifestation"/>
    <rdfs:range rdf:resource="http://www.w3.org/2000/01/rdf-schema#Literal"/>
    <rdf:type rdf:resource="http://www.w3.org/2002/07/owl#DatatypeProperty"/>
    <owl:equivalentProperty rdf:resource="http://id.loc.gov/ontologies/bibframe/lastIssue"/>
    <skos:definition xml:lang="en">BIBFRAME definition: Ending date of a resource and/or the sequential designations.</skos:definition>
  </rdf:Description>
  <rdf:Description rdf:about="http://urn.fi/URN:NBN:fi:schema:bffi:verticalScale">
    <dct:modified>2024-02-23 (New)</dct:modified>
    <rdfs:label xml:lang="en">vertical scale of cartographic content</rdfs:label>
    <rdfs:label xml:lang="fi">kartografisen sisällön vertikaalinen mittakaava</rdfs:label>
    <rdfs:domain rdf:resource="http://urn.fi/URN:NBN:fi:schema:bffi:CartographyExpression"/>
    <rdfs:range rdf:resource="http://urn.fi/URN:NBN:fi:schema:bffi:Scale"/>
    <rdf:type rdf:resource="http://www.w3.org/2002/07/owl#ObjectProperty"/>
    <bffi-meta:broadMatch rdf:resource="http://id.loc.gov/ontologies/bibframe/scale"/>
    <bffi-meta:exactMatch rdf:resource="http://rdaregistry.info/Elements/e/P20230"/>
    <rdfs:subPropertyOf rdf:resource="http://urn.fi/URN:NBN:fi:schema:bffi:scale"/>
  </rdf:Description>
  <rdf:Description rdf:about="http://urn.fi/URN:NBN:fi:schema:bffi:TableOfContents">
    <dct:modified>2024-11-22 (New)</dct:modified>
    <rdfs:label xml:lang="en">Table of contents</rdfs:label>
    <rdfs:label xml:lang="fi">Sisältöhuomautus</rdfs:label>
    <rdf:type rdf:resource="http://www.w3.org/2002/07/owl#Class"/>
    <owl:equivalentClass rdf:resource="http://id.loc.gov/ontologies/bibframe/TableOfContents"/>
    <skos:definition xml:lang="en">BIBFRAME definition: Table of contents of a resource</skos:definition>
  </rdf:Description>
  <rdf:Description rdf:about="http://urn.fi/URN:NBN:fi:schema:bffi:colorContent">
    <dct:modified>2024-04-16 (New)</dct:modified>
    <rdfs:label xml:lang="en">color content</rdfs:label>
    <rdfs:label xml:lang="fi">värisisältö</rdfs:label>
    <rdfs:domain rdf:resource="http://urn.fi/URN:NBN:fi:schema:bffi:Manifestation"/>
    <rdfs:range rdf:resource="http://urn.fi/URN:NBN:fi:schema:bffi:ColorContent"/>
    <rdf:type rdf:resource="http://www.w3.org/2002/07/owl#ObjectProperty"/>
    <owl:equivalentProperty rdf:resource="http://id.loc.gov/ontologies/bibframe/colorContent"/>
    <bffi-meta:exactMatch rdf:resource="http://rdaregistry.info/Elements/m/P30456"/>
    <skos:definition xml:lang="en">BIBFRAME definition: Color characteristics, e.g., black and white, multicolored.</skos:definition>
  </rdf:Description>
  <rdf:Description rdf:about="http://urn.fi/URN:NBN:fi:schema:bffi:Script">
    <dct:modified>2024-02-23 (New)</dct:modified>
    <rdfs:label xml:lang="en">Script</rdfs:label>
    <rdfs:label xml:lang="fi">Kirjoitusjärjestelmä</rdfs:label>
    <rdf:type rdf:resource="http://www.w3.org/2002/07/owl#Class"/>
    <owl:equivalentClass rdf:resource="http://id.loc.gov/ontologies/bibframe/Script"/>
    <rdfs:subClassOf rdf:resource="http://urn.fi/URN:NBN:fi:schema:bffi:Notation"/>
    <skos:definition xml:lang="en">BIBFRAME definition: Information on the script, or symbol system used to convey the content of a text resource</skos:definition>
  </rdf:Description>
  <rdf:Description rdf:nodeID="n71c313d9323b40c29dadafedf28680eeb5">
    <rdf:first rdf:resource="http://urn.fi/URN:NBN:fi:schema:bffi:Item"/>
    <rdf:rest rdf:resource="http://www.w3.org/1999/02/22-rdf-syntax-ns#nil"/>
  </rdf:Description>
  <rdf:Description rdf:nodeID="n3db75dd6e811409899be21399dda0ca7b3">
    <rdf:first rdf:resource="http://urn.fi/URN:NBN:fi:schema:bffi:Organization"/>
    <rdf:rest rdf:resource="http://www.w3.org/1999/02/22-rdf-syntax-ns#nil"/>
  </rdf:Description>
  <rdf:Description rdf:about="http://urn.fi/URN:NBN:fi:schema:bffi:ObjectCount">
    <dct:modified>2024-04-16 (New)</dct:modified>
    <rdfs:label xml:lang="en">Digital cartographic object count</rdfs:label>
    <rdfs:label xml:lang="fi">Objektien lukumäärä</rdfs:label>
    <rdf:type rdf:resource="http://www.w3.org/2002/07/owl#Class"/>
    <owl:equivalentClass rdf:resource="http://id.loc.gov/ontologies/bibframe/ObjectCount"/>
    <rdfs:subClassOf rdf:resource="http://urn.fi/URN:NBN:fi:schema:bffi:DigitalCharacteristic"/>
    <skos:definition xml:lang="en">BIBFRAME definition: Number of objects in encoded geospatial information in a cartographic resource</skos:definition>
  </rdf:Description>
  <rdf:Description rdf:about="http://urn.fi/URN:NBN:fi:schema:bffi:awards">
    <dct:modified>2024-02-23 (New)</dct:modified>
    <rdfs:label xml:lang="en">award</rdfs:label>
    <rdfs:label xml:lang="fi">palkinto</rdfs:label>
    <rdfs:domain rdf:resource="http://urn.fi/URN:NBN:fi:schema:bffi:Expression"/>
    <rdfs:range rdf:resource="http://www.w3.org/2000/01/rdf-schema#Literal"/>
    <rdf:type rdf:resource="http://www.w3.org/2002/07/owl#DatatypeProperty"/>
    <owl:equivalentProperty rdf:resource="http://id.loc.gov/ontologies/bibframe/awards"/>
    <bffi-meta:exactMatch rdf:resource="http://rdaregistry.info/Elements/e/P20005"/>
    <skos:definition xml:lang="en">BIBFRAME definition: Information on awards associated with the described resource.</skos:definition>
  </rdf:Description>
  <rdf:Description rdf:nodeID="n71c313d9323b40c29dadafedf28680eeb3">
    <rdf:first rdf:resource="http://urn.fi/URN:NBN:fi:schema:bffi:Expression"/>
    <rdf:rest rdf:nodeID="n71c313d9323b40c29dadafedf28680eeb4"/>
  </rdf:Description>
  <rdf:Description rdf:nodeID="n0a20977f4ff64f88b13306bf2d732ab6b3">
    <rdf:first rdf:resource="http://urn.fi/URN:NBN:fi:schema:bffi:Manifestation"/>
    <rdf:rest rdf:resource="http://www.w3.org/1999/02/22-rdf-syntax-ns#nil"/>
  </rdf:Description>
  <rdf:Description rdf:about="http://urn.fi/URN:NBN:fi:schema:bffi:Relationship">
    <dct:modified>2024-09-16 (New)</dct:modified>
    <rdfs:label xml:lang="en">Relationship</rdfs:label>
    <rdfs:label xml:lang="fi">Suhdetyyppi</rdfs:label>
    <rdf:type rdf:resource="http://www.w3.org/2002/07/owl#Class"/>
    <owl:equivalentClass rdf:resource="http://id.loc.gov/ontologies/bibframe/Relationship"/>
    <skos:definition xml:lang="en">BIBFRAME definition: Type of relationship between resources</skos:definition>
  </rdf:Description>
  <rdf:Description rdf:nodeID="n23d9c564949d4a53a71610ff1e9857f7b2">
    <rdf:first rdf:resource="http://urn.fi/URN:NBN:fi:schema:bffi:Manifestation"/>
    <rdf:rest rdf:nodeID="n23d9c564949d4a53a71610ff1e9857f7b3"/>
  </rdf:Description>
  <rdf:Description rdf:about="http://urn.fi/URN:NBN:fi:schema:bffi:projectionCharacteristic">
    <dct:modified>2024-11-22 (New)</dct:modified>
    <rdfs:label xml:lang="en">projection characteristic</rdfs:label>
    <rdfs:label xml:lang="fi">elokuvafilmin projisointiominaisuudet</rdfs:label>
    <rdfs:domain rdf:resource="http://urn.fi/URN:NBN:fi:schema:bffi:Manifestation"/>
    <rdfs:range rdf:resource="http://urn.fi/URN:NBN:fi:schema:bffi:ProjectionCharacteristic"/>
    <rdf:type rdf:resource="http://www.w3.org/2002/07/owl#ObjectProperty"/>
    <owl:equivalentProperty rdf:resource="http://id.loc.gov/ontologies/bibframe/projectionCharacteristic"/>
    <skos:definition xml:lang="en">BIBFRAME definition: Technical specification relating to the projection of a motion picture film.</skos:definition>
  </rdf:Description>
  <rdf:Description rdf:about="http://urn.fi/URN:NBN:fi:schema:bffi:Degree">
    <dct:modified>2024-02-23 (New)</dct:modified>
    <rdfs:label xml:lang="en">Degree</rdfs:label>
    <rdfs:label xml:lang="fi">Oppiarvo</rdfs:label>
    <rdf:type rdf:resource="http://www.w3.org/2002/07/owl#Class"/>
  </rdf:Description>
  <rdf:Description rdf:about="http://urn.fi/URN:NBN:fi:schema:bffi:Place">
    <dct:modified>2024-02-23 (New)</dct:modified>
    <rdfs:label xml:lang="en">Place</rdfs:label>
    <rdfs:label xml:lang="fi">Paikka</rdfs:label>
    <rdf:type rdf:resource="http://www.w3.org/2002/07/owl#Class"/>
    <owl:equivalentClass rdf:resource="http://id.loc.gov/ontologies/bibframe/Place"/>
    <bffi-meta:exactMatch rdf:resource="http://rdaregistry.info/Elements/c/C10009"/>
    <skos:definition xml:lang="en">BIBFRAME definition: Geographic location</skos:definition>
  </rdf:Description>
  <rdf:Description rdf:about="http://urn.fi/URN:NBN:fi:schema:bffi:SerialWork">
    <dct:modified>2024-02-23 (New)</dct:modified>
    <rdfs:label xml:lang="en">Serial work</rdfs:label>
    <rdfs:label xml:lang="fi">Sarjamaisesti ilmestynyt teos</rdfs:label>
    <rdf:type rdf:resource="http://www.w3.org/2002/07/owl#Class"/>
    <bffi-meta:broadMatch rdf:resource="http://id.loc.gov/ontologies/bibframe/Serial"/>
    <rdfs:subClassOf rdf:resource="http://urn.fi/URN:NBN:fi:schema:bffi:Work"/>
    <owl:disjointWith rdf:resource="http://urn.fi/URN:NBN:fi:schema:bffi:SeriesWork"/>
  </rdf:Description>
  <rdf:Description rdf:about="http://urn.fi/URN:NBN:fi:schema:bffi:AggregatingWork">
    <dct:modified>2024-02-23 (New)</dct:modified>
    <rdfs:label xml:lang="en">Aggregating work</rdfs:label>
    <rdfs:label xml:lang="fi">Aggregoiva teos</rdfs:label>
    <rdf:type rdf:resource="http://www.w3.org/2002/07/owl#Class"/>
    <bffi-meta:broadMatch rdf:resource="http://id.loc.gov/ontologies/bibframe/Work"/>
    <rdfs:subClassOf rdf:resource="http://urn.fi/URN:NBN:fi:schema:bffi:Work"/>
  </rdf:Description>
  <rdf:Description rdf:about="http://urn.fi/URN:NBN:fi:schema:bffi:Production">
    <dct:modified>2024-02-23 (New)</dct:modified>
    <rdfs:label xml:lang="en">Producer</rdfs:label>
    <rdfs:label xml:lang="fi">Tuottaja</rdfs:label>
    <rdf:type rdf:resource="http://www.w3.org/2002/07/owl#Class"/>
    <owl:equivalentClass rdf:resource="http://id.loc.gov/ontologies/bibframe/Production"/>
    <bffi-meta:broadMatch rdf:resource="http://rdaregistry.info/Elements/c/C10005"/>
    <rdfs:subClassOf rdf:resource="http://urn.fi/URN:NBN:fi:schema:bffi:ProvisionActivity"/>
    <skos:definition xml:lang="en">BIBFRAME definition: Information relating to production of a resource</skos:definition>
  </rdf:Description>
  <rdf:Description rdf:about="http://urn.fi/URN:NBN:fi:schema:bffi:cartographicProjectionOfRepresentativeExpression">
    <dct:modified>2024-04-16 (New)</dct:modified>
    <rdfs:label xml:lang="en">cartographic projection of representative expression</rdfs:label>
    <rdfs:label xml:lang="fi">edustavan ekspression karttaprojektio</rdfs:label>
    <rdfs:domain rdf:resource="http://urn.fi/URN:NBN:fi:schema:bffi:Work"/>
    <rdfs:range rdf:resource="http://urn.fi/URN:NBN:fi:schema:bffi:Projection"/>
    <rdf:type rdf:resource="http://www.w3.org/2002/07/owl#ObjectProperty"/>
    <bffi-meta:exactMatch rdf:resource="http://rdaregistry.info/Elements/w/P10355"/>
    <rdfs:subPropertyOf rdf:resource="http://id.loc.gov/ontologies/bibframe/projection"/>
  </rdf:Description>
  <rdf:Description rdf:about="http://urn.fi/URN:NBN:fi:schema:bffi:numberingOfSequence">
    <dct:modified>2025-01-02 (New)</dct:modified>
    <rdfs:label xml:lang="en">numbering of sequence</rdfs:label>
    <rdfs:label xml:lang="fi">numerointijakso</rdfs:label>
    <rdfs:domain rdf:resource="http://urn.fi/URN:NBN:fi:schema:bffi:Manifestation"/>
    <rdfs:range rdf:resource="http://www.w3.org/2000/01/rdf-schema#Literal"/>
    <rdf:type rdf:resource="http://www.w3.org/2002/07/owl#DatatypeProperty"/>
    <bffi-meta:narrowMatch rdf:resource="http://id.loc.gov/ontologies/bibframe/firstIssue"/>
    <bffi-meta:narrowMatch rdf:resource="http://id.loc.gov/ontologies/bibframe/lastIssue"/>
    <bffi-meta:exactMatch rdf:resource="http://rdaregistry.info/Elements/m/P30165"/>
  </rdf:Description>
  <rdf:Description rdf:about="http://urn.fi/URN:NBN:fi:schema:bffi:collectionArrangementOf">
    <owl:inverseOf rdf:resource="http://urn.fi/URN:NBN:fi:schema:bffi:collectionArrangement"/>
    <dct:modified>2024-04-16 (New)</dct:modified>
    <rdfs:label xml:lang="en">organization and arrangement of collection</rdfs:label>
    <rdfs:label xml:lang="fi">järjestämisperiaate aineistolle</rdfs:label>
    <rdfs:domain rdf:resource="http://urn.fi/URN:NBN:fi:schema:bffi:CollectionArrangement"/>
    <rdfs:range rdf:nodeID="n30938fe99dde46599fe6796e2af454deb1"/>
    <rdf:type rdf:resource="http://www.w3.org/2002/07/owl#ObjectProperty"/>
    <owl:equivalentProperty rdf:resource="http://id.loc.gov/ontologies/bibframe/collectionArrangementOf"/>
    <skos:definition xml:lang="en">BIBFRAME definition: Relates an Arrangement resource to that which it describes.</skos:definition>
  </rdf:Description>
  <rdf:Description rdf:about="http://urn.fi/URN:NBN:fi:schema:bffi:partNumber">
    <dct:modified>2024-02-23 (New)</dct:modified>
    <rdfs:label xml:lang="en">part number</rdfs:label>
    <rdfs:label xml:lang="fi">osan numero</rdfs:label>
    <rdfs:domain rdf:resource="http://urn.fi/URN:NBN:fi:schema:bffi:Title"/>
    <rdfs:range rdf:resource="http://www.w3.org/2000/01/rdf-schema#Literal"/>
    <rdf:type rdf:resource="http://www.w3.org/2002/07/owl#DatatypeProperty"/>
    <owl:equivalentProperty rdf:resource="http://id.loc.gov/ontologies/bibframe/partNumber"/>
    <bffi-meta:exactMatch rdf:resource="http://rdaregistry.info/Elements/w/P10012"/>
    <skos:definition xml:lang="en">BIBFRAME definition: Part or section enumeration of a title. Possible title component.</skos:definition>
  </rdf:Description>
  <rdf:Description rdf:about="http://urn.fi/URN:NBN:fi:schema:bffi:productionStatement">
    <dct:modified>2024-09-16 (New)</dct:modified>
    <rdfs:label xml:lang="en">production statement</rdfs:label>
    <rdfs:label xml:lang="fi">tuotantomerkintö</rdfs:label>
    <rdfs:domain rdf:resource="http://urn.fi/URN:NBN:fi:schema:bffi:Manifestation"/>
    <rdfs:range rdf:resource="http://www.w3.org/2000/01/rdf-schema#Literal"/>
    <rdf:type rdf:resource="http://www.w3.org/2002/07/owl#DatatypeProperty"/>
    <owl:equivalentProperty rdf:resource="http://id.loc.gov/ontologies/bibframe/productionStatement"/>
    <bffi-meta:exactMatch rdf:resource="http://rdaregistry.info/Elements/m/P30110"/>
    <skos:definition xml:lang="en">BIBFRAME definition: Statement related to the production of the resources; usually transcribed.</skos:definition>
  </rdf:Description>
  <rdf:Description rdf:about="http://urn.fi/URN:NBN:fi:schema:bffi:AspectRatio">
    <dct:modified>2024-11-22 (New)</dct:modified>
    <rdfs:label xml:lang="en">Aspect ratio</rdfs:label>
    <rdfs:label xml:lang="fi">Kuvasuhde</rdfs:label>
    <bffi-meta:relatedValueVocabulary rdf:resource="http://urn.fi/URN:NBN:fi:au:mts:m1988"/>
    <rdf:type rdf:resource="http://www.w3.org/2002/07/owl#Class"/>
    <owl:equivalentClass rdf:resource="http://id.loc.gov/ontologies/bibframe/AspectRatio"/>
    <rdfs:seeAlso rdf:resource="http://rdaregistry.info/termList/AspectRatio/"/>
    <skos:definition xml:lang="en">BIBFRAME definition: Proportional relationship between an image's width and its height</skos:definition>
  </rdf:Description>
  <rdf:Description rdf:about="http://urn.fi/URN:NBN:fi:schema:bffi:code">
    <dct:modified>2024-02-23 (New)</dct:modified>
    <rdfs:label xml:lang="en">code</rdfs:label>
    <rdfs:label xml:lang="fi">koodi</rdfs:label>
    <rdfs:domain rdf:resource="http://www.w3.org/2000/01/rdf-schema#Resource"/>
    <rdfs:range rdf:resource="http://www.w3.org/2000/01/rdf-schema#Literal"/>
    <rdf:type rdf:resource="http://www.w3.org/2002/07/owl#DatatypeProperty"/>
    <owl:equivalentProperty rdf:resource="http://id.loc.gov/ontologies/bibframe/code"/>
    <skos:definition xml:lang="en">BIBFRAME definition: String of characters that serves as a code representing information.</skos:definition>
  </rdf:Description>
  <rdf:Description rdf:about="http://urn.fi/URN:NBN:fi:schema:bffi:mainTitle">
    <dct:modified>2024-02-23 (New)</dct:modified>
    <rdfs:label xml:lang="en">main title</rdfs:label>
    <rdfs:label xml:lang="fi">nimekkeen merkkijono</rdfs:label>
    <rdfs:domain rdf:resource="http://urn.fi/URN:NBN:fi:schema:bffi:Title"/>
    <rdfs:range rdf:resource="http://www.w3.org/2000/01/rdf-schema#Literal"/>
    <rdf:type rdf:resource="http://www.w3.org/2002/07/owl#DatatypeProperty"/>
    <owl:equivalentProperty rdf:resource="http://id.loc.gov/ontologies/bibframe/mainTitle"/>
    <skos:definition xml:lang="en">BIBFRAME definition: Title being addressed. Possible title component.</skos:definition>
  </rdf:Description>
  <rdf:Description rdf:about="http://urn.fi/URN:NBN:fi:schema:bffi:scaleOfStillImageOrThreeDimensionalForm">
    <dct:modified>2024-04-16 (New)</dct:modified>
    <rdfs:label xml:lang="en">scale of still image or three-dimensional form</rdfs:label>
    <rdfs:label xml:lang="fi">stillkuvan tai kolmiulotteisen muodon mittakaava</rdfs:label>
    <rdfs:domain rdf:nodeID="na62f4311181e4083bd9b0ad0c31f158ab1"/>
    <rdfs:range rdf:resource="http://urn.fi/URN:NBN:fi:schema:bffi:Scale"/>
    <rdf:type rdf:resource="http://www.w3.org/2002/07/owl#ObjectProperty"/>
    <bffi-meta:broadMatch rdf:resource="http://id.loc.gov/ontologies/bibframe/scale"/>
    <bffi-meta:exactMatch rdf:resource="http://rdaregistry.info/Elements/e/P20227"/>
    <rdfs:subPropertyOf rdf:resource="http://urn.fi/URN:NBN:fi:schema:bffi:scale"/>
  </rdf:Description>
  <rdf:Description rdf:about="http://urn.fi/URN:NBN:fi:schema:bffi:aspectRatio">
    <dct:modified>2024-11-22 (New)</dct:modified>
    <rdfs:label xml:lang="en">aspect ratio</rdfs:label>
    <rdfs:label xml:lang="fi">kuvasuhde</rdfs:label>
    <rdfs:domain rdf:resource="http://urn.fi/URN:NBN:fi:schema:bffi:MovingImageExpression"/>
    <rdfs:range rdf:resource="http://urn.fi/URN:NBN:fi:schema:bffi:AspectRatio"/>
    <rdf:type rdf:resource="http://www.w3.org/2002/07/owl#ObjectProperty"/>
    <bffi-meta:exactMatch rdf:resource="http://rdaregistry.info/Elements/e/P20229"/>
    <rdfs:subPropertyOf rdf:resource="http://id.loc.gov/ontologies/bibframe/aspectRatio"/>
  </rdf:Description>
  <rdf:Description rdf:about="http://urn.fi/URN:NBN:fi:schema:bffi:PrimaryContribution">
    <dct:modified>2024-02-23 (New)</dct:modified>
    <rdfs:label xml:lang="en">Primary contribution</rdfs:label>
    <rdfs:label xml:lang="fi">Päävastuullinen tekijä</rdfs:label>
    <rdf:type rdf:resource="http://www.w3.org/2002/07/owl#Class"/>
    <owl:equivalentClass rdf:resource="http://id.loc.gov/ontologies/bibframe/PrimaryContribution"/>
    <rdfs:subClassOf rdf:resource="http://urn.fi/URN:NBN:fi:schema:bffi:Contribution"/>
    <skos:definition xml:lang="en">BIBFRAME definition: Contribution for which the agent is the name chosen as the name part of the name and title access point</skos:definition>
  </rdf:Description>
  <rdf:Description rdf:nodeID="n90e14c5f212f40b8a6a776d86788ca21b2">
    <rdf:first rdf:resource="http://urn.fi/URN:NBN:fi:schema:bffi:Work"/>
    <rdf:rest rdf:nodeID="n90e14c5f212f40b8a6a776d86788ca21b3"/>
  </rdf:Description>
  <rdf:Description rdf:about="http://urn.fi/URN:NBN:fi:schema:bffi:grantingInstitution">
    <dct:modified>2024-02-23 (New)</dct:modified>
    <rdfs:label xml:lang="en">degree granting institution</rdfs:label>
    <rdfs:label xml:lang="fi">oppiarvon myöntävä yhteisö</rdfs:label>
    <rdfs:domain rdf:resource="http://urn.fi/URN:NBN:fi:schema:bffi:Dissertation"/>
    <rdfs:range rdf:resource="http://urn.fi/URN:NBN:fi:schema:bffi:Organization"/>
    <rdf:type rdf:resource="http://www.w3.org/2002/07/owl#ObjectProperty"/>
    <bffi-meta:closeMatch rdf:resource="http://id.loc.gov/ontologies/bibframe/grantingInstitution"/>
    <bffi-meta:closeMatch rdf:resource="http://rdaregistry.info/Elements/w/P10006"/>
  </rdf:Description>
  <rdf:Description rdf:about="http://urn.fi/URN:NBN:fi:schema:bffi:musicKey">
    <dct:modified>2024-02-23 (New)</dct:modified>
    <rdfs:label xml:lang="en">music key</rdfs:label>
    <rdfs:label xml:lang="fi">sävellaji</rdfs:label>
    <rdfs:domain rdf:resource="http://urn.fi/URN:NBN:fi:schema:bffi:MusicWork"/>
    <rdfs:range rdf:resource="http://www.w3.org/2000/01/rdf-schema#Literal"/>
    <rdf:type rdf:resource="http://www.w3.org/2002/07/owl#DatatypeProperty"/>
    <owl:equivalentProperty rdf:resource="http://id.loc.gov/ontologies/bibframe/musicKey"/>
    <bffi-meta:narrowMatch rdf:resource="http://rdaregistry.info/Elements/e/P20326"/>
    <bffi-meta:narrowMatch rdf:resource="http://rdaregistry.info/Elements/w/P10221"/>
    <skos:definition xml:lang="en">BIBFRAME definition: Pitch and mode for music.</skos:definition>
  </rdf:Description>
  <rdf:Description rdf:about="http://urn.fi/URN:NBN:fi:schema:bffi:metadataLicensor">
    <dct:modified>2024-06-19 (New)</dct:modified>
    <rdfs:label xml:lang="en">metadata licensor</rdfs:label>
    <rdfs:label xml:lang="fi">metatiedon tekijänoikeus</rdfs:label>
    <rdfs:domain rdf:resource="http://urn.fi/URN:NBN:fi:schema:bffi:AdminMetadata"/>
    <rdfs:range rdf:resource="http://urn.fi/URN:NBN:fi:schema:bffi:MetadataLicensor"/>
    <rdf:type rdf:resource="http://www.w3.org/2002/07/owl#ObjectProperty"/>
    <owl:equivalentProperty rdf:resource="http://id.loc.gov/ontologies/bflc/metadataLicensor"/>
    <skos:definition xml:lang="en">BFLC definition: Organization that licenses the intellectual property rights to the data contained in the description.</skos:definition>
  </rdf:Description>
  <rdf:Description rdf:about="http://urn.fi/URN:NBN:fi:schema:bffi:nonSortNum">
    <dct:modified>2024-11-22 (New)</dct:modified>
    <rdfs:label xml:lang="en">non-sort character count</rdfs:label>
    <rdfs:label xml:lang="fi">ohitettavien merkkien määrä</rdfs:label>
    <rdfs:domain rdf:resource="http://urn.fi/URN:NBN:fi:schema:bffi:Title"/>
    <rdfs:range rdf:resource="http://www.w3.org/2000/01/rdf-schema#Literal"/>
    <rdf:type rdf:resource="http://www.w3.org/2002/07/owl#DatatypeProperty"/>
    <owl:equivalentProperty rdf:resource="http://id.loc.gov/ontologies/bflc/nonSortNum"/>
    <skos:definition xml:lang="en">BFLC definition: Number of characters at the start of a label that should be skipped for indexing and sorting.</skos:definition>
  </rdf:Description>
  <rdf:Description rdf:about="http://urn.fi/URN:NBN:fi:schema:bffi:OperatingSystem">
    <dct:modified>2024-11-22 (New)</dct:modified>
    <rdfs:label xml:lang="en">Operating system</rdfs:label>
    <rdfs:label xml:lang="fi">Käyttöjärjestelmä</rdfs:label>
    <rdf:type rdf:resource="http://www.w3.org/2002/07/owl#Class"/>
    <owl:equivalentClass rdf:resource="http://id.loc.gov/ontologies/bflc/OperatingSystem"/>
    <rdfs:subClassOf rdf:resource="http://urn.fi/URN:NBN:fi:schema:bffi:SystemRequirement"/>
    <skos:definition xml:lang="en">BFLC definition: Software that directly operates a system's hardware and serves as a platform for applications.</skos:definition>
  </rdf:Description>
  <rdf:Description rdf:about="http://urn.fi/URN:NBN:fi:schema:bffi:reductionRatio">
    <dct:modified>2024-11-22 (New)</dct:modified>
    <rdfs:label xml:lang="en">reduction ratio</rdfs:label>
    <rdfs:label xml:lang="fi">pienennyssuhde</rdfs:label>
    <rdfs:domain rdf:resource="http://urn.fi/URN:NBN:fi:schema:bffi:Microform"/>
    <rdfs:range rdf:resource="http://urn.fi/URN:NBN:fi:schema:bffi:ReductionRatio"/>
    <rdf:type rdf:resource="http://www.w3.org/2002/07/owl#ObjectProperty"/>
    <owl:equivalentProperty rdf:resource="http://id.loc.gov/ontologies/bibframe/reductionRatio"/>
    <bffi-meta:exactMatch rdf:resource="http://rdaregistry.info/Elements/m/P30198"/>
    <skos:definition xml:lang="en">BIBFRAME definition: Size of a micro-image in relation to the original from which it was produced.</skos:definition>
  </rdf:Description>
  <rdf:Description rdf:about="http://urn.fi/URN:NBN:fi:schema:bffi:validDate">
    <dct:modified>2024-11-22 (New)</dct:modified>
    <rdfs:label xml:lang="en">valid date</rdfs:label>
    <rdfs:label xml:lang="fi">voimassaoloaika</rdfs:label>
    <rdfs:domain rdf:resource="http://urn.fi/URN:NBN:fi:schema:bffi:Work"/>
    <rdfs:range rdf:resource="http://www.w3.org/2000/01/rdf-schema#Literal"/>
    <rdf:type rdf:resource="http://www.w3.org/2002/07/owl#DatatypeProperty"/>
    <owl:equivalentProperty rdf:resource="http://id.loc.gov/ontologies/bibframe/validDate"/>
    <bffi-meta:broadMatch rdf:resource="http://rdaregistry.info/Elements/w/P10317"/>
    <rdfs:subPropertyOf rdf:resource="http://urn.fi/URN:NBN:fi:schema:bffi:date"/>
    <skos:definition xml:lang="en">BIBFRAME definition: The date or date range during which the resource is accurate.</skos:definition>
  </rdf:Description>
  <rdf:Description rdf:about="http://urn.fi/URN:NBN:fi:schema:bffi:Material">
    <dct:modified>2024-09-16 (New)</dct:modified>
    <rdfs:label xml:lang="en">Material</rdfs:label>
    <rdfs:label xml:lang="fi">Materiaali</rdfs:label>
    <bffi-meta:relatedValueVocabulary rdf:resource="http://urn.fi/URN:NBN:fi:au:mts:m654"/>
    <rdf:type rdf:resource="http://www.w3.org/2002/07/owl#Class"/>
    <owl:equivalentClass rdf:resource="http://id.loc.gov/ontologies/bibframe/Material"/>
    <rdfs:seeAlso rdf:resource="http://rdaregistry.info/termList/RDAMaterial/"/>
    <skos:definition xml:lang="en">BIBFRAME definition: Substance or composition of the resource</skos:definition>
  </rdf:Description>
  <rdf:Description rdf:about="http://urn.fi/URN:NBN:fi:schema:bffi:cartographicAttributes">
    <dct:modified>2024-02-23 (New)</dct:modified>
    <rdfs:label xml:lang="en">cartographic data</rdfs:label>
    <rdfs:label xml:lang="fi">kartografinen data</rdfs:label>
    <rdfs:domain rdf:resource="http://urn.fi/URN:NBN:fi:schema:bffi:Work"/>
    <rdfs:range rdf:resource="http://urn.fi/URN:NBN:fi:schema:bffi:Cartographic"/>
    <rdf:type rdf:resource="http://www.w3.org/2002/07/owl#ObjectProperty"/>
    <owl:equivalentProperty rdf:resource="http://id.loc.gov/ontologies/bibframe/cartographicAttributes"/>
    <skos:definition xml:lang="en">BIBFRAME definition: Cartographic data that identifies characteristics of the resource, such as coordinates, projection, etc.</skos:definition>
  </rdf:Description>
  <rdf:Description rdf:about="http://urn.fi/URN:NBN:fi:schema:bffi:Enumeration">
    <dct:modified>2024-02-23 (New)</dct:modified>
    <rdfs:label xml:lang="en">Enumeration</rdfs:label>
    <rdfs:label xml:lang="fi">Numerointi</rdfs:label>
    <rdf:type rdf:resource="http://www.w3.org/2002/07/owl#Class"/>
    <owl:equivalentClass rdf:resource="http://id.loc.gov/ontologies/bibframe/Enumeration"/>
    <rdfs:subClassOf rdf:resource="http://urn.fi/URN:NBN:fi:schema:bffi:EnumerationAndChronology"/>
    <skos:definition xml:lang="en">BIBFRAME definition: Numbering or other enumeration associated with issues or items held</skos:definition>
  </rdf:Description>
  <rdf:Description rdf:nodeID="n1e5b766c1bf94ff9812af7b852f48486b3">
    <rdf:first rdf:resource="http://urn.fi/URN:NBN:fi:schema:bffi:Expression"/>
    <rdf:rest rdf:nodeID="n1e5b766c1bf94ff9812af7b852f48486b4"/>
  </rdf:Description>
  <rdf:Description rdf:about="http://urn.fi/URN:NBN:fi:schema:bffi:subject">
    <dct:modified>2024-02-23 (New)</dct:modified>
    <rdfs:label xml:lang="en">subject</rdfs:label>
    <rdfs:label xml:lang="fi">aihe</rdfs:label>
    <rdfs:domain rdf:resource="http://urn.fi/URN:NBN:fi:schema:bffi:Work"/>
    <rdfs:range rdf:resource="http://www.w3.org/2000/01/rdf-schema#Resource"/>
    <rdf:type rdf:resource="http://www.w3.org/2002/07/owl#ObjectProperty"/>
    <owl:equivalentProperty rdf:resource="http://id.loc.gov/ontologies/bibframe/subject"/>
    <bffi-meta:exactMatch rdf:resource="http://rdaregistry.info/Elements/w/P10256"/>
    <owl:inverseOf rdf:resource="http://urn.fi/URN:NBN:fi:schema:bffi:subjectOf"/>
    <skos:definition xml:lang="en">BIBFRAME definition: Subject term(s) describing a resource.</skos:definition>
  </rdf:Description>
  <rdf:Description rdf:about="http://urn.fi/URN:NBN:fi:schema:bffi:scaleOfRepresentativeExpression">
    <dct:modified>2024-04-16 (New)</dct:modified>
    <rdfs:label xml:lang="en">scale of representative expression</rdfs:label>
    <rdfs:label xml:lang="fi">edustavan ekspression mittakaava</rdfs:label>
    <rdfs:domain rdf:resource="http://urn.fi/URN:NBN:fi:schema:bffi:Work"/>
    <rdfs:range rdf:resource="http://urn.fi/URN:NBN:fi:schema:bffi:Scale"/>
    <rdf:type rdf:resource="http://www.w3.org/2002/07/owl#ObjectProperty"/>
    <bffi-meta:closeMatch rdf:resource="http://id.loc.gov/ontologies/bibframe/scale"/>
    <bffi-meta:exactMatch rdf:resource="http://rdaregistry.info/Elements/w/P10356"/>
  </rdf:Description>
  <rdf:Description rdf:about="http://urn.fi/URN:NBN:fi:schema:bffi:derivedFrom">
    <dct:modified>2024-02-23 (New)</dct:modified>
    <rdfs:label xml:lang="en">source metadata</rdfs:label>
    <rdfs:label xml:lang="fi">lähdemetatieto</rdfs:label>
    <rdfs:domain rdf:resource="http://urn.fi/URN:NBN:fi:schema:bffi:AdminMetadata"/>
    <rdfs:range rdf:resource="http://www.w3.org/2000/01/rdf-schema#Resource"/>
    <rdf:type rdf:resource="http://www.w3.org/2002/07/owl#ObjectProperty"/>
    <owl:equivalentProperty rdf:resource="http://id.loc.gov/ontologies/bibframe/derivedFrom"/>
    <skos:definition xml:lang="en">BIBFRAME definition: Link to the metadata that was the source of the data</skos:definition>
  </rdf:Description>
  <rdf:Description rdf:about="http://urn.fi/URN:NBN:fi:schema:bffi:EncodingFormat">
    <dct:modified>2024-11-22 (New)</dct:modified>
    <rdfs:label xml:lang="en">Encoding format</rdfs:label>
    <rdfs:label xml:lang="fi">Koodausmuoto</rdfs:label>
    <bffi-meta:relatedValueVocabulary rdf:resource="http://urn.fi/URN:NBN:fi:au:mts:m88"/>
    <rdf:type rdf:resource="http://www.w3.org/2002/07/owl#Class"/>
    <owl:equivalentClass rdf:resource="http://id.loc.gov/ontologies/bibframe/EncodingFormat"/>
    <rdfs:subClassOf rdf:resource="http://urn.fi/URN:NBN:fi:schema:bffi:DigitalCharacteristic"/>
    <skos:definition xml:lang="en">BIBFRAME definition: Schema, standard, etc., used to encode the digital content of a resource, e.g., MP3, XML, JPEG</skos:definition>
  </rdf:Description>
  <rdf:Description rdf:about="http://urn.fi/URN:NBN:fi:schema:bffi:BaseMaterial">
    <dct:modified>2024-09-16 (New)</dct:modified>
    <rdfs:label xml:lang="en">Base material</rdfs:label>
    <rdfs:label xml:lang="fi">Pohjamateriaali</rdfs:label>
    <bffi-meta:relatedValueVocabulary rdf:resource="http://urn.fi/URN:NBN:fi:au:mts:m654"/>
    <rdf:type rdf:resource="http://www.w3.org/2002/07/owl#Class"/>
    <owl:equivalentClass rdf:resource="http://id.loc.gov/ontologies/bibframe/BaseMaterial"/>
    <rdfs:seeAlso rdf:resource="http://rdaregistry.info/termList/RDAMaterial/"/>
    <rdfs:subClassOf rdf:resource="http://urn.fi/URN:NBN:fi:schema:bffi:Material"/>
    <skos:definition xml:lang="en">BIBFRAME definition: Underlying physical material of a resource</skos:definition>
  </rdf:Description>
  <rdf:Description rdf:about="http://urn.fi/URN:NBN:fi:schema:bffi:binding">
    <dct:modified>2024-09-16 (New)</dct:modified>
    <rdfs:label xml:lang="en">binding method</rdfs:label>
    <rdfs:label xml:lang="fi">sidostyyppi</rdfs:label>
    <rdfs:domain rdf:resource="http://urn.fi/URN:NBN:fi:schema:bffi:Manifestation"/>
    <rdfs:range rdf:resource="http://urn.fi/URN:NBN:fi:schema:bffi:Binding"/>
    <rdf:type rdf:resource="http://www.w3.org/2002/07/owl#ObjectProperty"/>
    <owl:equivalentProperty rdf:resource="http://id.loc.gov/ontologies/bibframe/binding"/>
    <bffi-meta:exactMatch rdf:resource="http://rdaregistry.info/Elements/m/P30309"/>
    <skos:definition xml:lang="en">BIBFRAME definition: A method used to bind a published or unpublished resource,or other binding information.</skos:definition>
  </rdf:Description>
  <rdf:Description rdf:about="http://urn.fi/URN:NBN:fi:schema:bffi:descriptionConventions">
    <dct:modified>2024-06-19 (New)</dct:modified>
    <rdfs:label xml:lang="en">description conventions</rdfs:label>
    <rdfs:label xml:lang="fi">kuvailusäännöt</rdfs:label>
    <rdfs:domain rdf:resource="http://urn.fi/URN:NBN:fi:schema:bffi:AdminMetadata"/>
    <rdfs:range rdf:resource="http://urn.fi/URN:NBN:fi:schema:bffi:DescriptionConventions"/>
    <rdf:type rdf:resource="http://www.w3.org/2002/07/owl#ObjectProperty"/>
    <owl:equivalentProperty rdf:resource="http://id.loc.gov/ontologies/bibframe/descriptionConventions"/>
    <bffi-meta:closeMatch rdf:resource="http://rdaregistry.info/Elements/w/P10309"/>
    <skos:definition xml:lang="en">BIBFRAME definition: Rules used for the descriptive content of the resource description</skos:definition>
  </rdf:Description>
  <rdf:Description rdf:nodeID="nd5a8377479bd46e890352259af2eb06cb3">
    <rdf:first rdf:resource="http://urn.fi/URN:NBN:fi:schema:bffi:NonMusicAudioExpression"/>
    <rdf:rest rdf:nodeID="nd5a8377479bd46e890352259af2eb06cb4"/>
  </rdf:Description>
  <rdf:Description rdf:about="http://urn.fi/URN:NBN:fi:schema:bffi:EncodedBitrate">
    <dct:modified>2024-11-22 (New)</dct:modified>
    <rdfs:label xml:lang="en">Encoded bitrate</rdfs:label>
    <rdfs:label xml:lang="fi">Koodattu bittinopeus</rdfs:label>
    <rdf:type rdf:resource="http://www.w3.org/2002/07/owl#Class"/>
    <owl:equivalentClass rdf:resource="http://id.loc.gov/ontologies/bibframe/EncodedBitrate"/>
    <rdfs:subClassOf rdf:resource="http://urn.fi/URN:NBN:fi:schema:bffi:DigitalCharacteristic"/>
    <skos:definition xml:lang="en">BIBFRAME definition: Speed at which streaming audio, video, etc., is designed to play, e.g., 32 kbps</skos:definition>
  </rdf:Description>
  <rdf:Description rdf:nodeID="n30938fe99dde46599fe6796e2af454deb1">
    <rdf:type rdf:resource="http://www.w3.org/2002/07/owl#Class"/>
    <owl:unionOf rdf:nodeID="n30938fe99dde46599fe6796e2af454deb2"/>
  </rdf:Description>
  <rdf:Description rdf:about="http://urn.fi/URN:NBN:fi:schema:bffi:assigner">
    <dct:modified>2024-06-19 (New)</dct:modified>
    <rdfs:label xml:lang="en">assigner</rdfs:label>
    <rdfs:label xml:lang="fi">antava taho</rdfs:label>
    <rdfs:domain rdf:resource="http://www.w3.org/2000/01/rdf-schema#Resource"/>
    <rdfs:range rdf:nodeID="n3db75dd6e811409899be21399dda0ca7b1"/>
    <rdf:type rdf:resource="http://www.w3.org/2002/07/owl#ObjectProperty"/>
    <owl:equivalentProperty rdf:resource="http://id.loc.gov/ontologies/bibframe/assigner"/>
    <bffi-meta:closeMatch rdf:resource="http://rdaregistry.info/Elements/w/P10437"/>
    <bffi-meta:closeMatch rdf:resource="http://rdaregistry.info/Elements/w/P10531"/>
    <bffi-meta:closeMatch rdf:resource="http://rdaregistry.info/Elements/n/P80075"/>
    <bffi-meta:closeMatch rdf:resource="http://rdaregistry.info/Elements/n/P80077"/>
    <skos:definition xml:lang="en">BIBFRAME definition: Entity that assigned the metadata, such as the entity that assigned a classification number, entity that assigned a name, entity that assigned an identifier.</skos:definition>
  </rdf:Description>
  <rdf:Description rdf:nodeID="naa57803e9b8e45bda2faf492b90c6d13b2">
    <rdf:first rdf:resource="http://urn.fi/URN:NBN:fi:schema:bffi:Manifestation"/>
    <rdf:rest rdf:nodeID="naa57803e9b8e45bda2faf492b90c6d13b3"/>
  </rdf:Description>
  <rdf:Description rdf:about="http://urn.fi/URN:NBN:fi:schema:bffi:musicMediumOfRepresentativeExpression">
    <dct:modified>2024-11-22 (New)</dct:modified>
    <rdfs:label xml:lang="en">medium of performance of musical content of representative expression</rdfs:label>
    <rdfs:label xml:lang="fi">edustavan ekspression musiikin esityskokoonpano</rdfs:label>
    <rdfs:domain rdf:resource="http://urn.fi/URN:NBN:fi:schema:bffi:MusicWork"/>
    <rdfs:range rdf:resource="http://urn.fi/URN:NBN:fi:schema:bffi:MusicMedium"/>
    <rdf:type rdf:resource="http://www.w3.org/2002/07/owl#ObjectProperty"/>
    <bffi-meta:exactMatch rdf:resource="http://rdaregistry.info/Elements/w/P10220"/>
    <rdfs:subPropertyOf rdf:resource="http://id.loc.gov/ontologies/bibframe/musicMedium"/>
  </rdf:Description>
  <rdf:Description rdf:about="http://urn.fi/URN:NBN:fi:schema:bffi:soundCharacteristic">
    <dct:modified>2024-11-22 (New)</dct:modified>
    <rdfs:label xml:lang="en">sound characteristic</rdfs:label>
    <rdfs:label xml:lang="fi">äänitallenteen ominaisuudet</rdfs:label>
    <rdfs:domain rdf:resource="http://urn.fi/URN:NBN:fi:schema:bffi:Manifestation"/>
    <rdfs:range rdf:resource="http://urn.fi/URN:NBN:fi:schema:bffi:SoundCharacteristic"/>
    <rdf:type rdf:resource="http://www.w3.org/2002/07/owl#ObjectProperty"/>
    <owl:equivalentProperty rdf:resource="http://id.loc.gov/ontologies/bibframe/soundCharacteristic"/>
    <bffi-meta:exactMatch rdf:resource="http://rdaregistry.info/Elements/m/P30125"/>
    <skos:definition xml:lang="en">BIBFRAME definition: Technical specification relating to the encoding of sound in a resource.</skos:definition>
  </rdf:Description>
  <rdf:Description rdf:nodeID="n0a20977f4ff64f88b13306bf2d732ab6b2">
    <rdf:first rdf:resource="http://urn.fi/URN:NBN:fi:schema:bffi:Expression"/>
    <rdf:rest rdf:nodeID="n0a20977f4ff64f88b13306bf2d732ab6b3"/>
  </rdf:Description>
  <rdf:Description rdf:about="http://urn.fi/URN:NBN:fi:schema:bffi:ClassificationDdc">
    <dct:modified>2024-06-19 (New)</dct:modified>
    <rdfs:label xml:lang="en">DDC classification</rdfs:label>
    <rdfs:label xml:lang="fi">Dewey-luokitus</rdfs:label>
    <rdf:type rdf:resource="http://www.w3.org/2002/07/owl#Class"/>
    <owl:equivalentClass rdf:resource="http://id.loc.gov/ontologies/bibframe/ClassificationDdc"/>
    <rdfs:subClassOf rdf:resource="http://urn.fi/URN:NBN:fi:schema:bffi:Classification"/>
    <skos:definition xml:lang="en">BIBFRAME definition: Dewey Decimal Classification number used for subject access</skos:definition>
  </rdf:Description>
  <rdf:Description rdf:about="http://urn.fi/URN:NBN:fi:schema:bffi:MusicMedium">
    <dct:modified>2024-02-23 (New)</dct:modified>
    <rdfs:label xml:lang="en">Music medium information</rdfs:label>
    <rdfs:label xml:lang="fi">Musiikin esityskokoonpano</rdfs:label>
    <rdf:type rdf:resource="http://www.w3.org/2002/07/owl#Class"/>
    <owl:equivalentClass rdf:resource="http://id.loc.gov/ontologies/bibframe/MusicMedium"/>
    <skos:definition xml:lang="fi">Ekspression musiikillisen sisällön esittämiseen käytetty tai käytettäväksi tarkoitettu soitin, lauluääni tai esittäjäryhmä ja stemmojen, esittäjien ja käsien lukumäärä.</skos:definition>
    <skos:definition xml:lang="en">An instrument, voice, or ensemble and the number of parts, performers and hands used, or intended to be used, to perform the musical content of an expression.</skos:definition>
  </rdf:Description>
  <rdf:Description rdf:about="http://urn.fi/URN:NBN:fi:schema:bffi:Projection">
    <dct:modified>2024-02-23 (New)</dct:modified>
    <rdfs:label xml:lang="en">Projection</rdfs:label>
    <rdfs:label xml:lang="fi">Projektio</rdfs:label>
    <rdf:type rdf:resource="http://www.w3.org/2002/07/owl#Class"/>
    <owl:equivalentClass rdf:resource="http://id.loc.gov/ontologies/bibframe/Projection"/>
    <skos:definition xml:lang="en">BIBFRAME definition: Method or system used to represent the surface of the earth or of a celestial sphere on a plane</skos:definition>
  </rdf:Description>
  <rdf:Description rdf:about="http://urn.fi/URN:NBN:fi:schema:bffi:GrooveCutting">
    <dct:modified>2024-11-22 (New)</dct:modified>
    <rdfs:label xml:lang="en">Groove cutting</rdfs:label>
    <rdfs:label xml:lang="fi">Leikkaustapa</rdfs:label>
    <rdf:type rdf:resource="http://www.w3.org/2002/07/owl#Class"/>
    <owl:equivalentProperty rdf:resource="http://id.loc.gov/ontologies/bflc/GrooveCutting"/>
    <rdfs:seeAlso rdf:resource="http://rdaregistry.info/termList/groovePitch/"/>
    <rdfs:subClassOf rdf:resource="http://urn.fi/URN:NBN:fi:schema:bffi:SoundCharacteristic"/>
    <skos:definition xml:lang="en">BFLC definition: Kind of cutting of the grooves used on a disc whose sound reproduction process involves a cutting head inscribing a modulated groove into the surface of a rotating cylinder or disc.</skos:definition>
  </rdf:Description>
  <rdf:Description rdf:about="http://urn.fi/URN:NBN:fi:schema:bffi:musicThematicNumber">
    <dct:modified>2024-02-23 (New)</dct:modified>
    <rdfs:label xml:lang="en">music thematic number</rdfs:label>
    <rdfs:label xml:lang="fi">temaattisen teosluettelon numero</rdfs:label>
    <rdfs:domain rdf:resource="http://urn.fi/URN:NBN:fi:schema:bffi:Work"/>
    <rdfs:range rdf:resource="http://www.w3.org/2000/01/rdf-schema#Literal"/>
    <rdf:type rdf:resource="http://www.w3.org/2002/07/owl#DatatypeProperty"/>
    <owl:equivalentProperty rdf:resource="http://id.loc.gov/ontologies/bibframe/musicThematicNumber"/>
    <bffi-meta:exactMatch rdf:resource="http://rdaregistry.info/Elements/w/P10335"/>
    <skos:definition xml:lang="en">BIBFRAME definition: Numeric designation for a musical work as found in a thematic index for the composer.</skos:definition>
  </rdf:Description>
  <rdf:Description rdf:about="http://urn.fi/URN:NBN:fi:schema:bffi:fontSize">
    <dct:modified>2024-09-16 (New)</dct:modified>
    <rdfs:label xml:lang="en">font size</rdfs:label>
    <rdfs:label xml:lang="fi">kirjasinkoko</rdfs:label>
    <rdfs:domain rdf:resource="http://urn.fi/URN:NBN:fi:schema:bffi:Manifestation"/>
    <rdfs:range rdf:resource="http://urn.fi/URN:NBN:fi:schema:bffi:FontSize"/>
    <rdf:type rdf:resource="http://www.w3.org/2002/07/owl#ObjectProperty"/>
    <owl:equivalentProperty rdf:resource="http://id.loc.gov/ontologies/bibframe/fontSize"/>
    <bffi-meta:exactMatch rdf:resource="http://rdaregistry.info/Elements/m/P30199"/>
    <skos:definition xml:lang="en">BIBFRAME definition: Size of the type used to represent the characters and symbols in a resource.</skos:definition>
  </rdf:Description>
  <rdf:Description rdf:about="http://urn.fi/URN:NBN:fi:schema:bffi:descriptionLevel">
    <dct:modified>2024-06-19 (New)</dct:modified>
    <rdfs:label xml:lang="en">description level</rdfs:label>
    <rdfs:label xml:lang="fi">kuvailun tietomalli</rdfs:label>
    <rdfs:domain rdf:resource="http://urn.fi/URN:NBN:fi:schema:bffi:AdminMetadata"/>
    <rdfs:range rdf:resource="http://urn.fi/URN:NBN:fi:schema:bffi:DescriptionLevel"/>
    <rdf:type rdf:resource="http://www.w3.org/2002/07/owl#ObjectProperty"/>
    <owl:equivalentProperty rdf:resource="http://id.loc.gov/ontologies/bibframe/descriptionLevel"/>
    <skos:definition xml:lang="en">BIBFRAME definition: Designation of the descriptive content of the metadata</skos:definition>
  </rdf:Description>
  <rdf:Description rdf:about="http://urn.fi/URN:NBN:fi:schema:bffi:ProductionMethod">
    <dct:modified>2024-09-16 (New)</dct:modified>
    <rdfs:label xml:lang="en">Production method</rdfs:label>
    <rdfs:label xml:lang="fi">Valmistusmenetelmä</rdfs:label>
    <bffi-meta:relatedValueVocabulary rdf:resource="http://urn.fi/URN:NBN:fi:au:mts:m417"/>
    <rdf:type rdf:resource="http://www.w3.org/2002/07/owl#Class"/>
    <owl:equivalentClass rdf:resource="http://id.loc.gov/ontologies/bibframe/ProductionMethod"/>
    <rdfs:seeAlso rdf:resource="http://rdaregistry.info/termList/RDAproductionMethod/"/>
    <skos:definition xml:lang="en">BIBFRAME definition: Process used to produce a resource</skos:definition>
  </rdf:Description>
  <rdf:Description rdf:nodeID="n3340e60e05a148bda7f556ae223dde3ab4">
    <rdf:first rdf:resource="http://urn.fi/URN:NBN:fi:schema:bffi:Manifestation"/>
    <rdf:rest rdf:nodeID="n3340e60e05a148bda7f556ae223dde3ab5"/>
  </rdf:Description>
  <rdf:Description rdf:about="http://urn.fi/URN:NBN:fi:schema:bffi:ShelfMark">
    <dct:modified>2025-01-02 (New)</dct:modified>
    <rdfs:label xml:lang="en">Shelf mark</rdfs:label>
    <rdfs:label xml:lang="fi">Hyllypaikka</rdfs:label>
    <rdf:type rdf:resource="http://www.w3.org/2002/07/owl#Class"/>
    <owl:equivalentClass rdf:resource="http://id.loc.gov/ontologies/bibframe/ShelfMark"/>
    <rdfs:subClassOf rdf:resource="http://urn.fi/URN:NBN:fi:schema:bffi:Identifier"/>
    <skos:definition xml:lang="en">BIBFRAME definition: Piece/item identifier, such as a call or other type of number</skos:definition>
  </rdf:Description>
  <rdf:Description rdf:about="http://urn.fi/URN:NBN:fi:schema:bffi:NotatedMovement">
    <dct:modified>2024-02-23 (New)</dct:modified>
    <rdfs:label xml:lang="en">Notated movement</rdfs:label>
    <rdfs:label xml:lang="fi">Liikenotaatio</rdfs:label>
    <rdf:type rdf:resource="http://www.w3.org/2002/07/owl#Class"/>
    <owl:equivalentClass rdf:resource="http://id.loc.gov/ontologies/bibframe/NotatedMovement"/>
    <rdfs:subClassOf rdf:resource="http://urn.fi/URN:NBN:fi:schema:bffi:Expression"/>
    <skos:definition xml:lang="en">BIBFRAME definition: Graphic, non-realized representations of movement intended to be perceived visually, e.g. dance</skos:definition>
  </rdf:Description>
  <rdf:Description rdf:about="http://urn.fi/URN:NBN:fi:schema:bffi:agent">
    <dct:modified>2024-02-23 (New)</dct:modified>
    <rdfs:label xml:lang="en">associated agent</rdfs:label>
    <rdfs:label xml:lang="fi">liittyvä toimija</rdfs:label>
    <rdfs:domain rdf:nodeID="na6088cd10c31435fa00ddf5ff7f94651b1"/>
    <rdfs:range rdf:resource="http://urn.fi/URN:NBN:fi:schema:bffi:Agent"/>
    <rdf:type rdf:resource="http://www.w3.org/2002/07/owl#ObjectProperty"/>
    <bffi-meta:closeMatch rdf:resource="http://rdaregistry.info/Elements/w/P10311"/>
    <rdfs:subPropertyOf rdf:resource="http://id.loc.gov/ontologies/bibframe/agent"/>
  </rdf:Description>
  <rdf:Description rdf:about="http://urn.fi/URN:NBN:fi:schema:bffi:CartographyExpression">
    <dct:modified>2024-02-23 (New)</dct:modified>
    <rdfs:label xml:lang="en">Cartographic expression</rdfs:label>
    <rdfs:label xml:lang="fi">Kartografinen ekspressio</rdfs:label>
    <rdf:type rdf:resource="http://www.w3.org/2002/07/owl#Class"/>
    <bffi-meta:broadMatch rdf:resource="http://id.loc.gov/ontologies/bibframe/Cartography"/>
    <rdfs:subClassOf rdf:resource="http://urn.fi/URN:NBN:fi:schema:bffi:Expression"/>
    <owl:disjointWith rdf:resource="http://urn.fi/URN:NBN:fi:schema:bffi:CartographyWork"/>
  </rdf:Description>
  <rdf:Description rdf:about="http://urn.fi/URN:NBN:fi:schema:bffi:ProjectionSpeed">
    <dct:modified>2024-11-22 (New)</dct:modified>
    <rdfs:label xml:lang="en">Projection speed</rdfs:label>
    <rdfs:label xml:lang="fi">Projisointinopeus</rdfs:label>
    <rdf:type rdf:resource="http://www.w3.org/2002/07/owl#Class"/>
    <owl:equivalentClass rdf:resource="http://id.loc.gov/ontologies/bibframe/ProjectionSpeed"/>
    <rdfs:subClassOf rdf:resource="http://urn.fi/URN:NBN:fi:schema:bffi:ProjectionCharacteristic"/>
    <skos:definition xml:lang="en">BIBFRAME definition: Speed at which a projected carrier must be operated to produce the moving image intended, e.g., 20 fps</skos:definition>
  </rdf:Description>
  <rdf:Description rdf:about="http://urn.fi/URN:NBN:fi:schema:bffi:ReductionRatio">
    <dct:modified>2024-11-22 (New)</dct:modified>
    <rdfs:label xml:lang="en">Reduction ratio</rdfs:label>
    <rdfs:label xml:lang="fi">Pienennyssuhde</rdfs:label>
    <bffi-meta:relatedValueVocabulary rdf:resource="http://urn.fi/URN:NBN:fi:au:mts:m573"/>
    <rdf:type rdf:resource="http://www.w3.org/2002/07/owl#Class"/>
    <owl:equivalentClass rdf:resource="http://id.loc.gov/ontologies/bibframe/ReductionRatio"/>
    <rdfs:seeAlso rdf:resource="http://rdaregistry.info/termList/RDAReductionRatio/"/>
    <skos:definition xml:lang="en">BIBFRAME definition: Size of a micro-image in relation to the original from which it was produced</skos:definition>
  </rdf:Description>
  <rdf:Description rdf:about="http://urn.fi/URN:NBN:fi:schema:bffi:VideoCharacteristic">
    <dct:modified>2024-11-22 (New)</dct:modified>
    <rdfs:label xml:lang="en">Video characteristic</rdfs:label>
    <rdfs:label xml:lang="fi">Videon ominaisuudet</rdfs:label>
    <rdf:type rdf:resource="http://www.w3.org/2002/07/owl#Class"/>
    <owl:equivalentClass rdf:resource="http://id.loc.gov/ontologies/bibframe/VideoCharacteristic"/>
    <skos:definition xml:lang="en">BIBFRAME definition: Technical specification relating to the encoding of video images in a resource</skos:definition>
  </rdf:Description>
  <rdf:Description rdf:about="http://urn.fi/URN:NBN:fi:schema:bffi:readMarc382">
    <dct:modified>2025-01-02 (New)</dct:modified>
    <rdfs:label xml:lang="en">read-only 382 field</rdfs:label>
    <rdfs:label xml:lang="fi">marc382-kentän sisältö</rdfs:label>
    <rdfs:domain rdf:resource="http://urn.fi/URN:NBN:fi:schema:bffi:MusicMedium"/>
    <rdfs:range rdf:resource="http://www.w3.org/2000/01/rdf-schema#Literal"/>
    <rdf:type rdf:resource="http://www.w3.org/2002/07/owl#DatatypeProperty"/>
    <owl:equivalentProperty rdf:resource="http://id.loc.gov/ontologies/bflc/readMarc382"/>
    <skos:definition xml:lang="en">BFLC definition: String representing the medium of performance information located in the 382 field of the original MARC record</skos:definition>
  </rdf:Description>
  <rdf:Description rdf:about="http://urn.fi/URN:NBN:fi:schema:bffi:MachineModel">
    <dct:modified>2024-11-22 (New)</dct:modified>
    <rdfs:label xml:lang="en">Make and model of machine</rdfs:label>
    <rdfs:label xml:lang="fi">Laitteen merkki ja malli</rdfs:label>
    <rdf:type rdf:resource="http://www.w3.org/2002/07/owl#Class"/>
    <owl:equivalentClass rdf:resource="http://id.loc.gov/ontologies/bflc/MachineModel"/>
    <rdfs:subClassOf rdf:resource="http://urn.fi/URN:NBN:fi:schema:bffi:SystemRequirement"/>
    <skos:definition xml:lang="en">BFLC definition: Model of the computing device on which the resource operates.</skos:definition>
  </rdf:Description>
  <rdf:Description rdf:about="http://urn.fi/URN:NBN:fi:schema:bffi:subtitle">
    <dct:modified>2024-02-23 (New)</dct:modified>
    <rdfs:label xml:lang="en">subtitle</rdfs:label>
    <rdfs:label xml:lang="fi">muu nimeketieto</rdfs:label>
    <rdfs:domain rdf:resource="http://urn.fi/URN:NBN:fi:schema:bffi:Title"/>
    <rdfs:range rdf:resource="http://www.w3.org/2000/01/rdf-schema#Literal"/>
    <rdf:type rdf:resource="http://www.w3.org/2002/07/owl#DatatypeProperty"/>
    <owl:equivalentProperty rdf:resource="http://id.loc.gov/ontologies/bibframe/subtitle"/>
    <bffi-meta:closeMatch rdf:resource="http://rdaregistry.info/Elements/m/P30142"/>
    <skos:definition xml:lang="en">BIBFRAME definition: Word, character, or group of words and/or characters that contains the remainder of the title after the main title. Possible title component.</skos:definition>
  </rdf:Description>
  <rdf:Description rdf:about="http://urn.fi/URN:NBN:fi:schema:bffi:MusicAudioExpression">
    <dct:modified>2024-02-23 (New)</dct:modified>
    <rdfs:label xml:lang="en">Music audio expression</rdfs:label>
    <rdfs:label xml:lang="fi">Musiikkiaudioekspressio</rdfs:label>
    <rdf:type rdf:resource="http://www.w3.org/2002/07/owl#Class"/>
    <bffi-meta:broadMatch rdf:resource="http://id.loc.gov/ontologies/bibframe/MusicAudio"/>
    <rdfs:subClassOf rdf:resource="http://urn.fi/URN:NBN:fi:schema:bffi:Expression"/>
  </rdf:Description>
  <rdf:Description rdf:nodeID="n90e14c5f212f40b8a6a776d86788ca21b5">
    <rdf:first rdf:resource="http://urn.fi/URN:NBN:fi:schema:bffi:Item"/>
    <rdf:rest rdf:resource="http://www.w3.org/1999/02/22-rdf-syntax-ns#nil"/>
  </rdf:Description>
  <rdf:Description rdf:nodeID="n68bca78492684c1398be6f6d4f77765db3">
    <rdf:first rdf:resource="http://urn.fi/URN:NBN:fi:schema:bffi:Expression"/>
    <rdf:rest rdf:nodeID="n68bca78492684c1398be6f6d4f77765db4"/>
  </rdf:Description>
  <rdf:Description rdf:about="http://urn.fi/URN:NBN:fi:schema:bffi:firstIssueChronology">
    <dct:modified>2024-02-23 (New)</dct:modified>
    <rdfs:label xml:lang="en">first chronological designation of sequence</rdfs:label>
    <rdfs:label xml:lang="fi">numerointijakson ensimmäinen aikamäärite</rdfs:label>
    <rdfs:domain rdf:resource="http://urn.fi/URN:NBN:fi:schema:bffi:Manifestation"/>
    <rdfs:range rdf:resource="http://www.w3.org/2000/01/rdf-schema#Literal"/>
    <rdf:type rdf:resource="http://www.w3.org/2002/07/owl#DatatypeProperty"/>
    <bffi-meta:broadMatch rdf:resource="http://id.loc.gov/ontologies/bibframe/firstIssue"/>
    <bffi-meta:exactMatch rdf:resource="http://rdaregistry.info/Elements/m/P30149"/>
  </rdf:Description>
  <rdf:Description rdf:about="http://urn.fi/URN:NBN:fi:schema:bffi:sublocation">
    <dct:modified>2024-04-16 (New)</dct:modified>
    <rdfs:label xml:lang="en">held in sublocation</rdfs:label>
    <rdfs:label xml:lang="fi">alayksikkö tai alakokoelma</rdfs:label>
    <rdfs:domain rdf:resource="http://urn.fi/URN:NBN:fi:schema:bffi:Item"/>
    <rdfs:range rdf:resource="http://urn.fi/URN:NBN:fi:schema:bffi:Sublocation"/>
    <rdf:type rdf:resource="http://www.w3.org/2002/07/owl#ObjectProperty"/>
    <owl:equivalentProperty rdf:resource="http://id.loc.gov/ontologies/bibframe/sublocation"/>
    <bffi-meta:broadMatch rdf:resource="http://rdaregistry.info/Elements/i/P40162"/>
    <skos:definition xml:lang="en">BIBFRAME definition: Specific place within the holding entity where the item is located or made available.</skos:definition>
  </rdf:Description>
  <rdf:Description rdf:about="http://urn.fi/URN:NBN:fi:schema:bffi:encodingLevel">
    <dct:modified>2024-11-22 (New)</dct:modified>
    <rdfs:label xml:lang="en">encoding level</rdfs:label>
    <rdfs:label xml:lang="fi">kuvailutaso</rdfs:label>
    <rdfs:domain rdf:resource="http://urn.fi/URN:NBN:fi:schema:bffi:AdminMetadata"/>
    <rdfs:range rdf:resource="http://urn.fi/URN:NBN:fi:schema:bffi:EncodingLevel"/>
    <rdf:type rdf:resource="http://www.w3.org/2002/07/owl#ObjectProperty"/>
    <owl:equivalentProperty rdf:resource="http://id.loc.gov/ontologies/bflc/encodingLevel"/>
    <skos:definition xml:lang="en">BFLC definition: Designation of the fullness of the bibliographic description.</skos:definition>
  </rdf:Description>
  <rdf:Description rdf:about="http://urn.fi/URN:NBN:fi:schema:bffi:SupplementaryContent">
    <dct:modified>2024-11-22 (New)</dct:modified>
    <rdfs:label xml:lang="en">Supplementary material</rdfs:label>
    <rdfs:label xml:lang="fi">Lisätty sisältö</rdfs:label>
    <bffi-meta:relatedValueVocabulary rdf:resource="http://urn.fi/URN:NBN:fi:au:mts:m4849"/>
    <rdf:type rdf:resource="http://www.w3.org/2002/07/owl#Class"/>
    <owl:equivalentClass rdf:resource="http://id.loc.gov/ontologies/bibframe/SupplementaryContent"/>
    <skos:definition xml:lang="en">BIBFRAME definition: Index, bibliography, appendix, etc. intended to supplement the primary content of a resource</skos:definition>
  </rdf:Description>
  <rdf:Description rdf:about="http://urn.fi/URN:NBN:fi:schema:bffi:Archival">
    <dct:modified>2024-09-16 (New)</dct:modified>
    <rdfs:label xml:lang="en">Archival controlled</rdfs:label>
    <rdfs:label xml:lang="fi">Arkistoaineisto</rdfs:label>
    <rdf:type rdf:resource="http://www.w3.org/2002/07/owl#Class"/>
    <owl:equivalentClass rdf:resource="http://id.loc.gov/ontologies/bibframe/Archival"/>
    <rdfs:seeAlso rdf:resource="http://rdaregistry.info/termList/RDATerms/1007"/>
    <rdfs:subClassOf rdf:resource="http://urn.fi/URN:NBN:fi:schema:bffi:Manifestation"/>
    <skos:definition xml:lang="en">BIBFRAME definition: Resources organically created, accumulated, and/or used by a person, family, or organization in the course of conduct of affairs and preserved because of their continuing value</skos:definition>
  </rdf:Description>
  <rdf:Description rdf:about="http://urn.fi/URN:NBN:fi:schema:bffi:SoundCharacteristic">
    <dct:modified>2024-11-22 (New)</dct:modified>
    <rdfs:label xml:lang="en">Sound characteristic</rdfs:label>
    <rdfs:label xml:lang="fi">Äänitallenteen ominaisuudet</rdfs:label>
    <rdf:type rdf:resource="http://www.w3.org/2002/07/owl#Class"/>
    <owl:equivalentClass rdf:resource="http://id.loc.gov/ontologies/bibframe/SoundCharacteristic"/>
    <skos:definition xml:lang="en">BIBFRAME definition: Technical specification relating to the encoding of sound in a resource</skos:definition>
  </rdf:Description>
  <rdf:Description rdf:about="http://urn.fi/URN:NBN:fi:schema:bffi:Uncontrolled">
    <dct:modified>2025-01-02 (New)</dct:modified>
    <rdfs:label xml:lang="en">Uncontrolled</rdfs:label>
    <rdfs:label xml:lang="fi">Auktorisoimaton</rdfs:label>
    <rdf:type rdf:resource="http://www.w3.org/2002/07/owl#Class"/>
    <owl:equivalentClass rdf:resource="http://id.loc.gov/ontologies/bflc/Uncontrolled"/>
    <skos:definition xml:lang="en">BFLC definition: Component of the resource that is not under authority control</skos:definition>
  </rdf:Description>
  <rdf:Description rdf:nodeID="n7333c8087d784d019f2d09a8a88483c5b2">
    <rdf:first rdf:resource="http://urn.fi/URN:NBN:fi:schema:bffi:Work"/>
    <rdf:rest rdf:nodeID="n7333c8087d784d019f2d09a8a88483c5b3"/>
  </rdf:Description>
  <rdf:Description rdf:about="http://urn.fi/URN:NBN:fi:schema:bffi:hierarchicalLevel">
    <dct:modified>2024-04-16 (New)</dct:modified>
    <rdfs:label xml:lang="en">hierarchical level of material</rdfs:label>
    <rdfs:label xml:lang="fi">hierarkkinen taso</rdfs:label>
    <rdfs:domain rdf:resource="http://urn.fi/URN:NBN:fi:schema:bffi:CollectionArrangement"/>
    <rdfs:range rdf:resource="http://www.w3.org/2000/01/rdf-schema#Literal"/>
    <rdf:type rdf:resource="http://www.w3.org/2002/07/owl#DatatypeProperty"/>
    <owl:equivalentProperty rdf:resource="http://id.loc.gov/ontologies/bibframe/hierarchicalLevel"/>
    <skos:definition xml:lang="en">BIBFRAME definition: Hierarchical position of the described materials relative to other material from the same source.</skos:definition>
  </rdf:Description>
  <rdf:Description rdf:about="http://urn.fi/URN:NBN:fi:schema:bffi:EnumerationAndChronology">
    <dct:modified>2024-02-23 (New)</dct:modified>
    <rdfs:label xml:lang="en">Enumeration and chronology</rdfs:label>
    <rdfs:label xml:lang="fi">Numerointi- ja julkaisuaikatiedot</rdfs:label>
    <rdf:type rdf:resource="http://www.w3.org/2002/07/owl#Class"/>
    <owl:equivalentClass rdf:resource="http://id.loc.gov/ontologies/bibframe/EnumerationAndChronology"/>
    <skos:definition xml:lang="en">BIBFRAME definition: Numbering or other enumeration and dates associated with issues or items held</skos:definition>
  </rdf:Description>
  <rdf:Description rdf:about="http://urn.fi/URN:NBN:fi:schema:bffi:musicSerialNumber">
    <dct:modified>2024-02-23 (New)</dct:modified>
    <rdfs:label xml:lang="en">music serial number</rdfs:label>
    <rdfs:label xml:lang="fi">musiikkiteoksen järjestysnumero</rdfs:label>
    <rdfs:domain rdf:resource="http://urn.fi/URN:NBN:fi:schema:bffi:Work"/>
    <rdfs:range rdf:resource="http://www.w3.org/2000/01/rdf-schema#Literal"/>
    <rdf:type rdf:resource="http://www.w3.org/2002/07/owl#DatatypeProperty"/>
    <owl:equivalentProperty rdf:resource="http://id.loc.gov/ontologies/bibframe/musicSerialNumber"/>
    <bffi-meta:exactMatch rdf:resource="http://rdaregistry.info/Elements/w/P10334"/>
    <skos:definition xml:lang="en">BIBFRAME definition: Numeric designation for musical works consecutively numbered in music reference sources.</skos:definition>
  </rdf:Description>
  <rdf:Description rdf:about="http://urn.fi/URN:NBN:fi:schema:bffi:lastIssueEnumeration">
    <dct:modified>2024-02-23 (New)</dct:modified>
    <rdfs:label xml:lang="en">last alphanumeric designation of alternative sequence</rdfs:label>
    <rdfs:label xml:lang="fi">numerointijakson viimeinen numero- ja/tai kirjainmäärite</rdfs:label>
    <rdfs:domain rdf:resource="http://urn.fi/URN:NBN:fi:schema:bffi:Manifestation"/>
    <rdfs:range rdf:resource="http://www.w3.org/2000/01/rdf-schema#Literal"/>
    <rdf:type rdf:resource="http://www.w3.org/2002/07/owl#DatatypeProperty"/>
    <bffi-meta:broadMatch rdf:resource="http://id.loc.gov/ontologies/bibframe/lastIssue"/>
    <bffi-meta:exactMatch rdf:resource="http://rdaregistry.info/Elements/m/P30148"/>
  </rdf:Description>
  <rdf:Description rdf:about="http://urn.fi/URN:NBN:fi:schema:bffi:BibframeWork">
    <dct:modified>2024-02-23 (New)</dct:modified>
    <rdfs:label xml:lang="en">BIBFRAME Work</rdfs:label>
    <rdfs:label xml:lang="fi">BIBFRAME-teos</rdfs:label>
    <rdf:type rdf:resource="http://www.w3.org/2002/07/owl#Class"/>
    <owl:equivalentClass rdf:resource="http://id.loc.gov/ontologies/bibframe/Work"/>
    <bffi-meta:narrowMatch rdf:resource="http://rdaregistry.info/Elements/c/C10001"/>
    <bffi-meta:narrowMatch rdf:resource="http://rdaregistry.info/Elements/c/C10006"/>
    <skos:definition xml:lang="en">BIBFRAME definition: Resource reflecting a conceptual essence of a cataloging resource</skos:definition>
  </rdf:Description>
  <rdf:Description rdf:about="http://urn.fi/URN:NBN:fi:schema:bffi:horizontalScale">
    <dct:modified>2024-02-23 (New)</dct:modified>
    <rdfs:label xml:lang="en">horizontal scale of cartographic content</rdfs:label>
    <rdfs:label xml:lang="fi">horisontaalinen mittakaava</rdfs:label>
    <rdfs:domain rdf:resource="http://urn.fi/URN:NBN:fi:schema:bffi:CartographyExpression"/>
    <rdfs:range rdf:resource="http://urn.fi/URN:NBN:fi:schema:bffi:Scale"/>
    <rdf:type rdf:resource="http://www.w3.org/2002/07/owl#ObjectProperty"/>
    <bffi-meta:broadMatch rdf:resource="http://id.loc.gov/ontologies/bibframe/scale"/>
    <bffi-meta:exactMatch rdf:resource="http://rdaregistry.info/Elements/e/P20226"/>
    <rdfs:subPropertyOf rdf:resource="http://urn.fi/URN:NBN:fi:schema:bffi:scale"/>
  </rdf:Description>
  <rdf:Description rdf:about="http://urn.fi/URN:NBN:fi:schema:bffi:copyrightDate">
    <dct:modified>2024-02-23 (New)</dct:modified>
    <rdfs:label xml:lang="en">copyright date</rdfs:label>
    <rdfs:label xml:lang="fi">copyright-vuosi</rdfs:label>
    <rdfs:domain rdf:resource="http://urn.fi/URN:NBN:fi:schema:bffi:Manifestation"/>
    <rdfs:range rdf:resource="http://www.w3.org/2000/01/rdf-schema#Literal"/>
    <rdf:type rdf:resource="http://www.w3.org/2002/07/owl#DatatypeProperty"/>
    <owl:equivalentProperty rdf:resource="http://id.loc.gov/ontologies/bibframe/copyrightDate"/>
    <bffi-meta:exactMatch rdf:resource="http://rdaregistry.info/Elements/m/P30007"/>
    <rdfs:subPropertyOf rdf:resource="http://urn.fi/URN:NBN:fi:schema:bffi:date"/>
    <skos:definition xml:lang="en">BIBFRAME definition: Date associated with a claim of protection under copyright or a similar regime.</skos:definition>
  </rdf:Description>
  <rdf:Description rdf:about="http://urn.fi/URN:NBN:fi:schema:bffi:SerialPubType">
    <dct:modified>2024-11-22 (New)</dct:modified>
    <rdfs:label xml:lang="en">Serial Publication Type</rdfs:label>
    <rdfs:label xml:lang="fi">Jatkuvan julkaisun tyyppi</rdfs:label>
    <rdf:type rdf:resource="http://www.w3.org/2002/07/owl#Class"/>
    <owl:equivalentClass rdf:resource="http://id.loc.gov/ontologies/bflc/SerialPubType"/>
    <skos:definition xml:lang="en">BFLC definition: Information recording the type of continuing resource.</skos:definition>
  </rdf:Description>
  <rdf:Description rdf:about="http://urn.fi/URN:NBN:fi:schema:bffi:aap">
    <dct:modified>2024-02-23 (New)</dct:modified>
    <rdfs:label xml:lang="en">authorized access point</rdfs:label>
    <rdfs:label xml:lang="fi">auktorisoitu hakutieto</rdfs:label>
    <rdfs:domain rdf:nodeID="n90e14c5f212f40b8a6a776d86788ca21b1"/>
    <rdfs:range rdf:resource="http://www.w3.org/2000/01/rdf-schema#Literal"/>
    <rdf:type rdf:resource="http://www.w3.org/2002/07/owl#DatatypeProperty"/>
    <owl:equivalentProperty rdf:resource="http://id.loc.gov/ontologies/bflc/aap"/>
    <bffi-meta:narrowMatch rdf:resource="http://rdaregistry.info/Elements/w/P10331"/>
    <bffi-meta:narrowMatch rdf:resource="http://rdaregistry.info/Elements/e/P20313"/>
    <bffi-meta:narrowMatch rdf:resource="http://rdaregistry.info/Elements/m/P30294"/>
    <bffi-meta:narrowMatch rdf:resource="http://rdaregistry.info/Elements/i/P40083"/>
    <skos:definition xml:lang="en">BFLC definition: A text string that represents the label of the resource. It could be a name/title combination, but could also include additional fields to make it unique within the catalog.</skos:definition>
  </rdf:Description>
  <rdf:Description rdf:about="http://urn.fi/URN:NBN:fi:schema:bffi-meta:narrowMatch">
    <rdfs:label xml:lang="en">narrow match</rdfs:label>
    <rdfs:label xml:lang="fi">suppeampi vastaavuus</rdfs:label>
    <skos:definition xml:lang="en">Semantically narrower class or property in another ontology or scheme.</skos:definition>
    <skos:definition xml:lang="fi">Merkitykseltään vastaava suppeampi luokka tai ominaisuus jossakin toisessa ontologiassa tai skeemassa.</skos:definition>
    <rdf:type rdf:resource="http://www.w3.org/2002/07/owl#AnnotationProperty"/>
    <dct:modified>2024-02-23 (New)</dct:modified>
    <rdfs:subPropertyOf rdf:resource="http://purl.org/dc/terms/relation"/>
  </rdf:Description>
  <rdf:Description rdf:nodeID="na62f4311181e4083bd9b0ad0c31f158ab2">
    <rdf:first rdf:resource="http://urn.fi/URN:NBN:fi:schema:bffi:StillImage"/>
    <rdf:rest rdf:nodeID="na62f4311181e4083bd9b0ad0c31f158ab3"/>
  </rdf:Description>
  <rdf:Description rdf:about="http://urn.fi/URN:NBN:fi:schema:bffi:Language">
    <dct:modified>2024-02-23 (New)</dct:modified>
    <rdfs:label xml:lang="en">Language entity</rdfs:label>
    <rdfs:label xml:lang="fi">Kieli</rdfs:label>
    <rdf:type rdf:resource="http://www.w3.org/2002/07/owl#Class"/>
    <owl:equivalentClass rdf:resource="http://id.loc.gov/ontologies/bibframe/Language"/>
    <skos:definition xml:lang="en">BIBFRAME definition: Language entity</skos:definition>
  </rdf:Description>
  <rdf:Description rdf:about="http://urn.fi/URN:NBN:fi:schema:bffi:ColorContent">
    <dct:modified>2024-04-16 (New)</dct:modified>
    <rdfs:label xml:lang="en">Color content</rdfs:label>
    <rdfs:label xml:lang="fi">Värisisältö</rdfs:label>
    <bffi-meta:relatedValueVocabulary rdf:resource="http://urn.fi/URN:NBN:fi:au:mts:m1668"/>
    <rdf:type rdf:resource="http://www.w3.org/2002/07/owl#Class"/>
    <owl:equivalentClass rdf:resource="http://id.loc.gov/ontologies/bibframe/ColorContent"/>
    <rdfs:seeAlso rdf:resource="http://rdaregistry.info/termList/RDAColourContent/"/>
    <skos:definition xml:lang="en">BIBFRAME definition: Color characteristics of a resource, e.g., black and white, multicolored, etc.</skos:definition>
  </rdf:Description>
  <rdf:Description rdf:about="http://urn.fi/URN:NBN:fi:schema:bffi:shelfMark">
    <dct:modified>2025-01-02 (New)</dct:modified>
    <rdfs:label xml:lang="en">shelf mark</rdfs:label>
    <rdfs:label xml:lang="fi">hyllypaikka</rdfs:label>
    <rdfs:domain rdf:resource="http://urn.fi/URN:NBN:fi:schema:bffi:Item"/>
    <rdfs:range rdf:resource="http://urn.fi/URN:NBN:fi:schema:bffi:ShelfMark"/>
    <rdf:type rdf:resource="http://www.w3.org/2002/07/owl#ObjectProperty"/>
    <owl:equivalentProperty rdf:resource="http://id.loc.gov/ontologies/bibframe/shelfMark"/>
    <skos:definition xml:lang="en">BIBFRAME definition: Piece identifier, such as a call or other type of number.</skos:definition>
  </rdf:Description>
  <rdf:Description rdf:about="http://urn.fi/URN:NBN:fi:schema:bffi:CollectionManifestation">
    <dct:modified>2024-04-16 (New)</dct:modified>
    <rdfs:label xml:lang="en">Collection instance</rdfs:label>
    <rdfs:label xml:lang="fi">Kokoelmamanifestaatio</rdfs:label>
    <rdf:type rdf:resource="http://www.w3.org/2002/07/owl#Class"/>
    <bffi-meta:broadMatch rdf:resource="http://id.loc.gov/ontologies/bibframe/Instance"/>
    <rdfs:subClassOf rdf:resource="http://urn.fi/URN:NBN:fi:schema:bffi:Manifestation"/>
  </rdf:Description>
  <rdf:Description rdf:nodeID="n0d5ef643a16a443a8864901b85eb32dbb2">
    <rdf:first rdf:resource="http://urn.fi/URN:NBN:fi:schema:bffi:Work"/>
    <rdf:rest rdf:nodeID="n0d5ef643a16a443a8864901b85eb32dbb3"/>
  </rdf:Description>
  <rdf:Description rdf:nodeID="n14ff77a0080346dbb0cd2218439611d1b1">
    <rdf:type rdf:resource="http://www.w3.org/2002/07/owl#Class"/>
    <owl:unionOf rdf:nodeID="n14ff77a0080346dbb0cd2218439611d1b2"/>
  </rdf:Description>
  <rdf:Description rdf:about="http://urn.fi/URN:NBN:fi:schema:bffi:holdingOf">
    <dct:modified>2024-04-16 (New)</dct:modified>
    <rdfs:label xml:lang="en">holding of</rdfs:label>
    <rdfs:label xml:lang="fi">kappale kokoelmassa</rdfs:label>
    <rdfs:domain rdf:resource="http://urn.fi/URN:NBN:fi:schema:bffi:Item"/>
    <rdfs:range rdf:resource="http://urn.fi/URN:NBN:fi:schema:bffi:CollectionManifestation"/>
    <rdf:type rdf:resource="http://www.w3.org/2002/07/owl#ObjectProperty"/>
    <bffi-meta:broadMatch rdf:resource="http://id.loc.gov/ontologies/bibframe/itemOf"/>
    <bffi-meta:exactMatch rdf:resource="http://rdaregistry.info/Elements/i/P40161"/>
    <rdfs:subPropertyOf rdf:resource="http://urn.fi/URN:NBN:fi:schema:bffi:relatedTo"/>
  </rdf:Description>
  <rdf:Description rdf:about="http://urn.fi/URN:NBN:fi:schema:bffi:ascensionAndDeclination">
    <dct:modified>2024-04-16 (New)</dct:modified>
    <rdfs:label xml:lang="en">cartographic ascension and declination</rdfs:label>
    <rdfs:label xml:lang="fi">rektaskensio ja deklinaatio</rdfs:label>
    <rdfs:domain rdf:resource="http://urn.fi/URN:NBN:fi:schema:bffi:Cartographic"/>
    <rdfs:range rdf:resource="http://www.w3.org/2000/01/rdf-schema#Literal"/>
    <rdf:type rdf:resource="http://www.w3.org/2002/07/owl#DatatypeProperty"/>
    <owl:equivalentProperty rdf:resource="http://id.loc.gov/ontologies/bibframe/ascensionAndDeclination"/>
    <bffi-meta:exactMatch rdf:resource="http://rdaregistry.info/Elements/w/P10082"/>
    <skos:definition xml:lang="en">BIBFRAME definition: System for identifying the location of a celestial object in the sky covered by the cartographic content of a resource using the angles of right ascension and declination.</skos:definition>
  </rdf:Description>
  <rdf:Description rdf:about="http://urn.fi/URN:NBN:fi:schema:bffi:CollectionArrangement">
    <dct:modified>2024-04-16 (New)</dct:modified>
    <rdfs:label xml:lang="en">Organization of materials information</rdfs:label>
    <rdfs:label xml:lang="fi">Järjestämisperiaate</rdfs:label>
    <rdf:type rdf:resource="http://www.w3.org/2002/07/owl#Class"/>
    <owl:equivalentClass rdf:resource="http://id.loc.gov/ontologies/bibframe/CollectionArrangement"/>
    <skos:definition xml:lang="en">BIBFRAME definition: Information about the organization and arrangement of a collection of items</skos:definition>
  </rdf:Description>
  <rdf:Description rdf:about="http://urn.fi/URN:NBN:fi:schema:bffi:intendedAudienceOfRepresentativeExpression">
    <dct:modified>2024-04-16 (New)</dct:modified>
    <rdfs:label xml:lang="en">intended audience of representative expression</rdfs:label>
    <rdfs:label xml:lang="fi">edustavan ekspression kohderyhmä</rdfs:label>
    <rdfs:domain rdf:resource="http://urn.fi/URN:NBN:fi:schema:bffi:Work"/>
    <rdfs:range rdf:resource="http://urn.fi/URN:NBN:fi:schema:bffi:IntendedAudience"/>
    <rdf:type rdf:resource="http://www.w3.org/2002/07/owl#ObjectProperty"/>
    <bffi-meta:closeMatch rdf:resource="http://id.loc.gov/ontologies/bibframe/intendedAudience"/>
    <bffi-meta:exactMatch rdf:resource="http://rdaregistry.info/Elements/w/P10217"/>
  </rdf:Description>
  <rdf:Description rdf:about="http://urn.fi/URN:NBN:fi:schema:bffi:workManifested">
    <owl:inverseOf rdf:resource="http://urn.fi/URN:NBN:fi:schema:bffi:manifestationOfWork"/>
    <dct:modified>2024-02-23 (New)</dct:modified>
    <rdfs:label xml:lang="en">work manifested</rdfs:label>
    <rdfs:label xml:lang="fi">manifestaatioon sisältyvä teos</rdfs:label>
    <rdfs:domain rdf:resource="http://urn.fi/URN:NBN:fi:schema:bffi:Manifestation"/>
    <rdfs:range rdf:resource="http://urn.fi/URN:NBN:fi:schema:bffi:Work"/>
    <rdf:type rdf:resource="http://www.w3.org/2002/07/owl#ObjectProperty"/>
    <bffi-meta:broadMatch rdf:resource="http://id.loc.gov/ontologies/bibframe/instanceOf"/>
    <bffi-meta:exactMatch rdf:resource="http://rdaregistry.info/Elements/m/P30135"/>
    <rdfs:subPropertyOf rdf:resource="http://urn.fi/URN:NBN:fi:schema:bffi:relatedTo"/>
  </rdf:Description>
  <rdf:Description rdf:about="http://urn.fi/URN:NBN:fi:schema:bffi:ProvisionActivity">
    <dct:modified>2024-02-23 (New)</dct:modified>
    <rdfs:label xml:lang="en">Provider entity</rdfs:label>
    <rdfs:label xml:lang="fi">Tuottamistiedot</rdfs:label>
    <rdf:type rdf:resource="http://www.w3.org/2002/07/owl#Class"/>
    <owl:equivalentClass rdf:resource="http://id.loc.gov/ontologies/bibframe/ProvisionActivity"/>
    <skos:definition xml:lang="en">BIBFRAME definition: Information about the agent or place relating to the publication, printing, distribution, issue, release, or production of a resource</skos:definition>
  </rdf:Description>
  <rdf:Description rdf:about="http://urn.fi/URN:NBN:fi:schema:bffi:scale">
    <dct:modified>2024-02-23 (New)</dct:modified>
    <rdfs:label xml:lang="en">scale</rdfs:label>
    <rdfs:label xml:lang="fi">mittakaava</rdfs:label>
    <rdfs:domain rdf:resource="http://urn.fi/URN:NBN:fi:schema:bffi:Expression"/>
    <rdfs:range rdf:resource="http://urn.fi/URN:NBN:fi:schema:bffi:Scale"/>
    <rdf:type rdf:resource="http://www.w3.org/2002/07/owl#ObjectProperty"/>
    <owl:equivalentProperty rdf:resource="http://id.loc.gov/ontologies/bibframe/scale"/>
    <bffi-meta:exactMatch rdf:resource="http://rdaregistry.info/Elements/e/P20228"/>
    <skos:scopeNote xml:lang="fi">Käytä stillkuvan tai kolmiulotteisen objektin skaalalle ominaisuutta bffi:scaleOfStilllimageOrThreeDimensionalForm.</skos:scopeNote>
    <skos:scopeNote xml:lang="en">Use bffi:scaleOfStillImageOrThreeDimensionalForm property for still image or three-dimensional object.</skos:scopeNote>
    <skos:definition xml:lang="en">BIBFRAME definition: Ratio of the dimensions of a form contained or embodied in a resource to the dimensions of the entity it represents, e.g., for images or cartographic resources.</skos:definition>
  </rdf:Description>
  <rdf:Description rdf:about="http://urn.fi/URN:NBN:fi:schema:bffi:Meeting">
    <dct:modified>2024-02-23 (New)</dct:modified>
    <rdfs:label xml:lang="en">Meeting</rdfs:label>
    <rdfs:label xml:lang="fi">Kokous</rdfs:label>
    <rdf:type rdf:resource="http://www.w3.org/2002/07/owl#Class"/>
    <owl:equivalentClass rdf:resource="http://id.loc.gov/ontologies/bibframe/Meeting"/>
    <bffi-meta:broadMatch rdf:resource="http://rdaregistry.info/Elements/c/C10005"/>
    <rdfs:subClassOf rdf:resource="http://urn.fi/URN:NBN:fi:schema:bffi:Agent"/>
    <skos:definition xml:lang="en">BIBFRAME definition: Gathering of individuals or representatives of various bodies for the purpose of discussing and/or acting on topics of common interest</skos:definition>
  </rdf:Description>
  <rdf:Description rdf:about="http://urn.fi/URN:NBN:fi:schema:bffi:Jurisdiction">
    <dct:modified>2025-01-02 (New)</dct:modified>
    <rdfs:label xml:lang="en">Jurisdiction</rdfs:label>
    <rdfs:label xml:lang="fi">Hallintoalue</rdfs:label>
    <rdf:type rdf:resource="http://www.w3.org/2002/07/owl#Class"/>
    <owl:equivalentClass rdf:resource="http://id.loc.gov/ontologies/bibframe/Jurisdiction"/>
    <rdfs:subClassOf rdf:resource="http://urn.fi/URN:NBN:fi:schema:bffi:Agent"/>
    <skos:definition xml:lang="en">BIBFRAME definition: Legal or political unit administering a geographic area</skos:definition>
  </rdf:Description>
  <rdf:Description rdf:about="http://urn.fi/URN:NBN:fi:schema:bffi:DemographicGroup">
    <dct:modified>2025-01-02 (New)</dct:modified>
    <rdfs:label xml:lang="en">Demographic group</rdfs:label>
    <rdfs:label xml:lang="fi">Väestöryhmä</rdfs:label>
    <rdf:type rdf:resource="http://www.w3.org/2002/07/owl#Class"/>
    <owl:equivalentClass rdf:resource="http://id.loc.gov/ontologies/bflc/DemographicGroup"/>
    <skos:definition xml:lang="en">BFLC definition: Characteristics of a group of agents.</skos:definition>
  </rdf:Description>
  <rdf:Description rdf:about="http://urn.fi/URN:NBN:fi:schema:bffi:outerGRing">
    <dct:modified>2024-04-16 (New)</dct:modified>
    <rdfs:label xml:lang="en">cartographic outer G ring area covered</rdfs:label>
    <rdfs:label xml:lang="fi">ulompi G-kehä</rdfs:label>
    <rdfs:domain rdf:resource="http://urn.fi/URN:NBN:fi:schema:bffi:Cartographic"/>
    <rdfs:range rdf:resource="http://www.w3.org/2000/01/rdf-schema#Literal"/>
    <rdf:type rdf:resource="http://www.w3.org/2002/07/owl#DatatypeProperty"/>
    <owl:equivalentProperty rdf:resource="http://id.loc.gov/ontologies/bibframe/outerGRing"/>
    <bffi-meta:closeMatch rdf:resource="http://rdaregistry.info/Elements/w/P10083"/>
    <skos:definition xml:lang="en">BIBFRAME definition: Coordinate pairs that identify the closed non-intersecting boundary of the area covered.</skos:definition>
  </rdf:Description>
  <rdf:Description rdf:about="http://urn.fi/URN:NBN:fi:schema:bffi:videoCharacteristic">
    <dct:modified>2024-11-22 (New)</dct:modified>
    <rdfs:label xml:lang="en">video characteristic</rdfs:label>
    <rdfs:label xml:lang="fi">videon ominaisuudet</rdfs:label>
    <rdfs:domain rdf:resource="http://urn.fi/URN:NBN:fi:schema:bffi:Manifestation"/>
    <rdfs:range rdf:resource="http://urn.fi/URN:NBN:fi:schema:bffi:VideoCharacteristic"/>
    <rdf:type rdf:resource="http://www.w3.org/2002/07/owl#ObjectProperty"/>
    <owl:equivalentProperty rdf:resource="http://id.loc.gov/ontologies/bibframe/videoCharacteristic"/>
    <skos:definition xml:lang="en">BIBFRAME definition: Technical specification relating to the encoding of video images in a resource</skos:definition>
  </rdf:Description>
  <rdf:Description rdf:about="http://urn.fi/URN:NBN:fi:schema:bffi:temporalCoverage">
    <dct:modified>2024-02-23 (New)</dct:modified>
    <rdfs:label xml:lang="en">temporal coverage</rdfs:label>
    <rdfs:label xml:lang="fi">ajanjakso</rdfs:label>
    <rdfs:domain rdf:resource="http://urn.fi/URN:NBN:fi:schema:bffi:Work"/>
    <rdfs:range rdf:resource="http://www.w3.org/2000/01/rdf-schema#Literal"/>
    <rdf:type rdf:resource="http://www.w3.org/2002/07/owl#DatatypeProperty"/>
    <owl:equivalentProperty rdf:resource="http://id.loc.gov/ontologies/bibframe/temporalCoverage"/>
    <bffi-meta:exactMatch rdf:resource="http://rdaregistry.info/Elements/w/P10322"/>
    <skos:definition xml:lang="en">BIBFRAME definition: Time period coverage of the content of the resource.</skos:definition>
  </rdf:Description>
  <rdf:Description rdf:about="http://urn.fi/URN:NBN:fi:schema:bffi:ProjectionCharacteristic">
    <dct:modified>2024-11-22 (New)</dct:modified>
    <rdfs:label xml:lang="en">Projection characteristic</rdfs:label>
    <rdfs:label xml:lang="fi">Elokuvafilmin projisointiominaisuudet</rdfs:label>
    <rdf:type rdf:resource="http://www.w3.org/2002/07/owl#Class"/>
    <owl:equivalentClass rdf:resource="http://id.loc.gov/ontologies/bibframe/ProjectionCharacteristic"/>
    <rdfs:seeAlso rdf:resource="http://rdaregistry.info/termList/presFormat"/>
    <skos:definition xml:lang="en">BIBFRAME definition: Technical specification relating to the projection of a motion picture film</skos:definition>
  </rdf:Description>
  <rdf:Description rdf:about="http://urn.fi/URN:NBN:fi:schema:bffi:Status">
    <dct:modified>2024-02-23 (New)</dct:modified>
    <rdfs:label xml:lang="en">Status</rdfs:label>
    <rdfs:label xml:lang="fi">Status</rdfs:label>
    <rdf:type rdf:resource="http://www.w3.org/2002/07/owl#Class"/>
    <owl:equivalentClass rdf:resource="http://id.loc.gov/ontologies/bibframe/Status"/>
    <skos:definition xml:lang="en">BIBFRAME definition: Designation of the validity or position of something, e.g., whether something is incorrect or available</skos:definition>
  </rdf:Description>
  <rdf:Description rdf:about="http://urn.fi/URN:NBN:fi:schema:bffi:variantAccessPoint">
    <dct:modified>2024-02-23 (New)</dct:modified>
    <rdfs:label xml:lang="en">variant access point</rdfs:label>
    <rdfs:label xml:lang="fi">varianttihakutieto</rdfs:label>
    <rdfs:domain rdf:nodeID="n02875ff463bf42a79835462fc328eac6b1"/>
    <rdfs:range rdf:resource="http://www.w3.org/2000/01/rdf-schema#Literal"/>
    <rdf:type rdf:resource="http://www.w3.org/2002/07/owl#DatatypeProperty"/>
    <bffi-meta:narrowMatch rdf:resource="http://rdaregistry.info/Elements/w/P10332"/>
    <bffi-meta:narrowMatch rdf:resource="http://rdaregistry.info/Elements/e/P20314"/>
    <bffi-meta:narrowMatch rdf:resource="http://rdaregistry.info/Elements/m/P30295"/>
    <bffi-meta:narrowMatch rdf:resource="http://rdaregistry.info/Elements/i/P40084"/>
    <bffi-meta:narrowMatch rdf:resource="http://rdaregistry.info/Elements/p/P70046"/>
    <bffi-meta:narrowMatch rdf:resource="http://rdaregistry.info/Elements/t/P70048"/>
  </rdf:Description>
  <rdf:Description rdf:about="http://urn.fi/URN:NBN:fi:schema:bffi:Publication">
    <dct:modified>2024-02-23 (New)</dct:modified>
    <rdfs:label xml:lang="en">Publisher</rdfs:label>
    <rdfs:label xml:lang="fi">Kustantaja</rdfs:label>
    <rdf:type rdf:resource="http://www.w3.org/2002/07/owl#Class"/>
    <owl:equivalentClass rdf:resource="http://id.loc.gov/ontologies/bibframe/Publication"/>
    <rdfs:subClassOf rdf:resource="http://urn.fi/URN:NBN:fi:schema:bffi:ProvisionActivity"/>
    <skos:definition xml:lang="en">BIBFRAME definition: Information relating to publication of a resource</skos:definition>
  </rdf:Description>
  <rdf:Description rdf:about="http://urn.fi/URN:NBN:fi:schema:bffi:DescriptionConventions">
    <dct:modified>2024-06-19 (New)</dct:modified>
    <rdfs:label xml:lang="en">Description conventions</rdfs:label>
    <rdfs:label xml:lang="fi">Kuvailusäännöt</rdfs:label>
    <rdf:type rdf:resource="http://www.w3.org/2002/07/owl#Class"/>
    <owl:equivalentClass rdf:resource="http://id.loc.gov/ontologies/bibframe/DescriptionConventions"/>
    <skos:definition xml:lang="en">BIBFRAME definition: Rules used for the descriptive content of the resource description</skos:definition>
  </rdf:Description>
  <rdf:Description rdf:about="http://urn.fi/URN:NBN:fi:schema:bffi:Electronic">
    <dct:modified>2024-09-16 (New)</dct:modified>
    <rdfs:label xml:lang="en">Electronic</rdfs:label>
    <rdfs:label xml:lang="fi">Elektroninen</rdfs:label>
    <rdf:type rdf:resource="http://www.w3.org/2002/07/owl#Class"/>
    <owl:equivalentClass rdf:resource="http://id.loc.gov/ontologies/bibframe/Electronic"/>
    <rdfs:subClassOf rdf:resource="http://urn.fi/URN:NBN:fi:schema:bffi:Manifestation"/>
    <skos:definition xml:lang="en">BIBFRAME definition: Resource that is intended for manipulation by a computer, accessed either directly or remotely</skos:definition>
  </rdf:Description>
  <rdf:Description rdf:about="http://urn.fi/URN:NBN:fi:schema:bffi:Emulsion">
    <dct:modified>2024-09-16 (New)</dct:modified>
    <rdfs:label xml:lang="en">Emulsion</rdfs:label>
    <rdfs:label xml:lang="fi">Mikrofilmin ja mikrokortin emulsio</rdfs:label>
    <rdf:type rdf:resource="http://www.w3.org/2002/07/owl#Class"/>
    <owl:equivalentClass rdf:resource="http://id.loc.gov/ontologies/bibframe/Emulsion"/>
    <skos:definition xml:lang="en">BIBFRAME definition: Suspension of light-sensitive chemicals used as a coating on a microfilm or microfiche, e.g., silver halide</skos:definition>
  </rdf:Description>
  <rdf:Description rdf:nodeID="n42dc8c45022c4e7c8886fe842cc1e72fb1">
    <rdf:type rdf:resource="http://www.w3.org/2002/07/owl#Class"/>
    <owl:unionOf rdf:nodeID="n42dc8c45022c4e7c8886fe842cc1e72fb2"/>
  </rdf:Description>
  <rdf:Description rdf:about="http://urn.fi/URN:NBN:fi:schema:bffi:Contribution">
    <dct:modified>2024-02-23 (New)</dct:modified>
    <rdfs:label xml:lang="en">Contribution</rdfs:label>
    <rdfs:label xml:lang="fi">Kontribuutio</rdfs:label>
    <rdf:type rdf:resource="http://www.w3.org/2002/07/owl#Class"/>
    <owl:equivalentClass rdf:resource="http://id.loc.gov/ontologies/bibframe/Contribution"/>
    <skos:definition xml:lang="en">BIBFRAME definition: Agent and role with respect to the resource being described</skos:definition>
  </rdf:Description>
  <rdf:Description rdf:about="http://urn.fi/URN:NBN:fi:schema:bffi:tableOfContents">
    <dct:modified>2024-11-22 (New)</dct:modified>
    <rdfs:label xml:lang="en">table of contents content</rdfs:label>
    <rdfs:label xml:lang="fi">sisältöhuomautus</rdfs:label>
    <rdfs:domain rdf:resource="http://urn.fi/URN:NBN:fi:schema:bffi:Manifestation"/>
    <rdfs:range rdf:resource="http://urn.fi/URN:NBN:fi:schema:bffi:TableOfContents"/>
    <rdf:type rdf:resource="http://www.w3.org/2002/07/owl#ObjectProperty"/>
    <owl:equivalentProperty rdf:resource="http://id.loc.gov/ontologies/bibframe/tableOfContents"/>
    <skos:definition xml:lang="en">BIBFRAME definition: Table of contents of the described resource.</skos:definition>
  </rdf:Description>
  <rdf:Description rdf:nodeID="n3fb00cccae3f45e2923b7c06d0716eb2b2">
    <rdf:first rdf:resource="http://urn.fi/URN:NBN:fi:schema:bffi:MonographWork"/>
    <rdf:rest rdf:nodeID="n3fb00cccae3f45e2923b7c06d0716eb2b3"/>
  </rdf:Description>
  <rdf:Description rdf:about="http://urn.fi/URN:NBN:fi:schema:bffi:collectionAccrualPolicy">
    <dct:modified>2024-04-16 (New)</dct:modified>
    <rdfs:label xml:lang="en">collection accrual policy</rdfs:label>
    <rdfs:label xml:lang="fi">kokoelman kartuttamisen linja</rdfs:label>
    <rdfs:domain rdf:resource="http://urn.fi/URN:NBN:fi:schema:bffi:CollectionWork"/>
    <rdfs:range rdf:resource="http://urn.fi/URN:NBN:fi:schema:bffi:CollectionAccrualPolicy"/>
    <rdf:type rdf:resource="http://www.w3.org/2002/07/owl#ObjectProperty"/>
    <bffi-meta:broadMatch rdf:resource="http://id.loc.gov/ontologies/bibframe/usageAndAccessPolicy"/>
    <bffi-meta:exactMatch rdf:resource="http://rdaregistry.info/Elements/w/P10609"/>
  </rdf:Description>
  <rdf:Description rdf:nodeID="n5cd48ce8767a480c888bcf43bfaa8780b2">
    <rdf:first rdf:resource="http://urn.fi/URN:NBN:fi:schema:bffi:Work"/>
    <rdf:rest rdf:nodeID="n5cd48ce8767a480c888bcf43bfaa8780b3"/>
  </rdf:Description>
  <rdf:Description rdf:about="http://urn.fi/URN:NBN:fi:schema:bffi:tableSeq">
    <dct:modified>2024-06-19 (New)</dct:modified>
    <rdfs:label xml:lang="en">classification table sequence number</rdfs:label>
    <rdfs:label xml:lang="fi">luokkataulun järjestysnumero</rdfs:label>
    <rdfs:domain rdf:resource="http://urn.fi/URN:NBN:fi:schema:bffi:Classification"/>
    <rdfs:range rdf:resource="http://www.w3.org/2000/01/rdf-schema#Literal"/>
    <rdf:type rdf:resource="http://www.w3.org/2002/07/owl#DatatypeProperty"/>
    <owl:equivalentProperty rdf:resource="http://id.loc.gov/ontologies/bibframe/tableSeq"/>
    <skos:definition xml:lang="en">BIBFRAME definition: Sequence number or other identifier for an internal classification sub arrangement or add in a classification scheme.</skos:definition>
  </rdf:Description>
  <rdf:Description rdf:about="http://urn.fi/URN:NBN:fi:schema:bffi:acquisitionTerms">
    <dct:modified>2024-04-16 (New)</dct:modified>
    <rdfs:label xml:lang="en">terms of acquisition</rdfs:label>
    <rdfs:label xml:lang="fi">hankintatieto</rdfs:label>
    <rdfs:domain rdf:resource="http://urn.fi/URN:NBN:fi:schema:bffi:Manifestation"/>
    <rdfs:range rdf:resource="http://www.w3.org/2000/01/rdf-schema#Literal"/>
    <rdf:type rdf:resource="http://www.w3.org/2002/07/owl#DatatypeProperty"/>
    <owl:equivalentProperty rdf:resource="http://id.loc.gov/ontologies/bibframe/acquisitionTerms"/>
    <bffi-meta:closeMatch rdf:resource="http://rdaregistry.info/Elements/m/P30160"/>
    <skos:definition xml:lang="en">BIBFRAME definition: Conditions under which the publisher, distributor, etc., will normally supply a resource, e.g., price of a resource.</skos:definition>
  </rdf:Description>
  <rdf:Description rdf:about="http://urn.fi/URN:NBN:fi:schema:bffi:Event">
    <dct:modified>2024-02-23 (New)</dct:modified>
    <rdfs:label xml:lang="en">Event entity</rdfs:label>
    <rdfs:label xml:lang="fi">Tapahtuma</rdfs:label>
    <rdf:type rdf:resource="http://www.w3.org/2002/07/owl#Class"/>
    <owl:equivalentClass rdf:resource="http://id.loc.gov/ontologies/bibframe/Event"/>
    <skos:definition xml:lang="en">BIBFRAME definition: Something that happens at a certain time and location, such as a performance, speech, or athletic event</skos:definition>
  </rdf:Description>
  <rdf:Description rdf:about="http://urn.fi/URN:NBN:fi:schema:bffi:IntendedAudience">
    <dct:modified>2024-02-23 (New)</dct:modified>
    <rdfs:label xml:lang="en">Intended audience information</rdfs:label>
    <rdfs:label xml:lang="fi">Kohderyhmä</rdfs:label>
    <rdf:type rdf:resource="http://www.w3.org/2002/07/owl#Class"/>
    <owl:equivalentClass rdf:resource="http://id.loc.gov/ontologies/bibframe/IntendedAudience"/>
    <skos:definition xml:lang="en">BIBFRAME definition: Information that identifies the specific intended or target audience or intellectual level for which the content described is considered appropriate; also used to record interest and motivation levels and special learner characteristics</skos:definition>
  </rdf:Description>
  <rdf:Description rdf:about="http://urn.fi/URN:NBN:fi:schema:bffi:Scale">
    <dct:modified>2024-02-23 (New)</dct:modified>
    <rdfs:label xml:lang="en">Scale</rdfs:label>
    <rdfs:label xml:lang="fi">Mittakaava</rdfs:label>
    <rdf:type rdf:resource="http://www.w3.org/2002/07/owl#Class"/>
    <owl:equivalentClass rdf:resource="http://id.loc.gov/ontologies/bibframe/Scale"/>
    <skos:definition xml:lang="en">BIBFRAME definition: Ratio of the dimensions of a form contained or embodied in a resource to the dimensions of the entity it represents, e.g., for images or cartographic resources</skos:definition>
  </rdf:Description>
  <rdf:Description rdf:nodeID="n14ff77a0080346dbb0cd2218439611d1b4">
    <rdf:first rdf:resource="http://urn.fi/URN:NBN:fi:schema:bffi:Manifestation"/>
    <rdf:rest rdf:nodeID="n14ff77a0080346dbb0cd2218439611d1b5"/>
  </rdf:Description>
  <rdf:Description rdf:about="http://urn.fi/URN:NBN:fi:schema:bffi:CaptureStorage">
    <dct:modified>2024-11-22 (New)</dct:modified>
    <rdfs:label xml:lang="en">Capture and Storage Technique</rdfs:label>
    <rdfs:label xml:lang="fi">Taltiointi- ja tallennustekniikka</rdfs:label>
    <bffi-meta:relatedValueVocabulary rdf:resource="http://urn.fi/URN:NBN:fi:au:mts:m4955"/>
    <rdf:type rdf:resource="http://www.w3.org/2002/07/owl#Class"/>
    <owl:equivalentClass rdf:resource="http://id.loc.gov/ontologies/bibframe/CaptureStorage"/>
    <rdfs:subClassOf rdf:resource="http://urn.fi/URN:NBN:fi:schema:bffi:SoundCharacteristic"/>
    <skos:definition xml:lang="en">BIBFRAME definition: Specifies the sound capture and storage technique used on a sound recording resource</skos:definition>
  </rdf:Description>
  <rdf:Description rdf:about="http://urn.fi/URN:NBN:fi:schema:bffi:BroadcastStandard">
    <dct:modified>2024-11-22 (New)</dct:modified>
    <rdfs:label xml:lang="en">Broadcast standard</rdfs:label>
    <rdfs:label xml:lang="fi">Lähetysstandardi</rdfs:label>
    <bffi-meta:relatedValueVocabulary rdf:resource="http://urn.fi/URN:NBN:fi:au:mts:m682"/>
    <rdf:type rdf:resource="http://www.w3.org/2002/07/owl#Class"/>
    <owl:equivalentClass rdf:resource="http://id.loc.gov/ontologies/bibframe/BroadcastStandard"/>
    <rdfs:seeAlso rdf:resource="http://rdaregistry.info/termList/broadcastStand/"/>
    <rdfs:subClassOf rdf:resource="http://urn.fi/URN:NBN:fi:schema:bffi:VideoCharacteristic"/>
    <skos:definition xml:lang="en">BIBFRAME definition: System used to format a video resource for television broadcast, e.g., HDTV, PAL</skos:definition>
  </rdf:Description>
  <rdf:Description rdf:about="http://urn.fi/URN:NBN:fi:schema:bffi:Print">
    <dct:modified>2024-09-16 (New)</dct:modified>
    <rdfs:label xml:lang="en">Printed</rdfs:label>
    <rdfs:label xml:lang="fi">Painettu</rdfs:label>
    <rdf:type rdf:resource="http://www.w3.org/2002/07/owl#Class"/>
    <owl:equivalentClass rdf:resource="http://id.loc.gov/ontologies/bibframe/Print"/>
    <rdfs:subClassOf rdf:resource="http://urn.fi/URN:NBN:fi:schema:bffi:Manifestation"/>
    <skos:definition xml:lang="en">BIBFRAME definition: Resource that is printed</skos:definition>
  </rdf:Description>
  <rdf:Description rdf:about="http://urn.fi/URN:NBN:fi:schema:bffi:Relief">
    <dct:modified>2024-04-16 (New)</dct:modified>
    <rdfs:label xml:lang="en">Relief</rdfs:label>
    <rdfs:label xml:lang="fi">Korkeuserojen esitystapa</rdfs:label>
    <rdf:type rdf:resource="http://www.w3.org/2002/07/owl#Class"/>
    <owl:equivalentClass rdf:resource="http://id.loc.gov/ontologies/bibframe/Relief"/>
    <skos:definition xml:lang="en">BIBFRAME definition: Relief term specified on a cartographic resource</skos:definition>
  </rdf:Description>
  <rdf:Description rdf:about="http://urn.fi/URN:NBN:fi:schema:bffi:creditsProduction">
    <dct:modified>2024-06-19 (New)</dct:modified>
    <rdfs:label xml:lang="en">creation or production credits</rdfs:label>
    <rdfs:label xml:lang="fi">huomautus tuotantoon osallistujista</rdfs:label>
    <rdfs:domain rdf:resource="http://urn.fi/URN:NBN:fi:schema:bffi:Manifestation"/>
    <rdfs:range rdf:resource="http://www.w3.org/2000/01/rdf-schema#Literal"/>
    <rdf:type rdf:resource="http://www.w3.org/2002/07/owl#DatatypeProperty"/>
    <bffi-meta:broadMatch rdf:resource="http://id.loc.gov/ontologies/bibframe/credits"/>
    <bffi-meta:broadMatch rdf:resource="http://rdaregistry.info/Elements/m/P30057"/>
    <rdfs:subPropertyOf rdf:resource="http://urn.fi/URN:NBN:fi:schema:bffi:credits"/>
  </rdf:Description>
  <rdf:Description rdf:about="http://urn.fi/URN:NBN:fi:schema:bffi:CollectionItem">
    <dct:modified>2024-04-16 (New)</dct:modified>
    <rdfs:label xml:lang="en">Collection item</rdfs:label>
    <rdfs:label xml:lang="fi">Kokoelmakappale</rdfs:label>
    <rdf:type rdf:resource="http://www.w3.org/2002/07/owl#Class"/>
    <bffi-meta:broadMatch rdf:resource="http://id.loc.gov/ontologies/bibframe/Item"/>
    <rdfs:subClassOf rdf:resource="http://urn.fi/URN:NBN:fi:schema:bffi:Item"/>
  </rdf:Description>
  <rdf:Description rdf:about="http://urn.fi/URN:NBN:fi:schema:bffi:responsibilityStatement">
    <dct:modified>2024-02-23 (New)</dct:modified>
    <rdfs:label xml:lang="en">creative responsibility statement</rdfs:label>
    <rdfs:label xml:lang="fi">vastuullisuusmerkintö</rdfs:label>
    <rdfs:domain rdf:resource="http://urn.fi/URN:NBN:fi:schema:bffi:Manifestation"/>
    <rdfs:range rdf:resource="http://www.w3.org/2000/01/rdf-schema#Literal"/>
    <rdf:type rdf:resource="http://www.w3.org/2002/07/owl#DatatypeProperty"/>
    <owl:equivalentProperty rdf:resource="http://id.loc.gov/ontologies/bibframe/responsibilityStatement"/>
    <bffi-meta:exactMatch rdf:resource="http://rdaregistry.info/Elements/m/P30105"/>
    <skos:definition xml:lang="en">BIBFRAME definition: Statement relating to any persons, families, or corporate bodies responsible for the creation of, or contributing to the content of a resource; usually transcribed.</skos:definition>
  </rdf:Description>
  <rdf:Description rdf:about="http://urn.fi/URN:NBN:fi:schema:bffi:Notation">
    <dct:modified>2024-02-23 (New)</dct:modified>
    <rdfs:label xml:lang="en">Notation</rdfs:label>
    <rdfs:label xml:lang="fi">Notaatio</rdfs:label>
    <rdf:type rdf:resource="http://www.w3.org/2002/07/owl#Class"/>
    <owl:equivalentClass rdf:resource="http://id.loc.gov/ontologies/bibframe/Notation"/>
    <skos:definition xml:lang="en">BIBFRAME definition: Information on the alphabet, script, or symbol system used to convey the content of the resource, including specialized scripts, typefaces, tactile notation, movement notation, and musical notation</skos:definition>
  </rdf:Description>
  <rdf:Description rdf:about="http://urn.fi/URN:NBN:fi:schema:bffi:AppliedMaterial">
    <dct:modified>2024-09-16 (New)</dct:modified>
    <rdfs:label xml:lang="en">Applied material</rdfs:label>
    <rdfs:label xml:lang="fi">Päällimateriaali</rdfs:label>
    <bffi-meta:relatedValueVocabulary rdf:resource="http://urn.fi/URN:NBN:fi:au:mts:m654"/>
    <rdf:type rdf:resource="http://www.w3.org/2002/07/owl#Class"/>
    <owl:equivalentClass rdf:resource="http://id.loc.gov/ontologies/bibframe/AppliedMaterial"/>
    <rdfs:seeAlso rdf:resource="http://rdaregistry.info/termList/RDAMaterial/"/>
    <rdfs:subClassOf rdf:resource="http://urn.fi/URN:NBN:fi:schema:bffi:Material"/>
    <skos:definition xml:lang="en">BIBFRAME definition: Physical or chemical substance applied to a base material of a resource</skos:definition>
  </rdf:Description>
  <rdf:Description rdf:nodeID="ne27b8fc3c7014a3a99b60051d23322e1b5">
    <rdf:first rdf:resource="http://urn.fi/URN:NBN:fi:schema:bffi:Item"/>
    <rdf:rest rdf:resource="http://www.w3.org/1999/02/22-rdf-syntax-ns#nil"/>
  </rdf:Description>
  <rdf:Description rdf:about="http://urn.fi/URN:NBN:fi:schema:bffi:Item">
    <dct:modified>2024-02-23 (New)</dct:modified>
    <rdfs:label xml:lang="en">Item</rdfs:label>
    <rdfs:label xml:lang="fi">Kappale</rdfs:label>
    <rdf:type rdf:resource="http://www.w3.org/2002/07/owl#Class"/>
    <owl:equivalentClass rdf:resource="http://id.loc.gov/ontologies/bibframe/Item"/>
    <bffi-meta:exactMatch rdf:resource="http://rdaregistry.info/Elements/c/C10003"/>
    <skos:definition xml:lang="en">BIBFRAME definition: Single example of an Instance</skos:definition>
  </rdf:Description>
  <rdf:Description rdf:about="http://urn.fi/URN:NBN:fi:schema:bffi-meta:broadMatch">
    <dct:modified>2024-02-23 (New)</dct:modified>
    <rdf:type rdf:resource="http://www.w3.org/2002/07/owl#AnnotationProperty"/>
    <rdfs:subPropertyOf rdf:resource="http://purl.org/dc/terms/relation"/>
    <rdfs:label xml:lang="en">broad match</rdfs:label>
    <rdfs:label xml:lang="fi">laajempi vastaavuus</rdfs:label>
    <skos:definition xml:lang="en">Semantically broader class or property in another ontology or scheme.</skos:definition>
    <skos:definition xml:lang="fi">Merkitykseltään vastaava laajempi luokka tai ominaisuus jossakin toisessa ontologiassa tai skeemassa.</skos:definition>
  </rdf:Description>
  <rdf:Description rdf:about="http://urn.fi/URN:NBN:fi:schema:bffi:Identifier">
    <dct:modified>2024-02-23 (New)</dct:modified>
    <rdfs:label xml:lang="en">Identifier</rdfs:label>
    <rdfs:label xml:lang="fi">Tunniste</rdfs:label>
    <rdf:type rdf:resource="http://www.w3.org/2002/07/owl#Class"/>
    <owl:equivalentClass rdf:resource="http://id.loc.gov/ontologies/bibframe/Identifier"/>
    <bffi-meta:broadMatch rdf:resource="http://rdaregistry.info/Elements/c/C10012"/>
    <skos:definition xml:lang="en">BIBFRAME definition: Token or name that is associated with a resource, such as a URI or an ISBN</skos:definition>
  </rdf:Description>
  <rdf:Description rdf:about="http://urn.fi/URN:NBN:fi:schema:bffi:CopyrightRegistration">
    <dct:modified>2024-02-23 (New)</dct:modified>
    <rdfs:label xml:lang="en">Copyright registration</rdfs:label>
    <rdfs:label xml:lang="fi">Tekijänoikeus- tai vapaakappaletiedot</rdfs:label>
    <rdf:type rdf:resource="http://www.w3.org/2002/07/owl#Class"/>
    <owl:equivalentClass rdf:resource="http://id.loc.gov/ontologies/bibframe/CopyrightRegistration"/>
    <skos:definition xml:lang="en">BIBFRAME definition: Copyright or Legal Deposit registration information</skos:definition>
  </rdf:Description>
  <rdf:Description rdf:nodeID="naa57803e9b8e45bda2faf492b90c6d13b1">
    <rdf:type rdf:resource="http://www.w3.org/2002/07/owl#Class"/>
    <owl:unionOf rdf:nodeID="naa57803e9b8e45bda2faf492b90c6d13b2"/>
  </rdf:Description>
  <rdf:Description rdf:about="http://urn.fi/URN:NBN:fi:schema:bffi:CartographyWork">
    <owl:disjointWith rdf:resource="http://urn.fi/URN:NBN:fi:schema:bffi:CartographyExpression"/>
    <dct:modified>2024-02-23 (New)</dct:modified>
    <rdfs:label xml:lang="en">Cartographic work</rdfs:label>
    <rdfs:label xml:lang="fi">Kartografinen teos</rdfs:label>
    <rdf:type rdf:resource="http://www.w3.org/2002/07/owl#Class"/>
    <bffi-meta:broadMatch rdf:resource="http://id.loc.gov/ontologies/bibframe/Cartography"/>
    <rdfs:subClassOf rdf:resource="http://urn.fi/URN:NBN:fi:schema:bffi:Work"/>
  </rdf:Description>
  <rdf:Description rdf:nodeID="n7333c8087d784d019f2d09a8a88483c5b3">
    <rdf:first rdf:resource="http://urn.fi/URN:NBN:fi:schema:bffi:Expression"/>
    <rdf:rest rdf:nodeID="n7333c8087d784d019f2d09a8a88483c5b4"/>
  </rdf:Description>
  <rdf:Description rdf:about="http://urn.fi/URN:NBN:fi:schema:bffi:ClassificationNlm">
    <dct:modified>2024-06-19 (New)</dct:modified>
    <rdfs:label xml:lang="en">NLM classification</rdfs:label>
    <rdfs:label xml:lang="fi">National Library of Medicine -luokitus</rdfs:label>
    <rdf:type rdf:resource="http://www.w3.org/2002/07/owl#Class"/>
    <owl:equivalentClass rdf:resource="http://id.loc.gov/ontologies/bibframe/ClassificationNlm"/>
    <rdfs:subClassOf rdf:resource="http://urn.fi/URN:NBN:fi:schema:bffi:Classification"/>
    <skos:definition xml:lang="en">BIBFRAME definition: National Library of Medicine Classification number used for subject access</skos:definition>
  </rdf:Description>
  <rdf:Description rdf:nodeID="n7b5ca739c46d4a329e0fe2325c944dbcb4">
    <rdf:first rdf:resource="http://urn.fi/URN:NBN:fi:schema:bffi:MovingImageWork"/>
    <rdf:rest rdf:resource="http://www.w3.org/1999/02/22-rdf-syntax-ns#nil"/>
  </rdf:Description>
  <rdf:Description rdf:nodeID="n02875ff463bf42a79835462fc328eac6b1">
    <rdf:type rdf:resource="http://www.w3.org/2002/07/owl#Class"/>
    <owl:unionOf rdf:nodeID="n02875ff463bf42a79835462fc328eac6b2"/>
  </rdf:Description>
  <rdf:Description rdf:about="http://urn.fi/URN:NBN:fi:schema:bffi:Content">
    <dct:modified>2024-02-23 (New)</dct:modified>
    <rdfs:label xml:lang="en">Content type</rdfs:label>
    <rdfs:label xml:lang="fi">Sisältötyyppi</rdfs:label>
    <rdf:type rdf:resource="http://www.w3.org/2002/07/owl#Class"/>
    <owl:equivalentClass rdf:resource="http://id.loc.gov/ontologies/bibframe/Content"/>
    <skos:definition xml:lang="en">BIBFRAME definition: Categorization reflecting the fundamental form of communication in which the content is expressed and the human sense through which it is intended to be perceived</skos:definition>
  </rdf:Description>
  <rdf:Description rdf:nodeID="ne27b8fc3c7014a3a99b60051d23322e1b4">
    <rdf:first rdf:resource="http://urn.fi/URN:NBN:fi:schema:bffi:Manifestation"/>
    <rdf:rest rdf:nodeID="ne27b8fc3c7014a3a99b60051d23322e1b5"/>
  </rdf:Description>
  <rdf:Description rdf:nodeID="n68bca78492684c1398be6f6d4f77765db4">
    <rdf:first rdf:resource="http://urn.fi/URN:NBN:fi:schema:bffi:Manifestation"/>
    <rdf:rest rdf:nodeID="n68bca78492684c1398be6f6d4f77765db5"/>
  </rdf:Description>
  <rdf:Description rdf:nodeID="n90e14c5f212f40b8a6a776d86788ca21b1">
    <rdf:type rdf:resource="http://www.w3.org/2002/07/owl#Class"/>
    <owl:unionOf rdf:nodeID="n90e14c5f212f40b8a6a776d86788ca21b2"/>
  </rdf:Description>
  <rdf:Description rdf:about="http://urn.fi/URN:NBN:fi:schema:bffi:Expression">
    <dct:modified>2024-02-23 (New)</dct:modified>
    <rdfs:label xml:lang="en">Expression</rdfs:label>
    <rdfs:label xml:lang="fi">Ekspressio</rdfs:label>
    <rdf:type rdf:resource="http://www.w3.org/2002/07/owl#Class"/>
    <bffi-meta:broadMatch rdf:resource="http://id.loc.gov/ontologies/bibframe/Work"/>
    <bffi-meta:exactMatch rdf:resource="http://rdaregistry.info/Elements/c/C10006"/>
    <rdfs:subClassOf rdf:resource="http://urn.fi/URN:NBN:fi:schema:bffi:BibframeWork"/>
    <owl:disjointWith rdf:resource="http://urn.fi/URN:NBN:fi:schema:bffi:Work"/>
  </rdf:Description>
  <rdf:Description rdf:about="http://urn.fi/URN:NBN:fi:schema:bffi:Family">
    <dct:modified>2024-02-23 (New)</dct:modified>
    <rdfs:label xml:lang="en">Family</rdfs:label>
    <rdfs:label xml:lang="fi">Suku</rdfs:label>
    <rdf:type rdf:resource="http://www.w3.org/2002/07/owl#Class"/>
    <owl:equivalentClass rdf:resource="http://id.loc.gov/ontologies/bibframe/Family"/>
    <bffi-meta:exactMatch rdf:resource="http://rdaregistry.info/Elements/c/C10008"/>
    <rdfs:subClassOf rdf:resource="http://urn.fi/URN:NBN:fi:schema:bffi:Agent"/>
    <skos:definition xml:lang="en">BIBFRAME definition: Two or more persons related by birth, marriage, adoption, civil union, or similar legal status, or who otherwise present themselves as a family</skos:definition>
  </rdf:Description>
  <rdf:Description rdf:nodeID="na6088cd10c31435fa00ddf5ff7f94651b2">
    <rdf:first rdf:resource="http://urn.fi/URN:NBN:fi:schema:bffi:Contribution"/>
    <rdf:rest rdf:nodeID="na6088cd10c31435fa00ddf5ff7f94651b3"/>
  </rdf:Description>
  <rdf:Description rdf:nodeID="n2ee3b3232b574a15b2a1faf6555dee4fb3">
    <rdf:first rdf:resource="http://urn.fi/URN:NBN:fi:schema:bffi:NonMusicAudioWork"/>
    <rdf:rest rdf:nodeID="n2ee3b3232b574a15b2a1faf6555dee4fb4"/>
  </rdf:Description>
  <rdf:Description rdf:about="http://urn.fi/URN:NBN:fi:schema:bffi:CollectionAccrualPolicy">
    <dct:modified>2024-04-16 (New)</dct:modified>
    <rdfs:label xml:lang="en">Collection accrual policy</rdfs:label>
    <rdfs:label xml:lang="fi">Kokoelman kartuttamisen linja</rdfs:label>
    <bffi-meta:relatedValueVocabulary rdf:resource="http://urn.fi/URN:NBN:fi:au:mts:m5108"/>
    <rdf:type rdf:resource="http://www.w3.org/2002/07/owl#Class"/>
    <bffi-meta:broadMatch rdf:resource="http://id.loc.gov/ontologies/bibframe/UsageAndAccessPolicy"/>
    <rdfs:seeAlso rdf:resource="http://rdaregistry.info/termList/RDACollectionAccrualPolicy"/>
  </rdf:Description>
  <rdf:Description rdf:about="http://urn.fi/URN:NBN:fi:schema:bffi:RegionalEncoding">
    <dct:modified>2024-11-22 (New)</dct:modified>
    <rdfs:label xml:lang="en">Regional encoding</rdfs:label>
    <rdfs:label xml:lang="fi">Aluekoodi</rdfs:label>
    <bffi-meta:relatedValueVocabulary rdf:resource="http://urn.fi/URN:NBN:fi:au:mts:m4400"/>
    <rdf:type rdf:resource="http://www.w3.org/2002/07/owl#Class"/>
    <owl:equivalentClass rdf:resource="http://id.loc.gov/ontologies/bibframe/RegionalEncoding"/>
    <rdfs:seeAlso rdf:resource="http://rdaregistry.info/termList/RDARegionalEncoding/"/>
    <rdfs:subClassOf rdf:resource="http://urn.fi/URN:NBN:fi:schema:bffi:DigitalCharacteristic"/>
    <skos:definition xml:lang="en">BIBFRAME definition: Identification of the region of the world for which a videodisc has been encoded, e.g., region 4</skos:definition>
  </rdf:Description>
  <rdf:Description rdf:nodeID="n3db75dd6e811409899be21399dda0ca7b1">
    <rdf:type rdf:resource="http://www.w3.org/2002/07/owl#Class"/>
    <owl:unionOf rdf:nodeID="n3db75dd6e811409899be21399dda0ca7b2"/>
  </rdf:Description>
  <rdf:Description rdf:about="http://urn.fi/URN:NBN:fi:schema:bffi:seriesStatement">
    <dct:modified>2024-02-23 (New)</dct:modified>
    <rdfs:label xml:lang="en">series statement</rdfs:label>
    <rdfs:label xml:lang="fi">sarjamerkintö</rdfs:label>
    <rdfs:domain rdf:resource="http://urn.fi/URN:NBN:fi:schema:bffi:Manifestation"/>
    <rdfs:range rdf:resource="http://www.w3.org/2000/01/rdf-schema#Literal"/>
    <rdf:type rdf:resource="http://www.w3.org/2002/07/owl#DatatypeProperty"/>
    <owl:equivalentProperty rdf:resource="http://id.loc.gov/ontologies/bibframe/seriesStatement"/>
    <bffi-meta:exactMatch rdf:resource="http://rdaregistry.info/Elements/m/P30106"/>
    <skos:definition xml:lang="en">BIBFRAME definition: Statement of the series the resource is in; usually transcribed; includes the ISSN if applicable.</skos:definition>
  </rdf:Description>
  <rdf:Description rdf:nodeID="n096c0702f8c64e3bbe53573a59499c9ab4">
    <rdf:first rdf:resource="http://urn.fi/URN:NBN:fi:schema:bffi:MovingImageExpression"/>
    <rdf:rest rdf:resource="http://www.w3.org/1999/02/22-rdf-syntax-ns#nil"/>
  </rdf:Description>
  <rdf:Description rdf:nodeID="n9f671517b9dd4b7c955826691e2215f4b2">
    <rdf:first rdf:resource="http://urn.fi/URN:NBN:fi:schema:bffi:Work"/>
    <rdf:rest rdf:nodeID="n9f671517b9dd4b7c955826691e2215f4b3"/>
  </rdf:Description>
  <rdf:Description rdf:about="http://urn.fi/URN:NBN:fi:schema:bffi:PresentationFormat">
    <dct:modified>2024-11-22 (New)</dct:modified>
    <rdfs:label xml:lang="en">Presentation format</rdfs:label>
    <rdfs:label xml:lang="fi">Esitysformaatti</rdfs:label>
    <bffi-meta:relatedValueVocabulary rdf:resource="http://urn.fi/URN:NBN:fi:au:mts:m169"/>
    <rdf:type rdf:resource="http://www.w3.org/2002/07/owl#Class"/>
    <owl:equivalentClass rdf:resource="http://id.loc.gov/ontologies/bibframe/PresentationFormat"/>
    <rdfs:seeAlso rdf:resource="http://rdaregistry.info/termList/presFormat/"/>
    <rdfs:subClassOf rdf:resource="http://urn.fi/URN:NBN:fi:schema:bffi:ProjectionCharacteristic"/>
    <skos:definition xml:lang="en">BIBFRAME definition: Format used in the production of a projected image, e.g., Cinerama, IMAX</skos:definition>
  </rdf:Description>
  <rdf:Description rdf:nodeID="n02875ff463bf42a79835462fc328eac6b4">
    <rdf:first rdf:resource="http://urn.fi/URN:NBN:fi:schema:bffi:Manifestation"/>
    <rdf:rest rdf:nodeID="n02875ff463bf42a79835462fc328eac6b5"/>
  </rdf:Description>
  <rdf:Description rdf:about="http://urn.fi/URN:NBN:fi:schema:bffi:language">
    <dct:modified>2024-02-23 (New)</dct:modified>
    <rdfs:label xml:lang="en">language information</rdfs:label>
    <rdfs:label xml:lang="fi">kieli</rdfs:label>
    <rdfs:domain rdf:resource="http://www.w3.org/2000/01/rdf-schema#Resource"/>
    <rdfs:range rdf:resource="http://www.w3.org/2000/01/rdf-schema#Resource"/>
    <rdf:type rdf:resource="http://www.w3.org/2002/07/owl#ObjectProperty"/>
    <owl:equivalentProperty rdf:resource="http://id.loc.gov/ontologies/bibframe/language"/>
    <bffi-meta:closeMatch rdf:resource="http://rdaregistry.info/Elements/u/P60099"/>
    <skos:definition xml:lang="en">BIBFRAME definition: Language associated with a resource or its parts.</skos:definition>
  </rdf:Description>
  <rdf:Description rdf:nodeID="n1e5b766c1bf94ff9812af7b852f48486b2">
    <rdf:first rdf:resource="http://urn.fi/URN:NBN:fi:schema:bffi:Work"/>
    <rdf:rest rdf:nodeID="n1e5b766c1bf94ff9812af7b852f48486b3"/>
  </rdf:Description>
  <rdf:Description rdf:nodeID="n30938fe99dde46599fe6796e2af454deb2">
    <rdf:first rdf:resource="http://urn.fi/URN:NBN:fi:schema:bffi:Work"/>
    <rdf:rest rdf:nodeID="n30938fe99dde46599fe6796e2af454deb3"/>
  </rdf:Description>
  <rdf:Description rdf:nodeID="n71c313d9323b40c29dadafedf28680eeb4">
    <rdf:first rdf:resource="http://urn.fi/URN:NBN:fi:schema:bffi:Manifestation"/>
    <rdf:rest rdf:nodeID="n71c313d9323b40c29dadafedf28680eeb5"/>
  </rdf:Description>
  <rdf:Description rdf:nodeID="n68bca78492684c1398be6f6d4f77765db5">
    <rdf:first rdf:resource="http://urn.fi/URN:NBN:fi:schema:bffi:Item"/>
    <rdf:rest rdf:resource="http://www.w3.org/1999/02/22-rdf-syntax-ns#nil"/>
  </rdf:Description>
  <rdf:Description rdf:nodeID="n26a54bed81f14ec98f0dfd0d8091fc72b1">
    <rdf:type rdf:resource="http://www.w3.org/2002/07/owl#Class"/>
    <owl:unionOf rdf:nodeID="n26a54bed81f14ec98f0dfd0d8091fc72b2"/>
  </rdf:Description>
  <rdf:Description rdf:nodeID="nd5a8377479bd46e890352259af2eb06cb4">
    <rdf:first rdf:resource="http://urn.fi/URN:NBN:fi:schema:bffi:MovingImageExpression"/>
    <rdf:rest rdf:resource="http://www.w3.org/1999/02/22-rdf-syntax-ns#nil"/>
  </rdf:Description>
  <rdf:Description rdf:about="http://urn.fi/URN:NBN:fi:schema:bffi:Carrier">
    <dct:modified>2024-02-23 (New)</dct:modified>
    <rdfs:label xml:lang="en">Carrier type</rdfs:label>
    <rdfs:label xml:lang="fi">Tallennetyyppi</rdfs:label>
    <bffi-meta:relatedValueVocabulary rdf:resource="http://urn.fi/URN:NBN:fi:au:mts:m180"/>
    <rdf:type rdf:resource="http://www.w3.org/2002/07/owl#Class"/>
    <owl:equivalentClass rdf:resource="http://id.loc.gov/ontologies/bibframe/Carrier"/>
    <rdfs:seeAlso rdf:resource="http://rdaregistry.info/termList/RDACarrierType/"/>
    <skos:definition xml:lang="en">BIBFRAME definition: Categorization reflecting the format of the storage medium and housing of a carrier</skos:definition>
  </rdf:Description>
  <rdf:Description rdf:nodeID="n7b5ca739c46d4a329e0fe2325c944dbcb2">
    <rdf:first rdf:resource="http://urn.fi/URN:NBN:fi:schema:bffi:MusicWork"/>
    <rdf:rest rdf:nodeID="n7b5ca739c46d4a329e0fe2325c944dbcb3"/>
  </rdf:Description>
  <rdf:Description rdf:nodeID="n26a54bed81f14ec98f0dfd0d8091fc72b3">
    <rdf:first rdf:resource="http://urn.fi/URN:NBN:fi:schema:bffi:Expression"/>
    <rdf:rest rdf:nodeID="n26a54bed81f14ec98f0dfd0d8091fc72b4"/>
  </rdf:Description>
  <rdf:Description rdf:nodeID="na62f4311181e4083bd9b0ad0c31f158ab1">
    <rdf:type rdf:resource="http://www.w3.org/2002/07/owl#Class"/>
    <owl:unionOf rdf:nodeID="na62f4311181e4083bd9b0ad0c31f158ab2"/>
  </rdf:Description>
  <rdf:Description rdf:about="http://urn.fi/URN:NBN:fi:schema:bffi:supplementaryContent">
    <dct:modified>2024-11-22 (New)</dct:modified>
    <rdfs:label xml:lang="en">supplementary material</rdfs:label>
    <rdfs:label xml:lang="fi">lisätty sisältö</rdfs:label>
    <rdfs:domain rdf:resource="http://urn.fi/URN:NBN:fi:schema:bffi:Manifestation"/>
    <rdfs:range rdf:resource="http://urn.fi/URN:NBN:fi:schema:bffi:SupplementaryContent"/>
    <rdf:type rdf:resource="http://www.w3.org/2002/07/owl#ObjectProperty"/>
    <owl:equivalentProperty rdf:resource="http://id.loc.gov/ontologies/bibframe/supplementaryContent"/>
    <bffi-meta:exactMatch rdf:resource="http://rdaregistry.info/Elements/m/P30455"/>
    <skos:definition xml:lang="en">BIBFRAME definition: Material such as an index, bibliography, appendix intended to supplement the primary content of a resource.</skos:definition>
  </rdf:Description>
  <rdf:Description rdf:nodeID="n2ee3b3232b574a15b2a1faf6555dee4fb1">
    <rdf:type rdf:resource="http://www.w3.org/2002/07/owl#Class"/>
    <owl:unionOf rdf:nodeID="n2ee3b3232b574a15b2a1faf6555dee4fb2"/>
  </rdf:Description>
  <rdf:Description rdf:about="http://urn.fi/URN:NBN:fi:schema:bffi:TitleNote">
    <dct:modified>2024-02-23 (New)</dct:modified>
    <rdfs:label xml:lang="en">Title note</rdfs:label>
    <rdfs:label xml:lang="fi">Huomautus nimekkeestä</rdfs:label>
    <rdf:type rdf:resource="http://www.w3.org/2002/07/owl#Class"/>
    <bffi-meta:broadMatch rdf:resource="http://id.loc.gov/ontologies/bibframe/Note"/>
    <rdfs:subClassOf rdf:resource="http://urn.fi/URN:NBN:fi:schema:bffi:Note"/>
  </rdf:Description>
  <rdf:Description rdf:nodeID="n90e14c5f212f40b8a6a776d86788ca21b3">
    <rdf:first rdf:resource="http://urn.fi/URN:NBN:fi:schema:bffi:Expression"/>
    <rdf:rest rdf:nodeID="n90e14c5f212f40b8a6a776d86788ca21b4"/>
  </rdf:Description>
  <rdf:Description rdf:about="http://urn.fi/URN:NBN:fi:schema:bffi:MonographWork">
    <dct:modified>2024-02-23 (New)</dct:modified>
    <rdfs:label xml:lang="en">Monograph work</rdfs:label>
    <rdfs:label xml:lang="fi">Monografiateos</rdfs:label>
    <rdf:type rdf:resource="http://www.w3.org/2002/07/owl#Class"/>
    <bffi-meta:broadMatch rdf:resource="http://id.loc.gov/ontologies/bibframe/Monograph"/>
    <rdfs:subClassOf rdf:resource="http://urn.fi/URN:NBN:fi:schema:bffi:Work"/>
  </rdf:Description>
  <rdf:Description rdf:about="http://urn.fi/URN:NBN:fi:schema:bffi:Local">
    <dct:modified>2024-06-19 (New)</dct:modified>
    <rdfs:label xml:lang="en">Local identifier</rdfs:label>
    <rdfs:label xml:lang="fi">Järjestelmän tunniste</rdfs:label>
    <rdf:type rdf:resource="http://www.w3.org/2002/07/owl#Class"/>
    <owl:equivalentClass rdf:resource="http://id.loc.gov/ontologies/bibframe/Local"/>
    <rdfs:subClassOf rdf:resource="http://urn.fi/URN:NBN:fi:schema:bffi:Identifier"/>
    <skos:definition xml:lang="en">BIBFRAME definition: Identifier established locally and not a standard number</skos:definition>
  </rdf:Description>
  <rdf:Description rdf:nodeID="n5cd48ce8767a480c888bcf43bfaa8780b5">
    <rdf:first rdf:resource="http://urn.fi/URN:NBN:fi:schema:bffi:Item"/>
    <rdf:rest rdf:resource="http://www.w3.org/1999/02/22-rdf-syntax-ns#nil"/>
  </rdf:Description>
  <rdf:Description rdf:about="http://urn.fi/URN:NBN:fi:schema:bffi:marcKey">
    <dct:modified>2024-06-19 (New)</dct:modified>
    <rdfs:label xml:lang="en">marc key for headings</rdfs:label>
    <rdfs:label xml:lang="fi">marc-kentän sisältö</rdfs:label>
    <rdfs:domain rdf:nodeID="n7333c8087d784d019f2d09a8a88483c5b1"/>
    <rdfs:range rdf:resource="http://www.w3.org/2000/01/rdf-schema#Literal"/>
    <rdf:type rdf:resource="http://www.w3.org/2002/07/owl#DatatypeProperty"/>
    <owl:equivalentProperty rdf:resource="http://id.loc.gov/ontologies/bflc/marcKey"/>
    <skos:definition xml:lang="en">BFLC definition: String to store MARC data</skos:definition>
  </rdf:Description>
  <rdf:Description rdf:nodeID="n3340e60e05a148bda7f556ae223dde3ab1">
    <rdf:type rdf:resource="http://www.w3.org/2002/07/owl#Class"/>
    <owl:unionOf rdf:nodeID="n3340e60e05a148bda7f556ae223dde3ab2"/>
  </rdf:Description>
  <rdf:Description rdf:nodeID="n42dc8c45022c4e7c8886fe842cc1e72fb2">
    <rdf:first rdf:resource="http://urn.fi/URN:NBN:fi:schema:bffi:Manifestation"/>
    <rdf:rest rdf:nodeID="n42dc8c45022c4e7c8886fe842cc1e72fb3"/>
  </rdf:Description>
  <rdf:Description rdf:nodeID="n0d5ef643a16a443a8864901b85eb32dbb4">
    <rdf:first rdf:resource="http://urn.fi/URN:NBN:fi:schema:bffi:Manifestation"/>
    <rdf:rest rdf:nodeID="n0d5ef643a16a443a8864901b85eb32dbb5"/>
  </rdf:Description>
  <rdf:Description rdf:nodeID="n5cd48ce8767a480c888bcf43bfaa8780b3">
    <rdf:first rdf:resource="http://urn.fi/URN:NBN:fi:schema:bffi:Expression"/>
    <rdf:rest rdf:nodeID="n5cd48ce8767a480c888bcf43bfaa8780b4"/>
  </rdf:Description>
  <rdf:Description rdf:nodeID="n9f671517b9dd4b7c955826691e2215f4b1">
    <rdf:type rdf:resource="http://www.w3.org/2002/07/owl#Class"/>
    <owl:unionOf rdf:nodeID="n9f671517b9dd4b7c955826691e2215f4b2"/>
  </rdf:Description>
  <rdf:Description rdf:nodeID="na62f4311181e4083bd9b0ad0c31f158ab3">
    <rdf:first rdf:resource="http://urn.fi/URN:NBN:fi:schema:bffi:Object"/>
    <rdf:rest rdf:resource="http://www.w3.org/1999/02/22-rdf-syntax-ns#nil"/>
  </rdf:Description>
  <rdf:Description rdf:nodeID="n7b5ca739c46d4a329e0fe2325c944dbcb3">
    <rdf:first rdf:resource="http://urn.fi/URN:NBN:fi:schema:bffi:NonMusicAudioWork"/>
    <rdf:rest rdf:nodeID="n7b5ca739c46d4a329e0fe2325c944dbcb4"/>
  </rdf:Description>
  <rdf:Description rdf:nodeID="n2ee3b3232b574a15b2a1faf6555dee4fb4">
    <rdf:first rdf:resource="http://urn.fi/URN:NBN:fi:schema:bffi:MovingImageWork"/>
    <rdf:rest rdf:resource="http://www.w3.org/1999/02/22-rdf-syntax-ns#nil"/>
  </rdf:Description>
  <rdf:Description rdf:nodeID="n5cd48ce8767a480c888bcf43bfaa8780b4">
    <rdf:first rdf:resource="http://urn.fi/URN:NBN:fi:schema:bffi:Manifestation"/>
    <rdf:rest rdf:nodeID="n5cd48ce8767a480c888bcf43bfaa8780b5"/>
  </rdf:Description>
  <rdf:Description rdf:nodeID="n68bca78492684c1398be6f6d4f77765db2">
    <rdf:first rdf:resource="http://urn.fi/URN:NBN:fi:schema:bffi:Work"/>
    <rdf:rest rdf:nodeID="n68bca78492684c1398be6f6d4f77765db3"/>
  </rdf:Description>
  <rdf:Description rdf:nodeID="n2ee3b3232b574a15b2a1faf6555dee4fb2">
    <rdf:first rdf:resource="http://urn.fi/URN:NBN:fi:schema:bffi:MusicWork"/>
    <rdf:rest rdf:nodeID="n2ee3b3232b574a15b2a1faf6555dee4fb3"/>
  </rdf:Description>
  <rdf:Description rdf:nodeID="ne27b8fc3c7014a3a99b60051d23322e1b1">
    <rdf:type rdf:resource="http://www.w3.org/2002/07/owl#Class"/>
    <owl:unionOf rdf:nodeID="ne27b8fc3c7014a3a99b60051d23322e1b2"/>
  </rdf:Description>
  <rdf:Description rdf:nodeID="n26a54bed81f14ec98f0dfd0d8091fc72b2">
    <rdf:first rdf:resource="http://urn.fi/URN:NBN:fi:schema:bffi:Work"/>
    <rdf:rest rdf:nodeID="n26a54bed81f14ec98f0dfd0d8091fc72b3"/>
  </rdf:Description>
  <rdf:Description rdf:nodeID="n14ff77a0080346dbb0cd2218439611d1b3">
    <rdf:first rdf:resource="http://urn.fi/URN:NBN:fi:schema:bffi:Expression"/>
    <rdf:rest rdf:nodeID="n14ff77a0080346dbb0cd2218439611d1b4"/>
  </rdf:Description>
  <rdf:Description rdf:nodeID="n0d5ef643a16a443a8864901b85eb32dbb3">
    <rdf:first rdf:resource="http://urn.fi/URN:NBN:fi:schema:bffi:Expression"/>
    <rdf:rest rdf:nodeID="n0d5ef643a16a443a8864901b85eb32dbb4"/>
  </rdf:Description>
  <rdf:Description rdf:nodeID="ne27b8fc3c7014a3a99b60051d23322e1b2">
    <rdf:first rdf:resource="http://urn.fi/URN:NBN:fi:schema:bffi:Work"/>
    <rdf:rest rdf:nodeID="ne27b8fc3c7014a3a99b60051d23322e1b3"/>
  </rdf:Description>
  <rdf:Description rdf:nodeID="n0a20977f4ff64f88b13306bf2d732ab6b1">
    <rdf:type rdf:resource="http://www.w3.org/2002/07/owl#Class"/>
    <owl:unionOf rdf:nodeID="n0a20977f4ff64f88b13306bf2d732ab6b2"/>
  </rdf:Description>
  <rdf:Description rdf:nodeID="n3db75dd6e811409899be21399dda0ca7b2">
    <rdf:first rdf:resource="http://urn.fi/URN:NBN:fi:schema:bffi:Person"/>
    <rdf:rest rdf:nodeID="n3db75dd6e811409899be21399dda0ca7b3"/>
  </rdf:Description>
  <rdf:Description rdf:nodeID="naa57803e9b8e45bda2faf492b90c6d13b3">
    <rdf:first rdf:resource="http://urn.fi/URN:NBN:fi:schema:bffi:Item"/>
    <rdf:rest rdf:resource="http://www.w3.org/1999/02/22-rdf-syntax-ns#nil"/>
  </rdf:Description>
  <rdf:Description rdf:nodeID="na6088cd10c31435fa00ddf5ff7f94651b3">
    <rdf:first rdf:resource="http://urn.fi/URN:NBN:fi:schema:bffi:ProvisionActivity"/>
    <rdf:rest rdf:resource="http://www.w3.org/1999/02/22-rdf-syntax-ns#nil"/>
  </rdf:Description>
  <rdf:Description rdf:nodeID="nbf7db4a78c624ed983d40041e8bb0721b1">
    <rdf:type rdf:resource="http://www.w3.org/2002/07/owl#Class"/>
    <owl:unionOf rdf:nodeID="nbf7db4a78c624ed983d40041e8bb0721b2"/>
  </rdf:Description>
  <rdf:Description rdf:nodeID="n30938fe99dde46599fe6796e2af454deb4">
    <rdf:first rdf:resource="http://urn.fi/URN:NBN:fi:schema:bffi:Manifestation"/>
    <rdf:rest rdf:resource="http://www.w3.org/1999/02/22-rdf-syntax-ns#nil"/>
  </rdf:Description>
  <rdf:Description rdf:nodeID="n14ff77a0080346dbb0cd2218439611d1b2">
    <rdf:first rdf:resource="http://urn.fi/URN:NBN:fi:schema:bffi:Work"/>
    <rdf:rest rdf:nodeID="n14ff77a0080346dbb0cd2218439611d1b3"/>
  </rdf:Description>
  <rdf:Description rdf:nodeID="nd5a8377479bd46e890352259af2eb06cb2">
    <rdf:first rdf:resource="http://urn.fi/URN:NBN:fi:schema:bffi:MusicAudioExpression"/>
    <rdf:rest rdf:nodeID="nd5a8377479bd46e890352259af2eb06cb3"/>
  </rdf:Description>
  <rdf:Description rdf:nodeID="n7333c8087d784d019f2d09a8a88483c5b4">
    <rdf:first rdf:resource="http://urn.fi/URN:NBN:fi:schema:bffi:Manifestation"/>
    <rdf:rest rdf:nodeID="n7333c8087d784d019f2d09a8a88483c5b5"/>
  </rdf:Description>
  <rdf:Description rdf:nodeID="n42dc8c45022c4e7c8886fe842cc1e72fb3">
    <rdf:first rdf:resource="http://urn.fi/URN:NBN:fi:schema:bffi:Item"/>
    <rdf:rest rdf:resource="http://www.w3.org/1999/02/22-rdf-syntax-ns#nil"/>
  </rdf:Description>
  <rdf:Description rdf:nodeID="n02875ff463bf42a79835462fc328eac6b5">
    <rdf:first rdf:resource="http://urn.fi/URN:NBN:fi:schema:bffi:Item"/>
    <rdf:rest rdf:resource="http://www.w3.org/1999/02/22-rdf-syntax-ns#nil"/>
  </rdf:Description>
  <rdf:Description rdf:nodeID="n7b5ca739c46d4a329e0fe2325c944dbcb1">
    <rdf:type rdf:resource="http://www.w3.org/2002/07/owl#Class"/>
    <owl:unionOf rdf:nodeID="n7b5ca739c46d4a329e0fe2325c944dbcb2"/>
  </rdf:Description>
  <rdf:Description rdf:nodeID="n71c313d9323b40c29dadafedf28680eeb1">
    <rdf:type rdf:resource="http://www.w3.org/2002/07/owl#Class"/>
    <owl:unionOf rdf:nodeID="n71c313d9323b40c29dadafedf28680eeb2"/>
  </rdf:Description>
  <rdf:Description rdf:nodeID="n9f671517b9dd4b7c955826691e2215f4b4">
    <rdf:first rdf:resource="http://urn.fi/URN:NBN:fi:schema:bffi:Manifestation"/>
    <rdf:rest rdf:nodeID="n9f671517b9dd4b7c955826691e2215f4b5"/>
  </rdf:Description>
  <rdf:Description rdf:nodeID="n096c0702f8c64e3bbe53573a59499c9ab2">
    <rdf:first rdf:resource="http://urn.fi/URN:NBN:fi:schema:bffi:MusicAudioExpression"/>
    <rdf:rest rdf:nodeID="n096c0702f8c64e3bbe53573a59499c9ab3"/>
  </rdf:Description>
  <rdf:Description rdf:nodeID="n02875ff463bf42a79835462fc328eac6b2">
    <rdf:first rdf:resource="http://urn.fi/URN:NBN:fi:schema:bffi:Work"/>
    <rdf:rest rdf:nodeID="n02875ff463bf42a79835462fc328eac6b3"/>
  </rdf:Description>
  <rdf:Description rdf:nodeID="n14ff77a0080346dbb0cd2218439611d1b5">
    <rdf:first rdf:resource="http://urn.fi/URN:NBN:fi:schema:bffi:Item"/>
    <rdf:rest rdf:resource="http://www.w3.org/1999/02/22-rdf-syntax-ns#nil"/>
  </rdf:Description>
  <rdf:Description rdf:nodeID="n9f671517b9dd4b7c955826691e2215f4b5">
    <rdf:first rdf:resource="http://urn.fi/URN:NBN:fi:schema:bffi:Item"/>
    <rdf:rest rdf:resource="http://www.w3.org/1999/02/22-rdf-syntax-ns#nil"/>
  </rdf:Description>
  <rdf:Description rdf:nodeID="n1e5b766c1bf94ff9812af7b852f48486b5">
    <rdf:first rdf:resource="http://urn.fi/URN:NBN:fi:schema:bffi:Item"/>
    <rdf:rest rdf:resource="http://www.w3.org/1999/02/22-rdf-syntax-ns#nil"/>
  </rdf:Description>
  <rdf:Description rdf:nodeID="na6088cd10c31435fa00ddf5ff7f94651b1">
    <rdf:type rdf:resource="http://www.w3.org/2002/07/owl#Class"/>
    <owl:unionOf rdf:nodeID="na6088cd10c31435fa00ddf5ff7f94651b2"/>
  </rdf:Description>
  <rdf:Description rdf:nodeID="nd5a8377479bd46e890352259af2eb06cb1">
    <rdf:type rdf:resource="http://www.w3.org/2002/07/owl#Class"/>
    <owl:unionOf rdf:nodeID="nd5a8377479bd46e890352259af2eb06cb2"/>
  </rdf:Description>
  <rdf:Description rdf:nodeID="n02875ff463bf42a79835462fc328eac6b3">
    <rdf:first rdf:resource="http://urn.fi/URN:NBN:fi:schema:bffi:Expression"/>
    <rdf:rest rdf:nodeID="n02875ff463bf42a79835462fc328eac6b4"/>
  </rdf:Description>
  <rdf:Description rdf:nodeID="n3fb00cccae3f45e2923b7c06d0716eb2b1">
    <rdf:type rdf:resource="http://www.w3.org/2002/07/owl#Class"/>
    <owl:unionOf rdf:nodeID="n3fb00cccae3f45e2923b7c06d0716eb2b2"/>
  </rdf:Description>
</rdf:RDF>
